@prefix dbo: <http://dbpedia.org/ontology/> .
@prefix dcterms: <http://purl.org/dc/terms/> .
@prefix foaf: <http://xmlns.com/foaf/0.1/> .
@prefix rdf: <http://www.w3.org/1999/02/22-rdf-syntax-ns#> .
@prefix rdfs: <http://www.w3.org/2000/01/rdf-schema#> .
@prefix roboprof: <http://roboprof.ca/schema/> .
@prefix roboprof_data: <http://roboprof.ca/data/> .
@prefix vcard: <https://www.w3.org/2006/vcard/ns/> .
@prefix vivo: <http://vivoweb.org/ontology/core/> .
@prefix xsd: <http://www.w3.org/2001/XMLSchema#> .

roboprof:CourseContent a rdfs:Class ;
    rdfs:label "Course Content"@en ;
    rdfs:comment "The content suggested or covered in a course."@en .

roboprof:CourseEvent a rdfs:Class ;
    rdfs:label "Course Event"@en ;
    rdfs:comment "Specifies the events in a course like lectures, labs, tutorials etc."@en .

roboprof:Grade a rdfs:Class ;
    rdfs:label "Grade"@en ;
    rdfs:comment "Refers to Grade received for a specific course."@en .

roboprof:InitialGrade a rdfs:Class ;
    rdfs:label "Initial Grade"@en ;
    rdfs:comment "Refers to Grade received for a specific course."@en ;
    rdfs:subClassOf roboprof:Grade .

roboprof:Lab a rdfs:Class ;
    rdfs:label "Lab"@en ;
    rdfs:comment "A single session of laboratory within a course, covering specific content."@en ;
    rdfs:subClassOf roboprof:CourseEvent .

roboprof:LabMaterial a rdfs:Class ;
    rdfs:label "Lab Material"@en ;
    rdfs:comment "Lab material suggested or covered in a course."@en ;
    rdfs:subClassOf roboprof:CourseContent .

roboprof:Lecture a rdfs:Class ;
    rdfs:label "Lecture"@en ;
    rdfs:comment "A single session of teaching within a course, covering specific content."@en ;
    rdfs:subClassOf roboprof:CourseEvent .

roboprof:OtherMaterial a rdfs:Class ;
    rdfs:label "Other Material"@en ;
    rdfs:comment "Other material suggested or covered in a course."@en ;
    rdfs:subClassOf roboprof:CourseContent .

roboprof:Reading a rdfs:Class ;
    rdfs:label "Reading"@en ;
    rdfs:comment "The readings covered in a course."@en ;
    rdfs:subClassOf roboprof:CourseContent .

roboprof:RetakeGrade a rdfs:Class ;
    rdfs:label "Retake Grade"@en ;
    rdfs:comment "Refers to Grade received for a specific course when retaken."@en ;
    rdfs:subClassOf roboprof:Grade .

roboprof:Slide a rdfs:Class ;
    rdfs:label "Slide"@en ;
    rdfs:comment "The powerpoint slides covered in a course."@en ;
    rdfs:subClassOf roboprof:CourseContent .

roboprof:Topic a rdfs:Class ;
    rdfs:label "Topic"@en ;
    rdfs:comment "A subject or theme covered in a course."@en .

roboprof:Worksheet a rdfs:Class ;
    rdfs:label "Worksheet"@en ;
    rdfs:comment "The worksheet covered in a course."@en ;
    rdfs:subClassOf roboprof:CourseContent .

<http://dbpedia.org/resource/10BASE2> a roboprof:Topic ;
    dbo:name "10BASE2" ;
    roboprof:provenanceInfo <file:///./dataset/Lecture%20Content/COMP%206461/OtherMaterial/ComputerNetwork.pdf> .

<http://dbpedia.org/resource/2> a roboprof:Topic ;
    dbo:name "HTTP/2" ;
    roboprof:provenanceInfo <file:///./dataset/Lab%20Content/COMP%206461/Lab%20Material/Lab%201.pdf> .

<http://dbpedia.org/resource/AIXI> a roboprof:Topic ;
    dbo:name "AIXI" ;
    roboprof:provenanceInfo <file:///./dataset/Lecture%20Content/COMP%206741/Readings/IntelligentAgent.pdf> .

<http://dbpedia.org/resource/AI_winter> a roboprof:Topic ;
    dbo:name "AI Winter" ;
    roboprof:provenanceInfo <file:///./dataset/Lecture%20Content/COMP%206741/Lectures/slides02.pdf> .

<http://dbpedia.org/resource/ALOHAnet> a roboprof:Topic ;
    dbo:name "Aloha",
        "Slotted Aloha" ;
    roboprof:provenanceInfo <file:///./dataset/Lecture%20Content/COMP%206461/Worksheets/TA3.pdf> .

<http://dbpedia.org/resource/ALPAC> a roboprof:Topic ;
    dbo:name "ALPAC" ;
    roboprof:provenanceInfo <file:///./dataset/Lecture%20Content/COMP%206741/Readings/NLP.pdf> .

<http://dbpedia.org/resource/ARPANET> a roboprof:Topic ;
    dbo:name "ARPANET",
        "Transmission Control Program" ;
    roboprof:provenanceInfo <file:///./dataset/Lecture%20Content/COMP%206461/OtherMaterial/TCP.pdf>,
        <file:///./dataset/Lecture%20Content/COMP%206461/Readings/InternetProtocolSuite.pdf> .

<http://dbpedia.org/resource/AT&T_Corporation> a roboprof:Topic ;
    dbo:name "AT&T Corporation" ;
    roboprof:provenanceInfo <file:///./dataset/Lecture%20Content/COMP%206461/OtherMaterial/ComputerNetwork.pdf> .

<http://dbpedia.org/resource/Aiman> a roboprof:Topic ;
    dbo:name "Aiman" ;
    roboprof:provenanceInfo <file:///./dataset/Lecture%20Content/COMP%206461/Lectures/2.ppt>,
        <file:///./dataset/Lecture%20Content/COMP%206461/Lectures/3.ppt>,
        <file:///./dataset/Lecture%20Content/COMP%206461/Lectures/4.ppt>,
        <file:///./dataset/Lecture%20Content/COMP%206461/Lectures/5.ppt>,
        <file:///./dataset/Lecture%20Content/COMP%206461/Lectures/6.ppt> .

<http://dbpedia.org/resource/Airbnb> a roboprof:Topic ;
    dbo:name "Airbnb" ;
    roboprof:provenanceInfo <file:///./dataset/Lecture%20Content/COMP%206741/Readings/KnowledgeGraph.pdf> .

<http://dbpedia.org/resource/Aksu_City> a roboprof:Topic ;
    dbo:name "GUMO" ;
    roboprof:provenanceInfo <file:///./dataset/Lecture%20Content/COMP%206741/Lectures/slides05.pdf> .

<http://dbpedia.org/resource/Alag> a roboprof:Topic ;
    dbo:name "Alag" ;
    roboprof:provenanceInfo <file:///./dataset/Lecture%20Content/COMP%206741/Lectures/slides05.pdf> .

<http://dbpedia.org/resource/Alan_Turing> a roboprof:Topic ;
    dbo:name "Alan Turing" ;
    roboprof:provenanceInfo <file:///./dataset/Lecture%20Content/COMP%206741/Readings/NLP.pdf> .

<http://dbpedia.org/resource/Algorithm> a roboprof:Topic ;
    dbo:name "algorithm" ;
    roboprof:provenanceInfo <file:///./dataset/Lecture%20Content/COMP%206461/Lectures/5.ppt>,
        <file:///./dataset/Lecture%20Content/COMP%206741/Lectures/slides06.pdf>,
        <file:///./dataset/Lecture%20Content/COMP%206741/Readings/RecommenderSystem.pdf> .

<http://dbpedia.org/resource/Alice_and_Bob> a roboprof:Topic ;
    dbo:name "Alice" ;
    roboprof:provenanceInfo <file:///./dataset/Lecture%20Content/COMP%206461/Lectures/2.ppt>,
        <file:///./dataset/Lecture%20Content/COMP%206461/Lectures/3.ppt>,
        <file:///./dataset/Lecture%20Content/COMP%206741/Lectures/slides02.pdf> .

<http://dbpedia.org/resource/Alison_DiLaurentis> a roboprof:Topic ;
    dbo:name "Alison" ;
    roboprof:provenanceInfo <file:///./dataset/Lecture%20Content/COMP%206741/Lectures/slides06.pdf> .

<http://dbpedia.org/resource/AlphaZero> a roboprof:Topic ;
    dbo:name "AlphaZero" ;
    roboprof:provenanceInfo <file:///./dataset/Lecture%20Content/COMP%206741/Readings/IntelligentAgent.pdf> .

<http://dbpedia.org/resource/Amazon_Alexa> a roboprof:Topic ;
    dbo:name "Alexa",
        "Amazon Alexa" ;
    roboprof:provenanceInfo <file:///./dataset/Lab%20Content/COMP%206741/Lab%20Material/Lab%203.pdf>,
        <file:///./dataset/Lecture%20Content/COMP%206741/Lectures/slides01.pdf>,
        <file:///./dataset/Lecture%20Content/COMP%206741/Readings/KnowledgeGraph.pdf> .

<http://dbpedia.org/resource/Amazon_Web_Services> a roboprof:Topic ;
    dbo:name "Amazon AWS" ;
    roboprof:provenanceInfo <file:///./dataset/Lecture%20Content/COMP%206741/Lectures/slides04.pdf> .

<http://dbpedia.org/resource/Anatoly_Kitov> a roboprof:Topic ;
    dbo:name "Anatoly Kitov" ;
    roboprof:provenanceInfo <file:///./dataset/Lecture%20Content/COMP%206461/OtherMaterial/ComputerNetwork.pdf> .

<http://dbpedia.org/resource/Andes> a roboprof:Topic ;
    dbo:name "Andes Mountains" ;
    roboprof:provenanceInfo <file:///./dataset/Lecture%20Content/COMP%206741/Lectures/slides01.pdf> .

<http://dbpedia.org/resource/Anthony_Julius> a roboprof:Topic ;
    dbo:name "Anthony Julius" ;
    roboprof:provenanceInfo <file:///./dataset/Lecture%20Content/COMP%206741/Lectures/slides05.pdf> .

<http://dbpedia.org/resource/Apache_HTTP_Server> a roboprof:Topic ;
    dbo:name "Apache",
        "Apache HTTP Server" ;
    roboprof:provenanceInfo <file:///./dataset/Lab%20Content/COMP%206461/Lab%20Material/Lab%202.pdf>,
        <file:///./dataset/Lecture%20Content/COMP%206461/Lectures/2.ppt> .

<http://dbpedia.org/resource/Apache_Lucene> a roboprof:Topic ;
    dbo:name "Lucene" ;
    roboprof:provenanceInfo <file:///./dataset/Lecture%20Content/COMP%206741/Lectures/slides01.pdf> .

<http://dbpedia.org/resource/Apache_Solr> a roboprof:Topic ;
    dbo:name "Solr" ;
    roboprof:provenanceInfo <file:///./dataset/Lecture%20Content/COMP%206741/Lectures/slides01.pdf> .

<http://dbpedia.org/resource/Apple_Inc.> a roboprof:Topic ;
    dbo:name "Apple" ;
    roboprof:provenanceInfo <file:///./dataset/Lecture%20Content/COMP%206741/Readings/KnowledgeGraph.pdf> .

<http://dbpedia.org/resource/Application_layer> a roboprof:Topic ;
    dbo:name "Application Layer" ;
    roboprof:provenanceInfo <file:///./dataset/Lecture%20Content/COMP%206461/Lectures/2.ppt>,
        <file:///./dataset/Lecture%20Content/COMP%206461/Lectures/3.ppt> .

<http://dbpedia.org/resource/Application_programming_interface> a roboprof:Topic ;
    dbo:name "API" ;
    roboprof:provenanceInfo <file:///./dataset/Lab%20Content/COMP%206461/Lab%20Material/Lab%201.pdf>,
        <file:///./dataset/Lecture%20Content/COMP%206461/Lectures/2.ppt>,
        <file:///./dataset/Lecture%20Content/COMP%206741/Lectures/slides01.pdf>,
        <file:///./dataset/Lecture%20Content/COMP%206741/Lectures/slides02.pdf> .

<http://dbpedia.org/resource/Artificial_intelligence> a roboprof:Topic ;
    dbo:name "AI",
        "Artificial Intelligence",
        "Intelligent Systems" ;
    roboprof:provenanceInfo <file:///./dataset/Lab%20Content/COMP%206741/Lab%20Material/Lab%202.pdf>,
        <file:///./dataset/Lab%20Content/COMP%206741/Lab%20Material/Lab%203.pdf>,
        <file:///./dataset/Lecture%20Content/COMP%206741/Lectures/slides01.pdf>,
        <file:///./dataset/Lecture%20Content/COMP%206741/Lectures/slides02.pdf>,
        <file:///./dataset/Lecture%20Content/COMP%206741/Lectures/slides03.pdf>,
        <file:///./dataset/Lecture%20Content/COMP%206741/Lectures/slides06.pdf>,
        <file:///./dataset/Lecture%20Content/COMP%206741/Readings/IntelligentAgent.pdf>,
        <file:///./dataset/Lecture%20Content/COMP%206741/Worksheets/worksheet01.pdf>,
        <file:///./dataset/Lecture%20Content/COMP%206741/Worksheets/worksheet03.pdf> .

<http://dbpedia.org/resource/Association_Control_Service_Element> a roboprof:Topic ;
    dbo:name "ACSE",
        "Association Control Service Element" ;
    roboprof:provenanceInfo <file:///./dataset/Lecture%20Content/COMP%206461/OtherMaterial/ApplicationLayer.pdf> .

<http://dbpedia.org/resource/Association_for_Computing_Machinery> a roboprof:Topic ;
    dbo:name "ACM" ;
    roboprof:provenanceInfo <file:///./dataset/Lecture%20Content/COMP%206741/Lectures/slides03.pdf> .

<http://dbpedia.org/resource/Asynchronous_transfer_mode> a roboprof:Topic ;
    dbo:name "ATM" ;
    roboprof:provenanceInfo <file:///./dataset/Lecture%20Content/COMP%206461/Lectures/6.ppt> .

<http://dbpedia.org/resource/Automatic_repeat_request> a roboprof:Topic ;
    dbo:name "ARQ" ;
    roboprof:provenanceInfo <file:///./dataset/Lab%20Content/COMP%206461/Lab%20Material/Lab%203.pdf>,
        <file:///./dataset/Lecture%20Content/COMP%206461/Lectures/4.ppt>,
        <file:///./dataset/Lecture%20Content/COMP%206461/Readings/GoBackN.pdf>,
        <file:///./dataset/Lecture%20Content/COMP%206461/Readings/SelectiveRepeat.pdf> .

<http://dbpedia.org/resource/BBN_Technologies> a roboprof:Topic ;
    dbo:name "BBN" ;
    roboprof:provenanceInfo <file:///./dataset/Lecture%20Content/COMP%206461/OtherMaterial/ComputerNetwork.pdf> .

<http://dbpedia.org/resource/BSD_licenses> a roboprof:Topic ;
    dbo:name "BSD License" ;
    roboprof:provenanceInfo <file:///./dataset/Lecture%20Content/COMP%206741/Lectures/slides06.pdf> .

<http://dbpedia.org/resource/BabelNet> a roboprof:Topic ;
    dbo:name "BabelNet" ;
    roboprof:provenanceInfo <file:///./dataset/Lecture%20Content/COMP%206741/Lectures/slides04.pdf> .

<http://dbpedia.org/resource/Battle_of_Fredericksburg> a roboprof:Topic ;
    dbo:name "Fredericksburg" ;
    roboprof:provenanceInfo <file:///./dataset/Lecture%20Content/COMP%206741/Lectures/slides01.pdf> .

<http://dbpedia.org/resource/Bertrand_Russell> a roboprof:Topic ;
    dbo:name "Russell" ;
    roboprof:provenanceInfo <file:///./dataset/Lecture%20Content/COMP%206741/Readings/IntelligentAgent.pdf> .

<http://dbpedia.org/resource/Bibcode> a roboprof:Topic ;
    dbo:name "Bibcode" ;
    roboprof:provenanceInfo <file:///./dataset/Lecture%20Content/COMP%206461/Readings/SelectiveRepeat.pdf> .

<http://dbpedia.org/resource/BioPAX> a roboprof:Topic ;
    dbo:name "BioPAX" ;
    roboprof:provenanceInfo <file:///./dataset/Lecture%20Content/COMP%206741/Lectures/slides04.pdf> .

<http://dbpedia.org/resource/BitTorrent> a roboprof:Topic ;
    dbo:name "BitTorrent" ;
    roboprof:provenanceInfo <file:///./dataset/Lecture%20Content/COMP%206461/Lectures/2.ppt>,
        <file:///./dataset/Lecture%20Content/COMP%206461/Lectures/3.ppt>,
        <file:///./dataset/Lecture%20Content/COMP%206461/Worksheets/TA1.pdf> .

<http://dbpedia.org/resource/Bit_error_rate> a roboprof:Topic ;
    dbo:name "BERT" ;
    roboprof:provenanceInfo <file:///./dataset/Lecture%20Content/COMP%206741/Lectures/slides01.pdf> .

<http://dbpedia.org/resource/BlackBerry_Priv> a roboprof:Topic ;
    dbo:name "Priv" ;
    roboprof:provenanceInfo <file:///./dataset/Lecture%20Content/COMP%206741/Lectures/slides02.pdf> .

<http://dbpedia.org/resource/Bob_Kahn> a roboprof:Topic ;
    dbo:name "Bob Kahn" ;
    roboprof:provenanceInfo <file:///./dataset/Lecture%20Content/COMP%206461/OtherMaterial/TCP.pdf>,
        <file:///./dataset/Lecture%20Content/COMP%206461/Readings/InternetProtocolSuite.pdf> .

<http://dbpedia.org/resource/Bootstrap_Protocol> a roboprof:Topic ;
    dbo:name "BOOTP" ;
    roboprof:provenanceInfo <file:///./dataset/Lecture%20Content/COMP%206461/OtherMaterial/ApplicationLayer.pdf> .

<http://dbpedia.org/resource/Brutus_the_Younger> a roboprof:Topic ;
    dbo:name "BRUTUS" ;
    roboprof:provenanceInfo <file:///./dataset/Lecture%20Content/COMP%206741/Lectures/slides05.pdf> .

<http://dbpedia.org/resource/Byte> a roboprof:Topic ;
    dbo:name "Byte" ;
    roboprof:provenanceInfo <file:///./dataset/Lab%20Content/COMP%206461/Lab%20Material/Lab%203.pdf> .

<http://dbpedia.org/resource/CLOUD_experiment> a roboprof:Topic ;
    dbo:name "CLOUD" ;
    roboprof:provenanceInfo <file:///./dataset/Lecture%20Content/COMP%206741/Lectures/slides02.pdf> .

<http://dbpedia.org/resource/CNAME_record> a roboprof:Topic ;
    dbo:name "CNAME" ;
    roboprof:provenanceInfo <file:///./dataset/Lecture%20Content/COMP%206461/Lectures/3.ppt> .

<http://dbpedia.org/resource/CURL> a roboprof:Topic ;
    dbo:name "cURL",
        "curl",
        "libcurl" ;
    roboprof:provenanceInfo <file:///./dataset/Lab%20Content/COMP%206461/Lab%20Material/Lab%201.pdf>,
        <file:///./dataset/Lab%20Content/COMP%206461/Lab%20Material/Lab%202.pdf> .

<http://dbpedia.org/resource/CYCLADES> a roboprof:Topic ;
    dbo:name "CYCLADES" ;
    roboprof:provenanceInfo <file:///./dataset/Lecture%20Content/COMP%206461/OtherMaterial/TCP.pdf> .

<http://dbpedia.org/resource/Cambridge_Analytica> a roboprof:Topic ;
    dbo:name "Cambridge Analytica" ;
    roboprof:provenanceInfo <file:///./dataset/Lecture%20Content/COMP%206741/Lectures/slides06.pdf> .

<http://dbpedia.org/resource/Canada> a roboprof:Topic ;
    dbo:name "Canada" ;
    roboprof:provenanceInfo <file:///./dataset/Lecture%20Content/COMP%206461/Lectures/2.ppt>,
        <file:///./dataset/Lecture%20Content/COMP%206461/Lectures/3.ppt>,
        <file:///./dataset/Lecture%20Content/COMP%206461/Lectures/6.ppt> .

<http://dbpedia.org/resource/Central_processing_unit> a roboprof:Topic ;
    dbo:name "CPU" ;
    roboprof:provenanceInfo <file:///./dataset/Lab%20Content/COMP%206461/Lab%20Material/Lab%201.pdf> .

<http://dbpedia.org/resource/Cerberus> a roboprof:Topic ;
    dbo:name "Kerberos" ;
    roboprof:provenanceInfo <file:///./dataset/Lab%20Content/COMP%206461/Lab%20Material/Lab%201.pdf> .

<http://dbpedia.org/resource/Chatbot> a roboprof:Topic ;
    dbo:name "Chatbot" ;
    roboprof:provenanceInfo <file:///./dataset/Lecture%20Content/COMP%206741/Lectures/slides01.pdf> .

<http://dbpedia.org/resource/Chavacano> a roboprof:Topic ;
    dbo:name "Chabacano" ;
    roboprof:provenanceInfo <file:///./dataset/Lecture%20Content/COMP%206741/Lectures/slides06.pdf> .

<http://dbpedia.org/resource/Checksum> a roboprof:Topic ;
    dbo:name "Checksum" ;
    roboprof:provenanceInfo <file:///./dataset/Lecture%20Content/COMP%206461/Lectures/4.ppt>,
        <file:///./dataset/Lecture%20Content/COMP%206461/OtherMaterial/UDP.pdf> .

<http://dbpedia.org/resource/Classless_Inter-Domain_Routing> a roboprof:Topic ;
    dbo:name "CIDR" ;
    roboprof:provenanceInfo <file:///./dataset/Lecture%20Content/COMP%206461/Worksheets/TA2.pdf> .

<http://dbpedia.org/resource/Cleopatra> a roboprof:Topic ;
    dbo:name "CLEOPATRA",
        "Cleopatra" ;
    roboprof:provenanceInfo <file:///./dataset/Lecture%20Content/COMP%206741/Lectures/slides05.pdf> .

<http://dbpedia.org/resource/Cole_Howard> a roboprof:Topic ;
    dbo:name "Cole Howard" ;
    roboprof:provenanceInfo <file:///./dataset/Lecture%20Content/COMP%206741/Lectures/slides01.pdf> .

<http://dbpedia.org/resource/Collective_intelligence> a roboprof:Topic ;
    dbo:name "Collective Intelligence" ;
    roboprof:provenanceInfo <file:///./dataset/Lecture%20Content/COMP%206741/Lectures/slides05.pdf> .

<http://dbpedia.org/resource/Comma-separated_values> a roboprof:Topic ;
    dbo:name "CSV" ;
    roboprof:provenanceInfo <file:///./dataset/Lecture%20Content/COMP%206741/Lectures/slides04.pdf> .

<http://dbpedia.org/resource/Common_Management_Information_Protocol> a roboprof:Topic ;
    dbo:name "CMIP",
        "Common Management Information Protocol" ;
    roboprof:provenanceInfo <file:///./dataset/Lecture%20Content/COMP%206461/OtherMaterial/ApplicationLayer.pdf> .

<http://dbpedia.org/resource/Compound_annual_growth_rate> a roboprof:Topic ;
    dbo:name "CAGR" ;
    roboprof:provenanceInfo <file:///./dataset/Lecture%20Content/COMP%206741/Lectures/slides01.pdf> .

<http://dbpedia.org/resource/Computer-aided_software_engineering> a roboprof:Topic ;
    dbo:name "CASE" ;
    roboprof:provenanceInfo <file:///./dataset/Lecture%20Content/COMP%206461/OtherMaterial/ApplicationLayer.pdf> .

<http://dbpedia.org/resource/Computer_science> a roboprof:Topic ;
    dbo:name "Computer Science" ;
    roboprof:provenanceInfo <file:///./dataset/Lecture%20Content/COMP%206461/Lectures/2.ppt>,
        <file:///./dataset/Lecture%20Content/COMP%206461/Lectures/3.ppt>,
        <file:///./dataset/Lecture%20Content/COMP%206461/Lectures/4.ppt>,
        <file:///./dataset/Lecture%20Content/COMP%206461/Lectures/5.ppt>,
        <file:///./dataset/Lecture%20Content/COMP%206461/Lectures/6.ppt>,
        <file:///./dataset/Lecture%20Content/COMP%206741/Lectures/slides01.pdf>,
        <file:///./dataset/Lecture%20Content/COMP%206741/Lectures/slides02.pdf>,
        <file:///./dataset/Lecture%20Content/COMP%206741/Lectures/slides03.pdf>,
        <file:///./dataset/Lecture%20Content/COMP%206741/Lectures/slides04.pdf>,
        <file:///./dataset/Lecture%20Content/COMP%206741/Lectures/slides05.pdf>,
        <file:///./dataset/Lecture%20Content/COMP%206741/Lectures/slides06.pdf> .

<http://dbpedia.org/resource/Concordia_University> a roboprof:Topic ;
    dbo:name "Concordia" ;
    roboprof:provenanceInfo <file:///./dataset/Lab%20Content/COMP%206741/Lab%20Material/Lab%203.pdf> .

<http://dbpedia.org/resource/Conference_on_Neural_Information_Processing_Systems> a roboprof:Topic ;
    dbo:name "NIPS" ;
    roboprof:provenanceInfo <file:///./dataset/Lecture%20Content/COMP%206741/OtherMaterial/WordEmbeddings.pdf> .

<http://dbpedia.org/resource/Coreference> a roboprof:Topic ;
    dbo:name "Coreference" ;
    roboprof:provenanceInfo <file:///./dataset/Lecture%20Content/COMP%206741/OtherMaterial/TextMining.pdf> .

<http://dbpedia.org/resource/Corpus_linguistics> a roboprof:Topic ;
    dbo:name "corpora" ;
    roboprof:provenanceInfo <file:///./dataset/Lecture%20Content/COMP%206741/Readings/NLP.pdf> .

<http://dbpedia.org/resource/Cortana> a roboprof:Topic ;
    dbo:name "Microsoft Cortana" ;
    roboprof:provenanceInfo <file:///./dataset/Lecture%20Content/COMP%206741/Lectures/slides01.pdf> .

<http://dbpedia.org/resource/Cyc> a roboprof:Topic ;
    dbo:name "Cyc" ;
    roboprof:provenanceInfo <file:///./dataset/Lecture%20Content/COMP%206741/Lectures/slides02.pdf> .

<http://dbpedia.org/resource/DARPA> a roboprof:Topic ;
    dbo:name "DARPA" ;
    roboprof:provenanceInfo <file:///./dataset/Lecture%20Content/COMP%206461/Readings/InternetProtocolSuite.pdf> .

<http://dbpedia.org/resource/DBpedia> a roboprof:Topic ;
    dbo:name "DBpedia" ;
    roboprof:provenanceInfo <file:///./dataset/Lab%20Content/COMP%206741/Lab%20Material/Lab%202.pdf>,
        <file:///./dataset/Lab%20Content/COMP%206741/Lab%20Material/Lab%203.pdf>,
        <file:///./dataset/Lecture%20Content/COMP%206741/Lectures/slides02.pdf>,
        <file:///./dataset/Lecture%20Content/COMP%206741/Lectures/slides04.pdf>,
        <file:///./dataset/Lecture%20Content/COMP%206741/Readings/KnowledgeGraph.pdf>,
        <file:///./dataset/Lecture%20Content/COMP%206741/Worksheets/worksheet03.pdf> .

<http://dbpedia.org/resource/DICT> a roboprof:Topic ;
    dbo:name "DICT" ;
    roboprof:provenanceInfo <file:///./dataset/Lab%20Content/COMP%206461/Lab%20Material/Lab%201.pdf> .

<http://dbpedia.org/resource/Dartmouth_Time_Sharing_System> a roboprof:Topic ;
    dbo:name "Dartmouth Time Sharing System" ;
    roboprof:provenanceInfo <file:///./dataset/Lecture%20Content/COMP%206461/OtherMaterial/ComputerNetwork.pdf> .

<http://dbpedia.org/resource/Data-rate_units> a roboprof:Topic ;
    dbo:name "Gbps",
        "Kbps",
        "Mbps",
        "kbps" ;
    roboprof:provenanceInfo <file:///./dataset/Lecture%20Content/COMP%206461/Lectures/2.ppt>,
        <file:///./dataset/Lecture%20Content/COMP%206461/Lectures/5.ppt>,
        <file:///./dataset/Lecture%20Content/COMP%206461/Lectures/6.ppt>,
        <file:///./dataset/Lecture%20Content/COMP%206461/Worksheets/TA1.pdf> .

<http://dbpedia.org/resource/Data_integration> a roboprof:Topic ;
    dbo:name "Data Integration" ;
    roboprof:provenanceInfo <file:///./dataset/Lab%20Content/COMP%206741/Lab%20Material/Lab%202.pdf>,
        <file:///./dataset/Lecture%20Content/COMP%206741/Lectures/slides02.pdf> .

<http://dbpedia.org/resource/Data_model> a roboprof:Topic ;
    dbo:name "schema" ;
    roboprof:provenanceInfo <file:///./dataset/Lecture%20Content/COMP%206741/Lectures/slides01.pdf>,
        <file:///./dataset/Lecture%20Content/COMP%206741/Lectures/slides02.pdf> .

<http://dbpedia.org/resource/Dedi> a roboprof:Topic ;
    dbo:name "dedi" ;
    roboprof:provenanceInfo <file:///./dataset/Lecture%20Content/COMP%206461/Worksheets/TA1.pdf> .

<http://dbpedia.org/resource/Deep_learning> a roboprof:Topic ;
    dbo:name "Deep Learning" ;
    roboprof:provenanceInfo <file:///./dataset/Lecture%20Content/COMP%206741/Lectures/slides01.pdf>,
        <file:///./dataset/Lecture%20Content/COMP%206741/Lectures/slides06.pdf> .

<http://dbpedia.org/resource/Deliverable> a roboprof:Topic ;
    dbo:name "Deliverable" ;
    roboprof:provenanceInfo <file:///./dataset/Lab%20Content/COMP%206461/Lab%20Material/Lab%201.pdf>,
        <file:///./dataset/Lab%20Content/COMP%206461/Lab%20Material/Lab%202.pdf>,
        <file:///./dataset/Lab%20Content/COMP%206461/Lab%20Material/Lab%203.pdf> .

<http://dbpedia.org/resource/Denial-of-service_attack> a roboprof:Topic ;
    dbo:name "DDoS" ;
    roboprof:provenanceInfo <file:///./dataset/Lecture%20Content/COMP%206461/Lectures/3.ppt> .

<http://dbpedia.org/resource/Description_logic> a roboprof:Topic ;
    dbo:name "Description Logic" ;
    roboprof:provenanceInfo <file:///./dataset/Lecture%20Content/COMP%206741/Lectures/slides02.pdf>,
        <file:///./dataset/Lecture%20Content/COMP%206741/Lectures/slides04.pdf> .

<http://dbpedia.org/resource/Design_Issues> a roboprof:Topic ;
    dbo:name "Design Issues" ;
    roboprof:provenanceInfo <file:///./dataset/Lecture%20Content/COMP%206741/Lectures/slides04.pdf> .

<http://dbpedia.org/resource/Dewey_Decimal_Classification> a roboprof:Topic ;
    dbo:name "Dewey Decimal" ;
    roboprof:provenanceInfo <file:///./dataset/Lecture%20Content/COMP%206741/Lectures/slides03.pdf> .

<http://dbpedia.org/resource/Dieter_Fensel> a roboprof:Topic ;
    dbo:name "Dieter Fensel" ;
    roboprof:provenanceInfo <file:///./dataset/Lecture%20Content/COMP%206741/Lectures/slides04.pdf> .

<http://dbpedia.org/resource/Digital_subscriber_line> a roboprof:Topic ;
    dbo:name "DSL" ;
    roboprof:provenanceInfo <file:///./dataset/Lecture%20Content/COMP%206461/Lectures/2.ppt>,
        <file:///./dataset/Lecture%20Content/COMP%206461/Worksheets/TA1.pdf> .

<http://dbpedia.org/resource/Dimension> a roboprof:Topic ;
    dbo:name "2D" ;
    roboprof:provenanceInfo <file:///./dataset/Lecture%20Content/COMP%206741/Lectures/slides05.pdf> .

<http://dbpedia.org/resource/Disconnect_Mobile> a roboprof:Topic ;
    dbo:name "Disconnect" ;
    roboprof:provenanceInfo <file:///./dataset/Lecture%20Content/COMP%206461/Lectures/6.ppt> .

<http://dbpedia.org/resource/Domain_Name_System> a roboprof:Topic ;
    dbo:name "DNS",
        "Domain Name System" ;
    roboprof:provenanceInfo <file:///./dataset/Lecture%20Content/COMP%206461/Lectures/2.ppt>,
        <file:///./dataset/Lecture%20Content/COMP%206461/Lectures/3.ppt>,
        <file:///./dataset/Lecture%20Content/COMP%206461/Lectures/4.ppt>,
        <file:///./dataset/Lecture%20Content/COMP%206461/OtherMaterial/ApplicationLayer.pdf>,
        <file:///./dataset/Lecture%20Content/COMP%206461/OtherMaterial/UDP.pdf> .

<http://dbpedia.org/resource/Donald_O._Hebb> a roboprof:Topic ;
    dbo:name "Donald Hebb" ;
    roboprof:provenanceInfo <file:///./dataset/Lecture%20Content/COMP%206741/OtherMaterial/MachineLearning.pdf> .

<http://dbpedia.org/resource/Dublin_Core> a roboprof:Topic ;
    dbo:name "Dublin Core" ;
    roboprof:provenanceInfo <file:///./dataset/Lecture%20Content/COMP%206741/Lectures/slides03.pdf> .

<http://dbpedia.org/resource/Due_Date> a roboprof:Topic ;
    dbo:name "Due Date" ;
    roboprof:provenanceInfo <file:///./dataset/Lab%20Content/COMP%206461/Lab%20Material/Lab%201.pdf>,
        <file:///./dataset/Lab%20Content/COMP%206461/Lab%20Material/Lab%202.pdf>,
        <file:///./dataset/Lab%20Content/COMP%206461/Lab%20Material/Lab%203.pdf>,
        <file:///./dataset/Lecture%20Content/COMP%206461/Worksheets/TA1.pdf>,
        <file:///./dataset/Lecture%20Content/COMP%206461/Worksheets/TA2.pdf> .

<http://dbpedia.org/resource/Dynamic_Host_Configuration_Protocol> a roboprof:Topic ;
    dbo:name "DHCP" ;
    roboprof:provenanceInfo <file:///./dataset/Lecture%20Content/COMP%206461/OtherMaterial/UDP.pdf> .

<http://dbpedia.org/resource/EBay> a roboprof:Topic ;
    dbo:name "eBay" ;
    roboprof:provenanceInfo <file:///./dataset/Lecture%20Content/COMP%206741/Readings/KnowledgeGraph.pdf> .

<http://dbpedia.org/resource/ELIZA> a roboprof:Topic ;
    dbo:name "ELIZA" ;
    roboprof:provenanceInfo <file:///./dataset/Lecture%20Content/COMP%206741/Readings/NLP.pdf> .

<http://dbpedia.org/resource/Educause> a roboprof:Topic ;
    dbo:name "Educause" ;
    roboprof:provenanceInfo <file:///./dataset/Lecture%20Content/COMP%206461/Lectures/3.ppt> .

<http://dbpedia.org/resource/Edward_S._Herman> a roboprof:Topic ;
    dbo:name "Herman" ;
    roboprof:provenanceInfo <file:///./dataset/Lecture%20Content/COMP%206741/Lectures/slides02.pdf> .

<http://dbpedia.org/resource/Electronic_design_automation> a roboprof:Topic ;
    dbo:name "EDA" ;
    roboprof:provenanceInfo <file:///./dataset/Lecture%20Content/COMP%206741/Lectures/slides06.pdf>,
        <file:///./dataset/Lecture%20Content/COMP%206741/OtherMaterial/MachineLearning.pdf> .

<http://dbpedia.org/resource/Email> a roboprof:Topic ;
    dbo:name "Internet Mail" ;
    roboprof:provenanceInfo <file:///./dataset/Lecture%20Content/COMP%206461/Lectures/2.ppt> .

<http://dbpedia.org/resource/Endianness> a roboprof:Topic ;
    dbo:name "Endianness" ;
    roboprof:provenanceInfo <file:///./dataset/Lab%20Content/COMP%206461/Lab%20Material/Lab%203.pdf> .

<http://dbpedia.org/resource/English_language> a roboprof:Topic ;
    dbo:name "English" ;
    roboprof:provenanceInfo <file:///./dataset/Lab%20Content/COMP%206741/Lab%20Material/Lab%203.pdf>,
        <file:///./dataset/Lecture%20Content/COMP%206741/Lectures/slides01.pdf>,
        <file:///./dataset/Lecture%20Content/COMP%206741/Readings/NLP.pdf> .

<http://dbpedia.org/resource/Essence> a roboprof:Topic ;
    dbo:name "Essence" ;
    roboprof:provenanceInfo <file:///./dataset/Lecture%20Content/COMP%206741/Lectures/slides06.pdf> .

<http://dbpedia.org/resource/Ethernet> a roboprof:Topic ;
    dbo:name "Ethernet" ;
    roboprof:provenanceInfo <file:///./dataset/Lecture%20Content/COMP%206461/OtherMaterial/ComputerNetwork.pdf>,
        <file:///./dataset/Lecture%20Content/COMP%206461/Readings/NetworkCongestion.pdf> .

<http://dbpedia.org/resource/FTAM> a roboprof:Topic ;
    dbo:name "FTAM" ;
    roboprof:provenanceInfo <file:///./dataset/Lecture%20Content/COMP%206461/OtherMaterial/ApplicationLayer.pdf> .

<http://dbpedia.org/resource/FTPS> a roboprof:Topic ;
    dbo:name "FTPS" ;
    roboprof:provenanceInfo <file:///./dataset/Lab%20Content/COMP%206461/Lab%20Material/Lab%201.pdf> .

<http://dbpedia.org/resource/Facebook_Graph_Search> a roboprof:Topic ;
    dbo:name "Facebook Graph Search" ;
    roboprof:provenanceInfo <file:///./dataset/Lecture%20Content/COMP%206741/Lectures/slides02.pdf> .

<http://dbpedia.org/resource/File_Transfer_Protocol> a roboprof:Topic ;
    dbo:name "FTP",
        "File Transfer Protocol",
        "SFTP" ;
    roboprof:provenanceInfo <file:///./dataset/Lab%20Content/COMP%206461/Lab%20Material/Lab%201.pdf>,
        <file:///./dataset/Lecture%20Content/COMP%206461/Lectures/2.ppt>,
        <file:///./dataset/Lecture%20Content/COMP%206461/OtherMaterial/ApplicationLayer.pdf> .

<http://dbpedia.org/resource/File_server> a roboprof:Topic ;
    dbo:name "File Server" ;
    roboprof:provenanceInfo <file:///./dataset/Lab%20Content/COMP%206461/Lab%20Material/Lab%202.pdf> .

<http://dbpedia.org/resource/Finite-state_machine> a roboprof:Topic ;
    dbo:name "Finite State Machine",
        "Finite State Machines" ;
    roboprof:provenanceInfo <file:///./dataset/Lecture%20Content/COMP%206461/Lectures/5.ppt> .

<http://dbpedia.org/resource/Finland> a roboprof:Topic ;
    dbo:name "FIN" ;
    roboprof:provenanceInfo <file:///./dataset/Lecture%20Content/COMP%206461/Lectures/6.ppt> .

<http://dbpedia.org/resource/Firefox> a roboprof:Topic ;
    dbo:name "Firefox" ;
    roboprof:provenanceInfo <file:///./dataset/Lecture%20Content/COMP%206461/Lectures/2.ppt> .

<http://dbpedia.org/resource/Flickr> a roboprof:Topic ;
    dbo:name "Flickr" ;
    roboprof:provenanceInfo <file:///./dataset/Lecture%20Content/COMP%206741/Lectures/slides03.pdf>,
        <file:///./dataset/Lecture%20Content/COMP%206741/Lectures/slides04.pdf> .

<http://dbpedia.org/resource/Freebase> a roboprof:Topic ;
    dbo:name "Freebase" ;
    roboprof:provenanceInfo <file:///./dataset/Lecture%20Content/COMP%206741/Lectures/slides04.pdf>,
        <file:///./dataset/Lecture%20Content/COMP%206741/Readings/KnowledgeGraph.pdf> .

<http://dbpedia.org/resource/Fuseki> a roboprof:Topic ;
    dbo:name "Fuseki" ;
    roboprof:provenanceInfo <file:///./dataset/Lecture%20Content/COMP%206741/Lectures/slides04.pdf> .

<http://dbpedia.org/resource/G.hn> a roboprof:Topic ;
    dbo:name "G.hn" ;
    roboprof:provenanceInfo <file:///./dataset/Lecture%20Content/COMP%206461/Readings/SelectiveRepeat.pdf> .

<http://dbpedia.org/resource/Gartner> a roboprof:Topic ;
    dbo:name "Gartner" ;
    roboprof:provenanceInfo <file:///./dataset/Lecture%20Content/COMP%206741/Lectures/slides01.pdf> .

<http://dbpedia.org/resource/Gene_ontology> a roboprof:Topic ;
    dbo:name "Gene Ontology" ;
    roboprof:provenanceInfo <file:///./dataset/Lecture%20Content/COMP%206741/Lectures/slides04.pdf> .

<http://dbpedia.org/resource/General_officer> a roboprof:Topic ;
    dbo:name "General" ;
    roboprof:provenanceInfo <file:///./dataset/Lecture%20Content/COMP%206741/Lectures/slides02.pdf> .

<http://dbpedia.org/resource/GeoNames> a roboprof:Topic ;
    dbo:name "Geonames" ;
    roboprof:provenanceInfo <file:///./dataset/Lecture%20Content/COMP%206741/Lectures/slides04.pdf>,
        <file:///./dataset/Lecture%20Content/COMP%206741/Readings/KnowledgeGraph.pdf> .

<http://dbpedia.org/resource/Git> a roboprof:Topic ;
    dbo:name "Git" ;
    roboprof:provenanceInfo <file:///./dataset/Lab%20Content/COMP%206461/Lab%20Material/Lab%201.pdf> .

<http://dbpedia.org/resource/GitHub> a roboprof:Topic ;
    dbo:name "GitHub" ;
    roboprof:provenanceInfo <file:///./dataset/Lab%20Content/COMP%206741/Lab%20Material/Lab%201.pdf> .

<http://dbpedia.org/resource/Glossary_of_ancient_Roman_religion> a roboprof:Topic ;
    dbo:name "fas" ;
    roboprof:provenanceInfo <file:///./dataset/Lecture%20Content/COMP%206741/Lectures/slides02.pdf> .

<http://dbpedia.org/resource/Google> a roboprof:Topic ;
    dbo:name "Google" ;
    roboprof:provenanceInfo <file:///./dataset/Lecture%20Content/COMP%206741/Lectures/slides01.pdf>,
        <file:///./dataset/Lecture%20Content/COMP%206741/Readings/KnowledgeGraph.pdf> .

<http://dbpedia.org/resource/Google_Assistant> a roboprof:Topic ;
    dbo:name "Google Assistant" ;
    roboprof:provenanceInfo <file:///./dataset/Lab%20Content/COMP%206741/Lab%20Material/Lab%203.pdf>,
        <file:///./dataset/Lecture%20Content/COMP%206741/Lectures/slides01.pdf> .

<http://dbpedia.org/resource/Google_Nexus> a roboprof:Topic ;
    dbo:name "Nexus" ;
    roboprof:provenanceInfo <file:///./dataset/Lecture%20Content/COMP%206741/Lectures/slides03.pdf> .

<http://dbpedia.org/resource/Google_Search> a roboprof:Topic ;
    dbo:name "Google Search" ;
    roboprof:provenanceInfo <file:///./dataset/Lecture%20Content/COMP%206741/Lectures/slides01.pdf> .

<http://dbpedia.org/resource/Graphiq> a roboprof:Topic ;
    dbo:name "GraphIQ" ;
    roboprof:provenanceInfo <file:///./dataset/Lecture%20Content/COMP%206741/Lectures/slides02.pdf> .

<http://dbpedia.org/resource/Greenwich_Mean_Time> a roboprof:Topic ;
    dbo:name "GMT" ;
    roboprof:provenanceInfo <file:///./dataset/Lab%20Content/COMP%206461/Lab%20Material/Lab%201.pdf> .

<http://dbpedia.org/resource/Gzip> a roboprof:Topic ;
    dbo:name "gzip" ;
    roboprof:provenanceInfo <file:///./dataset/Lecture%20Content/COMP%206461/Lectures/2.ppt> .

<http://dbpedia.org/resource/HTTP_ETag> a roboprof:Topic ;
    dbo:name "ETag" ;
    roboprof:provenanceInfo <file:///./dataset/Lecture%20Content/COMP%206461/Lectures/2.ppt> .

<http://dbpedia.org/resource/Hanover> a roboprof:Topic ;
    dbo:name "Hanover" ;
    roboprof:provenanceInfo <file:///./dataset/Lecture%20Content/COMP%206741/Lectures/slides02.pdf> .

<http://dbpedia.org/resource/HarperCollins> a roboprof:Topic ;
    dbo:name "Harper Collins" ;
    roboprof:provenanceInfo <file:///./dataset/Lecture%20Content/COMP%206741/Lectures/slides02.pdf>,
        <file:///./dataset/Lecture%20Content/COMP%206741/Lectures/slides03.pdf> .

<http://dbpedia.org/resource/Heidelberg> a roboprof:Topic ;
    dbo:name "Heidelberg" ;
    roboprof:provenanceInfo <file:///./dataset/Lecture%20Content/COMP%206741/Lectures/slides02.pdf> .

<http://dbpedia.org/resource/High-test_peroxide> a roboprof:Topic ;
    dbo:name "HTP" ;
    roboprof:provenanceInfo <file:///./dataset/Lecture%20Content/COMP%206461/Lectures/2.ppt> .

<http://dbpedia.org/resource/High_frequency> a roboprof:Topic ;
    dbo:name "HF" ;
    roboprof:provenanceInfo <file:///./dataset/Lecture%20Content/COMP%206461/Readings/SelectiveRepeat.pdf> .

<http://dbpedia.org/resource/Hulu> a roboprof:Topic ;
    dbo:name "Hulu" ;
    roboprof:provenanceInfo <file:///./dataset/Lecture%20Content/COMP%206461/Lectures/2.ppt> .

<http://dbpedia.org/resource/Hypertext> a roboprof:Topic ;
    dbo:name "Hypertext" ;
    roboprof:provenanceInfo <file:///./dataset/Lecture%20Content/COMP%206461/OtherMaterial/ApplicationLayer.pdf> .

<http://dbpedia.org/resource/Hypertext_Transfer_Protocol> a roboprof:Topic ;
    dbo:name "HTTP",
        "HTTP GET",
        "HTTPS",
        "Hypertext Transfer Protocol",
        "RFC2616" ;
    roboprof:provenanceInfo <file:///./dataset/Lab%20Content/COMP%206461/Lab%20Material/Lab%201.pdf>,
        <file:///./dataset/Lab%20Content/COMP%206461/Lab%20Material/Lab%202.pdf>,
        <file:///./dataset/Lab%20Content/COMP%206461/Lab%20Material/Lab%203.pdf>,
        <file:///./dataset/Lecture%20Content/COMP%206461/Lectures/2.ppt>,
        <file:///./dataset/Lecture%20Content/COMP%206461/Lectures/3.ppt>,
        <file:///./dataset/Lecture%20Content/COMP%206461/OtherMaterial/ApplicationLayer.pdf>,
        <file:///./dataset/Lecture%20Content/COMP%206461/Worksheets/TA2.pdf>,
        <file:///./dataset/Lecture%20Content/COMP%206741/Lectures/slides04.pdf> .

<http://dbpedia.org/resource/IBM> a roboprof:Topic ;
    dbo:name "IBM" ;
    roboprof:provenanceInfo <file:///./dataset/Lecture%20Content/COMP%206741/Lectures/slides01.pdf> .

<http://dbpedia.org/resource/IBM_Systems_Network_Architecture> a roboprof:Topic ;
    dbo:name "SNA" ;
    roboprof:provenanceInfo <file:///./dataset/Lecture%20Content/COMP%206461/Lectures/6.ppt> .

<http://dbpedia.org/resource/ICANN> a roboprof:Topic ;
    dbo:name "ICANN" ;
    roboprof:provenanceInfo <file:///./dataset/Lecture%20Content/COMP%206461/Lectures/3.ppt> .

<http://dbpedia.org/resource/ING_Group> a roboprof:Topic ;
    dbo:name "ing" ;
    roboprof:provenanceInfo <file:///./dataset/Lecture%20Content/COMP%206461/Worksheets/TA1.pdf> .

<http://dbpedia.org/resource/IPTV> a roboprof:Topic ;
    dbo:name "IPTV" ;
    roboprof:provenanceInfo <file:///./dataset/Lecture%20Content/COMP%206461/Lectures/2.ppt>,
        <file:///./dataset/Lecture%20Content/COMP%206461/OtherMaterial/UDP.pdf> .

<http://dbpedia.org/resource/Informa> a roboprof:Topic ;
    dbo:name "informa" ;
    roboprof:provenanceInfo <file:///./dataset/Lecture%20Content/COMP%206741/OtherMaterial/TextMining.pdf> .

<http://dbpedia.org/resource/Information_extraction> a roboprof:Topic ;
    dbo:name "Information Extraction" ;
    roboprof:provenanceInfo <file:///./dataset/Lecture%20Content/COMP%206741/Lectures/slides01.pdf> .

<http://dbpedia.org/resource/Information_retrieval> a roboprof:Topic ;
    dbo:name "Information Retrieval" ;
    roboprof:provenanceInfo <file:///./dataset/Lecture%20Content/COMP%206741/Lectures/slides01.pdf>,
        <file:///./dataset/Lecture%20Content/COMP%206741/Lectures/slides05.pdf> .

<http://dbpedia.org/resource/Institute_of_Electrical_and_Electronics_Engineers> a roboprof:Topic ;
    dbo:name "IEEE" ;
    roboprof:provenanceInfo <file:///./dataset/Lecture%20Content/COMP%206461/Readings/SelectiveRepeat.pdf> .

<http://dbpedia.org/resource/Integrated_development_environment> a roboprof:Topic ;
    dbo:name "IDE" ;
    roboprof:provenanceInfo <file:///./dataset/Lab%20Content/COMP%206461/Lab%20Material/Lab%201.pdf> .

<http://dbpedia.org/resource/Intelligent_agent> a roboprof:Topic ;
    dbo:name "Intelligent Agent" ;
    roboprof:provenanceInfo <file:///./dataset/Lab%20Content/COMP%206741/Lab%20Material/Lab%203.pdf> .

<http://dbpedia.org/resource/International_Organization_for_Standardization> a roboprof:Topic ;
    dbo:name "ISO" ;
    roboprof:provenanceInfo <file:///./dataset/Lecture%20Content/COMP%206741/Lectures/slides03.pdf> .

<http://dbpedia.org/resource/International_Standard_Book_Number> a roboprof:Topic ;
    dbo:name "ISBN" ;
    roboprof:provenanceInfo <file:///./dataset/Lecture%20Content/COMP%206741/Lectures/slides02.pdf> .

<http://dbpedia.org/resource/Internationalized_Resource_Identifier> a roboprof:Topic ;
    dbo:name "IRI" ;
    roboprof:provenanceInfo <file:///./dataset/Lecture%20Content/COMP%206741/Lectures/slides03.pdf>,
        <file:///./dataset/Lecture%20Content/COMP%206741/Lectures/slides04.pdf> .

<http://dbpedia.org/resource/Internet> a roboprof:Topic ;
    dbo:name "Internet" ;
    roboprof:provenanceInfo <file:///./dataset/Lecture%20Content/COMP%206461/OtherMaterial/TCP.pdf>,
        <file:///./dataset/Lecture%20Content/COMP%206461/Readings/InternetProtocolSuite.pdf> .

<http://dbpedia.org/resource/Internet_Assigned_Numbers_Authority> a roboprof:Topic ;
    dbo:name "IANA" ;
    roboprof:provenanceInfo <file:///./dataset/Lecture%20Content/COMP%206461/OtherMaterial/UDP.pdf> .

<http://dbpedia.org/resource/Internet_Engineering_Task_Force> a roboprof:Topic ;
    dbo:name "IETF",
        "Internet Engineering Task Force" ;
    roboprof:provenanceInfo <file:///./dataset/Lecture%20Content/COMP%206461/Lectures/3.ppt>,
        <file:///./dataset/Lecture%20Content/COMP%206461/Readings/InternetProtocolSuite.pdf> .

<http://dbpedia.org/resource/Internet_Message_Access_Protocol> a roboprof:Topic ;
    dbo:name "IMAP",
        "IMAPS" ;
    roboprof:provenanceInfo <file:///./dataset/Lab%20Content/COMP%206461/Lab%20Material/Lab%201.pdf>,
        <file:///./dataset/Lecture%20Content/COMP%206461/Lectures/2.ppt> .

<http://dbpedia.org/resource/Internet_Relay_Chat> a roboprof:Topic ;
    dbo:name "IRC" ;
    roboprof:provenanceInfo <file:///./dataset/Lecture%20Content/COMP%206461/OtherMaterial/ApplicationLayer.pdf> .

<http://dbpedia.org/resource/Internet_Standard> a roboprof:Topic ;
    dbo:name "Internet Standard" ;
    roboprof:provenanceInfo <file:///./dataset/Lab%20Content/COMP%206461/Lab%20Material/Lab%201.pdf> .

<http://dbpedia.org/resource/Internet_service_provider> a roboprof:Topic ;
    dbo:name "ISP" ;
    roboprof:provenanceInfo <file:///./dataset/Lecture%20Content/COMP%206461/Lectures/2.ppt>,
        <file:///./dataset/Lecture%20Content/COMP%206461/Lectures/3.ppt> .

<http://dbpedia.org/resource/Ion> a roboprof:Topic ;
    dbo:name "cation" ;
    roboprof:provenanceInfo <file:///./dataset/Lecture%20Content/COMP%206741/Worksheets/worksheet05.pdf> .

<http://dbpedia.org/resource/Israel_Defense_Forces> a roboprof:Topic ;
    dbo:name "idf" ;
    roboprof:provenanceInfo <file:///./dataset/Lecture%20Content/COMP%206741/Lectures/slides05.pdf>,
        <file:///./dataset/Lecture%20Content/COMP%206741/Worksheets/worksheet04.pdf> .

<http://dbpedia.org/resource/Israeli_new_shekel> a roboprof:Topic ;
    dbo:name "nis" ;
    roboprof:provenanceInfo <file:///./dataset/Lecture%20Content/COMP%206741/Lectures/slides06.pdf> .

<http://dbpedia.org/resource/JPEG> a roboprof:Topic ;
    dbo:name "JPEG" ;
    roboprof:provenanceInfo <file:///./dataset/Lecture%20Content/COMP%206461/Lectures/2.ppt> .

<http://dbpedia.org/resource/JSON> a roboprof:Topic ;
    dbo:name "Json" ;
    roboprof:provenanceInfo <file:///./dataset/Lecture%20Content/COMP%206741/Lectures/slides03.pdf> .

<http://dbpedia.org/resource/Jabberwacky> a roboprof:Topic ;
    dbo:name "Jabberwacky" ;
    roboprof:provenanceInfo <file:///./dataset/Lecture%20Content/COMP%206741/Readings/NLP.pdf> .

<http://dbpedia.org/resource/James_Pustejovsky> a roboprof:Topic ;
    dbo:name "James Pustejovsky" ;
    roboprof:provenanceInfo <file:///./dataset/Lecture%20Content/COMP%206741/Lectures/slides06.pdf> .

<http://dbpedia.org/resource/Java_virtual_machine> a roboprof:Topic ;
    dbo:name "Java" ;
    roboprof:provenanceInfo <file:///./dataset/Lab%20Content/COMP%206461/Lab%20Material/Lab%201.pdf>,
        <file:///./dataset/Lab%20Content/COMP%206741/Lab%20Material/Lab%202.pdf> .

<http://dbpedia.org/resource/Jim_Kurose> a roboprof:Topic ;
    dbo:name "Jim Kurose" ;
    roboprof:provenanceInfo <file:///./dataset/Lecture%20Content/COMP%206461/Lectures/2.ppt>,
        <file:///./dataset/Lecture%20Content/COMP%206461/Lectures/3.ppt>,
        <file:///./dataset/Lecture%20Content/COMP%206461/Lectures/4.ppt>,
        <file:///./dataset/Lecture%20Content/COMP%206461/Lectures/5.ppt>,
        <file:///./dataset/Lecture%20Content/COMP%206461/Lectures/6.ppt> .

<http://dbpedia.org/resource/John_Berryman> a roboprof:Topic ;
    dbo:name "John Berryman" ;
    roboprof:provenanceInfo <file:///./dataset/Lecture%20Content/COMP%206741/Lectures/slides05.pdf> .

<http://dbpedia.org/resource/John_Lennon> a roboprof:Topic ;
    dbo:name "Lennon" ;
    roboprof:provenanceInfo <file:///./dataset/Lecture%20Content/COMP%206741/Lectures/slides02.pdf> .

<http://dbpedia.org/resource/John_Searle> a roboprof:Topic ;
    dbo:name "John Searle" ;
    roboprof:provenanceInfo <file:///./dataset/Lecture%20Content/COMP%206741/Readings/IntelligentAgent.pdf>,
        <file:///./dataset/Lecture%20Content/COMP%206741/Readings/NLP.pdf> .

<http://dbpedia.org/resource/Joseph_Weizenbaum> a roboprof:Topic ;
    dbo:name "Weizenbaum" ;
    roboprof:provenanceInfo <file:///./dataset/Lecture%20Content/COMP%206741/Lectures/slides01.pdf> .

<http://dbpedia.org/resource/K-nearest_neighbors_algorithm> a roboprof:Topic ;
    dbo:name "kNN" ;
    roboprof:provenanceInfo <file:///./dataset/Lecture%20Content/COMP%206741/Lectures/slides06.pdf>,
        <file:///./dataset/Lecture%20Content/COMP%206741/Worksheets/worksheet05.pdf> .

<http://dbpedia.org/resource/Kaiser_Permanente> a roboprof:Topic ;
    dbo:name "Kaiser" ;
    roboprof:provenanceInfo <file:///./dataset/Lecture%20Content/COMP%206741/Lectures/slides01.pdf> .

<http://dbpedia.org/resource/Kankan> a roboprof:Topic ;
    dbo:name "KanKan" ;
    roboprof:provenanceInfo <file:///./dataset/Lecture%20Content/COMP%206461/Lectures/3.ppt> .

<http://dbpedia.org/resource/Karyotype> a roboprof:Topic ;
    dbo:name "FN" ;
    roboprof:provenanceInfo <file:///./dataset/Lecture%20Content/COMP%206741/Lectures/slides06.pdf> .

<http://dbpedia.org/resource/King_Arthur> a roboprof:Topic ;
    dbo:name "Arthur" ;
    roboprof:provenanceInfo <file:///./dataset/Lecture%20Content/COMP%206741/Lectures/slides06.pdf> .

<http://dbpedia.org/resource/Knowledge_Graph> a roboprof:Topic ;
    dbo:name "Knowledge Graph",
        "Knowledge Vault" ;
    roboprof:provenanceInfo <file:///./dataset/Lab%20Content/COMP%206741/Lab%20Material/Lab%203.pdf>,
        <file:///./dataset/Lecture%20Content/COMP%206741/Lectures/slides02.pdf>,
        <file:///./dataset/Lecture%20Content/COMP%206741/Readings/KnowledgeGraph.pdf> .

<http://dbpedia.org/resource/Knowledge_representation_and_reasoning> a roboprof:Topic ;
    dbo:name "Knowledge Representation" ;
    roboprof:provenanceInfo <file:///./dataset/Lecture%20Content/COMP%206741/Lectures/slides02.pdf> .

<http://dbpedia.org/resource/Knowledge_worker> a roboprof:Topic ;
    dbo:name "Knowledge Worker" ;
    roboprof:provenanceInfo <file:///./dataset/Lecture%20Content/COMP%206741/Lectures/slides01.pdf> .

<http://dbpedia.org/resource/La_Paz> a roboprof:Topic ;
    dbo:name "La Paz" ;
    roboprof:provenanceInfo <file:///./dataset/Lecture%20Content/COMP%206741/Lectures/slides01.pdf> .

<http://dbpedia.org/resource/Last.fm> a roboprof:Topic ;
    dbo:name "Last.fm" ;
    roboprof:provenanceInfo <file:///./dataset/Lecture%20Content/COMP%206741/Lectures/slides05.pdf>,
        <file:///./dataset/Lecture%20Content/COMP%206741/Readings/RecommenderSystem.pdf> .

<http://dbpedia.org/resource/Layer_cake> a roboprof:Topic ;
    dbo:name "Layer Cake" ;
    roboprof:provenanceInfo <file:///./dataset/Lecture%20Content/COMP%206741/Lectures/slides01.pdf>,
        <file:///./dataset/Lecture%20Content/COMP%206741/Lectures/slides02.pdf>,
        <file:///./dataset/Lecture%20Content/COMP%206741/Lectures/slides03.pdf> .

<http://dbpedia.org/resource/Le_Palais> a roboprof:Topic ;
    dbo:name "Le Palais" ;
    roboprof:provenanceInfo <file:///./dataset/Lecture%20Content/COMP%206741/Lectures/slides02.pdf>,
        <file:///./dataset/Lecture%20Content/COMP%206741/Lectures/slides03.pdf> .

<http://dbpedia.org/resource/Leonardo_da_Vinci> a roboprof:Topic ;
    dbo:name "Leonardo da Vinci" ;
    roboprof:provenanceInfo <file:///./dataset/Lecture%20Content/COMP%206741/Lectures/slides02.pdf> .

<http://dbpedia.org/resource/Lesk_algorithm> a roboprof:Topic ;
    dbo:name "Lesk algorithm" ;
    roboprof:provenanceInfo <file:///./dataset/Lecture%20Content/COMP%206741/Readings/NLP.pdf> .

<http://dbpedia.org/resource/Lightweight_Directory_Access_Protocol> a roboprof:Topic ;
    dbo:name "LDAP" ;
    roboprof:provenanceInfo <file:///./dataset/Lab%20Content/COMP%206461/Lab%20Material/Lab%201.pdf> .

<http://dbpedia.org/resource/Linguistic_Linked_Open_Data> a roboprof:Topic ;
    dbo:name "Linguistic Linked Open Data" ;
    roboprof:provenanceInfo <file:///./dataset/Lecture%20Content/COMP%206741/OtherMaterial/LinguisticLinkedOpenData.pdf> .

<http://dbpedia.org/resource/LinkedIn> a roboprof:Topic ;
    dbo:name "LinkedIn" ;
    roboprof:provenanceInfo <file:///./dataset/Lecture%20Content/COMP%206741/Readings/KnowledgeGraph.pdf>,
        <file:///./dataset/Lecture%20Content/COMP%206741/Worksheets/worksheet01.pdf> .

<http://dbpedia.org/resource/Linked_data> a roboprof:Topic ;
    dbo:name "Linked Data",
        "Linked Open Data" ;
    roboprof:provenanceInfo <file:///./dataset/Lecture%20Content/COMP%206741/Lectures/slides01.pdf>,
        <file:///./dataset/Lecture%20Content/COMP%206741/Lectures/slides03.pdf>,
        <file:///./dataset/Lecture%20Content/COMP%206741/Lectures/slides04.pdf>,
        <file:///./dataset/Lecture%20Content/COMP%206741/OtherMaterial/LinguisticLinkedOpenData.pdf>,
        <file:///./dataset/Lecture%20Content/COMP%206741/Readings/KnowledgeGraph.pdf>,
        <file:///./dataset/Lecture%20Content/COMP%206741/Worksheets/worksheet03.pdf> .

<http://dbpedia.org/resource/Linus_Torvalds> a roboprof:Topic ;
    dbo:name "Linus Torvalds" ;
    roboprof:provenanceInfo <file:///./dataset/Lab%20Content/COMP%206461/Lab%20Material/Lab%201.pdf> .

<http://dbpedia.org/resource/Linux> a roboprof:Topic ;
    dbo:name "Linux" ;
    roboprof:provenanceInfo <file:///./dataset/Lab%20Content/COMP%206461/Lab%20Material/Lab%201.pdf> .

<http://dbpedia.org/resource/Lio> a roboprof:Topic ;
    dbo:name "lio" ;
    roboprof:provenanceInfo <file:///./dataset/Lecture%20Content/COMP%206741/Lectures/slides02.pdf> .

<http://dbpedia.org/resource/Liyang> a roboprof:Topic ;
    dbo:name "Liyang" ;
    roboprof:provenanceInfo <file:///./dataset/Lecture%20Content/COMP%206741/Lectures/slides02.pdf>,
        <file:///./dataset/Lecture%20Content/COMP%206741/Lectures/slides03.pdf> .

<http://dbpedia.org/resource/Logic> a roboprof:Topic ;
    dbo:name "Logic" ;
    roboprof:provenanceInfo <file:///./dataset/Lecture%20Content/COMP%206741/Lectures/slides02.pdf> .

<http://dbpedia.org/resource/MIME> a roboprof:Topic ;
    dbo:name "MIME" ;
    roboprof:provenanceInfo <file:///./dataset/Lecture%20Content/COMP%206461/Lectures/2.ppt> .

<http://dbpedia.org/resource/MOS_Technology_TED> a roboprof:Topic ;
    dbo:name "TED" ;
    roboprof:provenanceInfo <file:///./dataset/Lecture%20Content/COMP%206741/Lectures/slides02.pdf>,
        <file:///./dataset/Lecture%20Content/COMP%206741/Lectures/slides03.pdf> .

<http://dbpedia.org/resource/MacOS> a roboprof:Topic ;
    dbo:name "MacOS" ;
    roboprof:provenanceInfo <file:///./dataset/Lab%20Content/COMP%206461/Lab%20Material/Lab%201.pdf>,
        <file:///./dataset/Lab%20Content/COMP%206461/Lab%20Material/Lab%203.pdf> .

<http://dbpedia.org/resource/Macbeth> a roboprof:Topic ;
    dbo:name "Macbeth" ;
    roboprof:provenanceInfo <file:///./dataset/Lecture%20Content/COMP%206741/Lectures/slides05.pdf> .

<http://dbpedia.org/resource/Machine_learning> a roboprof:Topic ;
    dbo:name "ML",
        "Machine Learning" ;
    roboprof:provenanceInfo <file:///./dataset/Lab%20Content/COMP%206741/Lab%20Material/Lab%202.pdf>,
        <file:///./dataset/Lecture%20Content/COMP%206741/Lectures/slides01.pdf>,
        <file:///./dataset/Lecture%20Content/COMP%206741/Lectures/slides06.pdf>,
        <file:///./dataset/Lecture%20Content/COMP%206741/OtherMaterial/MachineLearning.pdf>,
        <file:///./dataset/Lecture%20Content/COMP%206741/Worksheets/worksheet05.pdf> .

<http://dbpedia.org/resource/Main_Page> a roboprof:Topic ;
    dbo:name "Concordia University" ;
    roboprof:provenanceInfo <file:///./dataset/Lab%20Content/COMP%206741/Lab%20Material/Lab%202.pdf>,
        <file:///./dataset/Lab%20Content/COMP%206741/Lab%20Material/Lab%203.pdf>,
        <file:///./dataset/Lecture%20Content/COMP%206461/Lectures/2.ppt>,
        <file:///./dataset/Lecture%20Content/COMP%206461/Lectures/3.ppt>,
        <file:///./dataset/Lecture%20Content/COMP%206461/Lectures/4.ppt>,
        <file:///./dataset/Lecture%20Content/COMP%206461/Lectures/5.ppt>,
        <file:///./dataset/Lecture%20Content/COMP%206461/Lectures/6.ppt>,
        <file:///./dataset/Lecture%20Content/COMP%206741/Lectures/slides01.pdf>,
        <file:///./dataset/Lecture%20Content/COMP%206741/Lectures/slides02.pdf>,
        <file:///./dataset/Lecture%20Content/COMP%206741/Lectures/slides03.pdf>,
        <file:///./dataset/Lecture%20Content/COMP%206741/Lectures/slides05.pdf>,
        <file:///./dataset/Lecture%20Content/COMP%206741/Lectures/slides06.pdf>,
        <file:///./dataset/Lecture%20Content/COMP%206741/Worksheets/worksheet01.pdf> .

<http://dbpedia.org/resource/Manning_Publications> a roboprof:Topic ;
    dbo:name "Manning Publications" ;
    roboprof:provenanceInfo <file:///./dataset/Lecture%20Content/COMP%206741/Lectures/slides01.pdf>,
        <file:///./dataset/Lecture%20Content/COMP%206741/Lectures/slides03.pdf>,
        <file:///./dataset/Lecture%20Content/COMP%206741/Lectures/slides04.pdf>,
        <file:///./dataset/Lecture%20Content/COMP%206741/Lectures/slides05.pdf> .

<http://dbpedia.org/resource/Master_of_Laws> a roboprof:Topic ;
    dbo:name "LLM" ;
    roboprof:provenanceInfo <file:///./dataset/Lecture%20Content/COMP%206741/Lectures/slides02.pdf> .

<http://dbpedia.org/resource/Maximum_transmission_unit> a roboprof:Topic ;
    dbo:name "MTU" ;
    roboprof:provenanceInfo <file:///./dataset/Lecture%20Content/COMP%206461/OtherMaterial/ComputerNetwork.pdf>,
        <file:///./dataset/Lecture%20Content/COMP%206461/OtherMaterial/NetworkLayer.pdf> .

<http://dbpedia.org/resource/Metadata> a roboprof:Topic ;
    dbo:name "Metadata",
        "metadata" ;
    roboprof:provenanceInfo <file:///./dataset/Lecture%20Content/COMP%206741/Lectures/slides05.pdf> .

<http://dbpedia.org/resource/Metafiction> a roboprof:Topic ;
    dbo:name "Metafiction" ;
    roboprof:provenanceInfo <file:///./dataset/Lecture%20Content/COMP%206741/Lectures/slides03.pdf> .

<http://dbpedia.org/resource/Metaweb> a roboprof:Topic ;
    dbo:name "Metaweb" ;
    roboprof:provenanceInfo <file:///./dataset/Lecture%20Content/COMP%206741/Lectures/slides04.pdf> .

<http://dbpedia.org/resource/Microdata_Corporation> a roboprof:Topic ;
    dbo:name "Microdata" ;
    roboprof:provenanceInfo <file:///./dataset/Lecture%20Content/COMP%206741/Readings/KnowledgeGraph.pdf> .

<http://dbpedia.org/resource/Microsoft> a roboprof:Topic ;
    dbo:name "Microsoft" ;
    roboprof:provenanceInfo <file:///./dataset/Lecture%20Content/COMP%206741/Lectures/slides01.pdf> .

<http://dbpedia.org/resource/Microsoft_Windows> a roboprof:Topic ;
    dbo:name "Windows" ;
    roboprof:provenanceInfo <file:///./dataset/Lab%20Content/COMP%206461/Lab%20Material/Lab%201.pdf> .

<http://dbpedia.org/resource/Miroirs> a roboprof:Topic ;
    dbo:name "miroirs" ;
    roboprof:provenanceInfo <file:///./dataset/Lecture%20Content/COMP%206741/Lectures/slides02.pdf>,
        <file:///./dataset/Lecture%20Content/COMP%206741/Lectures/slides03.pdf> .

<http://dbpedia.org/resource/Mona_Lisa> a roboprof:Topic ;
    dbo:name "Mona Lisa" ;
    roboprof:provenanceInfo <file:///./dataset/Lecture%20Content/COMP%206741/Lectures/slides01.pdf>,
        <file:///./dataset/Lecture%20Content/COMP%206741/Lectures/slides02.pdf> .

<http://dbpedia.org/resource/Montreal> a roboprof:Topic ;
    dbo:name "Montreal" ;
    roboprof:provenanceInfo <file:///./dataset/Lecture%20Content/COMP%206461/Lectures/2.ppt> .

<http://dbpedia.org/resource/Moodle> a roboprof:Topic ;
    dbo:name "Moodle" ;
    roboprof:provenanceInfo <file:///./dataset/Lab%20Content/COMP%206461/Lab%20Material/Lab%201.pdf>,
        <file:///./dataset/Lab%20Content/COMP%206461/Lab%20Material/Lab%202.pdf>,
        <file:///./dataset/Lab%20Content/COMP%206461/Lab%20Material/Lab%203.pdf> .

<http://dbpedia.org/resource/Mozilla_Thunderbird> a roboprof:Topic ;
    dbo:name "Thunderbird" ;
    roboprof:provenanceInfo <file:///./dataset/Lecture%20Content/COMP%206461/Lectures/2.ppt> .

<http://dbpedia.org/resource/Multimedia_Messaging_Service> a roboprof:Topic ;
    dbo:name "MMS" ;
    roboprof:provenanceInfo <file:///./dataset/Lecture%20Content/COMP%206461/OtherMaterial/ApplicationLayer.pdf> .

<http://dbpedia.org/resource/Museum_of_the_Rockies> a roboprof:Topic ;
    dbo:name "mor" ;
    roboprof:provenanceInfo <file:///./dataset/Lecture%20Content/COMP%206741/Readings/KnowledgeGraph.pdf> .

<http://dbpedia.org/resource/MusicBrainz> a roboprof:Topic ;
    dbo:name "MusicBrainz" ;
    roboprof:provenanceInfo <file:///./dataset/Lecture%20Content/COMP%206741/Lectures/slides04.pdf> .

<http://dbpedia.org/resource/Music_Genome_Project> a roboprof:Topic ;
    dbo:name "Music Genome Project" ;
    roboprof:provenanceInfo <file:///./dataset/Lecture%20Content/COMP%206741/Readings/RecommenderSystem.pdf> .

<http://dbpedia.org/resource/NAKS> a roboprof:Topic ;
    dbo:name "NAKs" ;
    roboprof:provenanceInfo <file:///./dataset/Lecture%20Content/COMP%206461/Lectures/4.ppt> .

<http://dbpedia.org/resource/NASA> a roboprof:Topic ;
    dbo:name "NASA" ;
    roboprof:provenanceInfo <file:///./dataset/Lecture%20Content/COMP%206461/Lectures/3.ppt> .

<http://dbpedia.org/resource/NCR_CRAM> a roboprof:Topic ;
    dbo:name "CRAM" ;
    roboprof:provenanceInfo <file:///./dataset/Lab%20Content/COMP%206461/Lab%20Material/Lab%201.pdf> .

<http://dbpedia.org/resource/NT_LAN_Manager> a roboprof:Topic ;
    dbo:name "NTLM" ;
    roboprof:provenanceInfo <file:///./dataset/Lab%20Content/COMP%206461/Lab%20Material/Lab%201.pdf> .

<http://dbpedia.org/resource/Naive_Bayes_classifier> a roboprof:Topic ;
    dbo:name "Nave Bayes" ;
    roboprof:provenanceInfo <file:///./dataset/Lecture%20Content/COMP%206741/Lectures/slides06.pdf> .

<http://dbpedia.org/resource/National_Cancer_Institute> a roboprof:Topic ;
    dbo:name "National Cancer Institute" ;
    roboprof:provenanceInfo <file:///./dataset/Lecture%20Content/COMP%206741/Lectures/slides04.pdf> .

<http://dbpedia.org/resource/National_Science_Foundation> a roboprof:Topic ;
    dbo:name "NSF" ;
    roboprof:provenanceInfo <file:///./dataset/Lecture%20Content/COMP%206741/Lectures/slides06.pdf> .

<http://dbpedia.org/resource/National_Science_Foundation_Network> a roboprof:Topic ;
    dbo:name "NSFNET" ;
    roboprof:provenanceInfo <file:///./dataset/Lecture%20Content/COMP%206461/Readings/NetworkCongestion.pdf> .

<http://dbpedia.org/resource/Natural_language_processing> a roboprof:Topic ;
    dbo:name "NLP",
        "Natural Language Processing" ;
    roboprof:provenanceInfo <file:///./dataset/Lecture%20Content/COMP%206741/Lectures/slides01.pdf>,
        <file:///./dataset/Lecture%20Content/COMP%206741/Lectures/slides04.pdf>,
        <file:///./dataset/Lecture%20Content/COMP%206741/OtherMaterial/TextMining.pdf>,
        <file:///./dataset/Lecture%20Content/COMP%206741/OtherMaterial/WordEmbeddings.pdf>,
        <file:///./dataset/Lecture%20Content/COMP%206741/Readings/NLP.pdf> .

<http://dbpedia.org/resource/Neo4j> a roboprof:Topic ;
    dbo:name "Neo4j" ;
    roboprof:provenanceInfo <file:///./dataset/Lecture%20Content/COMP%206741/Lectures/slides02.pdf> .

<http://dbpedia.org/resource/Netflix> a roboprof:Topic ;
    dbo:name "Netflix" ;
    roboprof:provenanceInfo <file:///./dataset/Lecture%20Content/COMP%206461/Lectures/2.ppt> .

<http://dbpedia.org/resource/Network_Control_Program> a roboprof:Topic ;
    dbo:name "Network Control Program" ;
    roboprof:provenanceInfo <file:///./dataset/Lecture%20Content/COMP%206461/Readings/InternetProtocolSuite.pdf> .

<http://dbpedia.org/resource/Network_File_System> a roboprof:Topic ;
    dbo:name "Network File System" ;
    roboprof:provenanceInfo <file:///./dataset/Lecture%20Content/COMP%206461/OtherMaterial/UDP.pdf> .

<http://dbpedia.org/resource/Network_Solutions> a roboprof:Topic ;
    dbo:name "Network Solutions" ;
    roboprof:provenanceInfo <file:///./dataset/Lecture%20Content/COMP%206461/Lectures/3.ppt> .

<http://dbpedia.org/resource/Network_Time_Protocol> a roboprof:Topic ;
    dbo:name "NTP",
        "Network Time Protocol" ;
    roboprof:provenanceInfo <file:///./dataset/Lab%20Content/COMP%206461/Lab%20Material/Lab%201.pdf>,
        <file:///./dataset/Lecture%20Content/COMP%206461/OtherMaterial/UDP.pdf> .

<http://dbpedia.org/resource/Network_packet> a roboprof:Topic ;
    dbo:name "packet" ;
    roboprof:provenanceInfo <file:///./dataset/Lecture%20Content/COMP%206461/Lectures/5.ppt> .

<http://dbpedia.org/resource/New_Jersey> a roboprof:Topic ;
    dbo:name "New Jersey" ;
    roboprof:provenanceInfo <file:///./dataset/Lecture%20Content/COMP%206461/Readings/SelectiveRepeat.pdf> .

<http://dbpedia.org/resource/Newline> a roboprof:Topic ;
    dbo:name "lf" ;
    roboprof:provenanceInfo <file:///./dataset/Lecture%20Content/COMP%206461/Lectures/2.ppt> .

<http://dbpedia.org/resource/Noam_Chomsky> a roboprof:Topic ;
    dbo:name "Chomskyan" ;
    roboprof:provenanceInfo <file:///./dataset/Lecture%20Content/COMP%206741/Readings/NLP.pdf> .

<http://dbpedia.org/resource/Notation3> a roboprof:Topic ;
    dbo:name "N3" ;
    roboprof:provenanceInfo <file:///./dataset/Lecture%20Content/COMP%206741/Lectures/slides02.pdf>,
        <file:///./dataset/Lecture%20Content/COMP%206741/Lectures/slides03.pdf>,
        <file:///./dataset/Lecture%20Content/COMP%206741/Worksheets/worksheet02.pdf> .

<http://dbpedia.org/resource/OBO_Foundry> a roboprof:Topic ;
    dbo:name "Open Biomedical Ontologies Foundry" ;
    roboprof:provenanceInfo <file:///./dataset/Lecture%20Content/COMP%206741/Lectures/slides04.pdf> .

<http://dbpedia.org/resource/OSI_model> a roboprof:Topic ;
    dbo:name "OSI",
        "Open Systems Interconnection" ;
    roboprof:provenanceInfo <file:///./dataset/Lab%20Content/COMP%206461/Lab%20Material/Lab%201.pdf>,
        <file:///./dataset/Lecture%20Content/COMP%206461/OtherMaterial/ApplicationLayer.pdf>,
        <file:///./dataset/Lecture%20Content/COMP%206461/OtherMaterial/NetworkLayer.pdf> .

<http://dbpedia.org/resource/Ontology> a roboprof:Topic ;
    dbo:name "Ontology" ;
    roboprof:provenanceInfo <file:///./dataset/Lab%20Content/COMP%206741/Lab%20Material/Lab%203.pdf>,
        <file:///./dataset/Lecture%20Content/COMP%206741/Lectures/slides01.pdf> .

<http://dbpedia.org/resource/OpenAI> a roboprof:Topic ;
    dbo:name "OpenAI" ;
    roboprof:provenanceInfo <file:///./dataset/Lecture%20Content/COMP%206741/Lectures/slides01.pdf> .

<http://dbpedia.org/resource/Open_Mind_Common_Sense> a roboprof:Topic ;
    dbo:name "ConceptNet" ;
    roboprof:provenanceInfo <file:///./dataset/Lecture%20Content/COMP%206741/Lectures/slides02.pdf> .

<http://dbpedia.org/resource/Open_data> a roboprof:Topic ;
    dbo:name "Open Data" ;
    roboprof:provenanceInfo <file:///./dataset/Lecture%20Content/COMP%206741/Lectures/slides04.pdf> .

<http://dbpedia.org/resource/Operating_system> a roboprof:Topic ;
    dbo:name "OS" ;
    roboprof:provenanceInfo <file:///./dataset/Lecture%20Content/COMP%206461/Lectures/2.ppt> .

<http://dbpedia.org/resource/Oracle_Spatial_and_Graph> a roboprof:Topic ;
    dbo:name "Oracle Spatial" ;
    roboprof:provenanceInfo <file:///./dataset/Lecture%20Content/COMP%206741/Lectures/slides02.pdf> .

<http://dbpedia.org/resource/Outlier> a roboprof:Topic ;
    dbo:name "Outliers" ;
    roboprof:provenanceInfo <file:///./dataset/Lecture%20Content/COMP%206741/Lectures/slides06.pdf> .

<http://dbpedia.org/resource/Outlook.com> a roboprof:Topic ;
    dbo:name "Hotmail" ;
    roboprof:provenanceInfo <file:///./dataset/Lecture%20Content/COMP%206461/Lectures/2.ppt> .

<http://dbpedia.org/resource/Ovid> a roboprof:Topic ;
    dbo:name "Ovid" ;
    roboprof:provenanceInfo <file:///./dataset/Lecture%20Content/COMP%206741/Lectures/slides01.pdf> .

<http://dbpedia.org/resource/PHP> a roboprof:Topic ;
    dbo:name "PHP" ;
    roboprof:provenanceInfo <file:///./dataset/Lecture%20Content/COMP%206741/Lectures/slides02.pdf> .

<http://dbpedia.org/resource/POWER7> a roboprof:Topic ;
    dbo:name "POWER7" ;
    roboprof:provenanceInfo <file:///./dataset/Lecture%20Content/COMP%206741/Lectures/slides01.pdf> .

<http://dbpedia.org/resource/Pandora_Radio> a roboprof:Topic ;
    dbo:name "Pandora",
        "Pandora Radio" ;
    roboprof:provenanceInfo <file:///./dataset/Lecture%20Content/COMP%206741/Readings/RecommenderSystem.pdf> .

<http://dbpedia.org/resource/Paris> a roboprof:Topic ;
    dbo:name "Paris" ;
    roboprof:provenanceInfo <file:///./dataset/Lecture%20Content/COMP%206461/Lectures/2.ppt> .

<http://dbpedia.org/resource/Peer-to-peer> a roboprof:Topic ;
    dbo:name "P2P" ;
    roboprof:provenanceInfo <file:///./dataset/Lecture%20Content/COMP%206461/Lectures/2.ppt>,
        <file:///./dataset/Lecture%20Content/COMP%206461/Lectures/3.ppt> .

<http://dbpedia.org/resource/Perceptron> a roboprof:Topic ;
    dbo:name "Perceptrons" ;
    roboprof:provenanceInfo <file:///./dataset/Lecture%20Content/COMP%206741/Lectures/slides02.pdf> .

<http://dbpedia.org/resource/Personalization> a roboprof:Topic ;
    dbo:name "Personalization" ;
    roboprof:provenanceInfo <file:///./dataset/Lecture%20Content/COMP%206741/Lectures/slides05.pdf> .

<http://dbpedia.org/resource/Poems_by_Edgar_Allan_Poe> a roboprof:Topic ;
    dbo:name "Alone" ;
    roboprof:provenanceInfo <file:///./dataset/Lecture%20Content/COMP%206741/Lectures/slides02.pdf> .

<http://dbpedia.org/resource/Post_Office_Protocol> a roboprof:Topic ;
    dbo:name "POP",
        "POP3",
        "Post Office Protocol" ;
    roboprof:provenanceInfo <file:///./dataset/Lab%20Content/COMP%206461/Lab%20Material/Lab%201.pdf>,
        <file:///./dataset/Lecture%20Content/COMP%206461/Lectures/2.ppt> .

<http://dbpedia.org/resource/Power-on_self-test> a roboprof:Topic ;
    dbo:name "POST" ;
    roboprof:provenanceInfo <file:///./dataset/Lab%20Content/COMP%206461/Lab%20Material/Lab%201.pdf>,
        <file:///./dataset/Lab%20Content/COMP%206461/Lab%20Material/Lab%202.pdf>,
        <file:///./dataset/Lab%20Content/COMP%206461/Lab%20Material/Lab%203.pdf>,
        <file:///./dataset/Lecture%20Content/COMP%206461/Lectures/2.ppt> .

<http://dbpedia.org/resource/Prabhakar_Raghavan> a roboprof:Topic ;
    dbo:name "Prabhakar Raghavan" ;
    roboprof:provenanceInfo <file:///./dataset/Lecture%20Content/COMP%206741/Lectures/slides05.pdf> .

<http://dbpedia.org/resource/Precision_Time_Protocol> a roboprof:Topic ;
    dbo:name "Precision Time Protocol" ;
    roboprof:provenanceInfo <file:///./dataset/Lecture%20Content/COMP%206461/OtherMaterial/UDP.pdf> .

<http://dbpedia.org/resource/Prentice_Hall> a roboprof:Topic ;
    dbo:name "Prentice Hall" ;
    roboprof:provenanceInfo <file:///./dataset/Lecture%20Content/COMP%206461/Readings/SelectiveRepeat.pdf> .

<http://dbpedia.org/resource/Psychotherapy> a roboprof:Topic ;
    dbo:name "psychotherapist" ;
    roboprof:provenanceInfo <file:///./dataset/Lecture%20Content/COMP%206741/Lectures/slides01.pdf> .

<http://dbpedia.org/resource/QUIC> a roboprof:Topic ;
    dbo:name "QUIC" ;
    roboprof:provenanceInfo <file:///./dataset/Lecture%20Content/COMP%206461/OtherMaterial/UDP.pdf> .

<http://dbpedia.org/resource/RDF_Schema> a roboprof:Topic ;
    dbo:name "RDF Schema",
        "RDF schema",
        "RDFS",
        "rdfs" ;
    roboprof:provenanceInfo <file:///./dataset/Lab%20Content/COMP%206741/Lab%20Material/Lab%202.pdf>,
        <file:///./dataset/Lab%20Content/COMP%206741/Lab%20Material/Lab%203.pdf>,
        <file:///./dataset/Lecture%20Content/COMP%206741/Lectures/slides02.pdf>,
        <file:///./dataset/Lecture%20Content/COMP%206741/Lectures/slides03.pdf>,
        <file:///./dataset/Lecture%20Content/COMP%206741/Lectures/slides04.pdf>,
        <file:///./dataset/Lecture%20Content/COMP%206741/Lectures/slides06.pdf> .

<http://dbpedia.org/resource/RDF_query_language> a roboprof:Topic ;
    dbo:name "RDF Query Language" ;
    roboprof:provenanceInfo <file:///./dataset/Lecture%20Content/COMP%206741/Readings/SPARQL.pdf> .

<http://dbpedia.org/resource/RDFa> a roboprof:Topic ;
    dbo:name "RDFa" ;
    roboprof:provenanceInfo <file:///./dataset/Lecture%20Content/COMP%206741/Lectures/slides02.pdf>,
        <file:///./dataset/Lecture%20Content/COMP%206741/Lectures/slides03.pdf> .

<http://dbpedia.org/resource/RELA> a roboprof:Topic ;
    dbo:name "rela" ;
    roboprof:provenanceInfo <file:///./dataset/Lecture%20Content/COMP%206741/Lectures/slides02.pdf> .

<http://dbpedia.org/resource/RIPE> a roboprof:Topic ;
    dbo:name "RIPE" ;
    roboprof:provenanceInfo <file:///./dataset/Lecture%20Content/COMP%206461/Lectures/3.ppt> .

<http://dbpedia.org/resource/Racter> a roboprof:Topic ;
    dbo:name "Racter" ;
    roboprof:provenanceInfo <file:///./dataset/Lecture%20Content/COMP%206741/Readings/NLP.pdf> .

<http://dbpedia.org/resource/Raphael_Weldon> a roboprof:Topic ;
    dbo:name "Weldon" ;
    roboprof:provenanceInfo <file:///./dataset/Lecture%20Content/COMP%206461/Readings/SelectiveRepeat.pdf> .

<http://dbpedia.org/resource/Raytheon> a roboprof:Topic ;
    dbo:name "Raytheon Company" ;
    roboprof:provenanceInfo <file:///./dataset/Lecture%20Content/COMP%206741/OtherMaterial/MachineLearning.pdf> .

<http://dbpedia.org/resource/Reading> a roboprof:Topic ;
    dbo:name "Reading" ;
    roboprof:provenanceInfo <file:///./dataset/Lecture%20Content/COMP%206741/Lectures/slides01.pdf>,
        <file:///./dataset/Lecture%20Content/COMP%206741/Lectures/slides02.pdf>,
        <file:///./dataset/Lecture%20Content/COMP%206741/Lectures/slides03.pdf>,
        <file:///./dataset/Lecture%20Content/COMP%206741/Lectures/slides05.pdf>,
        <file:///./dataset/Lecture%20Content/COMP%206741/Lectures/slides06.pdf> .

<http://dbpedia.org/resource/Real-Time_Messaging_Protocol> a roboprof:Topic ;
    dbo:name "RTMP" ;
    roboprof:provenanceInfo <file:///./dataset/Lab%20Content/COMP%206461/Lab%20Material/Lab%201.pdf> .

<http://dbpedia.org/resource/Real-time_Transport_Protocol> a roboprof:Topic ;
    dbo:name "RTP" ;
    roboprof:provenanceInfo <file:///./dataset/Lecture%20Content/COMP%206461/OtherMaterial/TCP.pdf> .

<http://dbpedia.org/resource/Real_Time_Streaming_Protocol> a roboprof:Topic ;
    dbo:name "RTSP" ;
    roboprof:provenanceInfo <file:///./dataset/Lab%20Content/COMP%206461/Lab%20Material/Lab%201.pdf> .

<http://dbpedia.org/resource/Recommender_system> a roboprof:Topic ;
    dbo:name "Recommender Systems" ;
    roboprof:provenanceInfo <file:///./dataset/Lecture%20Content/COMP%206741/Lectures/slides01.pdf>,
        <file:///./dataset/Lecture%20Content/COMP%206741/Lectures/slides05.pdf>,
        <file:///./dataset/Lecture%20Content/COMP%206741/Worksheets/worksheet04.pdf> .

<http://dbpedia.org/resource/Regional_rail> a roboprof:Topic ;
    dbo:name "ter" ;
    roboprof:provenanceInfo <file:///./dataset/Lecture%20Content/COMP%206461/OtherMaterial/ComputerNetwork.pdf> .

<http://dbpedia.org/resource/Reinforcement_learning> a roboprof:Topic ;
    dbo:name "Reinforcement Learning" ;
    roboprof:provenanceInfo <file:///./dataset/Lecture%20Content/COMP%206741/Lectures/slides06.pdf> .

<http://dbpedia.org/resource/Remote_Database_Access> a roboprof:Topic ;
    dbo:name "Remote Database Access" ;
    roboprof:provenanceInfo <file:///./dataset/Lecture%20Content/COMP%206461/OtherMaterial/ApplicationLayer.pdf> .

<http://dbpedia.org/resource/Resource_Description_Framework> a roboprof:Topic ;
    dbo:name "RDF",
        "Resource Description Framework",
        "rdf" ;
    roboprof:provenanceInfo <file:///./dataset/Lab%20Content/COMP%206741/Lab%20Material/Lab%202.pdf>,
        <file:///./dataset/Lab%20Content/COMP%206741/Lab%20Material/Lab%203.pdf>,
        <file:///./dataset/Lecture%20Content/COMP%206741/Lectures/slides02.pdf>,
        <file:///./dataset/Lecture%20Content/COMP%206741/Lectures/slides03.pdf>,
        <file:///./dataset/Lecture%20Content/COMP%206741/Lectures/slides04.pdf>,
        <file:///./dataset/Lecture%20Content/COMP%206741/OtherMaterial/LinguisticLinkedOpenData.pdf>,
        <file:///./dataset/Lecture%20Content/COMP%206741/Readings/SPARQL.pdf>,
        <file:///./dataset/Lecture%20Content/COMP%206741/Worksheets/worksheet01.pdf>,
        <file:///./dataset/Lecture%20Content/COMP%206741/Worksheets/worksheet02.pdf> .

<http://dbpedia.org/resource/Rhetorical_structure_theory> a roboprof:Topic ;
    dbo:name "Rhetorical Structure Theory" ;
    roboprof:provenanceInfo <file:///./dataset/Lecture%20Content/COMP%206741/Readings/NLP.pdf> .

<http://dbpedia.org/resource/Roadgeek> a roboprof:Topic ;
    dbo:name "SABRE" ;
    roboprof:provenanceInfo <file:///./dataset/Lecture%20Content/COMP%206461/OtherMaterial/ComputerNetwork.pdf> .

<http://dbpedia.org/resource/Ross_Geller> a roboprof:Topic ;
    dbo:name "Ross" ;
    roboprof:provenanceInfo <file:///./dataset/Lecture%20Content/COMP%206461/Lectures/2.ppt>,
        <file:///./dataset/Lecture%20Content/COMP%206461/Lectures/6.ppt> .

<http://dbpedia.org/resource/Routing_Information_Protocol> a roboprof:Topic ;
    dbo:name "Routing Information Protocol" ;
    roboprof:provenanceInfo <file:///./dataset/Lecture%20Content/COMP%206461/OtherMaterial/UDP.pdf> .

<http://dbpedia.org/resource/Rup_dialects> a roboprof:Topic ;
    dbo:name "Rup" ;
    roboprof:provenanceInfo <file:///./dataset/Lecture%20Content/COMP%206741/OtherMaterial/WordEmbeddings.pdf> .

<http://dbpedia.org/resource/SHRDLU> a roboprof:Topic ;
    dbo:name "SHRDLU" ;
    roboprof:provenanceInfo <file:///./dataset/Lecture%20Content/COMP%206741/Lectures/slides02.pdf> .

<http://dbpedia.org/resource/SOAP> a roboprof:Topic ;
    dbo:name "SOAP" ;
    roboprof:provenanceInfo <file:///./dataset/Lecture%20Content/COMP%206741/Lectures/slides04.pdf> .

<http://dbpedia.org/resource/SPARQL> a roboprof:Topic ;
    dbo:name "SPARQL" ;
    roboprof:provenanceInfo <file:///./dataset/Lab%20Content/COMP%206741/Lab%20Material/Lab%203.pdf>,
        <file:///./dataset/Lecture%20Content/COMP%206741/Lectures/slides02.pdf>,
        <file:///./dataset/Lecture%20Content/COMP%206741/Lectures/slides04.pdf>,
        <file:///./dataset/Lecture%20Content/COMP%206741/Readings/SPARQL.pdf> .

<http://dbpedia.org/resource/SQL> a roboprof:Topic ;
    dbo:name "SQL" ;
    roboprof:provenanceInfo <file:///./dataset/Lecture%20Content/COMP%206741/Readings/SPARQL.pdf> .

<http://dbpedia.org/resource/Safari> a roboprof:Topic ;
    dbo:name "Safari" ;
    roboprof:provenanceInfo <file:///./dataset/Lecture%20Content/COMP%206461/Lectures/2.ppt> .

<http://dbpedia.org/resource/Sameer_(lyricist)> a roboprof:Topic ;
    dbo:name "Sameer" ;
    roboprof:provenanceInfo <file:///./dataset/Lecture%20Content/COMP%206741/Lectures/slides02.pdf> .

<http://dbpedia.org/resource/Satori> a roboprof:Topic ;
    dbo:name "Satori" ;
    roboprof:provenanceInfo <file:///./dataset/Lecture%20Content/COMP%206741/Lectures/slides02.pdf>,
        <file:///./dataset/Lecture%20Content/COMP%206741/Readings/KnowledgeGraph.pdf> .

<http://dbpedia.org/resource/Scale-invariant_feature_transform> a roboprof:Topic ;
    dbo:name "SIFT" ;
    roboprof:provenanceInfo <file:///./dataset/Lecture%20Content/COMP%206741/OtherMaterial/BagOfWords.pdf> .

<http://dbpedia.org/resource/Schema.org> a roboprof:Topic ;
    dbo:name "Schema.org",
        "schema.org" ;
    roboprof:provenanceInfo <file:///./dataset/Lecture%20Content/COMP%206741/Lectures/slides02.pdf>,
        <file:///./dataset/Lecture%20Content/COMP%206741/Lectures/slides03.pdf> .

<http://dbpedia.org/resource/Searing> a roboprof:Topic ;
    dbo:name "sear" ;
    roboprof:provenanceInfo <file:///./dataset/Lecture%20Content/COMP%206741/Lectures/slides02.pdf> .

<http://dbpedia.org/resource/Secure_Shell> a roboprof:Topic ;
    dbo:name "Secure Shell" ;
    roboprof:provenanceInfo <file:///./dataset/Lecture%20Content/COMP%206461/OtherMaterial/ApplicationLayer.pdf>,
        <file:///./dataset/Lecture%20Content/COMP%206461/OtherMaterial/TCP.pdf> .

<http://dbpedia.org/resource/Selective_Repeat_ARQ> a roboprof:Topic ;
    dbo:name "Selective Repeat",
        "Selective Repeat ARQ" ;
    roboprof:provenanceInfo <file:///./dataset/Lab%20Content/COMP%206461/Lab%20Material/Lab%203.pdf>,
        <file:///./dataset/Lecture%20Content/COMP%206461/Lectures/5.ppt>,
        <file:///./dataset/Lecture%20Content/COMP%206461/Lectures/6.ppt>,
        <file:///./dataset/Lecture%20Content/COMP%206461/Readings/GoBackN.pdf>,
        <file:///./dataset/Lecture%20Content/COMP%206461/Readings/SelectiveRepeat.pdf> .

<http://dbpedia.org/resource/Semantic_Web> a roboprof:Topic ;
    dbo:name "Semantic Web" ;
    roboprof:provenanceInfo <file:///./dataset/Lecture%20Content/COMP%206741/Lectures/slides02.pdf>,
        <file:///./dataset/Lecture%20Content/COMP%206741/Lectures/slides03.pdf>,
        <file:///./dataset/Lecture%20Content/COMP%206741/Lectures/slides04.pdf>,
        <file:///./dataset/Lecture%20Content/COMP%206741/Readings/KnowledgeGraph.pdf> .

<http://dbpedia.org/resource/Semantic_network> a roboprof:Topic ;
    dbo:name "Semantic Networks" ;
    roboprof:provenanceInfo <file:///./dataset/Lecture%20Content/COMP%206741/Lectures/slides02.pdf> .

<http://dbpedia.org/resource/Semantic_triple> a roboprof:Topic ;
    dbo:name "RDF Triple" ;
    roboprof:provenanceInfo <file:///./dataset/Lecture%20Content/COMP%206741/Lectures/slides03.pdf> .

<http://dbpedia.org/resource/Semantics> a roboprof:Topic ;
    dbo:name "Semantics" ;
    roboprof:provenanceInfo <file:///./dataset/Lecture%20Content/COMP%206461/Lectures/2.ppt>,
        <file:///./dataset/Lecture%20Content/COMP%206741/Lectures/slides03.pdf> .

<http://dbpedia.org/resource/Semi-Automatic_Ground_Environment> a roboprof:Topic ;
    dbo:name "SAGE" ;
    roboprof:provenanceInfo <file:///./dataset/Lecture%20Content/COMP%206461/OtherMaterial/ComputerNetwork.pdf> .

<http://dbpedia.org/resource/Sentiment_analysis> a roboprof:Topic ;
    dbo:name "Sentiment Analysis" ;
    roboprof:provenanceInfo <file:///./dataset/Lecture%20Content/COMP%206741/Lectures/slides01.pdf> .

<http://dbpedia.org/resource/Serialization> a roboprof:Topic ;
    dbo:name "Serialization" ;
    roboprof:provenanceInfo <file:///./dataset/Lecture%20Content/COMP%206741/Lectures/slides02.pdf>,
        <file:///./dataset/Lecture%20Content/COMP%206741/Lectures/slides04.pdf> .

<http://dbpedia.org/resource/Server_Message_Block> a roboprof:Topic ;
    dbo:name "SMB" ;
    roboprof:provenanceInfo <file:///./dataset/Lab%20Content/COMP%206461/Lab%20Material/Lab%201.pdf> .

<http://dbpedia.org/resource/Shay_locomotive> a roboprof:Topic ;
    dbo:name "Shay" ;
    roboprof:provenanceInfo <file:///./dataset/Lecture%20Content/COMP%206461/Lectures/2.ppt>,
        <file:///./dataset/Lecture%20Content/COMP%206461/Lectures/3.ppt>,
        <file:///./dataset/Lecture%20Content/COMP%206461/Lectures/4.ppt>,
        <file:///./dataset/Lecture%20Content/COMP%206461/Lectures/5.ppt>,
        <file:///./dataset/Lecture%20Content/COMP%206461/Lectures/6.ppt> .

<http://dbpedia.org/resource/Simple_Knowledge_Organization_System> a roboprof:Topic ;
    dbo:name "SKOS" ;
    roboprof:provenanceInfo <file:///./dataset/Lecture%20Content/COMP%206741/Lectures/slides02.pdf>,
        <file:///./dataset/Lecture%20Content/COMP%206741/Lectures/slides03.pdf> .

<http://dbpedia.org/resource/Simple_Mail_Transfer_Protocol> a roboprof:Topic ;
    dbo:name "HELO",
        "SMTP",
        "Simple Mail Transfer Protocol" ;
    roboprof:provenanceInfo <file:///./dataset/Lab%20Content/COMP%206461/Lab%20Material/Lab%201.pdf>,
        <file:///./dataset/Lecture%20Content/COMP%206461/Lectures/2.ppt>,
        <file:///./dataset/Lecture%20Content/COMP%206461/OtherMaterial/ApplicationLayer.pdf>,
        <file:///./dataset/Lecture%20Content/COMP%206461/Worksheets/TA2.pdf> .

<http://dbpedia.org/resource/Simple_Network_Management_Protocol> a roboprof:Topic ;
    dbo:name "SNMP",
        "Simple Network Management Protocol" ;
    roboprof:provenanceInfo <file:///./dataset/Lecture%20Content/COMP%206461/Lectures/4.ppt>,
        <file:///./dataset/Lecture%20Content/COMP%206461/OtherMaterial/ApplicationLayer.pdf> .

<http://dbpedia.org/resource/Siri> a roboprof:Topic ;
    dbo:name "Siri" ;
    roboprof:provenanceInfo <file:///./dataset/Lab%20Content/COMP%206741/Lab%20Material/Lab%203.pdf>,
        <file:///./dataset/Lecture%20Content/COMP%206741/Readings/KnowledgeGraph.pdf> .

<http://dbpedia.org/resource/Skype> a roboprof:Topic ;
    dbo:name "Skype" ;
    roboprof:provenanceInfo <file:///./dataset/Lecture%20Content/COMP%206461/Lectures/2.ppt> .

<http://dbpedia.org/resource/Sliding_window_protocol> a roboprof:Topic ;
    dbo:name "Sliding Window Protocol" ;
    roboprof:provenanceInfo <file:///./dataset/Lecture%20Content/COMP%206461/Lectures/5.ppt> .

<http://dbpedia.org/resource/Software_engineering> a roboprof:Topic ;
    dbo:name "Software Engineering" ;
    roboprof:provenanceInfo <file:///./dataset/Lecture%20Content/COMP%206461/Lectures/2.ppt>,
        <file:///./dataset/Lecture%20Content/COMP%206461/Lectures/3.ppt>,
        <file:///./dataset/Lecture%20Content/COMP%206461/Lectures/4.ppt>,
        <file:///./dataset/Lecture%20Content/COMP%206461/Lectures/5.ppt>,
        <file:///./dataset/Lecture%20Content/COMP%206461/Lectures/6.ppt>,
        <file:///./dataset/Lecture%20Content/COMP%206741/Lectures/slides01.pdf>,
        <file:///./dataset/Lecture%20Content/COMP%206741/Lectures/slides02.pdf>,
        <file:///./dataset/Lecture%20Content/COMP%206741/Lectures/slides03.pdf>,
        <file:///./dataset/Lecture%20Content/COMP%206741/Lectures/slides04.pdf>,
        <file:///./dataset/Lecture%20Content/COMP%206741/Lectures/slides05.pdf>,
        <file:///./dataset/Lecture%20Content/COMP%206741/Lectures/slides06.pdf> .

<http://dbpedia.org/resource/South_Korea> a roboprof:Topic ;
    dbo:name "KR" ;
    roboprof:provenanceInfo <file:///./dataset/Lecture%20Content/COMP%206741/Lectures/slides02.pdf> .

<http://dbpedia.org/resource/Springer_Nature> a roboprof:Topic ;
    dbo:name "Springer International Publishing" ;
    roboprof:provenanceInfo <file:///./dataset/Lecture%20Content/COMP%206741/Lectures/slides04.pdf> .

<http://dbpedia.org/resource/Standardization_Agreement> a roboprof:Topic ;
    dbo:name "STANAG" ;
    roboprof:provenanceInfo <file:///./dataset/Lecture%20Content/COMP%206461/Readings/SelectiveRepeat.pdf> .

<http://dbpedia.org/resource/Steve_Crocker> a roboprof:Topic ;
    dbo:name "Steve Crocker" ;
    roboprof:provenanceInfo <file:///./dataset/Lecture%20Content/COMP%206461/Readings/InternetProtocolSuite.pdf> .

<http://dbpedia.org/resource/Steve_Jobs> a roboprof:Topic ;
    dbo:name "Steve Jobs" ;
    roboprof:provenanceInfo <file:///./dataset/Lecture%20Content/COMP%206741/Lectures/slides01.pdf> .

<http://dbpedia.org/resource/Stevedore> a roboprof:Topic ;
    dbo:name "Docker" ;
    roboprof:provenanceInfo <file:///./dataset/Lab%20Content/COMP%206461/Lab%20Material/Lab%201.pdf> .

<http://dbpedia.org/resource/Straitjacket_Fits> a roboprof:Topic ;
    dbo:name "David Wood" ;
    roboprof:provenanceInfo <file:///./dataset/Lecture%20Content/COMP%206741/Lectures/slides03.pdf> .

<http://dbpedia.org/resource/Stream_Control_Transmission_Protocol> a roboprof:Topic ;
    dbo:name "SCTP",
        "Stream Control Transmission Protocol" ;
    roboprof:provenanceInfo <file:///./dataset/Lecture%20Content/COMP%206461/OtherMaterial/UDP.pdf> .

<http://dbpedia.org/resource/Sun_Microsystems> a roboprof:Topic ;
    dbo:name "Sun" ;
    roboprof:provenanceInfo <file:///./dataset/Lecture%20Content/COMP%206461/Lectures/2.ppt> .

<http://dbpedia.org/resource/TCP_congestion_control> a roboprof:Topic ;
    dbo:name "TCP RENO",
        "TCP Slow Start" ;
    roboprof:provenanceInfo <file:///./dataset/Lecture%20Content/COMP%206461/Lectures/6.ppt> .

<http://dbpedia.org/resource/TaleSpin> a roboprof:Topic ;
    dbo:name "TaleSpin" ;
    roboprof:provenanceInfo <file:///./dataset/Lecture%20Content/COMP%206741/Readings/NLP.pdf> .

<http://dbpedia.org/resource/Telnet> a roboprof:Topic ;
    dbo:name "Telnet",
        "telnet" ;
    roboprof:provenanceInfo <file:///./dataset/Lab%20Content/COMP%206461/Lab%20Material/Lab%201.pdf>,
        <file:///./dataset/Lab%20Content/COMP%206461/Lab%20Material/Lab%202.pdf>,
        <file:///./dataset/Lecture%20Content/COMP%206461/Lectures/2.ppt>,
        <file:///./dataset/Lecture%20Content/COMP%206461/Lectures/6.ppt>,
        <file:///./dataset/Lecture%20Content/COMP%206461/OtherMaterial/ApplicationLayer.pdf> .

<http://dbpedia.org/resource/Terry_Winograd> a roboprof:Topic ;
    dbo:name "Winograd" ;
    roboprof:provenanceInfo <file:///./dataset/Lecture%20Content/COMP%206741/Lectures/slides02.pdf> .

<http://dbpedia.org/resource/Text_mining> a roboprof:Topic ;
    dbo:name "Text Mining" ;
    roboprof:provenanceInfo <file:///./dataset/Lecture%20Content/COMP%206741/Lectures/slides01.pdf> .

<http://dbpedia.org/resource/The_Tempest> a roboprof:Topic ;
    dbo:name "Tempest" ;
    roboprof:provenanceInfo <file:///./dataset/Lecture%20Content/COMP%206741/Lectures/slides05.pdf> .

<http://dbpedia.org/resource/The_World_Factbook> a roboprof:Topic ;
    dbo:name "CIA World Factbook" ;
    roboprof:provenanceInfo <file:///./dataset/Lecture%20Content/COMP%206741/Readings/KnowledgeGraph.pdf> .

<http://dbpedia.org/resource/Time-division_multiplexing> a roboprof:Topic ;
    dbo:name "TDM" ;
    roboprof:provenanceInfo <file:///./dataset/Lecture%20Content/COMP%206741/OtherMaterial/TextMining.pdf> .

<http://dbpedia.org/resource/Time_to_live> a roboprof:Topic ;
    dbo:name "TTL" ;
    roboprof:provenanceInfo <file:///./dataset/Lecture%20Content/COMP%206461/Lectures/3.ppt> .

<http://dbpedia.org/resource/Token_ring> a roboprof:Topic ;
    dbo:name "Token Ring" ;
    roboprof:provenanceInfo <file:///./dataset/Lecture%20Content/COMP%206461/Worksheets/TA3.pdf> .

<http://dbpedia.org/resource/Top-level_domain> a roboprof:Topic ;
    dbo:name "TLD" ;
    roboprof:provenanceInfo <file:///./dataset/Lecture%20Content/COMP%206461/Lectures/3.ppt> .

<http://dbpedia.org/resource/Traceroute> a roboprof:Topic ;
    dbo:name "Traceroute" ;
    roboprof:provenanceInfo <file:///./dataset/Lecture%20Content/COMP%206461/Worksheets/TA1.pdf> .

<http://dbpedia.org/resource/Transmission_Control_Protocol> a roboprof:Topic ;
    dbo:name "ACK",
        "TCP",
        "Transmission Control Protocol" ;
    roboprof:provenanceInfo <file:///./dataset/Lab%20Content/COMP%206461/Lab%20Material/Lab%201.pdf>,
        <file:///./dataset/Lab%20Content/COMP%206461/Lab%20Material/Lab%203.pdf>,
        <file:///./dataset/Lecture%20Content/COMP%206461/Lectures/2.ppt>,
        <file:///./dataset/Lecture%20Content/COMP%206461/Lectures/4.ppt>,
        <file:///./dataset/Lecture%20Content/COMP%206461/Lectures/5.ppt>,
        <file:///./dataset/Lecture%20Content/COMP%206461/Lectures/6.ppt>,
        <file:///./dataset/Lecture%20Content/COMP%206461/OtherMaterial/TCP.pdf>,
        <file:///./dataset/Lecture%20Content/COMP%206461/OtherMaterial/UDP.pdf>,
        <file:///./dataset/Lecture%20Content/COMP%206461/Readings/GoBackN.pdf>,
        <file:///./dataset/Lecture%20Content/COMP%206461/Readings/InternetProtocolSuite.pdf>,
        <file:///./dataset/Lecture%20Content/COMP%206461/Readings/SelectiveRepeat.pdf>,
        <file:///./dataset/Lecture%20Content/COMP%206461/Worksheets/TA2.pdf> .

<http://dbpedia.org/resource/Transport_Layer_Security> a roboprof:Topic ;
    dbo:name "SSL" ;
    roboprof:provenanceInfo <file:///./dataset/Lab%20Content/COMP%206461/Lab%20Material/Lab%201.pdf>,
        <file:///./dataset/Lecture%20Content/COMP%206461/Lectures/2.ppt> .

<http://dbpedia.org/resource/Trigonometric_functions> a roboprof:Topic ;
    dbo:name "Cosine" ;
    roboprof:provenanceInfo <file:///./dataset/Lecture%20Content/COMP%206741/Lectures/slides05.pdf> .

<http://dbpedia.org/resource/Trivial_File_Transfer_Protocol> a roboprof:Topic ;
    dbo:name "TFTP",
        "Trivial File Transfer Protocol" ;
    roboprof:provenanceInfo <file:///./dataset/Lab%20Content/COMP%206461/Lab%20Material/Lab%201.pdf>,
        <file:///./dataset/Lecture%20Content/COMP%206461/OtherMaterial/ApplicationLayer.pdf>,
        <file:///./dataset/Lecture%20Content/COMP%206461/OtherMaterial/UDP.pdf> .

<http://dbpedia.org/resource/Turing_Award> a roboprof:Topic ;
    dbo:name "Turing Award" ;
    roboprof:provenanceInfo <file:///./dataset/Lecture%20Content/COMP%206461/OtherMaterial/TCP.pdf> .

<http://dbpedia.org/resource/UIMA> a roboprof:Topic ;
    dbo:name "UIMA" ;
    roboprof:provenanceInfo <file:///./dataset/Lecture%20Content/COMP%206741/Lectures/slides01.pdf> .

<http://dbpedia.org/resource/URL> a roboprof:Topic ;
    dbo:name "URL",
        "Uniform Resource Locator" ;
    roboprof:provenanceInfo <file:///./dataset/Lab%20Content/COMP%206461/Lab%20Material/Lab%201.pdf>,
        <file:///./dataset/Lecture%20Content/COMP%206461/Lectures/2.ppt>,
        <file:///./dataset/Lecture%20Content/COMP%206741/Lectures/slides03.pdf> .

<http://dbpedia.org/resource/Uber> a roboprof:Topic ;
    dbo:name "Uber" ;
    roboprof:provenanceInfo <file:///./dataset/Lecture%20Content/COMP%206741/Readings/KnowledgeGraph.pdf> .

<http://dbpedia.org/resource/UniProt> a roboprof:Topic ;
    dbo:name "UniProt" ;
    roboprof:provenanceInfo <file:///./dataset/Lecture%20Content/COMP%206741/Lectures/slides04.pdf> .

<http://dbpedia.org/resource/Uniform_Resource_Identifier> a roboprof:Topic ;
    dbo:name "URI" ;
    roboprof:provenanceInfo <file:///./dataset/Lab%20Content/COMP%206741/Lab%20Material/Lab%202.pdf>,
        <file:///./dataset/Lab%20Content/COMP%206741/Lab%20Material/Lab%203.pdf>,
        <file:///./dataset/Lecture%20Content/COMP%206741/Lectures/slides02.pdf>,
        <file:///./dataset/Lecture%20Content/COMP%206741/Lectures/slides03.pdf>,
        <file:///./dataset/Lecture%20Content/COMP%206741/Lectures/slides04.pdf>,
        <file:///./dataset/Lecture%20Content/COMP%206741/OtherMaterial/LinguisticLinkedOpenData.pdf>,
        <file:///./dataset/Lecture%20Content/COMP%206741/Worksheets/worksheet01.pdf>,
        <file:///./dataset/Lecture%20Content/COMP%206741/Worksheets/worksheet03.pdf> .

<http://dbpedia.org/resource/United_States_Army_Research_Laboratory> a roboprof:Topic ;
    dbo:name "ARL" ;
    roboprof:provenanceInfo <file:///./dataset/Lecture%20Content/COMP%206461/Lectures/3.ppt> .

<http://dbpedia.org/resource/United_States_Department_of_Defense> a roboprof:Topic ;
    dbo:name "US DoD" ;
    roboprof:provenanceInfo <file:///./dataset/Lecture%20Content/COMP%206461/Lectures/3.ppt> .

<http://dbpedia.org/resource/University_of_Manchester> a roboprof:Topic ;
    dbo:name "msec" ;
    roboprof:provenanceInfo <file:///./dataset/Lecture%20Content/COMP%206461/Lectures/2.ppt>,
        <file:///./dataset/Lecture%20Content/COMP%206461/Lectures/5.ppt> .

<http://dbpedia.org/resource/Unix> a roboprof:Topic ;
    dbo:name "UNIX" ;
    roboprof:provenanceInfo <file:///./dataset/Lab%20Content/COMP%206461/Lab%20Material/Lab%202.pdf> .

<http://dbpedia.org/resource/Unsupervised_learning> a roboprof:Topic ;
    dbo:name "Unsupervised" ;
    roboprof:provenanceInfo <file:///./dataset/Lecture%20Content/COMP%206741/Lectures/slides06.pdf> .

<http://dbpedia.org/resource/Urban_area> a roboprof:Topic ;
    dbo:name "UA" ;
    roboprof:provenanceInfo <file:///./dataset/Lecture%20Content/COMP%206461/Lectures/2.ppt> .

<http://dbpedia.org/resource/User_Datagram_Protocol> a roboprof:Topic ;
    dbo:name "UDP",
        "User Datagram Protocol" ;
    roboprof:provenanceInfo <file:///./dataset/Lab%20Content/COMP%206461/Lab%20Material/Lab%201.pdf>,
        <file:///./dataset/Lab%20Content/COMP%206461/Lab%20Material/Lab%203.pdf>,
        <file:///./dataset/Lecture%20Content/COMP%206461/Lectures/2.ppt>,
        <file:///./dataset/Lecture%20Content/COMP%206461/Lectures/4.ppt>,
        <file:///./dataset/Lecture%20Content/COMP%206461/Lectures/6.ppt>,
        <file:///./dataset/Lecture%20Content/COMP%206461/OtherMaterial/TCP.pdf>,
        <file:///./dataset/Lecture%20Content/COMP%206461/OtherMaterial/UDP.pdf>,
        <file:///./dataset/Lecture%20Content/COMP%206461/Readings/InternetProtocolSuite.pdf>,
        <file:///./dataset/Lecture%20Content/COMP%206461/Readings/SelectiveRepeat.pdf>,
        <file:///./dataset/Lecture%20Content/COMP%206461/Worksheets/TA2.pdf> .

<http://dbpedia.org/resource/User_modeling> a roboprof:Topic ;
    dbo:name "User Modeling" ;
    roboprof:provenanceInfo <file:///./dataset/Lecture%20Content/COMP%206741/Lectures/slides05.pdf> .

<http://dbpedia.org/resource/VVV-Venlo> a roboprof:Topic ;
    dbo:name "vvv" ;
    roboprof:provenanceInfo <file:///./dataset/Lecture%20Content/COMP%206741/Lectures/slides03.pdf> .

<http://dbpedia.org/resource/Van_Jacobson> a roboprof:Topic ;
    dbo:name "Van Jacobson" ;
    roboprof:provenanceInfo <file:///./dataset/Lecture%20Content/COMP%206461/Readings/NetworkCongestion.pdf> .

<http://dbpedia.org/resource/Vector_space_model> a roboprof:Topic ;
    dbo:name "Vector Space Model" ;
    roboprof:provenanceInfo <file:///./dataset/Lecture%20Content/COMP%206741/Lectures/slides05.pdf>,
        <file:///./dataset/Lecture%20Content/COMP%206741/Lectures/slides06.pdf> .

<http://dbpedia.org/resource/Verbosity> a roboprof:Topic ;
    dbo:name "Verbosity" ;
    roboprof:provenanceInfo <file:///./dataset/Lab%20Content/COMP%206461/Lab%20Material/Lab%201.pdf> .

<http://dbpedia.org/resource/Vint_Cerf> a roboprof:Topic ;
    dbo:name "Vint Cerf",
        "Vinton Cerf" ;
    roboprof:provenanceInfo <file:///./dataset/Lecture%20Content/COMP%206461/OtherMaterial/TCP.pdf>,
        <file:///./dataset/Lecture%20Content/COMP%206461/Readings/InternetProtocolSuite.pdf> .

<http://dbpedia.org/resource/VirtualBox> a roboprof:Topic ;
    dbo:name "VirtualBox" ;
    roboprof:provenanceInfo <file:///./dataset/Lab%20Content/COMP%206461/Lab%20Material/Lab%201.pdf> .

<http://dbpedia.org/resource/Voltaire> a roboprof:Topic ;
    dbo:name "Voltaire" ;
    roboprof:provenanceInfo <file:///./dataset/Lecture%20Content/COMP%206741/Lectures/slides06.pdf> .

<http://dbpedia.org/resource/Walter_Pitts> a roboprof:Topic ;
    dbo:name "Walter Pitts" ;
    roboprof:provenanceInfo <file:///./dataset/Lecture%20Content/COMP%206741/OtherMaterial/MachineLearning.pdf> .

<http://dbpedia.org/resource/Warren_Sturgis_McCulloch> a roboprof:Topic ;
    dbo:name "McCulloch",
        "Warren McCulloch" ;
    roboprof:provenanceInfo <file:///./dataset/Lecture%20Content/COMP%206741/Lectures/slides02.pdf>,
        <file:///./dataset/Lecture%20Content/COMP%206741/OtherMaterial/MachineLearning.pdf> .

<http://dbpedia.org/resource/Web_Ontology_Language> a roboprof:Topic ;
    dbo:name "OWL",
        "OWL DL",
        "OWL2",
        "Web Ontology Language" ;
    roboprof:provenanceInfo <file:///./dataset/Lab%20Content/COMP%206741/Lab%20Material/Lab%203.pdf>,
        <file:///./dataset/Lecture%20Content/COMP%206741/Lectures/slides02.pdf>,
        <file:///./dataset/Lecture%20Content/COMP%206741/Lectures/slides04.pdf> .

<http://dbpedia.org/resource/Web_cache> a roboprof:Topic ;
    dbo:name "cache" ;
    roboprof:provenanceInfo <file:///./dataset/Lecture%20Content/COMP%206461/Lectures/2.ppt> .

<http://dbpedia.org/resource/Web_server> a roboprof:Topic ;
    dbo:name "server" ;
    roboprof:provenanceInfo <file:///./dataset/Lab%20Content/COMP%206461/Lab%20Material/Lab%203.pdf>,
        <file:///./dataset/Lecture%20Content/COMP%206461/Lectures/2.ppt> .

<http://dbpedia.org/resource/Webmail> a roboprof:Topic ;
    dbo:name "Webmail" ;
    roboprof:provenanceInfo <file:///./dataset/Lecture%20Content/COMP%206461/Lectures/2.ppt> .

<http://dbpedia.org/resource/Wikidata> a roboprof:Topic ;
    dbo:name "Wikidata" ;
    roboprof:provenanceInfo <file:///./dataset/Lab%20Content/COMP%206741/Lab%20Material/Lab%202.pdf>,
        <file:///./dataset/Lab%20Content/COMP%206741/Lab%20Material/Lab%203.pdf>,
        <file:///./dataset/Lecture%20Content/COMP%206741/Lectures/slides02.pdf>,
        <file:///./dataset/Lecture%20Content/COMP%206741/Lectures/slides04.pdf>,
        <file:///./dataset/Lecture%20Content/COMP%206741/Readings/KnowledgeGraph.pdf>,
        <file:///./dataset/Lecture%20Content/COMP%206741/Worksheets/worksheet01.pdf>,
        <file:///./dataset/Lecture%20Content/COMP%206741/Worksheets/worksheet03.pdf> .

<http://dbpedia.org/resource/Wikipedia> a roboprof:Topic ;
    dbo:name "Wikipedia" ;
    roboprof:provenanceInfo <file:///./dataset/Lecture%20Content/COMP%206741/Lectures/slides02.pdf>,
        <file:///./dataset/Lecture%20Content/COMP%206741/OtherMaterial/TextMining.pdf>,
        <file:///./dataset/Lecture%20Content/COMP%206741/Readings/KnowledgeGraph.pdf> .

<http://dbpedia.org/resource/Wireshark> a roboprof:Topic ;
    dbo:name "Wireshark" ;
    roboprof:provenanceInfo <file:///./dataset/Lab%20Content/COMP%206461/Lab%20Material/Lab%201.pdf> .

<http://dbpedia.org/resource/Wolfram_Alpha> a roboprof:Topic ;
    dbo:name "WolframAlpha" ;
    roboprof:provenanceInfo <file:///./dataset/Lecture%20Content/COMP%206741/Readings/KnowledgeGraph.pdf> .

<http://dbpedia.org/resource/WordNet> a roboprof:Topic ;
    dbo:name "Wordnet" ;
    roboprof:provenanceInfo <file:///./dataset/Lecture%20Content/COMP%206741/Readings/KnowledgeGraph.pdf> .

<http://dbpedia.org/resource/WordPress.com> a roboprof:Topic ;
    dbo:name "Wordpress.com" ;
    roboprof:provenanceInfo <file:///./dataset/Lecture%20Content/COMP%206741/Lectures/slides04.pdf> .

<http://dbpedia.org/resource/World_Wide_Web> a roboprof:Topic ;
    dbo:name "WWW" ;
    roboprof:provenanceInfo <file:///./dataset/Lecture%20Content/COMP%206461/OtherMaterial/TCP.pdf>,
        <file:///./dataset/Lecture%20Content/COMP%206741/Lectures/slides02.pdf> .

<http://dbpedia.org/resource/World_Wide_Web_Consortium> a roboprof:Topic ;
    dbo:name "W3C",
        "W3C Recommendation",
        "World Wide Web Consortium" ;
    roboprof:provenanceInfo <file:///./dataset/Lecture%20Content/COMP%206741/Lectures/slides01.pdf>,
        <file:///./dataset/Lecture%20Content/COMP%206741/Lectures/slides02.pdf>,
        <file:///./dataset/Lecture%20Content/COMP%206741/Lectures/slides03.pdf>,
        <file:///./dataset/Lecture%20Content/COMP%206741/Lectures/slides04.pdf>,
        <file:///./dataset/Lecture%20Content/COMP%206741/Readings/SPARQL.pdf> .

<http://dbpedia.org/resource/X86> a roboprof:Topic ;
    dbo:name "DL" ;
    roboprof:provenanceInfo <file:///./dataset/Lecture%20Content/COMP%206741/Lectures/slides06.pdf> .

<http://dbpedia.org/resource/XHTML> a roboprof:Topic ;
    dbo:name "XHTML" ;
    roboprof:provenanceInfo <file:///./dataset/Lecture%20Content/COMP%206741/Lectures/slides04.pdf> .

<http://dbpedia.org/resource/XQuery> a roboprof:Topic ;
    dbo:name "XQuery" ;
    roboprof:provenanceInfo <file:///./dataset/Lecture%20Content/COMP%206741/Readings/SPARQL.pdf> .

<http://dbpedia.org/resource/Yann_LeCun> a roboprof:Topic ;
    dbo:name "Yann LeCun" ;
    roboprof:provenanceInfo <file:///./dataset/Lecture%20Content/COMP%206741/Readings/IntelligentAgent.pdf> .

<http://dbpedia.org/resource/Yext> a roboprof:Topic ;
    dbo:name "Yext" ;
    roboprof:provenanceInfo <file:///./dataset/Lecture%20Content/COMP%206741/Readings/KnowledgeGraph.pdf> .

<http://dbpedia.org/resource/Yoshua_Bengio> a roboprof:Topic ;
    dbo:name "Bengio" ;
    roboprof:provenanceInfo <file:///./dataset/Lecture%20Content/COMP%206741/OtherMaterial/WordEmbeddings.pdf> .

<http://dbpedia.org/resource/YouTube> a roboprof:Topic ;
    dbo:name "YouTube" ;
    roboprof:provenanceInfo <file:///./dataset/Lecture%20Content/COMP%206461/Lectures/2.ppt>,
        <file:///./dataset/Lecture%20Content/COMP%206741/Lectures/slides02.pdf> .

roboprof_data:40225156 a vivo:Student ;
    roboprof:achievedGrade <http://roboprof.ca/data/COMP_6231_B+>,
        <http://roboprof.ca/data/COMP_6421_A+>,
        <http://roboprof.ca/data/COMP_6461_B+>,
        roboprof_data:COMP_6521_A,
        roboprof_data:COMP_6721_A,
        roboprof_data:COMP_6731_A-,
        <http://roboprof.ca/data/COMP_6741_A+> ;
    roboprof:completedCourse roboprof_data:COMP_6231,
        roboprof_data:COMP_6421,
        roboprof_data:COMP_6461,
        roboprof_data:COMP_6521,
        roboprof_data:COMP_6721,
        roboprof_data:COMP_6731,
        roboprof_data:COMP_6741 ;
    roboprof:studiesAt roboprof_data:ConcordiaUniversity ;
    foaf:firstName "Jatish" ;
    foaf:lastName "Bhatia" ;
    vcard:hasEmail "jb@gmail.com" .

roboprof_data:40226157 a vivo:Student ;
    roboprof:achievedGrade roboprof_data:COMP_6231_A,
        roboprof_data:COMP_6411_A,
        roboprof_data:COMP_6551_A-,
        <http://roboprof.ca/data/COMP_6741_A+>,
        roboprof_data:COMP_6761_A,
        roboprof_data:COMP_6771_A-,
        <http://roboprof.ca/data/COMP_6791_B+> ;
    roboprof:completedCourse roboprof_data:COMP_6231,
        roboprof_data:COMP_6411,
        roboprof_data:COMP_6551,
        roboprof_data:COMP_6741,
        roboprof_data:COMP_6761,
        roboprof_data:COMP_6771,
        roboprof_data:COMP_6791 ;
    roboprof:studiesAt roboprof_data:ConcordiaUniversity ;
    foaf:firstName "Shruti" ;
    foaf:lastName "Bibra" ;
    vcard:hasEmail "sb@gmail.com" .

roboprof_data:40227120 a vivo:Student ;
    roboprof:achievedGrade roboprof_data:COMP_6231_F,
        roboprof_data:COMP_6461_A-,
        roboprof_data:COMP_6481_A-,
        roboprof_data:COMP_6521_F,
        roboprof_data:COMP_6741_A-,
        <http://roboprof.ca/data/Retake/COMP_6231_A>,
        <http://roboprof.ca/data/Retake/COMP_6521_B+> ;
    roboprof:completedCourse roboprof_data:COMP_6231,
        roboprof_data:COMP_6461,
        roboprof_data:COMP_6481,
        roboprof_data:COMP_6521,
        roboprof_data:COMP_6741 ;
    roboprof:studiesAt roboprof_data:ConcordiaUniversity ;
    foaf:firstName "Nandini" ;
    foaf:lastName "Bibra" ;
    vcard:hasEmail "nb@gmail.com" .

roboprof_data:COMP_6461_Lab_4 a roboprof:Lab ;
    dbo:name "Lab 1 : HTTP Client" ;
    dbo:number 4 ;
    roboprof:coversCourseContent <file:///./dataset/Lab%20Content/COMP%206461/Lab%20Material/Lab%201.pdf> .

roboprof_data:COMP_6461_Lab_5 a roboprof:Lab ;
    dbo:name "Lab 2 : HTTP Server" ;
    dbo:number 5 ;
    roboprof:coversCourseContent <file:///./dataset/Lab%20Content/COMP%206461/Lab%20Material/Lab%202.pdf> .

roboprof_data:COMP_6461_Lab_6 a roboprof:Lab ;
    dbo:name "Lab 3 : UDP Client Server" ;
    dbo:number 6 ;
    roboprof:coversCourseContent <file:///./dataset/Lab%20Content/COMP%206461/Lab%20Material/Lab%203.pdf> .

roboprof:achievedGrade a rdf:Property ;
    rdfs:label "Grade Achieved"@en ;
    rdfs:comment "Specifies the grade achieved by a student."@en ;
    rdfs:domain vivo:Student ;
    rdfs:range roboprof:Grade .

roboprof:completedCourse a rdf:Property ;
    rdfs:label "Course Compeleted"@en ;
    rdfs:comment "Specifies the courses completed by a student."@en ;
    rdfs:domain vivo:Student ;
    rdfs:range vivo:Course .

roboprof:courseOutline a rdf:Property ;
    rdfs:label "Course Outline"@en ;
    rdfs:comment "Refers to a document containing the course outline."@en ;
    rdfs:domain roboprof:Lecture ;
    rdfs:range dbo:Document .

roboprof:coversCourseContent a rdf:Property ;
    rdfs:label "Covers Course Content"@en ;
    rdfs:comment "Specifies the content covered in the course."@en ;
    rdfs:domain roboprof:CourseEvent ;
    rdfs:range roboprof:CourseContent .

roboprof:gradeInCourse a rdf:Property ;
    rdfs:label "Grade in Course"@en ;
    rdfs:comment "Specifies the grade that can be achieved in a particular course."@en ;
    rdfs:domain roboprof:Grade ;
    rdfs:range vivo:Course .

roboprof:gradeValue a rdf:Property ;
    rdfs:label "Value of the Grade"@en ;
    rdfs:comment "Specifies the letter grade."@en ;
    rdfs:domain roboprof:Grade ;
    rdfs:range xsd:string .

roboprof:hasCourseEvent a rdf:Property ;
    rdfs:label "Has Course Event"@en ;
    rdfs:comment "Specifies to the events that are part of a course."@en ;
    rdfs:domain vivo:Course ;
    rdfs:range roboprof:CourseEvent .

roboprof:offersCourse a rdf:Property ;
    rdfs:label "Course Offered"@en ;
    rdfs:comment "Specifies to the courses offered by the University."@en ;
    rdfs:domain dbo:University ;
    rdfs:range vivo:Course .

roboprof:provenanceInfo a rdf:Property ;
    rdfs:label "Provenance Information"@en ;
    rdfs:comment "Records where the topic was identified as being covered in the course (e.g., the calendar, the course outline or a specific lecture)"@en ;
    rdfs:domain roboprof:Topic ;
    rdfs:range roboprof:CourseContent .

roboprof:studiesAt a rdf:Property ;
    rdfs:label "Studies At"@en ;
    rdfs:comment "Specifies the university where the student studies."@en ;
    rdfs:domain vivo:Student ;
    rdfs:range dbo:University .

<file:///./dataset/Lecture%20Content/COMP%206461/Lectures/1.ppt> a roboprof:Slide ;
    dbo:name "1.ppt" .

<file:///./dataset/Lecture%20Content/COMP%206741/Readings/DeepLearning.pdf> a roboprof:Reading ;
    dbo:name "DeepLearning.pdf" .

roboprof_data:ACCO_330 a vivo:Course ;
    dbo:name "Cost and Management Accounting" ;
    dbo:number 330 ;
    dcterms:description "This course provides an examination of the techniques, systems, and procedures applicable to the managerial use of accounting information for planning, decision making, and control. Topics include cost accumulation and allocation, product and process costing, flexible budgeting and variance analysis, evaluation of managerial performance, and transfer pricing." ;
    vivo:courseCredits 3 ;
    vivo:hasSubjectArea "ACCO" .

roboprof_data:ACCO_355 a vivo:Course ;
    dbo:name "Analysis of Financial Statements" ;
    dbo:number 355 ;
    dcterms:description "Real life accounting case discussions and a project based on a real company" ;
    vivo:courseCredits 3 ;
    vivo:hasSubjectArea "ACCO" .

roboprof_data:ACCO_400 a vivo:Course ;
    dbo:name "Accounting in Society / Accounting Theory" ;
    dbo:number 400 ;
    dcterms:description "Research-based group project, written report, and recorded presentation" ;
    vivo:courseCredits 3 ;
    vivo:hasSubjectArea "ACCO" .

roboprof_data:ACCO_420 a vivo:Course ;
    dbo:name "Financial Reporting III" ;
    dbo:number 420 ;
    dcterms:description "All consolidation and foreign currency translation done using Excel worksheets as would be done in reality; case analysis done for all topics." ;
    vivo:courseCredits 3 ;
    vivo:hasSubjectArea "ACCO" .

roboprof_data:ACCO_425 a vivo:Course ;
    dbo:name "Financial Reporting IV" ;
    dbo:number 425 ;
    dcterms:description "Prepare financial statements for a fictitious company" ;
    vivo:courseCredits 3 ;
    vivo:hasSubjectArea "ACCO" .

roboprof_data:ACCO_435 a vivo:Course ;
    dbo:name "Strategic Accounting Case Analysis" ;
    dbo:number 435 ;
    dcterms:description "Comprehensive multi-subject strategic cases analysis (individual and group levels)" ;
    vivo:courseCredits 3 ;
    vivo:hasSubjectArea "ACCO" .

roboprof_data:ACCO_455 a vivo:Course ;
    dbo:name "Fraud Prevention and Investigation" ;
    dbo:number 455 ;
    dcterms:description "Reallife fraud case analyses, discussions and presentations" ;
    vivo:courseCredits 3 ;
    vivo:hasSubjectArea "ACCO" .

roboprof_data:ACCO_465 a vivo:Course ;
    dbo:name "Advanced Assurance Services" ;
    dbo:number 465 ;
    dcterms:description "This course covers important topics and concepts in auditing and assurance services. It builds on audit principles covered in previous courses and introduces specialized and advanced topics that are of particular importance to professional accountants. In covering topics and their application, the course focuses on decision-making processes followed by auditors." ;
    vivo:courseCredits 3 ;
    vivo:hasSubjectArea "ACCO" .

roboprof_data:ACCO_495 a vivo:Course ;
    dbo:name "Honours Seminar in Accountancy" ;
    dbo:number 495 ;
    dcterms:description "Writing a teaching case and solution or conducting an applied research project" ;
    vivo:courseCredits 4 ;
    vivo:hasSubjectArea "ACCO" .

roboprof_data:ACCO_650 a vivo:Course ;
    dbo:name "Financial Reporting in Practice" ;
    dbo:number 650 ;
    dcterms:description "Case Analysis" ;
    vivo:courseCredits 3 ;
    vivo:hasSubjectArea "ACCO" .

roboprof_data:ACCO_651 a vivo:Course ;
    dbo:name "Financial Reporting: Comprehensive Applications" ;
    dbo:number 651 ;
    dcterms:description "Case Analysis" ;
    vivo:courseCredits 3 ;
    vivo:hasSubjectArea "ACCO" .

roboprof_data:ACCO_652 a vivo:Course ;
    dbo:name "Business Advisory Services" ;
    dbo:number 652 ;
    dcterms:description "Case Analysis and Fictitious BOD Group Presentation" ;
    vivo:courseCredits 3 ;
    vivo:hasSubjectArea "ACCO" .

roboprof_data:ACCO_653 a vivo:Course ;
    dbo:name "Information Systems and Internal Control" ;
    dbo:number 653 ;
    dcterms:description "Case Analysis" ;
    vivo:courseCredits 4 ;
    vivo:hasSubjectArea "ACCO" .

roboprof_data:ACCO_654 a vivo:Course ;
    dbo:name "Assurance and Professional Practice" ;
    dbo:number 654 ;
    dcterms:description "Case Analysis" ;
    vivo:courseCredits 4 ;
    vivo:hasSubjectArea "ACCO" .

roboprof_data:ACCO_655 a vivo:Course ;
    dbo:name "Taxation and Decision-Making" ;
    dbo:number 655 ;
    dcterms:description "Case Analysis" ;
    vivo:courseCredits 4 ;
    vivo:hasSubjectArea "ACCO" .

roboprof_data:ACCO_656 a vivo:Course ;
    dbo:name "Performance Management" ;
    dbo:number 656 ;
    dcterms:description "Case Analysis and Fictitious BOD Group Presentation" ;
    vivo:courseCredits 3 ;
    vivo:hasSubjectArea "ACCO" .

roboprof_data:ACCO_657 a vivo:Course ;
    dbo:name "Financial Strategies and Decisions" ;
    dbo:number 657 ;
    dcterms:description "Case Analysis" ;
    vivo:courseCredits 4 ;
    vivo:hasSubjectArea "ACCO" .

roboprof_data:ACCO_658 a vivo:Course ;
    dbo:name "Capstone I Seminar" ;
    dbo:number 658 ;
    dcterms:description "Group Case Analysis, Written Report, and Fictitious BOD Group Presentation" ;
    vivo:courseCredits 4 ;
    vivo:hasSubjectArea "ACCO" .

roboprof_data:ACCO_659 a vivo:Course ;
    dbo:name "Capstone II Examination Preparation" ;
    dbo:number 659 ;
    dcterms:description "Case Analysis" ;
    vivo:courseCredits 4 ;
    vivo:hasSubjectArea "ACCO" .

roboprof_data:ACTT_201 a vivo:Course ;
    dbo:name "INTRODUCTION TO ACTING I",
        "Introduction to Acting" ;
    dbo:number 201 ;
    dcterms:description "NaN"^^xsd:double,
        "Development of imagination and physical expression" ;
    vivo:courseCredits 3,
        4 ;
    vivo:hasSubjectArea "ACTT" .

roboprof_data:ACTT_202 a vivo:Course ;
    dbo:name "INTRODUCTION TO ACTING II",
        "Introduction to Acting ll" ;
    dbo:number 202 ;
    dcterms:description "NaN"^^xsd:double,
        "Development of skills pertaining to language, character, and text" ;
    vivo:courseCredits 3,
        4 ;
    vivo:hasSubjectArea "ACTT" .

roboprof_data:ACTT_209 a vivo:Course ;
    dbo:name "The Engaged Theatre Artist" ;
    dbo:number 209 ;
    dcterms:description "Combines theoretical readings and practical explorations relating to diverse perspectives on an artists role in society" ;
    vivo:courseCredits 4 ;
    vivo:hasSubjectArea "ACTT " .

roboprof_data:ACTT_210 a vivo:Course ;
    dbo:name "Scene Study l" ;
    dbo:number 210 ;
    dcterms:description "Emphasis on movement, voice, and text interpretation" ;
    vivo:courseCredits 4 ;
    vivo:hasSubjectArea "ACTT " .

roboprof_data:ACTT_211 a vivo:Course ;
    dbo:name "Voice and Movement for the Stage l" ;
    dbo:number 211 ;
    dcterms:description "Cultivates the expressive potential of the actors instrument: the body, voice, and imagination" ;
    vivo:courseCredits 4 ;
    vivo:hasSubjectArea "ACTT " .

roboprof_data:ACTT_231 a vivo:Course ;
    dbo:name "Ensembles l" ;
    dbo:number 231 ;
    dcterms:description "Preparation for theatrical presentation with emphasis on the cooperative nature of theatre" ;
    vivo:courseCredits 4 ;
    vivo:hasSubjectArea "ACTT" .

roboprof_data:ACTT_321 a vivo:Course ;
    dbo:name "Movement for the Stage ll" ;
    dbo:number 321 ;
    dcterms:description "Various movement-based ensemble performance techniques and methods" ;
    vivo:courseCredits 4 ;
    vivo:hasSubjectArea "ACTT" .

roboprof_data:ACTT_325 a vivo:Course ;
    dbo:name "Voice for the Stage ll" ;
    dbo:number 325 ;
    dcterms:description "Course emphasizes embodiment, selfawareness" ;
    vivo:courseCredits 3 ;
    vivo:hasSubjectArea "ACTT" .

roboprof_data:ACTT_331 a vivo:Course ;
    dbo:name "Scene Study ll" ;
    dbo:number 331 ;
    dcterms:description "Course focus on nonrealistic genres " ;
    vivo:courseCredits 3 ;
    vivo:hasSubjectArea "ACTT " .

roboprof_data:ACTT_332 a vivo:Course ;
    dbo:name "Improvisation" ;
    dbo:number 332 ;
    dcterms:description "Introduction to improvisation as a method of creation for the stage" ;
    vivo:courseCredits 3 ;
    vivo:hasSubjectArea "ACTT" .

roboprof_data:ACTT_355 a vivo:Course ;
    dbo:name "Voice for the Stage lll" ;
    dbo:number 355 ;
    dcterms:description "Thorough introduction to a particular voicebased performance technique" ;
    vivo:courseCredits 4 ;
    vivo:hasSubjectArea "ACTT" .

roboprof_data:ACTT_358 a vivo:Course ;
    dbo:name "Movement for the Stage lll" ;
    dbo:number 358 ;
    dcterms:description "Course deepens student learning in a particular movement-based performance technique" ;
    vivo:courseCredits 4 ;
    vivo:hasSubjectArea "ACTT" .

roboprof_data:ACTT_360 a vivo:Course ;
    dbo:name "Ensembles ll" ;
    dbo:number 360 ;
    dcterms:description "Course focuses on skill development and performance of a particular theatrical genre" ;
    vivo:courseCredits 4 ;
    vivo:hasSubjectArea "ACTT" .

roboprof_data:ACTT_362 a vivo:Course ;
    dbo:name "Laban for the Actor" ;
    dbo:number 362 ;
    dcterms:description "Using Labans effort actions to investigate movement and space" ;
    vivo:courseCredits 4 ;
    vivo:hasSubjectArea "ACTT" .

roboprof_data:ACTT_370 a vivo:Course ;
    dbo:name "Clown for the Actor" ;
    dbo:number 370 ;
    dcterms:description "Course focuses on the development of clown characters and situations" ;
    vivo:courseCredits 4 ;
    vivo:hasSubjectArea "ACTT" .

roboprof_data:ACTT_372 a vivo:Course ;
    dbo:name "Stage Combat" ;
    dbo:number 372 ;
    dcterms:description "Course focuses on the development of unarmed and armed stage combat" ;
    vivo:courseCredits 3 ;
    vivo:hasSubjectArea "ACTT" .

roboprof_data:ACTT_398 a vivo:Course ;
    dbo:name "Special Topics in Acting" ;
    dbo:number 398 ;
    dcterms:description "Provides opportunities for studies in selected styles or modes of theatre performance" ;
    vivo:courseCredits 4 ;
    vivo:hasSubjectArea "ACTT" .

roboprof_data:ACTT_399 a vivo:Course ;
    dbo:name "Special Topics in Acting" ;
    dbo:number 399 ;
    dcterms:description "Provides opportunities for studies in selected styles or modes of theatre performance" ;
    vivo:courseCredits 4 ;
    vivo:hasSubjectArea "ACTT" .

roboprof_data:ACTT_432 a vivo:Course ;
    dbo:name "Rasa Boxes" ;
    dbo:number 432 ;
    dcterms:description "Course provides an intensive introduction to the performance of emotion" ;
    vivo:courseCredits 3 ;
    vivo:hasSubjectArea "ACTT" .

roboprof_data:ACTT_435 a vivo:Course ;
    dbo:name "Creation Project" ;
    dbo:number 435 ;
    dcterms:description "Course offers supervised application of theatrical skills" ;
    vivo:courseCredits 4 ;
    vivo:hasSubjectArea "ACTT" .

roboprof_data:ACTT_436 a vivo:Course ;
    dbo:name "One Act Project" ;
    dbo:number 436 ;
    dcterms:description "Public production of a one-act text from the worldwide body of dramatic literature" ;
    vivo:courseCredits 3 ;
    vivo:hasSubjectArea "ACTT" .

roboprof_data:ACTT_440 a vivo:Course ;
    dbo:name "Supervised Acting Performance Project" ;
    dbo:number 440 ;
    dcterms:description "Work in selfselected teams to develop short projects" ;
    vivo:courseCredits 3 ;
    vivo:hasSubjectArea "ACTT" .

roboprof_data:ACTT_450 a vivo:Course ;
    dbo:name "Advanced Acting Studio" ;
    dbo:number 450 ;
    dcterms:description "Provides advanced students with the opportunity to apply their skills to text study and character development" ;
    vivo:courseCredits 4 ;
    vivo:hasSubjectArea "ACTT" .

roboprof_data:ACTT_455 a vivo:Course ;
    dbo:name "Voice for Stage lV" ;
    dbo:number 455 ;
    dcterms:description "Advanced exploration of a particular voicebased performance technique, method, or approach" ;
    vivo:courseCredits 4 ;
    vivo:hasSubjectArea "ACTT" .

roboprof_data:ACTT_458 a vivo:Course ;
    dbo:name "Movement for Stage lV" ;
    dbo:number 458 ;
    dcterms:description "Exploration of a particular movementbased performance technique, method, or approach" ;
    vivo:courseCredits 3 ;
    vivo:hasSubjectArea "ACTT" .

roboprof_data:ACTT_460 a vivo:Course ;
    dbo:name "Classical Text Project" ;
    dbo:number 460 ;
    dcterms:description "Production of an iconic text from the worldwide body of dramatic literature" ;
    vivo:courseCredits 4 ;
    vivo:hasSubjectArea "ACTT" .

roboprof_data:ACTT_465 a vivo:Course ;
    dbo:name "The Actor's Profession" ;
    dbo:number 465 ;
    dcterms:description "Development of audition technique, on camera technique, interview skills, and other career-oriented skills" ;
    vivo:courseCredits 4 ;
    vivo:hasSubjectArea "ACTT" .

roboprof_data:ACTT_480 a vivo:Course ;
    dbo:name "Designing an Acting Workshop" ;
    dbo:number 480 ;
    dcterms:description "Opportunity to design a course framework under the guidance of the instructor that includes curriculum, implementation, and assessment for students" ;
    vivo:courseCredits 3 ;
    vivo:hasSubjectArea "ACTT" .

roboprof_data:ACTT_481 a vivo:Course ;
    dbo:name "Conducting Acting Workshop" ;
    dbo:number 481 ;
    dcterms:description "Conducting an acting workshop: active observation, instructional strategies to deliver the curriculum, and assessment" ;
    vivo:courseCredits 3 ;
    vivo:hasSubjectArea "ACTT" .

roboprof_data:ACTT_498 a vivo:Course ;
    dbo:name "Special Topics in Acting" ;
    dbo:number 498 ;
    dcterms:description "Provides opportunities for studies in selected styles or modes of theatre performance" ;
    vivo:courseCredits 3 ;
    vivo:hasSubjectArea "ACTT" .

roboprof_data:ACTT_499 a vivo:Course ;
    dbo:name "Special Topics in Acting" ;
    dbo:number 499 ;
    dcterms:description "Provides opportunities for studies in selected styles or modes of theatre performance" ;
    vivo:courseCredits 4 ;
    vivo:hasSubjectArea "ACTT" .

roboprof_data:ACTU_286 a vivo:Course ;
    dbo:name "Actuarial Mathematics Lab I" ;
    dbo:number 286 ;
    dcterms:description "Lab" ;
    vivo:courseCredits 3 ;
    vivo:hasSubjectArea "ACTU" .

roboprof_data:ACTU_386 a vivo:Course ;
    dbo:name "Actuarial Mathematics Lab II" ;
    dbo:number 386 ;
    dcterms:description "Lab" ;
    vivo:courseCredits 3 ;
    vivo:hasSubjectArea "ACTU" .

roboprof_data:ACTU_486 a vivo:Course ;
    dbo:name "Actuarial Mathematics Lab III" ;
    dbo:number 486 ;
    dcterms:description "Lab, workshop" ;
    vivo:courseCredits 3 ;
    vivo:hasSubjectArea "ACTU" .

roboprof_data:ADED_230 a vivo:Course ;
    dbo:name "Roles and Competencies of Adult Educators" ;
    dbo:number 230 ;
    dcterms:description "According to the participants needs & interests, an opportunity is given to explore competencies related to the particular roles" ;
    vivo:courseCredits 3 ;
    vivo:hasSubjectArea "ADED" .

roboprof_data:ADED_344 a vivo:Course ;
    dbo:name "Design of Adult Learning Projects" ;
    dbo:number 344 ;
    dcterms:description "Design & conduct a learning activity in the area of subject matter specialty" ;
    vivo:courseCredits 4 ;
    vivo:hasSubjectArea "ADED" .

roboprof_data:ADED_345 a vivo:Course ;
    dbo:name "Evaluating Adult Learning Projects" ;
    dbo:number 345 ;
    dcterms:description "Conduct an evaluation of an adult learning project in the area of subject matter specialty" ;
    vivo:courseCredits 4 ;
    vivo:hasSubjectArea "ADED" .

roboprof_data:ADED_370 a vivo:Course ;
    dbo:name "Workshops for Adult Educators" ;
    dbo:number 370 ;
    dcterms:description "Workshop" ;
    vivo:courseCredits 4 ;
    vivo:hasSubjectArea "ADED" .

roboprof_data:AERO_201 a vivo:Course ;
    dbo:name "Introduction to Flight and Aerospace Systems" ;
    dbo:number 201 ;
    dcterms:description "Laboratory: 4 hours per week, alternate weeks" ;
    vivo:courseCredits 3 ;
    vivo:hasSubjectArea "AERO" .

roboprof_data:AERO_371 a vivo:Course ;
    dbo:name "Modelling and Control Systems" ;
    dbo:number 371 ;
    dcterms:description "Laboratory: 2 hours per week, alternate weeks" ;
    vivo:courseCredits 4 ;
    vivo:hasSubjectArea "AERO" .

roboprof_data:AERO_390 a vivo:Course ;
    dbo:name "Aerospace Engineering Design Project" ;
    dbo:number 390 ;
    dcterms:description "Team-based project, design, implement, alternate weeks" ;
    vivo:courseCredits 4 ;
    vivo:hasSubjectArea "AERO" .

roboprof_data:AERO_455 a vivo:Course ;
    dbo:name "Computational Fluid Dynamics for Aerospace Applications" ;
    dbo:number 455 ;
    dcterms:description "Laboratory: 3 hours per week, alternate weeks" ;
    vivo:courseCredits 3 ;
    vivo:hasSubjectArea "AERO" .

roboprof_data:AERO_465 a vivo:Course ;
    dbo:name "Gas Turbine Design" ;
    dbo:number 465 ;
    dcterms:description "Laboratory: 2 hours per week, alternate weeks" ;
    vivo:courseCredits 3 ;
    vivo:hasSubjectArea "AERO" .

roboprof_data:AERO_480 a vivo:Course ;
    dbo:name "Flight Control Systems" ;
    dbo:number 480 ;
    dcterms:description "Laboratory: 2 hours per week, alternate weeks" ;
    vivo:courseCredits 4 ;
    vivo:hasSubjectArea "AERO" .

roboprof_data:AERO_481 a vivo:Course ;
    dbo:name "Materials Engineering for Aerospace" ;
    dbo:number 481 ;
    dcterms:description "Laboratory: 2 hours per week, alternate weeks" ;
    vivo:courseCredits 4 ;
    vivo:hasSubjectArea "AERO" .

roboprof_data:AERO_482 a vivo:Course ;
    dbo:name "Avionic Navigation Systems (3 credits)" ;
    dbo:number 482 ;
    dcterms:description "Laboratory: 1 hour per week" ;
    vivo:courseCredits 3 ;
    vivo:hasSubjectArea "AERO" .

roboprof_data:AERO_490 a vivo:Course ;
    dbo:name "Capstone Aerospace Engineering Design Project" ;
    dbo:number 490 ;
    dcterms:description "supervised design, simulation or experimental capstone design project" ;
    vivo:courseCredits 3 ;
    vivo:hasSubjectArea "AERO" .

roboprof_data:AHSC_225 a vivo:Course ;
    dbo:name "Self-Managed Learning" ;
    dbo:number 225 ;
    dcterms:description "Enables students to create clear personal visions, set relevant learning goals, create, organize related activities, & assess their progress" ;
    vivo:courseCredits 4 ;
    vivo:hasSubjectArea "AHSC" .

roboprof_data:AHSC_232 a vivo:Course ;
    dbo:name "Working in Task Groups" ;
    dbo:number 232 ;
    dcterms:description "Opportunities to integrate the theory they learn with their experiences in a task group" ;
    vivo:courseCredits 4 ;
    vivo:hasSubjectArea "AHSC" .

roboprof_data:AHSC_260 a vivo:Course ;
    dbo:name "Program Planning, design & evaluation" ;
    dbo:number 260 ;
    dcterms:description "Opportunities to integrate the theory they learn with their experiences in a task group" ;
    vivo:courseCredits 3 ;
    vivo:hasSubjectArea "AHSC" .

roboprof_data:AHSC_322 a vivo:Course ;
    dbo:name "Fundamentals of Child and YouthCare Work" ;
    dbo:number 322 ;
    dcterms:description "Simulations" ;
    vivo:courseCredits 3 ;
    vivo:hasSubjectArea "AHSC" .

roboprof_data:AHSC_332 a vivo:Course ;
    dbo:name "Organization Development 1" ;
    dbo:number 332 ;
    dcterms:description "Learn the phases and skills of OD consulting by participating in several workplace simulations" ;
    vivo:courseCredits 4 ;
    vivo:hasSubjectArea "AHSC" .

roboprof_data:AHSC_350 a vivo:Course ;
    dbo:name "Leisure Education" ;
    dbo:number 350 ;
    dcterms:description "The development and implementation of leisure education with children in the BASE after school program" ;
    vivo:courseCredits 4 ;
    vivo:hasSubjectArea "AHSC" .

roboprof_data:AHSC_360 a vivo:Course ;
    dbo:name "Play, Adult Learning and Development" ;
    dbo:number 360 ;
    dcterms:description "Design and implement play based simulations appropriate for various levels according to life stage development. Moot programs in class with peer groups" ;
    vivo:courseCredits 3 ;
    vivo:hasSubjectArea "AHSC" .

roboprof_data:AHSC_361 a vivo:Course ;
    dbo:name "Leisure Services Leadership" ;
    dbo:number 361 ;
    dcterms:description "Experiential learning through simulation with peers and off campus retreat" ;
    vivo:courseCredits 4 ;
    vivo:hasSubjectArea "AHSC" .

roboprof_data:AHSC_371 a vivo:Course ;
    dbo:name "Community Recreation Planning" ;
    dbo:number 371 ;
    dcterms:description "Practical experience, field experience, project planning " ;
    vivo:courseCredits 3 ;
    vivo:hasSubjectArea "AHSC" .

roboprof_data:AHSC_384 a vivo:Course ;
    dbo:name "Therapeutic Recreation: Cognitive Disabilities and Illness" ;
    dbo:number 384 ;
    dcterms:description "Volunteer placements - students are actively involved in assisting with recreation and leisure programs at community organizations; Living Library component  a method of informal education involving students as readers who engage in conversations with living books (individuals with mental illness)" ;
    vivo:courseCredits 3 ;
    vivo:hasSubjectArea "AHSC" .

roboprof_data:AHSC_410 a vivo:Course ;
    dbo:name "Advanced Youth Work Intervention" ;
    dbo:number 410 ;
    dcterms:description "Simulations" ;
    vivo:courseCredits 4 ;
    vivo:hasSubjectArea "AHSC" .

roboprof_data:AHSC_422 a vivo:Course ;
    dbo:name "Youth and Leisure" ;
    dbo:number 422 ;
    dcterms:description "Laboratory" ;
    vivo:courseCredits 3 ;
    vivo:hasSubjectArea "AHSC" .

roboprof_data:AHSC_425 a vivo:Course ;
    dbo:name "Organization Development II" ;
    dbo:number 425 ;
    dcterms:description "Experiential approaches, in-class applications" ;
    vivo:courseCredits 3 ;
    vivo:hasSubjectArea "AHSC" .

roboprof_data:AHSC_432 a vivo:Course ;
    dbo:name "Seminar in Therapeutic Recreation" ;
    dbo:number 432 ;
    dcterms:description "Students use their knowledge of TR and the various skills and interests of the class to design a community project for the benefit of the community" ;
    vivo:courseCredits 4 ;
    vivo:hasSubjectArea "AHSC" .

roboprof_data:AHSC_435 a vivo:Course ;
    dbo:name "Fieldwork Practice" ;
    dbo:number 435 ;
    dcterms:description "Fieldwork, lead one small task or learning group in a community, an organizational or an institutional setting" ;
    vivo:courseCredits 4 ;
    vivo:hasSubjectArea "AHSC" .

roboprof_data:AHSC_436 a vivo:Course ;
    dbo:name "Internship in Youth and Family Work" ;
    dbo:number 436 ;
    dcterms:description "360-hour internship, supervised placement implementing family life education programs in such settings as community organizations, education, and health care",
        "Work with youth and families in such settings as child welfare, schools, non-profit organizations, residential care, or outreach" ;
    vivo:courseCredits 4 ;
    vivo:hasSubjectArea "AHSC" .

roboprof_data:AHSC_437 a vivo:Course ;
    dbo:name "Internships in Leisure Sciences" ;
    dbo:number 437 ;
    dcterms:description "Opportunity to design, implement, and evaluate programs; to facilitate groups in a variety of settings; and to establish working relationships with field personnel" ;
    vivo:courseCredits 4 ;
    vivo:hasSubjectArea "AHSC" .

roboprof_data:AHSC_438 a vivo:Course ;
    dbo:name "Internship in Therapeutic Recreation" ;
    dbo:number 438 ;
    dcterms:description "Opportunity to design, implement, and evaluate programs, to facilitate groups in a variety of settings, and to establish working relationships with field personnel" ;
    vivo:courseCredits 3 ;
    vivo:hasSubjectArea "AHSC" .

roboprof_data:AHSC_439 a vivo:Course ;
    dbo:name "Internship in Human Relations" ;
    dbo:number 439 ;
    dcterms:description "Opportunity to design, implement, and evaluate small group leadership in several settings, and to negotiate working relationships with site personnel" ;
    vivo:courseCredits 3 ;
    vivo:hasSubjectArea "AHSC" .

roboprof_data:AHSC_442 a vivo:Course ;
    dbo:name "Community Development and Leisure" ;
    dbo:number 442 ;
    dcterms:description "Development, application, and evaluation of a community development approach in the community" ;
    vivo:courseCredits 4 ;
    vivo:hasSubjectArea "AHSC" .

roboprof_data:AHSC_443 a vivo:Course ;
    dbo:name "Community Development I" ;
    dbo:number 443 ;
    dcterms:description "Community" ;
    vivo:courseCredits 3 ;
    vivo:hasSubjectArea "AHSC" .

roboprof_data:AHSC_444 a vivo:Course ;
    dbo:name "The Older Adult and Leisure" ;
    dbo:number 444 ;
    dcterms:description "Students form small working groups with older adults from local community organizations to design and facilitate a conversation caf" ;
    vivo:courseCredits 3 ;
    vivo:hasSubjectArea "AHSC" .

roboprof_data:AHSC_451 a vivo:Course ;
    dbo:name "Counselling Skills and Concepts" ;
    dbo:number 451 ;
    dcterms:description "in-class simulations" ;
    vivo:courseCredits 4 ;
    vivo:hasSubjectArea "AHSC" .

roboprof_data:AHSC_456 a vivo:Course ;
    dbo:name "Advanced Family Life Education" ;
    dbo:number 456 ;
    dcterms:description "Fieldwork, 1 hour per week of observation in a family life education setting" ;
    vivo:courseCredits 3 ;
    vivo:hasSubjectArea "AHSC" .

roboprof_data:AHSC_470 a vivo:Course ;
    dbo:name "Basic Human Relations Laboratory" ;
    dbo:number 470 ;
    dcterms:description "Laboratory" ;
    vivo:courseCredits 4 ;
    vivo:hasSubjectArea "AHSC" .

roboprof_data:AHSC_490 a vivo:Course ;
    dbo:name "Independent Study I" ;
    dbo:number 490 ;
    dcterms:description "Field studies, and/or research" ;
    vivo:courseCredits 3 ;
    vivo:hasSubjectArea "AHSC" .

roboprof_data:AHSC_491 a vivo:Course ;
    dbo:name "Independent Study II" ;
    dbo:number 491 ;
    dcterms:description "Field studies, and/or research" ;
    vivo:courseCredits 4 ;
    vivo:hasSubjectArea "AHSC" .

roboprof_data:AHSC_498 a vivo:Course ;
    dbo:name """Leadership,_x000D_
 Change &_x000D_
 Social_x000D_
 Innovation""" ;
    dbo:number 498 ;
    dcterms:description "Students join a learning community made up of undergraduate and graduate students, university staff and members of the local community. Together they engage in u.lab - a process of innovation and change that connects inner change to outer action." ;
    vivo:courseCredits 3 ;
    vivo:hasSubjectArea "AHSC" .

roboprof_data:AHSC_510 a vivo:Course ;
    dbo:name "Advanced Research Methods in Youth Work" ;
    dbo:number 510 ;
    dcterms:description "Applied research project" ;
    vivo:courseCredits 4 ;
    vivo:hasSubjectArea "AHSC" .

roboprof_data:AHSC_525 a vivo:Course ;
    dbo:name "Individual and Group Intervention with Youth" ;
    dbo:number 525 ;
    dcterms:description "Fieldwork component, 1 hour per week of observation in a youth work setting" ;
    vivo:courseCredits 3 ;
    vivo:hasSubjectArea "AHSC" .

roboprof_data:AHSC_527 a vivo:Course ;
    dbo:name "Advanced Youth Work Intervention: Case Management and Supervision" ;
    dbo:number 527 ;
    dcterms:description "Implementing & monitoring effective and collaborative case plans with young people & their families" ;
    vivo:courseCredits 4 ;
    vivo:hasSubjectArea "AHSC" .

roboprof_data:AHSC_530 a vivo:Course ;
    dbo:name "Community Youth Development" ;
    dbo:number 530 ;
    dcterms:description "Practical applications for community-based youth programs" ;
    vivo:courseCredits 3 ;
    vivo:hasSubjectArea "AHSC" .

roboprof_data:AHSC_533 a vivo:Course ;
    dbo:name "Internship I in Youth Work" ;
    dbo:number 533 ;
    dcterms:description "100 hours in settings such as schools, community organizations, hospitals, or rehabilitation centres",
        "Entry-level internship designed to provide  a first field experience that promotes integration into a clinical or normative youth work setting. A major focus is on participatory observation. One day per week, for a total of 100 hours in settings such as schools, community organizations, hospitals, or rehabilitation centres. " ;
    vivo:courseCredits 3,
        4 ;
    vivo:hasSubjectArea "AHSC" .

roboprof_data:AHSC_537 a vivo:Course ;
    dbo:name "Internship II in Youth Work" ;
    dbo:number 537 ;
    dcterms:description "220-hour internship, supervised apprenticeship in either a clinical or normative youth work setting that builds on the students previous courses",
        "Any programs" ;
    vivo:courseCredits 4 ;
    vivo:hasSubjectArea "AHSC" .

roboprof_data:AHSC_538 a vivo:Course ;
    dbo:name "Extended Internship in Youth Work" ;
    dbo:number 538 ;
    dcterms:description "320-hour internship, full-time supervised experience in either a clinical or a normative youth work setting, additional hours to assist the student in building his/her application for licensing",
        "320-hour internship. Full-time supervised experience in either a clinical or a normative youth work setting and requires additional hours to assist the student in building his/her application for licensing. The student fully assumes all the duties and responsibilities of a youth worker in the same site selected for the first internship. Work is supervised and evaluated by an on-site field supervisor." ;
    vivo:courseCredits 3 ;
    vivo:hasSubjectArea "AHSC" .

roboprof_data:AHSC_599 a vivo:Course ;
    dbo:name "Independent Study" ;
    dbo:number 599 ;
    dcterms:description "Field studies, and/or research" ;
    vivo:courseCredits 3 ;
    vivo:hasSubjectArea "AHSC" .

roboprof_data:AHSC_610 a vivo:Course ;
    dbo:name "Group Process Intervention" ;
    dbo:number 610 ;
    dcterms:description """Residential Laboratory; Course-integrated_x000D_
projects""" ;
    vivo:courseCredits 3 ;
    vivo:hasSubjectArea "AHSC" .

roboprof_data:AHSC_620 a vivo:Course ;
    dbo:name "Learning and Individual Change Processes" ;
    dbo:number 620 ;
    dcterms:description "Course-integrated projects; Capstone project" ;
    vivo:courseCredits 4 ;
    vivo:hasSubjectArea "AHSC" .

roboprof_data:AHSC_631 a vivo:Course ;
    dbo:name "Research Methods" ;
    dbo:number 631 ;
    dcterms:description "Course-integrated projects; Simulations; Participatory action research" ;
    vivo:courseCredits 3 ;
    vivo:hasSubjectArea "AHSC" .

roboprof_data:AHSC_632 a vivo:Course ;
    dbo:name "Planning Human Systems Intervention" ;
    dbo:number 632 ;
    dcterms:description "Course-integrated projects; Simulations; Case studies" ;
    vivo:courseCredits 3 ;
    vivo:hasSubjectArea "AHSC" .

roboprof_data:AHSC_660 a vivo:Course ;
    dbo:name "Philosophy and Ethics of Intervention" ;
    dbo:number 660 ;
    dcterms:description """Course-integrated project; Case studies; Hands-on_x000D_
workshops""" ;
    vivo:courseCredits 4 ;
    vivo:hasSubjectArea "AHSC" .

roboprof_data:AHSC_670 a vivo:Course ;
    dbo:name "Consultation Methods" ;
    dbo:number 670 ;
    dcterms:description "Establish effective client-consultant relationships " ;
    vivo:courseCredits 3 ;
    vivo:hasSubjectArea "AHSC" .

roboprof_data:AHSC_675 a vivo:Course ;
    dbo:name "Introduction to Open Systems Theory" ;
    dbo:number 675 ;
    dcterms:description "Course-integrated projects; Simulations" ;
    vivo:courseCredits 3 ;
    vivo:hasSubjectArea "AHSC" .

roboprof_data:AHSC_680 a vivo:Course ;
    dbo:name "Facilitating Individual and Group Learning Processes" ;
    dbo:number 680 ;
    dcterms:description "Laboratory setting",
        "Laboratory setting plus delivery of a workshop to a community client" ;
    vivo:courseCredits 4 ;
    vivo:hasSubjectArea "AHSC" .

roboprof_data:AHSC_685 a vivo:Course ;
    dbo:name "Coaching Interventions and Processes" ;
    dbo:number 685 ;
    dcterms:description "Practical components" ;
    vivo:courseCredits 3 ;
    vivo:hasSubjectArea "AHSC" .

roboprof_data:AHSC_690 a vivo:Course ;
    dbo:name "Practicum A" ;
    dbo:number 690 ;
    dcterms:description "Practicum" ;
    vivo:courseCredits 3 ;
    vivo:hasSubjectArea "AHSC" .

roboprof_data:AHSC_691 a vivo:Course ;
    dbo:name "Practicum B" ;
    dbo:number 691 ;
    dcterms:description "Practicum" ;
    vivo:courseCredits 4 ;
    vivo:hasSubjectArea "AHSC" .

roboprof_data:AHSC_698 a vivo:Course ;
    dbo:name "Masters Project" ;
    dbo:number 698 ;
    dcterms:description "Contracting with the client, gathering and analyzing data, implementing relevant intervention activities, and evaluating the intervention as well as their role" ;
    vivo:courseCredits 4 ;
    vivo:hasSubjectArea "AHSC" .

roboprof_data:ANTH_315 a vivo:Course ;
    dbo:name "Field Research" ;
    dbo:number 315 ;
    dcterms:description "Field, practice" ;
    vivo:courseCredits 3 ;
    vivo:hasSubjectArea "ANTH" .

roboprof_data:ANTH_450 a vivo:Course ;
    dbo:name "Social Economy & Sustainable Futures" ;
    dbo:number 450 ;
    dcterms:description "Community Service Learning & Group project" ;
    vivo:courseCredits 4 ;
    vivo:hasSubjectArea "ANTH" .

roboprof_data:APLI_601 a vivo:Course ;
    dbo:name "Graduate Phonology" ;
    dbo:number 601 ;
    dcterms:description "Evaluation of pronunciation textbooks; assessment of teaching techniques for pronunciation instructions; preparation of teaching materials targeting L2 pronunciation; analysis of L2 learner data; use of computer-assisted tools for pronunciation teaching and learning; conduct needs analysis (e.g., based on pronunciation problems in a specific learning context)" ;
    vivo:courseCredits 4 ;
    vivo:hasSubjectArea "APLI" .

roboprof_data:APLI_604 a vivo:Course ;
    dbo:name "Applied Language Studies" ;
    dbo:number 604 ;
    dcterms:description "Analysis of language data (e.g., phonological, morphosyntactic phenomena); synthesize research for various presentation formats: abstract, reviews, 3-min./10-min/20-min oral presentations, research papers, etc.;" ;
    vivo:courseCredits 3 ;
    vivo:hasSubjectArea "APLI" .

roboprof_data:APLI_610 a vivo:Course ;
    dbo:name "Teaching and Learning Second Language Vocabulary" ;
    dbo:number 610 ;
    dcterms:description "Students complete projects that has direct social impact: 1) a vocabulary language task for social justice education, which they can apply in their own teaching; 2) a digital presentation in which they demonstrate how to use computer tools to teach vocabulary, which is made available online for the community; 3) a research paper or a professional magazine article which students are encourage to submit for publication" ;
    vivo:courseCredits 3 ;
    vivo:hasSubjectArea "APLI" .

roboprof_data:APLI_616 a vivo:Course ;
    dbo:name "Pedagogical Grammar" ;
    dbo:number 616 ;
    dcterms:description "Final teaching research project: design, implement, and evaluate the teaching of an original set of materials on a grammar feature; write up the analysis in a final report" ;
    vivo:courseCredits 3 ;
    vivo:hasSubjectArea "APLI" .

roboprof_data:APLI_623 a vivo:Course ;
    dbo:name "Sociolinguistics" ;
    dbo:number 623 ;
    dcterms:description "Students complete a project targeting a sociolinguistic topic of their choice. The project can be either data driven (based on language data collected by students) or conceptual (involving a critical review of relevant issues on a given topic). Students write up the results of this project in a brief report format and present its content in a 10-minute presentation." ;
    vivo:courseCredits 3 ;
    vivo:hasSubjectArea "APLI" .

roboprof_data:APLI_626 a vivo:Course ;
    dbo:name "Variationist Approaches to Second Language Acquisition" ;
    dbo:number 626 ;
    dcterms:description "Conceptualize, design and implement a pilot study using variationist analytical tools; review and critique studies in the field; create sociolinguistically-influenced pedagogical materials for language teaching" ;
    vivo:courseCredits 3 ;
    vivo:hasSubjectArea "APLI" .

roboprof_data:APLI_630 a vivo:Course ;
    dbo:name "Second Language Syllabus Design and Curriculum Planning" ;
    dbo:number 630 ;
    dcterms:description "Students conduct a needs analysis based on a language program in their community with the aim to improve language instruction. They also complete a final project: design language curriculum based on the needs analysis. Knowledge of theories learned during the course is disseminated through a digital presentation and a blog post or research paper which students are encouraged to publish online and/or submit for publication" ;
    vivo:courseCredits 4 ;
    vivo:hasSubjectArea "APLI" .

roboprof_data:APLI_634 a vivo:Course ;
    dbo:name "Cross-linguistic Influence" ;
    dbo:number 634 ;
    dcterms:description "Final research project: students design and pilot (collect data) a study, and analyze and write up results; many students present their findings at the annual Graduate Student Symposium" ;
    vivo:courseCredits 3 ;
    vivo:hasSubjectArea "APLI" .

roboprof_data:APLI_635 a vivo:Course ;
    dbo:name "Language Assessment" ;
    dbo:number 635 ;
    dcterms:description "Students complete projects in which they analyze and deconstruct existing language assessments, as well as writing blueprints for language assessments in specific contexts of their own choice" ;
    vivo:courseCredits 3 ;
    vivo:hasSubjectArea "APLI" .

roboprof_data:APLI_636 a vivo:Course ;
    dbo:name "Language Awareness" ;
    dbo:number 636 ;
    dcterms:description "Students research and teach language awareness techniques to the entire class." ;
    vivo:courseCredits 3 ;
    vivo:hasSubjectArea "APLI" .

roboprof_data:APLI_644 a vivo:Course ;
    dbo:name "Technology in Language Teaching" ;
    dbo:number 644 ;
    dcterms:description "Design, create and assess pedagogical materials involving reading and writing (including lesson plans, activities, textbooks, virtual learning environments, website, games, etc.); final projects: develop a full-fledged virtual learning environment and a research project to implement computer technology in language teaching and/or learning" ;
    vivo:courseCredits 4 ;
    vivo:hasSubjectArea "APLI" .

roboprof_data:APLI_647 a vivo:Course ;
    dbo:name "Supervision of Practice Teaching" ;
    dbo:number 647 ;
    dcterms:description "Students observe and assist novice ESL teachers and provide one-on-one mentoring." ;
    vivo:courseCredits 4 ;
    vivo:hasSubjectArea "APLI" .

roboprof_data:APLI_660 a vivo:Course ;
    dbo:name "Research Methods" ;
    dbo:number 660 ;
    dcterms:description "Students engage in a project leading to a proposal for an MA-level research study. The research proposal consists of two parts: (a) review of the literature and (b) method section, organized as a single, coherent document. The research proposal also includes an oral presentation, and a response to peer feedback document." ;
    vivo:courseCredits 4 ;
    vivo:hasSubjectArea "APLI" .

roboprof_data:ARTE_201 a vivo:Course ;
    dbo:name "ART IN EARLY CHILDHOOD I" ;
    dbo:number 201 ;
    dcterms:description "NaN"^^xsd:double ;
    vivo:courseCredits 4 ;
    vivo:hasSubjectArea "ARTE" .

roboprof_data:ARTT_470 a vivo:Course ;
    dbo:name "Professional Internship" ;
    dbo:number 470 ;
    dcterms:description "Students wishing to work in an internship capacity within an artistic/cultural environment may apply for academic credit." ;
    vivo:courseCredits 4 ;
    vivo:hasSubjectArea "ARTT" .

roboprof_data:ARTT_471 a vivo:Course ;
    dbo:name "Professional Internship I " ;
    dbo:number 471 ;
    dcterms:description "Students wishing to work in an internship capacity within an artistic/cultural environment may apply for academic credit." ;
    vivo:courseCredits 4 ;
    vivo:hasSubjectArea "ARTT" .

roboprof_data:ARTT_472 a vivo:Course ;
    dbo:name "Professional Internship II" ;
    dbo:number 472 ;
    dcterms:description "Students wishing to work in an internship capacity within an artistic/cultural environment may apply for academic credit." ;
    vivo:courseCredits 4 ;
    vivo:hasSubjectArea "ARTT" .

roboprof_data:ARTX_201 a vivo:Course ;
    dbo:name "Introduction to Contemporary Art Practices" ;
    dbo:number 201 ;
    dcterms:description "Studio course" ;
    vivo:courseCredits 3 ;
    vivo:hasSubjectArea "ARTX" .

roboprof_data:ARTX_280 a vivo:Course ;
    dbo:name "Integrated Studio in Contemporary Art Practices I" ;
    dbo:number 280 ;
    dcterms:description "Studio course" ;
    vivo:courseCredits 4 ;
    vivo:hasSubjectArea "ARTX" .

roboprof_data:ARTX_380 a vivo:Course ;
    dbo:name "Intermediate Integrated Studio in Contemporary Art Practices" ;
    dbo:number 380 ;
    dcterms:description "Studio course" ;
    vivo:courseCredits 3 ;
    vivo:hasSubjectArea "ARTX" .

roboprof_data:ARTX_398 a vivo:Course ;
    dbo:name "Special Topics in Contemporary Studio Arts Practice" ;
    dbo:number 398 ;
    dcterms:description "Studio course" ;
    vivo:courseCredits 3 ;
    vivo:hasSubjectArea "ARTX" .

roboprof_data:ARTX_399 a vivo:Course ;
    dbo:name "Special Topics in Contemporary Studio Arts Practice" ;
    dbo:number 399 ;
    dcterms:description "Studio course" ;
    vivo:courseCredits 3 ;
    vivo:hasSubjectArea "ARTX" .

roboprof_data:ARTX_480 a vivo:Course ;
    dbo:name "Advanced Integrated Studio in Contemporary Art Practices" ;
    dbo:number 480 ;
    dcterms:description "Studio course" ;
    vivo:courseCredits 4 ;
    vivo:hasSubjectArea "ARTX" .

roboprof_data:ARTX_490 a vivo:Course ;
    dbo:name "Independent Study" ;
    dbo:number 490 ;
    dcterms:description "This course provides a limited number of students the opportunity to pursue advanced studies in a specific interdisciplinary project under the supervision of a fulltime ARTX faculty member." ;
    vivo:courseCredits 4 ;
    vivo:hasSubjectArea "ARTX" .

roboprof_data:ARTX_491 a vivo:Course ;
    dbo:name "Independent Study II" ;
    dbo:number 491 ;
    dcterms:description "This course provides a limited number of students the opportunity to pursue advanced studies in a specific interdisciplinary project under the supervision of a fulltime ARTX faculty member." ;
    vivo:courseCredits 3 ;
    vivo:hasSubjectArea "ARTX" .

roboprof_data:ARTX_492 a vivo:Course ;
    dbo:name "Independent Study II" ;
    dbo:number 492 ;
    dcterms:description "This course provides a limited number of students the opportunity to pursue advanced studies in a specific interdisciplinary project under the supervision of a fulltime ARTX faculty member. " ;
    vivo:courseCredits 3 ;
    vivo:hasSubjectArea "ARTX" .

roboprof_data:BCEE_371 a vivo:Course ;
    dbo:name "Surveying" ;
    dbo:number 371 ;
    dcterms:description "Fieldwork" ;
    vivo:courseCredits 3 ;
    vivo:hasSubjectArea "BCEE" .

roboprof_data:BIOL_201 a vivo:Course ;
    dbo:name "Introductory Biology" ;
    dbo:number 201 ;
    dcterms:description "Laboratory" ;
    vivo:courseCredits 4 ;
    vivo:hasSubjectArea "BIOL" .

roboprof_data:BIOL_227 a vivo:Course ;
    dbo:name "Laboratory Studies in Biodiversity" ;
    dbo:number 227 ;
    dcterms:description "Laboratory" ;
    vivo:courseCredits 3 ;
    vivo:hasSubjectArea "BIOL" .

roboprof_data:BIOL_322 a vivo:Course ;
    dbo:name "Biostatistics" ;
    dbo:number 322 ;
    dcterms:description "Laboratory" ;
    vivo:courseCredits 4 ;
    vivo:hasSubjectArea "BIOL" .

roboprof_data:BIOL_330 a vivo:Course ;
    dbo:name "Vertebrate Biology" ;
    dbo:number 330 ;
    dcterms:description "Laboratory" ;
    vivo:courseCredits 4 ;
    vivo:hasSubjectArea "BIOL" .

roboprof_data:BIOL_337 a vivo:Course ;
    dbo:name "Invertebrate Biology" ;
    dbo:number 337 ;
    dcterms:description "Laboratory" ;
    vivo:courseCredits 3 ;
    vivo:hasSubjectArea "BIOL" .

roboprof_data:BIOL_340 a vivo:Course ;
    dbo:name "Plant Biology" ;
    dbo:number 340 ;
    dcterms:description "Laboratory" ;
    vivo:courseCredits 4 ;
    vivo:hasSubjectArea "BIOL" .

roboprof_data:BIOL_351 a vivo:Course ;
    dbo:name "Basic Population Ecology" ;
    dbo:number 351 ;
    dcterms:description "Computer lab" ;
    vivo:courseCredits 4 ;
    vivo:hasSubjectArea "BIOL" .

roboprof_data:BIOL_368 a vivo:Course ;
    dbo:name "Genetics and Cell Biology Laboratory" ;
    dbo:number 368 ;
    dcterms:description "Laboratory" ;
    vivo:courseCredits 3 ;
    vivo:hasSubjectArea "BIOL" .

roboprof_data:BIOL_382 a vivo:Course ;
    dbo:name "Comparative Animal Physiology" ;
    dbo:number 382 ;
    dcterms:description "Laboratory" ;
    vivo:courseCredits 3 ;
    vivo:hasSubjectArea "BIOL" .

roboprof_data:BIOL_398 a vivo:Course ;
    dbo:name "Intermediate Topics in Biology: Ecology of Urban Environments" ;
    dbo:number 398 ;
    dcterms:description "Field work" ;
    vivo:courseCredits 3 ;
    vivo:hasSubjectArea "BIOL" .

roboprof_data:BIOL_422 a vivo:Course ;
    dbo:name "Advanced Statistics in Biological Science" ;
    dbo:number 422 ;
    dcterms:description "Computer lab" ;
    vivo:courseCredits 3 ;
    vivo:hasSubjectArea "BIOL" .

roboprof_data:BIOL_423 a vivo:Course ;
    dbo:name "Scientific Communication" ;
    dbo:number 423 ;
    dcterms:description "Workshops" ;
    vivo:courseCredits 4 ;
    vivo:hasSubjectArea "BIOL" .

roboprof_data:BIOL_450 a vivo:Course ;
    dbo:name "Techniques in Ecology" ;
    dbo:number 450 ;
    dcterms:description "Laboratory" ;
    vivo:courseCredits 3 ;
    vivo:hasSubjectArea "BIOL" .

roboprof_data:BIOL_451 a vivo:Course ;
    dbo:name "Field Ecology" ;
    dbo:number 451 ;
    dcterms:description "2 weeks of fieldwork in a research station " ;
    vivo:courseCredits 4 ;
    vivo:hasSubjectArea "BIOL" .

roboprof_data:BIOL_466 a vivo:Course ;
    dbo:name "Advanced Techniques in Molecular Biology" ;
    dbo:number 466 ;
    dcterms:description "Laboratory" ;
    vivo:courseCredits 3 ;
    vivo:hasSubjectArea "BIOL" .

roboprof_data:BIOL_480 a vivo:Course ;
    dbo:name "Bioinformatics" ;
    dbo:number 480 ;
    dcterms:description "Computer lab" ;
    vivo:courseCredits 4 ;
    vivo:hasSubjectArea "BIOL" .

roboprof_data:BIOL_486 a vivo:Course ;
    dbo:name "High-throughput Instrumentation" ;
    dbo:number 486 ;
    dcterms:description "Real-world project/assignment" ;
    vivo:courseCredits 3 ;
    vivo:hasSubjectArea "BIOL" .

roboprof_data:BIOL_490 a vivo:Course ;
    dbo:name "Independent Study" ;
    dbo:number 490 ;
    dcterms:description "Research project" ;
    vivo:courseCredits 3 ;
    vivo:hasSubjectArea "BIOL" .

roboprof_data:BIOL_498 a vivo:Course ;
    dbo:name "Internship In Tropical Biology" ;
    dbo:number 498 ;
    dcterms:description "Internship field work in tropical environment/seminar" ;
    vivo:courseCredits 3 ;
    vivo:hasSubjectArea "BIOL" .

roboprof_data:BIOL_510 a vivo:Course ;
    dbo:name "Bioinformatics" ;
    dbo:number 510 ;
    dcterms:description "Computer lab" ;
    vivo:courseCredits 4 ;
    vivo:hasSubjectArea "BIOL" .

roboprof_data:BIOL_515 a vivo:Course ;
    dbo:name "Biotechnology and Genomics Laboratory" ;
    dbo:number 515 ;
    dcterms:description "Laboratory" ;
    vivo:courseCredits 3 ;
    vivo:hasSubjectArea "BIOL" .

roboprof_data:BIOL_516 a vivo:Course ;
    dbo:name "Project in Biotechnology and Genomics" ;
    dbo:number 516 ;
    dcterms:description "Research project" ;
    vivo:courseCredits 4 ;
    vivo:hasSubjectArea "BIOL" .

roboprof_data:BIOL_524 a vivo:Course ;
    dbo:name "High-throughput Instrumentation" ;
    dbo:number 524 ;
    dcterms:description "Real-world project/assignment" ;
    vivo:courseCredits 3 ;
    vivo:hasSubjectArea "BIOL" .

roboprof_data:BIOL_614 a vivo:Course ;
    dbo:name "Advanced Topics in Ecology: Advanced Field Ecology" ;
    dbo:number 614 ;
    dcterms:description "2 weeks of fieldwork in a research station " ;
    vivo:courseCredits 4 ;
    vivo:hasSubjectArea "BIOL" .

roboprof_data:BIOL_622 a vivo:Course ;
    dbo:name "Advanced Techniques in Ecology" ;
    dbo:number 622 ;
    dcterms:description "Laboratory" ;
    vivo:courseCredits 4 ;
    vivo:hasSubjectArea "BIOL" .

roboprof_data:BIOL_630 a vivo:Course ;
    dbo:name "Bioinformatics" ;
    dbo:number 630 ;
    dcterms:description "Computer lab" ;
    vivo:courseCredits 3 ;
    vivo:hasSubjectArea "BIOL" .

roboprof_data:BIOL_631 a vivo:Course ;
    dbo:name "Advanced Top/Biotechnology: Synthetic Biology and Industrial Applications",
        "Advanced Top/Biotechnology: Tools of Synthetic Biology" ;
    dbo:number 631 ;
    dcterms:description "Real-world project/assignment" ;
    vivo:courseCredits 3,
        4 ;
    vivo:hasSubjectArea "BIOL" .

roboprof_data:BIOL_670 a vivo:Course ;
    dbo:name "Scientific Communication" ;
    dbo:number 670 ;
    dcterms:description "Workshops" ;
    vivo:courseCredits 4 ;
    vivo:hasSubjectArea "BIOL" .

roboprof_data:BIOL_680 a vivo:Course ;
    dbo:name "Advanced Topics in Biology: Advanced Statistics in Biological Science",
        "High-throughput Instrumentation" ;
    dbo:number 680 ;
    dcterms:description "Computer lab",
        "Real-world project/assignment" ;
    vivo:courseCredits 3 ;
    vivo:hasSubjectArea "BIOL" .

roboprof_data:BIOL_689 a vivo:Course ;
    dbo:name "Advanced Techniques in Molecular Biology" ;
    dbo:number 689 ;
    dcterms:description "Laboratory" ;
    vivo:courseCredits 4 ;
    vivo:hasSubjectArea "BIOL" .

roboprof_data:BIOL_801 a vivo:Course ;
    dbo:name "Pedagogical Training" ;
    dbo:number 801 ;
    dcterms:description "Pedagogical Practicum" ;
    vivo:courseCredits 3 ;
    vivo:hasSubjectArea "BIOL" .

roboprof_data:BIOL_802 a vivo:Course ;
    dbo:name "Research Seminar" ;
    dbo:number 802 ;
    dcterms:description "Research seminar" ;
    vivo:courseCredits 4 ;
    vivo:hasSubjectArea "BIOL" .

roboprof_data:BLDG_365 a vivo:Course ;
    dbo:name "Building Science" ;
    dbo:number 365 ;
    dcterms:description "Laboratory: 2 hours per week, alternate weeks" ;
    vivo:courseCredits 3 ;
    vivo:hasSubjectArea "BLDG" .

roboprof_data:BLDG_366 a vivo:Course ;
    dbo:name "Acoustics and Lighting" ;
    dbo:number 366 ;
    dcterms:description "Laboratory: 2 hours per week, alternate weeks" ;
    vivo:courseCredits 3 ;
    vivo:hasSubjectArea "BLDG" .

roboprof_data:BLDG_371 a vivo:Course ;
    dbo:name "Building Service Systems" ;
    dbo:number 371 ;
    dcterms:description "Laboratory: 2 hours per week, alternate weeks" ;
    vivo:courseCredits 3 ;
    vivo:hasSubjectArea "BLDG" .

roboprof_data:BLDG_390 a vivo:Course ;
    dbo:name "Building Engineering Design Project" ;
    dbo:number 390 ;
    dcterms:description "Laboratory: 2 hours per week, alternate weeks" ;
    vivo:courseCredits 4 ;
    vivo:hasSubjectArea "BLDG" .

roboprof_data:BLDG_463 a vivo:Course ;
    dbo:name "Building Envelope Design" ;
    dbo:number 463 ;
    dcterms:description "On-site investigation" ;
    vivo:courseCredits 3 ;
    vivo:hasSubjectArea "BLDG" .

roboprof_data:BLDG_471 a vivo:Course ;
    dbo:name "HVAC System Design" ;
    dbo:number 471 ;
    dcterms:description "Laboratory: 2 hours per week" ;
    vivo:courseCredits 4 ;
    vivo:hasSubjectArea "BLDG" .

roboprof_data:BLDG_476 a vivo:Course ;
    dbo:name "Thermal Analysis of Buildings" ;
    dbo:number 476 ;
    dcterms:description "Laboratory: 1 hour per week" ;
    vivo:courseCredits 4 ;
    vivo:hasSubjectArea "BLDG" .

roboprof_data:BLDG_490 a vivo:Course ;
    dbo:name "Capstone Building Engineering Design Project (also listed as BLDG 490A, BLDG 490B)" ;
    dbo:number 490 ;
    dcterms:description "capstone, team project" ;
    vivo:courseCredits 3 ;
    vivo:hasSubjectArea "BLDG" .

roboprof_data:BLDG_492 a vivo:Course ;
    dbo:name "Construction Processes" ;
    dbo:number 492 ;
    dcterms:description "Site visits" ;
    vivo:courseCredits 3 ;
    vivo:hasSubjectArea "BLDG" .

roboprof_data:BLDG_6071 a vivo:Course ;
    dbo:name "Wind Engineering and Building Aerodynamics" ;
    dbo:number 6071 ;
    dcterms:description "A case study or a project is required" ;
    vivo:courseCredits 4 ;
    vivo:hasSubjectArea "BLDG" .

roboprof_data:BLDG_6111 a vivo:Course ;
    dbo:name "Computer-Aided Building Operation" ;
    dbo:number 6111 ;
    dcterms:description "A project is required" ;
    vivo:courseCredits 3 ;
    vivo:hasSubjectArea "BLDG" .

roboprof_data:BLDG_6151 a vivo:Course ;
    dbo:name "Database Applications in Building and Civil Engineering" ;
    dbo:number 6151 ;
    dcterms:description "A project is required" ;
    vivo:courseCredits 3 ;
    vivo:hasSubjectArea "BLDG" .

roboprof_data:BLDG_6221 a vivo:Course ;
    dbo:name "Design of Computer-Aided Systems in Building and Civil Engineering" ;
    dbo:number 6221 ;
    dcterms:description "Project on implementation of a small scale computer-aided engineering system" ;
    vivo:courseCredits 4 ;
    vivo:hasSubjectArea "BLDG" .

roboprof_data:BLDG_6231 a vivo:Course ;
    dbo:name "Applications of Artificial Intelligence in Building and Civil Engineering" ;
    dbo:number 6231 ;
    dcterms:description "A project is required" ;
    vivo:courseCredits 3 ;
    vivo:hasSubjectArea "BLDG" .

roboprof_data:BLDG_6241 a vivo:Course ;
    dbo:name "Building Information Modelling in Construction" ;
    dbo:number 6241 ;
    dcterms:description "A project is required" ;
    vivo:courseCredits 4 ;
    vivo:hasSubjectArea "BLDG" .

roboprof_data:BLDG_6561 a vivo:Course ;
    dbo:name "Building Economics I" ;
    dbo:number 6561 ;
    dcterms:description "A project is required" ;
    vivo:courseCredits 4 ;
    vivo:hasSubjectArea "BLDG" .

roboprof_data:BLDG_6571 a vivo:Course ;
    dbo:name "Project Management" ;
    dbo:number 6571 ;
    dcterms:description "A project is required" ;
    vivo:courseCredits 3 ;
    vivo:hasSubjectArea "BLDG" .

roboprof_data:BLDG_6581 a vivo:Course ;
    dbo:name "Decision Analysis" ;
    dbo:number 6581 ;
    dcterms:description "A project is required" ;
    vivo:courseCredits 4 ;
    vivo:hasSubjectArea "BLDG" .

roboprof_data:BLDG_6591 a vivo:Course ;
    dbo:name "Computer-Aided Building Design" ;
    dbo:number 6591 ;
    dcterms:description "A project is required" ;
    vivo:courseCredits 3 ;
    vivo:hasSubjectArea "BLDG" .

roboprof_data:BLDG_6601 a vivo:Course ;
    dbo:name "Building Enclosure" ;
    dbo:number 6601 ;
    dcterms:description "A project is required" ;
    vivo:courseCredits 3 ;
    vivo:hasSubjectArea "BLDG" .

roboprof_data:BLDG_6611 a vivo:Course ;
    dbo:name "Building Science" ;
    dbo:number 6611 ;
    dcterms:description "A case study or a project is required" ;
    vivo:courseCredits 3 ;
    vivo:hasSubjectArea "BLDG" .

roboprof_data:BLDG_6621 a vivo:Course ;
    dbo:name "Modern Building Materials" ;
    dbo:number 6621 ;
    dcterms:description "A project is required" ;
    vivo:courseCredits 3 ;
    vivo:hasSubjectArea "BLDG" .

roboprof_data:BLDG_6641 a vivo:Course ;
    dbo:name "Industrialized Building" ;
    dbo:number 6641 ;
    dcterms:description "A case study & a project" ;
    vivo:courseCredits 3 ;
    vivo:hasSubjectArea "BLDG" .

roboprof_data:BLDG_6651 a vivo:Course ;
    dbo:name "Fire and Smoke Control in Buildings" ;
    dbo:number 6651 ;
    dcterms:description "A project is required" ;
    vivo:courseCredits 3 ;
    vivo:hasSubjectArea "BLDG" .

roboprof_data:BLDG_6661 a vivo:Course ;
    dbo:name "Hygrothermal Performance of the Building Envelope" ;
    dbo:number 6661 ;
    dcterms:description "A project is required" ;
    vivo:courseCredits 3 ;
    vivo:hasSubjectArea "BLDG" .

roboprof_data:BLDG_6701 a vivo:Course ;
    dbo:name "Building Environment" ;
    dbo:number 6701 ;
    dcterms:description "2 projects" ;
    vivo:courseCredits 3 ;
    vivo:hasSubjectArea "BLDG" .

roboprof_data:BLDG_6711 a vivo:Course ;
    dbo:name "Mechanical Systems in Building" ;
    dbo:number 6711 ;
    dcterms:description "A project is required" ;
    vivo:courseCredits 3 ;
    vivo:hasSubjectArea "BLDG" .

roboprof_data:BLDG_6721 a vivo:Course ;
    dbo:name "Building Acoustics" ;
    dbo:number 6721 ;
    dcterms:description "Case studies and a project are required" ;
    vivo:courseCredits 4 ;
    vivo:hasSubjectArea "BLDG" .

roboprof_data:BLDG_6731 a vivo:Course ;
    dbo:name "Building Illumination" ;
    dbo:number 6731 ;
    dcterms:description "A project is required" ;
    vivo:courseCredits 3 ;
    vivo:hasSubjectArea "BLDG" .

roboprof_data:BLDG_6741 a vivo:Course ;
    dbo:name "HVAC Control Systems" ;
    dbo:number 6741 ;
    dcterms:description "A project is required" ;
    vivo:courseCredits 4 ;
    vivo:hasSubjectArea "BLDG" .

roboprof_data:BLDG_6751 a vivo:Course ;
    dbo:name "Indoor Air Quality and Ventilation" ;
    dbo:number 6751 ;
    dcterms:description "A case study or project" ;
    vivo:courseCredits 4 ;
    vivo:hasSubjectArea "BLDG" .

roboprof_data:BLDG_6761 a vivo:Course ;
    dbo:name "Intelligent Buildings" ;
    dbo:number 6761 ;
    dcterms:description "A project is required" ;
    vivo:courseCredits 4 ;
    vivo:hasSubjectArea "BLDG" .

roboprof_data:BLDG_6781 a vivo:Course ;
    dbo:name "Energy Management in Buildings" ;
    dbo:number 6781 ;
    dcterms:description "A case study & project" ;
    vivo:courseCredits 4 ;
    vivo:hasSubjectArea "BLDG" .

roboprof_data:BLDG_6791 a vivo:Course ;
    dbo:name "Thermal Building Simulation" ;
    dbo:number 6791 ;
    dcterms:description "A project is required" ;
    vivo:courseCredits 4 ;
    vivo:hasSubjectArea "BLDG" .

roboprof_data:BLDG_6801 a vivo:Course ;
    dbo:name "Construction Planning and Control" ;
    dbo:number 6801 ;
    dcterms:description "A case study & project" ;
    vivo:courseCredits 4 ;
    vivo:hasSubjectArea "BLDG" .

roboprof_data:BLDG_6851 a vivo:Course ;
    dbo:name "Project Cost Estimating" ;
    dbo:number 6851 ;
    dcterms:description "A project is required" ;
    vivo:courseCredits 4 ;
    vivo:hasSubjectArea "BLDG" .

roboprof_data:BLDG_6861 a vivo:Course ;
    dbo:name "Simulations and Design of Construction Operations" ;
    dbo:number 6861 ;
    dcterms:description "A project is required" ;
    vivo:courseCredits 3 ;
    vivo:hasSubjectArea "BLDG" .

roboprof_data:BLDG_6951 a vivo:Course ;
    dbo:name "Solar Building Modelling and Design" ;
    dbo:number 6951 ;
    dcterms:description "A project is required" ;
    vivo:courseCredits 3 ;
    vivo:hasSubjectArea "BLDG" .

roboprof_data:BLDG_7401 a vivo:Course ;
    dbo:name "Dispersion of Building Exhaust" ;
    dbo:number 7401 ;
    dcterms:description "A case study or project is required" ;
    vivo:courseCredits 4 ;
    vivo:hasSubjectArea "BLDG" .

roboprof_data:BLDG_7511 a vivo:Course ;
    dbo:name "Integrated Building Design" ;
    dbo:number 7511 ;
    dcterms:description "A project is required" ;
    vivo:courseCredits 4 ;
    vivo:hasSubjectArea "BLDG" .

roboprof_data:BLDG_7521 a vivo:Course ;
    dbo:name "Advanced Computer-Aided Building Design" ;
    dbo:number 7521 ;
    dcterms:description "A project is required" ;
    vivo:courseCredits 4 ;
    vivo:hasSubjectArea "BLDG" .

roboprof_data:BLDG_7601 a vivo:Course ;
    dbo:name "Durability of Building Materials" ;
    dbo:number 7601 ;
    dcterms:description "A case study & project" ;
    vivo:courseCredits 4 ;
    vivo:hasSubjectArea "BLDG" .

roboprof_data:BLDG_7811 a vivo:Course ;
    dbo:name "Project Acquisition and Control" ;
    dbo:number 7811 ;
    dcterms:description "A project is required" ;
    vivo:courseCredits 4 ;
    vivo:hasSubjectArea "BLDG" .

roboprof_data:BLDG_7831 a vivo:Course ;
    dbo:name "Building Economics II" ;
    dbo:number 7831 ;
    dcterms:description "A project is required" ;
    vivo:courseCredits 3 ;
    vivo:hasSubjectArea "BLDG" .

roboprof_data:BLDG_7841 a vivo:Course ;
    dbo:name "Information Technology Applications in Construction" ;
    dbo:number 7841 ;
    dcterms:description "A project is required" ;
    vivo:courseCredits 3 ;
    vivo:hasSubjectArea "BLDG" .

roboprof_data:BLDG_7861 a vivo:Course ;
    dbo:name "Business Practices in Construction" ;
    dbo:number 7861 ;
    dcterms:description "A project is required" ;
    vivo:courseCredits 4 ;
    vivo:hasSubjectArea "BLDG" .

roboprof_data:BLDG_7871 a vivo:Course ;
    dbo:name "Construction Equipment Management" ;
    dbo:number 7871 ;
    dcterms:description "A project is required" ;
    vivo:courseCredits 4 ;
    vivo:hasSubjectArea "BLDG" .

roboprof_data:BSTA_445 a vivo:Course ;
    dbo:name "Statistical Software for Data Management and Analysis" ;
    dbo:number 445 ;
    dcterms:description "Lab work" ;
    vivo:courseCredits 3 ;
    vivo:hasSubjectArea "BSTA" .

roboprof_data:BSTA_450 a vivo:Course ;
    dbo:name "Statistical Models for Data Analysis" ;
    dbo:number 450 ;
    dcterms:description "Analyses of real-life data using statistical software packages" ;
    vivo:courseCredits 4 ;
    vivo:hasSubjectArea "BSTA" .

roboprof_data:BSTA_477 a vivo:Course ;
    dbo:name "Managerial Forecasting" ;
    dbo:number 477 ;
    dcterms:description "Business and economic databases are analyzed using statistical software packages" ;
    vivo:courseCredits 4 ;
    vivo:hasSubjectArea "BSTA" .

roboprof_data:BSTA_478 a vivo:Course ;
    dbo:name "Data Mining Techniques" ;
    dbo:number 478 ;
    dcterms:description "Practical experience" ;
    vivo:courseCredits 4 ;
    vivo:hasSubjectArea "BSTA" .

roboprof_data:BTM_430 a vivo:Course ;
    dbo:name "Enterprise Resources Planning and Technology Integration" ;
    dbo:number 430 ;
    dcterms:description "Integration of technological and business resources for analysis of practical business problems and processes via the use of enterprise resource planning applications" ;
    vivo:courseCredits 3 ;
    vivo:hasSubjectArea "BTM" .

roboprof_data:BTM_480 a vivo:Course ;
    dbo:name "Project Management" ;
    dbo:number 480 ;
    dcterms:description "Use of project management software and business cases" ;
    vivo:courseCredits 3 ;
    vivo:hasSubjectArea "BTM" .

roboprof_data:BTM_481 a vivo:Course ;
    dbo:name "Information Systems Analysis" ;
    dbo:number 481 ;
    dcterms:description "Analysis of real business processes for the development of requirements for information systems applications" ;
    vivo:courseCredits 3 ;
    vivo:hasSubjectArea "BTM" .

roboprof_data:BTM_495 a vivo:Course ;
    dbo:name "Information Systems Design and Implementation" ;
    dbo:number 495 ;
    dcterms:description "Designing and prototyping IT solutions for real-life projects" ;
    vivo:courseCredits 4 ;
    vivo:hasSubjectArea "BTM" .

roboprof_data:BTM_496 a vivo:Course ;
    dbo:name "Information Technology Strategy, Management and Sourcing" ;
    dbo:number 496 ;
    dcterms:description "Development of the request for proposal for information systems for real life business applications" ;
    vivo:courseCredits 3 ;
    vivo:hasSubjectArea "BTM" .

roboprof_data:BTM_633 a vivo:Course ;
    dbo:name "Strategic Management of Information Technology" ;
    dbo:number 633 ;
    dcterms:description "Students critically evaluate IT and business problems with a focus on strategic management of IT for competitive advantage." ;
    vivo:courseCredits 4 ;
    vivo:hasSubjectArea "BTM" .

roboprof_data:CART_451 a vivo:Course ;
    dbo:name "NETWORKED MEDIA STUDIO" ;
    dbo:number 451 ;
    dcterms:description "NaN"^^xsd:double ;
    vivo:courseCredits 3 ;
    vivo:hasSubjectArea "CART" .

roboprof_data:CATA_262 a vivo:Course ;
    dbo:name "Emergency Care in Sport and Exercise" ;
    dbo:number 262 ;
    dcterms:description "Laboratory" ;
    vivo:courseCredits 4 ;
    vivo:hasSubjectArea "CATA" .

roboprof_data:CATA_263 a vivo:Course ;
    dbo:name "Principles of Athletic Therapy" ;
    dbo:number 263 ;
    dcterms:description "Laboratory" ;
    vivo:courseCredits 3 ;
    vivo:hasSubjectArea "CATA" .

roboprof_data:CATA_337 a vivo:Course ;
    dbo:name "Assessment of the Upper and Lower Extremities" ;
    dbo:number 337 ;
    dcterms:description "Laboratory" ;
    vivo:courseCredits 3 ;
    vivo:hasSubjectArea "CATA" .

roboprof_data:CATA_339 a vivo:Course ;
    dbo:name "Rehabilitation of the Upper and Lower Extremities" ;
    dbo:number 339 ;
    dcterms:description "Laboratory" ;
    vivo:courseCredits 3 ;
    vivo:hasSubjectArea "CATA" .

roboprof_data:CATA_348 a vivo:Course ;
    dbo:name "Therapeutic Modalities in Sports Medicine" ;
    dbo:number 348 ;
    dcterms:description "Laboratory" ;
    vivo:courseCredits 4 ;
    vivo:hasSubjectArea "CATA" .

roboprof_data:CATA_365 a vivo:Course ;
    dbo:name "Athletic Therapy Field Internship I " ;
    dbo:number 365 ;
    dcterms:description "Internship" ;
    vivo:courseCredits 3 ;
    vivo:hasSubjectArea "CATA" .

roboprof_data:CATA_437 a vivo:Course ;
    dbo:name "Assessment of the Hip, Spine and Pelvis" ;
    dbo:number 437 ;
    dcterms:description "Laboratory" ;
    vivo:courseCredits 4 ;
    vivo:hasSubjectArea "CATA" .

roboprof_data:CATA_439 a vivo:Course ;
    dbo:name "Rehabilitation of the Hip, Spine and Pelvis" ;
    dbo:number 439 ;
    dcterms:description "Laboratory" ;
    vivo:courseCredits 4 ;
    vivo:hasSubjectArea "CATA" .

roboprof_data:CATA_441 a vivo:Course ;
    dbo:name "Concepts in Manual Therapy" ;
    dbo:number 441 ;
    dcterms:description "Laboratory" ;
    vivo:courseCredits 3 ;
    vivo:hasSubjectArea "CATA" .

roboprof_data:CATA_462 a vivo:Course ;
    dbo:name "Advanced Emergency Care" ;
    dbo:number 462 ;
    dcterms:description "Laboratory" ;
    vivo:courseCredits 3 ;
    vivo:hasSubjectArea "CATA" .

roboprof_data:CATA_475 a vivo:Course ;
    dbo:name "Athletic Therapy Clinical Internship I" ;
    dbo:number 475 ;
    dcterms:description "Internship" ;
    vivo:courseCredits 4 ;
    vivo:hasSubjectArea "CATA" .

roboprof_data:CATA_485 a vivo:Course ;
    dbo:name "Athletic Therapy Field Internship II" ;
    dbo:number 485 ;
    dcterms:description "Internship" ;
    vivo:courseCredits 4 ;
    vivo:hasSubjectArea "CATA" .

roboprof_data:CATA_495 a vivo:Course ;
    dbo:name "Athletic Therapy Clinical Internship II" ;
    dbo:number 495 ;
    dcterms:description "Internship" ;
    vivo:courseCredits 3 ;
    vivo:hasSubjectArea "CATA" .

roboprof_data:CERA_201 a vivo:Course ;
    dbo:name "Introduction to Ceramics" ;
    dbo:number 201 ;
    dcterms:description "An introduction to clay as an art medium employing the various techniques of forming, shaping, and decorating for firing and glazing." ;
    vivo:courseCredits 4 ;
    vivo:hasSubjectArea "CERA" .

roboprof_data:CERA_230 a vivo:Course ;
    dbo:name "Ceramics I " ;
    dbo:number 230 ;
    dcterms:description "An introduction to clay as an art medium employing the various techniques of forming, shaping, and decorating for firing and glazing." ;
    vivo:courseCredits 4 ;
    vivo:hasSubjectArea "CERA" .

roboprof_data:CERA_330 a vivo:Course ;
    dbo:name "Ceramics II " ;
    dbo:number 330 ;
    dcterms:description "An advanced course in technical and historical research in various ceramic processes with an emphasis on glazes and the use of different clay bodies." ;
    vivo:courseCredits 3 ;
    vivo:hasSubjectArea "CERA" .

roboprof_data:CERA_391 a vivo:Course ;
    dbo:name "Urban Clay" ;
    dbo:number 391 ;
    dcterms:description "This course expands the way ceramics can be experienced in relation to the city through the production of public artworks." ;
    vivo:courseCredits 4 ;
    vivo:hasSubjectArea "CERA" .

roboprof_data:CERA_392 a vivo:Course ;
    dbo:name "Surface Tension" ;
    dbo:number 392 ;
    dcterms:description "This course involves an indepth study of the ceramic surface including print and transfer techniques, and layering glaze through multiple firings. " ;
    vivo:courseCredits 4 ;
    vivo:hasSubjectArea "CERA" .

roboprof_data:CERA_398 a vivo:Course ;
    dbo:name "Special Topics in Ceramics" ;
    dbo:number 398 ;
    dcterms:description "A workshop/seminar, providing an opportunity for the study of specialized aspects of ceramics. " ;
    vivo:courseCredits 3 ;
    vivo:hasSubjectArea "CERA" .

roboprof_data:CERA_399 a vivo:Course ;
    dbo:name "Special Topics in Ceramics" ;
    dbo:number 399 ;
    dcterms:description "A workshop/seminar course providing an opportunity for the study of specialized aspects in ceramics." ;
    vivo:courseCredits 3 ;
    vivo:hasSubjectArea "CERA" .

roboprof_data:CERA_430 a vivo:Course ;
    dbo:name "Ceramics III" ;
    dbo:number 430 ;
    dcterms:description "The development of a body of personal work and a refinement of specific problems in clay." ;
    vivo:courseCredits 3 ;
    vivo:hasSubjectArea "CERA" .

roboprof_data:CERA_450 a vivo:Course ;
    dbo:name "Independent Study" ;
    dbo:number 450 ;
    dcterms:description "This course provides a limited number of students the opportunity to pursue advanced studies in ceramics under the supervision of a fulltime ceramics faculty member." ;
    vivo:courseCredits 3 ;
    vivo:hasSubjectArea "CERA" .

roboprof_data:CERA_451 a vivo:Course ;
    dbo:name "INDEPENDENT STUDY I",
        "Independent Study I" ;
    dbo:number 451 ;
    dcterms:description "NaN"^^xsd:double,
        "This course provides a limited number of students the opportunity to pursue advanced studies in ceramics under the supervision of a fulltime ceramics faculty member." ;
    vivo:courseCredits 4 ;
    vivo:hasSubjectArea "CERA" .

roboprof_data:CERA_452 a vivo:Course ;
    dbo:name "Independent Study II" ;
    dbo:number 452 ;
    dcterms:description "This course provides a limited number of students the opportunity to pursue advanced studies in ceramics under the supervision of a fulltime ceramics faculty member." ;
    vivo:courseCredits 3 ;
    vivo:hasSubjectArea "CERA" .

roboprof_data:CERA_498 a vivo:Course ;
    dbo:name "Special Topics in Ceramics" ;
    dbo:number 498 ;
    dcterms:description "An advanced studio course that provides an opportunity for the study of more specialized aspects of ceramics." ;
    vivo:courseCredits 4 ;
    vivo:hasSubjectArea "CERA" .

roboprof_data:CERA_499 a vivo:Course ;
    dbo:name "Special Topics in Ceramics" ;
    dbo:number 499 ;
    dcterms:description "An advanced studio course which provides an opportunity for the study of more specialized aspects of ceramics." ;
    vivo:courseCredits 3 ;
    vivo:hasSubjectArea "CERA" .

roboprof_data:CHEM_205 a vivo:Course ;
    dbo:name "General Chemistry I" ;
    dbo:number 205 ;
    dcterms:description "Laboratory" ;
    vivo:courseCredits 4 ;
    vivo:hasSubjectArea "CHEM" .

roboprof_data:CHEM_206 a vivo:Course ;
    dbo:name "General Chemistry II" ;
    dbo:number 206 ;
    dcterms:description "Laboratory" ;
    vivo:courseCredits 4 ;
    vivo:hasSubjectArea "CHEM" .

roboprof_data:CHEM_212 a vivo:Course ;
    dbo:name "Analytical Chemistry for Biologists" ;
    dbo:number 212 ;
    dcterms:description "Laboratory" ;
    vivo:courseCredits 3 ;
    vivo:hasSubjectArea "CHEM" .

roboprof_data:CHEM_217 a vivo:Course ;
    dbo:name "Introductory Analytical Chemistry I" ;
    dbo:number 217 ;
    dcterms:description "Laboratory" ;
    vivo:courseCredits 3 ;
    vivo:hasSubjectArea "CHEM" .

roboprof_data:CHEM_218 a vivo:Course ;
    dbo:name "Introductory Analytical Chemistry II" ;
    dbo:number 218 ;
    dcterms:description "Laboratory" ;
    vivo:courseCredits 3 ;
    vivo:hasSubjectArea "CHEM" .

roboprof_data:CHEM_221 a vivo:Course ;
    dbo:name "Introductory Organic Chemistry I" ;
    dbo:number 221 ;
    dcterms:description "Laboratory" ;
    vivo:courseCredits 4 ;
    vivo:hasSubjectArea "CHEM" .

roboprof_data:CHEM_222 a vivo:Course ;
    dbo:name "Introductory Organic Chemistry II" ;
    dbo:number 222 ;
    dcterms:description "Laboratory" ;
    vivo:courseCredits 3 ;
    vivo:hasSubjectArea "CHEM" .

roboprof_data:CHEM_235 a vivo:Course ;
    dbo:name "Physical Chemistry II: Kinetics of Chemical Reactions" ;
    dbo:number 235 ;
    dcterms:description "Laboratory" ;
    vivo:courseCredits 4 ;
    vivo:hasSubjectArea "CHEM" .

roboprof_data:CHEM_241 a vivo:Course ;
    dbo:name "Inorganic Chemistry I: Introduction to Periodicity and Valence Theory" ;
    dbo:number 241 ;
    dcterms:description "Laboratory" ;
    vivo:courseCredits 4 ;
    vivo:hasSubjectArea "CHEM" .

roboprof_data:CHEM_242 a vivo:Course ;
    dbo:name "Inorganic Chemistry II: The Chemistry of the Main Group Elements" ;
    dbo:number 242 ;
    dcterms:description "Laboratory" ;
    vivo:courseCredits 4 ;
    vivo:hasSubjectArea "CHEM" .

roboprof_data:CHEM_271 a vivo:Course ;
    dbo:name "Biochemistry I" ;
    dbo:number 271 ;
    dcterms:description "Laboratory" ;
    vivo:courseCredits 4 ;
    vivo:hasSubjectArea "CHEM" .

roboprof_data:CHEM_293 a vivo:Course ;
    dbo:name "Spectroscopy and Structure of Organic Compounds" ;
    dbo:number 293 ;
    dcterms:description "Laboratory" ;
    vivo:courseCredits 4 ;
    vivo:hasSubjectArea "CHEM" .

roboprof_data:CHEM_312 a vivo:Course ;
    dbo:name "Intermediate Analytical Chemistry" ;
    dbo:number 312 ;
    dcterms:description "Laboratory" ;
    vivo:courseCredits 4 ;
    vivo:hasSubjectArea "CHEM" .

roboprof_data:CHEM_324 a vivo:Course ;
    dbo:name "Organic Chemistry III: Organic Reactions" ;
    dbo:number 324 ;
    dcterms:description "Laboratory" ;
    vivo:courseCredits 4 ;
    vivo:hasSubjectArea "CHEM" .

roboprof_data:CHEM_325 a vivo:Course ;
    dbo:name "Organic Chemistry IV: Organic Structure and Stereochemistry" ;
    dbo:number 325 ;
    dcterms:description "Laboratory" ;
    vivo:courseCredits 4 ;
    vivo:hasSubjectArea "CHEM" .

roboprof_data:CHEM_333 a vivo:Course ;
    dbo:name "Introduction to Quantum Theory" ;
    dbo:number 333 ;
    dcterms:description "he course introduces students to the concept of quantum mechanics and the electronic structure of atoms and molecules. Topics include the origins and postulates of quantum theory, the Schrdinger equation and applications to simple systems such as the harmonic oscillator, rigid rotor and the hydrogen atom. The course looks at the quantum mechanical treatment of the chemical bond and provides an introduction to spectroscopy." ;
    vivo:courseCredits 3 ;
    vivo:hasSubjectArea "CHEM" .

roboprof_data:CHEM_335 a vivo:Course ;
    dbo:name "Biophysical Chemistry" ;
    dbo:number 335 ;
    dcterms:description "Laboratory" ;
    vivo:courseCredits 3 ;
    vivo:hasSubjectArea "CHEM" .

roboprof_data:CHEM_341 a vivo:Course ;
    dbo:name "Inorganic Chemistry III: The Transition Metals" ;
    dbo:number 341 ;
    dcterms:description "Laboratory" ;
    vivo:courseCredits 4 ;
    vivo:hasSubjectArea "CHEM" .

roboprof_data:CHEM_375 a vivo:Course ;
    dbo:name "Biochemistry II" ;
    dbo:number 375 ;
    dcterms:description "Laboratory" ;
    vivo:courseCredits 4 ;
    vivo:hasSubjectArea "CHEM" .

roboprof_data:CHEM_419 a vivo:Course ;
    dbo:name "Independent Study and Practicum" ;
    dbo:number 419 ;
    dcterms:description "Practicum" ;
    vivo:courseCredits 4 ;
    vivo:hasSubjectArea "CHEM" .

roboprof_data:CHEM_431 a vivo:Course ;
    dbo:name "Computational Chemistry for Chemists and Biochemists" ;
    dbo:number 431 ;
    dcterms:description "Hands-on experience, Laboratory" ;
    vivo:courseCredits 3 ;
    vivo:hasSubjectArea "CHEM" .

roboprof_data:CHEM_436 a vivo:Course ;
    dbo:name "Molecular Modelling of Proteins" ;
    dbo:number 436 ;
    dcterms:description "Hands-on introduction, Computer laboratory" ;
    vivo:courseCredits 3 ;
    vivo:hasSubjectArea "CHEM" .

roboprof_data:CHEM_450 a vivo:Course ;
    dbo:name "Research Project and Thesis " ;
    dbo:number 450 ;
    dcterms:description "NaN"^^xsd:double ;
    vivo:courseCredits 3 ;
    vivo:hasSubjectArea "CHEM" .

roboprof_data:CHEM_477 a vivo:Course ;
    dbo:name "Advanced Laboratory in Biochemistry" ;
    dbo:number 477 ;
    dcterms:description "Laboratory" ;
    vivo:courseCredits 3 ;
    vivo:hasSubjectArea "CHEM" .

roboprof_data:CHEM_487 a vivo:Course ;
    dbo:name "Capstone Seminar in Environmental Science " ;
    dbo:number 487 ;
    dcterms:description "NaN"^^xsd:double ;
    vivo:courseCredits 3 ;
    vivo:hasSubjectArea "CHEM" .

roboprof_data:CHEM_614 a vivo:Course ;
    dbo:name "Modern Aspects of Practical Mass Spectrometry" ;
    dbo:number 614 ;
    dcterms:description "Independent mass spectrometry project" ;
    vivo:courseCredits 3 ;
    vivo:hasSubjectArea "CHEM" .

roboprof_data:CHEM_631 a vivo:Course ;
    dbo:name "Computational Chemistry" ;
    dbo:number 631 ;
    dcterms:description "Laboratory" ;
    vivo:courseCredits 3 ;
    vivo:hasSubjectArea "CHEM" .

roboprof_data:CHEM_651 a vivo:Course ;
    dbo:name "Nanochemistry" ;
    dbo:number 651 ;
    dcterms:description "Term project carried out using the nanoscience facilities held in the department research labs" ;
    vivo:courseCredits 4 ;
    vivo:hasSubjectArea "CHEM" .

roboprof_data:CHEM_692 a vivo:Course ;
    dbo:name "Experimental Protein Chemistry" ;
    dbo:number 692 ;
    dcterms:description "Hands-on course, Laboratory" ;
    vivo:courseCredits 3 ;
    vivo:hasSubjectArea "CHEM" .

roboprof_data:CHST_605 a vivo:Course ;
    dbo:name "Quantitative Methods of Inquiry" ;
    dbo:number 605 ;
    dcterms:description "Laboratory work, practical experience" ;
    vivo:courseCredits 4 ;
    vivo:hasSubjectArea "CHST" .

roboprof_data:CHST_606 a vivo:Course ;
    dbo:name "Qualitative Methods of Inquiry" ;
    dbo:number 606 ;
    dcterms:description "Laboratory work, practical experience" ;
    vivo:courseCredits 3 ;
    vivo:hasSubjectArea "CHST" .

roboprof_data:CHST_608 a vivo:Course ;
    dbo:name "Field Observations" ;
    dbo:number 608 ;
    dcterms:description "2-3 hours weekly in an appropriate setting" ;
    vivo:courseCredits 4 ;
    vivo:hasSubjectArea "CHST" .

roboprof_data:CHST_618 a vivo:Course ;
    dbo:name "Childhood Settings" ;
    dbo:number 618 ;
    dcterms:description "Field trips to different types of settings" ;
    vivo:courseCredits 4 ;
    vivo:hasSubjectArea "CHST" .

roboprof_data:CIVI_231 a vivo:Course ;
    dbo:name "Geology for Civil Engineers" ;
    dbo:number 231 ;
    dcterms:description "Site investigation" ;
    vivo:courseCredits 4 ;
    vivo:hasSubjectArea "CIVI" .

roboprof_data:CIVI_321 a vivo:Course ;
    dbo:name "Engineering Materials" ;
    dbo:number 321 ;
    dcterms:description "Laboratory: 3 hours per week, alternate weeks" ;
    vivo:courseCredits 3 ;
    vivo:hasSubjectArea "CIVI" .

roboprof_data:CIVI_361 a vivo:Course ;
    dbo:name "Introduction to Environmental Engineering" ;
    dbo:number 361 ;
    dcterms:description "Laboratory: 2 hours per week, alternate weeks" ;
    vivo:courseCredits 4 ;
    vivo:hasSubjectArea "CIVI" .

roboprof_data:CIVI_381 a vivo:Course ;
    dbo:name "Hydraulics" ;
    dbo:number 381 ;
    dcterms:description "Laboratory: 2 hours per week, alternate weeks" ;
    vivo:courseCredits 3 ;
    vivo:hasSubjectArea "CIVI" .

roboprof_data:CIVI_382 a vivo:Course ;
    dbo:name "Water Resources Engineering" ;
    dbo:number 382 ;
    dcterms:description "Laboratory: 2 hours per week, alternate weeks" ;
    vivo:courseCredits 4 ;
    vivo:hasSubjectArea "CIVI" .

roboprof_data:CIVI_390 a vivo:Course ;
    dbo:name "Civil Engineering Design Project" ;
    dbo:number 390 ;
    dcterms:description "Team project, Laboratory: 2 hours per week, alternate weeks" ;
    vivo:courseCredits 4 ;
    vivo:hasSubjectArea "CIVI" .

roboprof_data:CIVI_432 a vivo:Course ;
    dbo:name "Soil Mechanics" ;
    dbo:number 432 ;
    dcterms:description "Laboratory: 2 hours per week, alternate weeks" ;
    vivo:courseCredits 3 ;
    vivo:hasSubjectArea "CIVI" .

roboprof_data:CIVI_440 a vivo:Course ;
    dbo:name "Computer Applications in Civil Engineering Practice" ;
    dbo:number 440 ;
    dcterms:description "Laboratory: 2 hours per week, alternate weeks" ;
    vivo:courseCredits 3 ;
    vivo:hasSubjectArea "CIVI" .

roboprof_data:CIVI_453 a vivo:Course ;
    dbo:name "Design of Reinforced Concrete Structures" ;
    dbo:number 453 ;
    dcterms:description "Laboratory: 2 hours per week, alternate weeks" ;
    vivo:courseCredits 4 ;
    vivo:hasSubjectArea "CIVI" .

roboprof_data:CIVI_454 a vivo:Course ;
    dbo:name "Design of Steel Structures" ;
    dbo:number 454 ;
    dcterms:description "Design project, Laboratory: 2 hours per week, alternate weeks" ;
    vivo:courseCredits 4 ;
    vivo:hasSubjectArea "CIVI" .

roboprof_data:CIVI_465 a vivo:Course ;
    dbo:name "Water Pollution and Control" ;
    dbo:number 465 ;
    dcterms:description "Laboratory: 2 hours per week, alternate weeks" ;
    vivo:courseCredits 3 ;
    vivo:hasSubjectArea "CIVI" .

roboprof_data:CIVI_469 a vivo:Course ;
    dbo:name "Geo-Environmental Engineering" ;
    dbo:number 469 ;
    dcterms:description "Laboratory: 2 hours per week, alternate weeks" ;
    vivo:courseCredits 3 ;
    vivo:hasSubjectArea "CIVI" .

roboprof_data:CIVI_484 a vivo:Course ;
    dbo:name "Hydraulic Engineering" ;
    dbo:number 484 ;
    dcterms:description "Laboratory: 2 hours per week, alternate weeks" ;
    vivo:courseCredits 3 ;
    vivo:hasSubjectArea "CIVI" .

roboprof_data:CIVI_6001 a vivo:Course ;
    dbo:name "Advanced Reinforced Concrete" ;
    dbo:number 6001 ;
    dcterms:description "A project is required" ;
    vivo:courseCredits 3 ;
    vivo:hasSubjectArea "CIVI" .

roboprof_data:CIVI_6011 a vivo:Course ;
    dbo:name "Precast and Prestressed Concrete Structures" ;
    dbo:number 6011 ;
    dcterms:description "A project is required" ;
    vivo:courseCredits 3 ;
    vivo:hasSubjectArea "CIVI" .

roboprof_data:CIVI_6021 a vivo:Course ;
    dbo:name "Durability of Concrete Materials" ;
    dbo:number 6021 ;
    dcterms:description "A project is required" ;
    vivo:courseCredits 4 ;
    vivo:hasSubjectArea "CIVI" .

roboprof_data:CIVI_6031 a vivo:Course ;
    dbo:name "Seismic Assessment and Retrofit of Structures" ;
    dbo:number 6031 ;
    dcterms:description "Case studies & a project are required" ;
    vivo:courseCredits 4 ;
    vivo:hasSubjectArea "CIVI" .

roboprof_data:CIVI_6051 a vivo:Course ;
    dbo:name "Design of Industrial Structures" ;
    dbo:number 6051 ;
    dcterms:description "A case study & project" ;
    vivo:courseCredits 3 ;
    vivo:hasSubjectArea "CIVI" .

roboprof_data:CIVI_6061 a vivo:Course ;
    dbo:name "Structural Health Monitoring" ;
    dbo:number 6061 ;
    dcterms:description "Field application, A project is required" ;
    vivo:courseCredits 3 ;
    vivo:hasSubjectArea "CIVI" .

roboprof_data:CIVI_6071 a vivo:Course ;
    dbo:name "Advanced Steel Structures Design" ;
    dbo:number 6071 ;
    dcterms:description "A project is required" ;
    vivo:courseCredits 4 ;
    vivo:hasSubjectArea "CIVI" .

roboprof_data:CIVI_6101 a vivo:Course ;
    dbo:name "Planning and Design of Bridges" ;
    dbo:number 6101 ;
    dcterms:description "A project is required" ;
    vivo:courseCredits 4 ;
    vivo:hasSubjectArea "CIVI" .

roboprof_data:CIVI_6301 a vivo:Course ;
    dbo:name "Hydrology" ;
    dbo:number 6301 ;
    dcterms:description "A case study & a project are required" ;
    vivo:courseCredits 3 ;
    vivo:hasSubjectArea "CIVI" .

roboprof_data:CIVI_6331 a vivo:Course ;
    dbo:name "Hydraulic Engineering" ;
    dbo:number 6331 ;
    dcterms:description "A case study & a project are required" ;
    vivo:courseCredits 4 ;
    vivo:hasSubjectArea "CIVI" .

roboprof_data:CIVI_6381 a vivo:Course ;
    dbo:name "Hydraulic Structures" ;
    dbo:number 6381 ;
    dcterms:description "A project is required" ;
    vivo:courseCredits 4 ;
    vivo:hasSubjectArea "CIVI" .

roboprof_data:CIVI_6401 a vivo:Course ;
    dbo:name "Transportation Systems Analysis" ;
    dbo:number 6401 ;
    dcterms:description "A project is required" ;
    vivo:courseCredits 4 ;
    vivo:hasSubjectArea "CIVI" .

roboprof_data:CIVI_6411 a vivo:Course ;
    dbo:name "Urban Transportation Planning" ;
    dbo:number 6411 ;
    dcterms:description "A project is required" ;
    vivo:courseCredits 4 ;
    vivo:hasSubjectArea "CIVI" .

roboprof_data:CIVI_6441 a vivo:Course ;
    dbo:name "Traffic Engineering" ;
    dbo:number 6441 ;
    dcterms:description "A project is required" ;
    vivo:courseCredits 3 ;
    vivo:hasSubjectArea "CIVI" .

roboprof_data:CIVI_6451 a vivo:Course ;
    dbo:name "Pavement Design" ;
    dbo:number 6451 ;
    dcterms:description "A project is required" ;
    vivo:courseCredits 4 ;
    vivo:hasSubjectArea "CIVI" .

roboprof_data:CIVI_6461 a vivo:Course ;
    dbo:name "Pavement Management Systems" ;
    dbo:number 6461 ;
    dcterms:description "A project is required" ;
    vivo:courseCredits 4 ;
    vivo:hasSubjectArea "CIVI" .

roboprof_data:CIVI_6481 a vivo:Course ;
    dbo:name "Sustainable Management of Industrial Waste" ;
    dbo:number 6481 ;
    dcterms:description "A project is required" ;
    vivo:courseCredits 4 ;
    vivo:hasSubjectArea "CIVI" .

roboprof_data:CIVI_6491 a vivo:Course ;
    dbo:name "Engineering Aspects of Site Remediation" ;
    dbo:number 6491 ;
    dcterms:description "Lab demonstrations, A project is required" ;
    vivo:courseCredits 4 ;
    vivo:hasSubjectArea "CIVI" .

roboprof_data:CIVI_6501 a vivo:Course ;
    dbo:name "Foundation Engineering" ;
    dbo:number 6501 ;
    dcterms:description "A project is required" ;
    vivo:courseCredits 3 ;
    vivo:hasSubjectArea "CIVI" .

roboprof_data:CIVI_6521 a vivo:Course ;
    dbo:name "Soil Behaviour" ;
    dbo:number 6521 ;
    dcterms:description "A project is required" ;
    vivo:courseCredits 3 ;
    vivo:hasSubjectArea "CIVI" .

roboprof_data:CIVI_6531 a vivo:Course ;
    dbo:name "Soil Testing and Properties" ;
    dbo:number 6531 ;
    dcterms:description "A project is required" ;
    vivo:courseCredits 3 ;
    vivo:hasSubjectArea "CIVI" .

roboprof_data:CIVI_6541 a vivo:Course ;
    dbo:name "Reinforced Earth" ;
    dbo:number 6541 ;
    dcterms:description "A project is required" ;
    vivo:courseCredits 4 ;
    vivo:hasSubjectArea "CIVI" .

roboprof_data:CIVI_6601 a vivo:Course ;
    dbo:name "Modelling in Building and Environmental Engineering" ;
    dbo:number 6601 ;
    dcterms:description "A case study and project" ;
    vivo:courseCredits 4 ;
    vivo:hasSubjectArea "CIVI" .

roboprof_data:CIVI_6611 a vivo:Course ;
    dbo:name "Environmental Engineering" ;
    dbo:number 6611 ;
    dcterms:description "A case study and a project are required" ;
    vivo:courseCredits 3 ;
    vivo:hasSubjectArea "CIVI" .

roboprof_data:CIVI_6621 a vivo:Course ;
    dbo:name "Engineering Aspects of Biological Treatment of Water and Air" ;
    dbo:number 6621 ;
    dcterms:description "Lab demonstration, case study and project" ;
    vivo:courseCredits 4 ;
    vivo:hasSubjectArea "CIVI" .

roboprof_data:CIVI_6631 a vivo:Course ;
    dbo:name "Hazardous Material Management and Transportation" ;
    dbo:number 6631 ;
    dcterms:description "A project is required" ;
    vivo:courseCredits 3 ;
    vivo:hasSubjectArea "CIVI" .

roboprof_data:CIVI_6641 a vivo:Course ;
    dbo:name "Unit Operations in Environmental Engineering" ;
    dbo:number 6641 ;
    dcterms:description "A case study and a project are required" ;
    vivo:courseCredits 4 ;
    vivo:hasSubjectArea "CIVI" .

roboprof_data:CIVI_6651 a vivo:Course ;
    dbo:name "Water Pollution and Control" ;
    dbo:number 6651 ;
    dcterms:description "A case study and a project are required" ;
    vivo:courseCredits 3 ;
    vivo:hasSubjectArea "CIVI" .

roboprof_data:CIVI_6661 a vivo:Course ;
    dbo:name "Environmental Impact Assessment" ;
    dbo:number 6661 ;
    dcterms:description "Case studies and project" ;
    vivo:courseCredits 4 ;
    vivo:hasSubjectArea "CIVI" .

roboprof_data:CIVI_6671 a vivo:Course ;
    dbo:name "Fate and Transport of Contaminants in the Environment" ;
    dbo:number 6671 ;
    dcterms:description "A project is required" ;
    vivo:courseCredits 4 ;
    vivo:hasSubjectArea "CIVI" .

roboprof_data:CIVI_6681 a vivo:Course ;
    dbo:name "Environmental Nanotechnology" ;
    dbo:number 6681 ;
    dcterms:description "A project is required" ;
    vivo:courseCredits 4 ;
    vivo:hasSubjectArea "CIVI" .

roboprof_data:CIVI_6691 a vivo:Course ;
    dbo:name "Greenhouse Gases and Control" ;
    dbo:number 6691 ;
    dcterms:description "A project is required" ;
    vivo:courseCredits 3 ;
    vivo:hasSubjectArea "CIVI" .

roboprof_data:CIVI_6711 a vivo:Course ;
    dbo:name "Asset Management for Sustainable Civil Infrastructure" ;
    dbo:number 6711 ;
    dcterms:description "A project is required" ;
    vivo:courseCredits 3 ;
    vivo:hasSubjectArea "CIVI" .

roboprof_data:CIVI_7001 a vivo:Course ;
    dbo:name "Earthquake Engineering" ;
    dbo:number 7001 ;
    dcterms:description "A project is required" ;
    vivo:courseCredits 4 ;
    vivo:hasSubjectArea "CIVI" .

roboprof_data:CIVI_7031 a vivo:Course ;
    dbo:name "Dynamics of Foundations" ;
    dbo:number 7031 ;
    dcterms:description "A project is required" ;
    vivo:courseCredits 4 ;
    vivo:hasSubjectArea "CIVI" .

roboprof_data:CIVI_7101 a vivo:Course ;
    dbo:name "Theory and Design of Orthotropic Bridges" ;
    dbo:number 7101 ;
    dcterms:description "A project is required" ;
    vivo:courseCredits 3 ;
    vivo:hasSubjectArea "CIVI" .

roboprof_data:CIVI_7111 a vivo:Course ;
    dbo:name "Theory and Design of Modern Bridge Systems" ;
    dbo:number 7111 ;
    dcterms:description "A project is required" ;
    vivo:courseCredits 3 ;
    vivo:hasSubjectArea "CIVI" .

roboprof_data:CIVI_7121 a vivo:Course ;
    dbo:name "Cable Stayed Bridges" ;
    dbo:number 7121 ;
    dcterms:description "A project is required" ;
    vivo:courseCredits 3 ;
    vivo:hasSubjectArea "CIVI" .

roboprof_data:CIVI_7311 a vivo:Course ;
    dbo:name "Advanced Analysis of Groundwater Flow and Contamination" ;
    dbo:number 7311 ;
    dcterms:description "A project is required" ;
    vivo:courseCredits 3 ;
    vivo:hasSubjectArea "CIVI" .

roboprof_data:CIVI_7401 a vivo:Course ;
    dbo:name "Design of Transportation Terminals" ;
    dbo:number 7401 ;
    dcterms:description "A project is required" ;
    vivo:courseCredits 4 ;
    vivo:hasSubjectArea "CIVI" .

roboprof_data:CIVI_7901 a vivo:Course ;
    dbo:name "Environmental Engineering Research Project" ;
    dbo:number 7901 ;
    dcterms:description "Research project, supervision of full-time faculty member" ;
    vivo:courseCredits 3 ;
    vivo:hasSubjectArea "CIVI" .

roboprof_data:CLAS_370 a vivo:Course ;
    dbo:name "Practicum in Archaeology" ;
    dbo:number 370 ;
    dcterms:description "At least 1 month in the field" ;
    vivo:courseCredits 3 ;
    vivo:hasSubjectArea "CLAS" .

roboprof_data:CLAS_383 a vivo:Course ;
    dbo:name "Intermediate Ancient Greek I: Prose" ;
    dbo:number 383 ;
    dcterms:description "NaN"^^xsd:double ;
    vivo:courseCredits 3 ;
    vivo:hasSubjectArea "CLAS" .

roboprof_data:CLAS_384 a vivo:Course ;
    dbo:name "Intermediate Ancient Greek II: Poetry" ;
    dbo:number 384 ;
    dcterms:description "NaN"^^xsd:double ;
    vivo:courseCredits 4 ;
    vivo:hasSubjectArea "CLAS" .

roboprof_data:CLAS_391 a vivo:Course ;
    dbo:name "Intermediate Latin I: Prose" ;
    dbo:number 391 ;
    dcterms:description "NaN"^^xsd:double ;
    vivo:courseCredits 3 ;
    vivo:hasSubjectArea "CLAS" .

roboprof_data:CLAS_392 a vivo:Course ;
    dbo:name "Intermediate Latin II: Poetry" ;
    dbo:number 392 ;
    dcterms:description "NaN"^^xsd:double ;
    vivo:courseCredits 3 ;
    vivo:hasSubjectArea "CLAS" .

roboprof_data:CLAS_410 a vivo:Course ;
    dbo:name "Advanced Ancient Greek I: Prose" ;
    dbo:number 410 ;
    dcterms:description "NaN"^^xsd:double ;
    vivo:courseCredits 4 ;
    vivo:hasSubjectArea "CLAS" .

roboprof_data:CLAS_411 a vivo:Course ;
    dbo:name "Advanced Ancient Greek II: Poetry" ;
    dbo:number 411 ;
    dcterms:description "NaN"^^xsd:double ;
    vivo:courseCredits 4 ;
    vivo:hasSubjectArea "CLAS" .

roboprof_data:CLAS_420 a vivo:Course ;
    dbo:name "Advanced Latin I: Prose" ;
    dbo:number 420 ;
    dcterms:description "NaN"^^xsd:double ;
    vivo:courseCredits 3 ;
    vivo:hasSubjectArea "CLAS" .

roboprof_data:CLAS_421 a vivo:Course ;
    dbo:name "Advanced Latin II: Poetry" ;
    dbo:number 421 ;
    dcterms:description "NaN"^^xsd:double ;
    vivo:courseCredits 4 ;
    vivo:hasSubjectArea "CLAS" .

roboprof_data:CLAS_460 a vivo:Course ;
    dbo:name "Ancient Pottery:  History, Analysis and Interpretation" ;
    dbo:number 460 ;
    dcterms:description "Artifact handling, materials analysis" ;
    vivo:courseCredits 3 ;
    vivo:hasSubjectArea "CLAS" .

roboprof_data:CLAS_470 a vivo:Course ;
    dbo:name "Advanced Seminar in Archaeology" ;
    dbo:number 470 ;
    dcterms:description "Artifact and materials analysis" ;
    vivo:courseCredits 4 ;
    vivo:hasSubjectArea "CLAS" .

roboprof_data:CLAS_490 a vivo:Course ;
    dbo:name "Honours Thesis" ;
    dbo:number 490 ;
    dcterms:description "NaN"^^xsd:double ;
    vivo:courseCredits 3 ;
    vivo:hasSubjectArea "CLAS" .

roboprof_data:COEN_212 a vivo:Course ;
    dbo:name "Digital Systems Design I" ;
    dbo:number 212 ;
    dcterms:description "Laboratory: 15 hours total" ;
    vivo:courseCredits 3,
        4 ;
    vivo:hasSubjectArea "COEN" .

roboprof_data:COEN_311 a vivo:Course ;
    dbo:name "Computer Organization and Software" ;
    dbo:number 311 ;
    dcterms:description "Laboratory: 15 hours total" ;
    vivo:courseCredits 3 ;
    vivo:hasSubjectArea "COEN" .

roboprof_data:COEN_313 a vivo:Course ;
    dbo:name "Digital Systems Design II" ;
    dbo:number 313 ;
    dcterms:description "Laboratory: 15 hours total" ;
    vivo:courseCredits 4 ;
    vivo:hasSubjectArea "COEN" .

roboprof_data:COEN_315 a vivo:Course ;
    dbo:name "Digital Electronics" ;
    dbo:number 315 ;
    dcterms:description "Laboratory: 15 hours total" ;
    vivo:courseCredits 3 ;
    vivo:hasSubjectArea "COEN" .

roboprof_data:COEN_316 a vivo:Course ;
    dbo:name "Computer Architecture and Design" ;
    dbo:number 316 ;
    dcterms:description "Laboratory: 15 hours total" ;
    vivo:courseCredits 3 ;
    vivo:hasSubjectArea "COEN" .

roboprof_data:COEN_317 a vivo:Course ;
    dbo:name "Microprocessor Systems" ;
    dbo:number 317 ;
    dcterms:description "Laboratory: 15 hours total" ;
    vivo:courseCredits 4 ;
    vivo:hasSubjectArea "COEN" .

roboprof_data:COEN_345 a vivo:Course ;
    dbo:name "Software Testing and Validation" ;
    dbo:number 345 ;
    dcterms:description "Laboratory: 15 hours total" ;
    vivo:courseCredits 3 ;
    vivo:hasSubjectArea "COEN" .

roboprof_data:COEN_346 a vivo:Course ;
    dbo:name "Operating Systems" ;
    dbo:number 346 ;
    dcterms:description "Laboratory: 15 hours total" ;
    vivo:courseCredits 4 ;
    vivo:hasSubjectArea "COEN" .

roboprof_data:COEN_390 a vivo:Course ;
    dbo:name "Computer Engineering Product Design Project" ;
    dbo:number 390 ;
    dcterms:description "Team project, develop system/device, equivalent laboratory time: 6 hours per week" ;
    vivo:courseCredits 4 ;
    vivo:hasSubjectArea "COEN" .

roboprof_data:COEN_421 a vivo:Course ;
    dbo:name "Embedded Systems Design" ;
    dbo:number 421 ;
    dcterms:description "Laboratory: 30 hours total" ;
    vivo:courseCredits 3 ;
    vivo:hasSubjectArea "COEN" .

roboprof_data:COEN_445 a vivo:Course ;
    dbo:name "Communication Networks and Protocols" ;
    dbo:number 445 ;
    dcterms:description "Laboratory: 15 hours total" ;
    vivo:courseCredits 3 ;
    vivo:hasSubjectArea "COEN" .

roboprof_data:COEN_451 a vivo:Course ;
    dbo:name "VLSI Circuit Design" ;
    dbo:number 451 ;
    dcterms:description "Laboratory: 30 hours total" ;
    vivo:courseCredits 3 ;
    vivo:hasSubjectArea "COEN" .

roboprof_data:COEN_490 a vivo:Course ;
    dbo:name "Capstone Computer Engineering Design Project" ;
    dbo:number 490 ;
    dcterms:description "capstone, group project" ;
    vivo:courseCredits 3 ;
    vivo:hasSubjectArea "COEN" .

roboprof_data:COEN_6211 a vivo:Course ;
    dbo:name "Biological Computing and Synthetic Biology" ;
    dbo:number 6211 ;
    dcterms:description "A project is required" ;
    vivo:courseCredits 4 ;
    vivo:hasSubjectArea "COEN" .

roboprof_data:COEN_6311 a vivo:Course ;
    dbo:name "Software Engineering" ;
    dbo:number 6311 ;
    dcterms:description "A project is required" ;
    vivo:courseCredits 4 ;
    vivo:hasSubjectArea "COEN" .

roboprof_data:COEN_6312 a vivo:Course ;
    dbo:name "Model-Driven Software Engineering" ;
    dbo:number 6312 ;
    dcterms:description "A project is required" ;
    vivo:courseCredits 4 ;
    vivo:hasSubjectArea "COEN" .

roboprof_data:COEN_6313 a vivo:Course ;
    dbo:name "Programming on the Cloud" ;
    dbo:number 6313 ;
    dcterms:description "A project is required" ;
    vivo:courseCredits 4 ;
    vivo:hasSubjectArea "COEN" .

roboprof_data:COEN_6321 a vivo:Course ;
    dbo:name "Applied Evolutionary and Learning Algorithms" ;
    dbo:number 6321 ;
    dcterms:description "A project is required" ;
    vivo:courseCredits 4 ;
    vivo:hasSubjectArea "COEN" .

roboprof_data:COEN_6331 a vivo:Course ;
    dbo:name "Neural Networks" ;
    dbo:number 6331 ;
    dcterms:description "A project is required" ;
    vivo:courseCredits 4 ;
    vivo:hasSubjectArea "COEN" .

roboprof_data:COEN_6341 a vivo:Course ;
    dbo:name "Embedded System Modelling" ;
    dbo:number 6341 ;
    dcterms:description "A project is required" ;
    vivo:courseCredits 3 ;
    vivo:hasSubjectArea "COEN" .

roboprof_data:COEN_6501 a vivo:Course ;
    dbo:name "Digital System Design and Synthesis" ;
    dbo:number 6501 ;
    dcterms:description "Project involving system design and modelling, a project is required" ;
    vivo:courseCredits 3 ;
    vivo:hasSubjectArea "COEN" .

roboprof_data:COEN_6511 a vivo:Course ;
    dbo:name "VLSI Circuit Design" ;
    dbo:number 6511 ;
    dcterms:description "A project is required" ;
    vivo:courseCredits 4 ;
    vivo:hasSubjectArea "COEN" .

roboprof_data:COEN_6521 a vivo:Course ;
    dbo:name "Design for Testability" ;
    dbo:number 6521 ;
    dcterms:description "A project is required" ;
    vivo:courseCredits 4 ;
    vivo:hasSubjectArea "COEN" .

roboprof_data:COEN_6531 a vivo:Course ;
    dbo:name "ASIC Synthesis" ;
    dbo:number 6531 ;
    dcterms:description "A project is required" ;
    vivo:courseCredits 4 ;
    vivo:hasSubjectArea "COEN" .

roboprof_data:COEN_6541 a vivo:Course ;
    dbo:name "Functional Hardware Verification" ;
    dbo:number 6541 ;
    dcterms:description "A project is required" ;
    vivo:courseCredits 3 ;
    vivo:hasSubjectArea "COEN" .

roboprof_data:COEN_6551 a vivo:Course ;
    dbo:name "Formal Hardware Verification" ;
    dbo:number 6551 ;
    dcterms:description "A project is required" ;
    vivo:courseCredits 4 ;
    vivo:hasSubjectArea "COEN" .

roboprof_data:COEN_6611 a vivo:Course ;
    dbo:name "Real-time Systems" ;
    dbo:number 6611 ;
    dcterms:description "A project is required" ;
    vivo:courseCredits 4 ;
    vivo:hasSubjectArea "COEN" .

roboprof_data:COEN_6711 a vivo:Course ;
    dbo:name "Microprocessors and Their Applications" ;
    dbo:number 6711 ;
    dcterms:description "A project is required" ;
    vivo:courseCredits 4 ;
    vivo:hasSubjectArea "COEN" .

roboprof_data:COEN_6721 a vivo:Course ;
    dbo:name "Fault-Tolerant Distributed Systems" ;
    dbo:number 6721 ;
    dcterms:description "A project is required" ;
    vivo:courseCredits 4 ;
    vivo:hasSubjectArea "COEN" .

roboprof_data:COEN_6741 a vivo:Course ;
    dbo:name "Computer Architecture and Design" ;
    dbo:number 6741 ;
    dcterms:description "A project is required" ;
    vivo:courseCredits 3 ;
    vivo:hasSubjectArea "COEN" .

roboprof_data:COEN_7311 a vivo:Course ;
    dbo:name "Protocol Design and Validation" ;
    dbo:number 7311 ;
    dcterms:description "A project is required" ;
    vivo:courseCredits 3 ;
    vivo:hasSubjectArea "COEN" .

roboprof_data:COEN_7741 a vivo:Course ;
    dbo:name "Advanced Computer Architecture" ;
    dbo:number 7741 ;
    dcterms:description "A project is required" ;
    vivo:courseCredits 3 ;
    vivo:hasSubjectArea "COEN" .

roboprof_data:COMM_205 a vivo:Course ;
    dbo:name "Business Communication" ;
    dbo:number 205 ;
    dcterms:description "Project proposal to improve the communications strategy of an existing business" ;
    vivo:courseCredits 4 ;
    vivo:hasSubjectArea "COMM" .

roboprof_data:COMM_401 a vivo:Course ;
    dbo:name "Strategy and Competition" ;
    dbo:number 401 ;
    dcterms:description "This capstone course requires graduating students to demonstrate their ability to integrate the knowledge and skills they have acquired during their program. This course introduces the major models and theories in strategic management." ;
    vivo:courseCredits 3 ;
    vivo:hasSubjectArea "COMM" .

roboprof_data:COMM_499 a vivo:Course ;
    dbo:name "Case Competition in Marketing (Seminar)",
        "Seminar Course: Business Case Writing " ;
    dbo:number 499 ;
    dcterms:description "This is not a case competition course. Instead, under the auspices of l'Association des Agences de Communication Crative (A2C), every year two Quebec inter-university competitions are organized and conducted. The Relve Communication was initiated in 1992 and the Relve Marketing in 1999. JMSB has entered teams of six students in both of these competitions since their inception. For both, participating university teams are given a day-long briefing in January by a company, not-for-profit organization or government agency and one or more of its communications agencies. The brief concludes with a mandate for which teams must create a complete communications or marketing plan for the client with a due date in late April. Their recommended plans are presented to the clients in their boardrooms or in their agency's pitch rooms. The judging panels include senior executives from the client (often its CEO), from the client's communications agencies and from A2C members. Throughout the academic term during which the competitions occur, students have the opportunity to apply the theories that they have learned so far in their BComm program to situations which are as close to 'real life' as possible in an academic setting.",
        "Uses case based approach and has students present in front of a panel of judges" ;
    vivo:courseCredits 3 ;
    vivo:hasSubjectArea "COMM",
        "COMM " .

roboprof_data:COMP_107 a vivo:Course ;
    dbo:name "Computer Science Industrial Experience Work Term I" ;
    dbo:number 107 ;
    dcterms:description "Industrial experience work term" ;
    vivo:courseCredits 4 ;
    vivo:hasSubjectArea "COMP" .

roboprof_data:COMP_108 a vivo:Course ;
    dbo:name "Computer ScienceIndustrial Experience Reflective Learning I" ;
    dbo:number 108 ;
    dcterms:description "Associated reflective learning course to industrial experience work term I" ;
    vivo:courseCredits 4 ;
    vivo:hasSubjectArea "COMP" .

roboprof_data:COMP_207 a vivo:Course ;
    dbo:name "Computer Science Industrial Experience Work Term II" ;
    dbo:number 207 ;
    dcterms:description "Industrial experience work term" ;
    vivo:courseCredits 4 ;
    vivo:hasSubjectArea "COMP" .

roboprof_data:COMP_208 a vivo:Course ;
    dbo:name "Computer Science Industrial Experience Reflective Learning II" ;
    dbo:number 208 ;
    dcterms:description "Associated reflective learning course to industrial experience work term II" ;
    vivo:courseCredits 4 ;
    vivo:hasSubjectArea "COMP" .

roboprof_data:COMP_248 a vivo:Course ;
    dbo:name "ObjectOriented Programming I" ;
    dbo:number 248 ;
    dcterms:description "Laboratory: 12 hours total" ;
    vivo:courseCredits 4 ;
    vivo:hasSubjectArea "COMP" .

roboprof_data:COMP_249 a vivo:Course ;
    dbo:name "ObjectOriented Programming I" ;
    dbo:number 249 ;
    dcterms:description "Laboratory: 12 hours total" ;
    vivo:courseCredits 4 ;
    vivo:hasSubjectArea "COMP" .

roboprof_data:COMP_345 a vivo:Course ;
    dbo:name "Advanced Program Design with C++" ;
    dbo:number 345 ;
    dcterms:description "Laboratory: 24 hours total, group project" ;
    vivo:courseCredits 4 ;
    vivo:hasSubjectArea "COMP" .

roboprof_data:COMP_346 a vivo:Course ;
    dbo:name "Operating Systems" ;
    dbo:number 346 ;
    dcterms:description "Laboratory: 24 hours total" ;
    vivo:courseCredits 4 ;
    vivo:hasSubjectArea "COMP" .

roboprof_data:COMP_353 a vivo:Course ;
    dbo:name "Databases" ;
    dbo:number 353 ;
    dcterms:description "Laboratory: 24 hours total, group project" ;
    vivo:courseCredits 4 ;
    vivo:hasSubjectArea "COMP" .

roboprof_data:COMP_354 a vivo:Course ;
    dbo:name "Introduction to Software Engineering" ;
    dbo:number 354 ;
    dcterms:description "Laboratory: 24 hours total, group project" ;
    vivo:courseCredits 4 ;
    vivo:hasSubjectArea "COMP" .

roboprof_data:COMP_371 a vivo:Course ;
    dbo:name "Computer Graphics" ;
    dbo:number 371 ;
    dcterms:description "Laboratory: 24 hours total, group project" ;
    vivo:courseCredits 4 ;
    vivo:hasSubjectArea "COMP" .

roboprof_data:COMP_376 a vivo:Course ;
    dbo:name "Introduction to Game Development" ;
    dbo:number 376 ;
    dcterms:description "Laboratory: 24 hours total, group project" ;
    vivo:courseCredits 4 ;
    vivo:hasSubjectArea "COMP" .

roboprof_data:COMP_426 a vivo:Course ;
    dbo:name "Multicore Programming" ;
    dbo:number 426 ;
    dcterms:description "Laboratory: 24 hours total, group project" ;
    vivo:courseCredits 4 ;
    vivo:hasSubjectArea "COMP" .

roboprof_data:COMP_428 a vivo:Course ;
    dbo:name "Parallel Programming" ;
    dbo:number 428 ;
    dcterms:description "Laboratory: 24 hours total, group project" ;
    vivo:courseCredits 4 ;
    vivo:hasSubjectArea "COMP" .

roboprof_data:COMP_442 a vivo:Course ;
    dbo:name "Compiler Design" ;
    dbo:number 442 ;
    dcterms:description "Laboratory: 24 hours total, project" ;
    vivo:courseCredits 4 ;
    vivo:hasSubjectArea "COMP" .

roboprof_data:COMP_444 a vivo:Course ;
    dbo:name "System Software Design" ;
    dbo:number 444 ;
    dcterms:description "Laboratory: 24 hours total, project" ;
    vivo:courseCredits 4 ;
    vivo:hasSubjectArea "COMP" .

roboprof_data:COMP_445 a vivo:Course ;
    dbo:name "Data Communication and Computer Networks" ;
    dbo:number 445 ;
    dcterms:description "Laboratory: 24 hours total" ;
    vivo:courseCredits 4 ;
    vivo:hasSubjectArea "COMP" .

roboprof_data:COMP_451 a vivo:Course ;
    dbo:name "Database Design" ;
    dbo:number 451 ;
    dcterms:description "Laboratory: 24 hours total" ;
    vivo:courseCredits 4 ;
    vivo:hasSubjectArea "COMP" .

roboprof_data:COMP_472 a vivo:Course ;
    dbo:name "Artificial Intelligence" ;
    dbo:number 472 ;
    dcterms:description "Laboratory: 24 hours total, project" ;
    vivo:courseCredits 4 ;
    vivo:hasSubjectArea "COMP" .

roboprof_data:COMP_473 a vivo:Course ;
    dbo:name "Pattern Recognition" ;
    dbo:number 473 ;
    dcterms:description "Laboratory: 24 hours total, project" ;
    vivo:courseCredits 4 ;
    vivo:hasSubjectArea "COMP" .

roboprof_data:COMP_474 a vivo:Course ;
    dbo:name "Intelligent Systems" ;
    dbo:number 474 ;
    dcterms:description "Laboratory: 24 hours total, project" ;
    vivo:courseCredits 4 ;
    vivo:hasSubjectArea "COMP" .

roboprof_data:COMP_476 a vivo:Course ;
    dbo:name "Advanced Game Development" ;
    dbo:number 476 ;
    dcterms:description "Laboratory: 24 hours total, group project" ;
    vivo:courseCredits 4 ;
    vivo:hasSubjectArea "COMP" .

roboprof_data:COMP_477 a vivo:Course ;
    dbo:name "Animation for Computer Games" ;
    dbo:number 477 ;
    dcterms:description "Laboratory: 24 hours total, project" ;
    vivo:courseCredits 4 ;
    vivo:hasSubjectArea "COMP" .

roboprof_data:COMP_478 a vivo:Course ;
    dbo:name "Image Processing" ;
    dbo:number 478 ;
    dcterms:description "Laboratory: 24 hours total, project" ;
    vivo:courseCredits 4 ;
    vivo:hasSubjectArea "COMP" .

roboprof_data:COMP_479 a vivo:Course ;
    dbo:name "Information Retrieval and Web Search" ;
    dbo:number 479 ;
    dcterms:description "Laboratory: 24 hours total, project" ;
    vivo:courseCredits 4 ;
    vivo:hasSubjectArea "COMP" .

roboprof_data:COMP_490 a vivo:Course ;
    dbo:name "Computer Science Project I" ;
    dbo:number 490 ;
    dcterms:description "capstone project" ;
    vivo:courseCredits 4 ;
    vivo:hasSubjectArea "COMP" .

roboprof_data:COMP_492 a vivo:Course ;
    dbo:name "Computer Science Project II" ;
    dbo:number 492 ;
    dcterms:description "capstone project" ;
    vivo:courseCredits 4 ;
    vivo:hasSubjectArea "COMP" .

roboprof_data:COMP_5201 a vivo:Course ;
    dbo:name "Computer Organization and Assembly Language" ;
    dbo:number 5201 ;
    dcterms:description "Laboratory: 24 hours total, project" ;
    vivo:courseCredits 4 ;
    vivo:hasSubjectArea "COMP" .

roboprof_data:COMP_5361 a vivo:Course ;
    dbo:name "Discrete Structures and Formal Languages" ;
    dbo:number 5361 ;
    dcterms:description "Laboratory: 24 hours total" ;
    vivo:courseCredits 4 ;
    vivo:hasSubjectArea "COMP" .

roboprof_data:COMP_5461 a vivo:Course ;
    dbo:name "Operating Systems" ;
    dbo:number 5461 ;
    dcterms:description "Laboratory: 24 hours total" ;
    vivo:courseCredits 4 ;
    vivo:hasSubjectArea "COMP" .

roboprof_data:COMP_5511 a vivo:Course ;
    dbo:name "Principles of Data Structures" ;
    dbo:number 5511 ;
    dcterms:description "Laboratory: 24 hours total" ;
    vivo:courseCredits 4 ;
    vivo:hasSubjectArea "COMP" .

roboprof_data:COMP_5541 a vivo:Course ;
    dbo:name "Tools and Techniques for Software Engineering" ;
    dbo:number 5541 ;
    dcterms:description "Laboratory: 24 hours total, project" ;
    vivo:courseCredits 4 ;
    vivo:hasSubjectArea "COMP" .

roboprof_data:COMP_6231_A a roboprof:InitialGrade ;
    roboprof:gradeInCourse roboprof_data:COMP_6231 ;
    roboprof:gradeValue "A" .

<http://roboprof.ca/data/COMP_6231_B+> a roboprof:InitialGrade ;
    roboprof:gradeInCourse roboprof_data:COMP_6231 ;
    roboprof:gradeValue "B+" .

roboprof_data:COMP_6231_F a roboprof:InitialGrade ;
    roboprof:gradeInCourse roboprof_data:COMP_6231 ;
    roboprof:gradeValue "F" .

roboprof_data:COMP_628 a vivo:Course ;
    dbo:name "Parallel Programming" ;
    dbo:number 628 ;
    dcterms:description "Laboratory: 24 hours total, group project" ;
    vivo:courseCredits 4 ;
    vivo:hasSubjectArea "COMP" .

roboprof_data:COMP_6311 a vivo:Course ;
    dbo:name "Animation for Computer Games" ;
    dbo:number 6311 ;
    dcterms:description "Laboratory: 24 hours total, project" ;
    vivo:courseCredits 4 ;
    vivo:hasSubjectArea "COMP" .

roboprof_data:COMP_6321 a vivo:Course ;
    dbo:name "Machine Learning" ;
    dbo:number 6321 ;
    dcterms:description "Laboratory: 24 hours total, project" ;
    vivo:courseCredits 4 ;
    vivo:hasSubjectArea "COMP" .

roboprof_data:COMP_6331 a vivo:Course ;
    dbo:name "Advanced Game Development" ;
    dbo:number 6331 ;
    dcterms:description "Laboratory: 24 hours total, project" ;
    vivo:courseCredits 4 ;
    vivo:hasSubjectArea "COMP" .

roboprof_data:COMP_6411_A a roboprof:InitialGrade ;
    roboprof:gradeInCourse roboprof_data:COMP_6411 ;
    roboprof:gradeValue "A" .

<http://roboprof.ca/data/COMP_6421_A+> a roboprof:InitialGrade ;
    roboprof:gradeInCourse roboprof_data:COMP_6421 ;
    roboprof:gradeValue "A+" .

roboprof_data:COMP_6461_A- a roboprof:InitialGrade ;
    roboprof:gradeInCourse roboprof_data:COMP_6461 ;
    roboprof:gradeValue "A-" .

<http://roboprof.ca/data/COMP_6461_B+> a roboprof:InitialGrade ;
    roboprof:gradeInCourse roboprof_data:COMP_6461 ;
    roboprof:gradeValue "B+" .

roboprof_data:COMP_6461_Lecture_1 a roboprof:Lecture ;
    dbo:name "Computer Networks & Internet" ;
    dbo:number 1 ;
    roboprof:coversCourseContent <file:///./dataset/Lecture%20Content/COMP%206461/Lectures/1.ppt>,
        <file:///./dataset/Lecture%20Content/COMP%206461/OtherMaterial/ComputerNetwork.pdf>,
        <file:///./dataset/Lecture%20Content/COMP%206461/Readings/InternetProtocolSuite.pdf>,
        <file:///./dataset/Lecture%20Content/COMP%206461/Worksheets/TA1.pdf> ;
    rdfs:seeAlso <https://www.concordia.ca/academics/graduate/calendar/current/gina-cody-school-of-engineering-and-computer-science-courses/computer-science-and-software-engineering-master-s-and-phd-courses.html> .

roboprof_data:COMP_6461_Lecture_2 a roboprof:Lecture ;
    dbo:name "Application Layer -1" ;
    dbo:number 2 ;
    roboprof:coversCourseContent <file:///./dataset/Lecture%20Content/COMP%206461/Lectures/2.ppt>,
        <file:///./dataset/Lecture%20Content/COMP%206461/OtherMaterial/ApplicationLayer.pdf>,
        <file:///./dataset/Lecture%20Content/COMP%206461/Readings/GoBackN.pdf>,
        <file:///./dataset/Lecture%20Content/COMP%206461/Worksheets/TA1.pdf> ;
    rdfs:seeAlso <https://www.concordia.ca/academics/graduate/calendar/current/gina-cody-school-of-engineering-and-computer-science-courses/computer-science-and-software-engineering-master-s-and-phd-courses.html> .

roboprof_data:COMP_6461_Lecture_3 a roboprof:Lecture ;
    dbo:name "Application Layer -2" ;
    dbo:number 3 ;
    roboprof:coversCourseContent <file:///./dataset/Lecture%20Content/COMP%206461/Lectures/3.ppt>,
        <file:///./dataset/Lecture%20Content/COMP%206461/OtherMaterial/ApplicationLayer.pdf>,
        <file:///./dataset/Lecture%20Content/COMP%206461/Readings/GoBackN.pdf>,
        <file:///./dataset/Lecture%20Content/COMP%206461/Worksheets/TA2.pdf> ;
    rdfs:seeAlso <https://www.concordia.ca/academics/graduate/calendar/current/gina-cody-school-of-engineering-and-computer-science-courses/computer-science-and-software-engineering-master-s-and-phd-courses.html> .

roboprof_data:COMP_6461_Lecture_4 a roboprof:Lecture ;
    dbo:name "Transport Layer - 1" ;
    dbo:number 4 ;
    roboprof:coversCourseContent <file:///./dataset/Lecture%20Content/COMP%206461/Lectures/4.ppt>,
        <file:///./dataset/Lecture%20Content/COMP%206461/OtherMaterial/NetworkLayer.pdf>,
        <file:///./dataset/Lecture%20Content/COMP%206461/Readings/SelectiveRepeat.pdf>,
        <file:///./dataset/Lecture%20Content/COMP%206461/Worksheets/TA2.pdf> ;
    rdfs:seeAlso <https://aits.encs.concordia.ca/aits/public/top/courses/20212/05/COMP6461.html> .

roboprof_data:COMP_6461_Lecture_5 a roboprof:Lecture ;
    dbo:name "Transport Layer - 2" ;
    dbo:number 5 ;
    roboprof:coversCourseContent <file:///./dataset/Lecture%20Content/COMP%206461/Lectures/5.ppt>,
        <file:///./dataset/Lecture%20Content/COMP%206461/OtherMaterial/TCP.pdf>,
        <file:///./dataset/Lecture%20Content/COMP%206461/Readings/SelectiveRepeat.pdf>,
        <file:///./dataset/Lecture%20Content/COMP%206461/Worksheets/TA3.pdf> ;
    rdfs:seeAlso <https://aits.encs.concordia.ca/aits/public/top/courses/20212/05/COMP6461.html> .

roboprof_data:COMP_6461_Lecture_6 a roboprof:Lecture ;
    dbo:name "Transport Layer - 3" ;
    dbo:number 6 ;
    roboprof:coversCourseContent <file:///./dataset/Lecture%20Content/COMP%206461/Lectures/6.ppt>,
        <file:///./dataset/Lecture%20Content/COMP%206461/OtherMaterial/UDP.pdf>,
        <file:///./dataset/Lecture%20Content/COMP%206461/Readings/NetworkCongestion.pdf>,
        <file:///./dataset/Lecture%20Content/COMP%206461/Worksheets/TA3.pdf> ;
    rdfs:seeAlso <https://aits.encs.concordia.ca/aits/public/top/courses/20212/05/COMP6461.html> .

roboprof_data:COMP_6481_A- a roboprof:InitialGrade ;
    roboprof:gradeInCourse roboprof_data:COMP_6481 ;
    roboprof:gradeValue "A-" .

roboprof_data:COMP_6521_A a roboprof:InitialGrade ;
    roboprof:gradeInCourse roboprof_data:COMP_6521 ;
    roboprof:gradeValue "A" .

roboprof_data:COMP_6521_F a roboprof:InitialGrade ;
    roboprof:gradeInCourse roboprof_data:COMP_6521 ;
    roboprof:gradeValue "F" .

roboprof_data:COMP_6551_A- a roboprof:InitialGrade ;
    roboprof:gradeInCourse roboprof_data:COMP_6551 ;
    roboprof:gradeValue "A-" .

roboprof_data:COMP_6721_A a roboprof:InitialGrade ;
    roboprof:gradeInCourse roboprof_data:COMP_6721 ;
    roboprof:gradeValue "A" .

roboprof_data:COMP_6731_A- a roboprof:InitialGrade ;
    roboprof:gradeInCourse roboprof_data:COMP_6731 ;
    roboprof:gradeValue "A-" .

roboprof_data:COMP_6741_A- a roboprof:InitialGrade ;
    roboprof:gradeInCourse roboprof_data:COMP_6741 ;
    roboprof:gradeValue "A-" .

roboprof_data:COMP_6741_Lab_1 a roboprof:Lab ;
    dbo:name "Lab 1 : Python" ;
    dbo:number 1 ;
    roboprof:coversCourseContent <file:///./dataset/Lab%20Content/COMP%206741/Lab%20Material/Lab%201.pdf> .

roboprof_data:COMP_6741_Lab_2 a roboprof:Lab ;
    dbo:name "Lab 2 : RDF" ;
    dbo:number 2 ;
    roboprof:coversCourseContent <file:///./dataset/Lab%20Content/COMP%206741/Lab%20Material/Lab%202.pdf> .

roboprof_data:COMP_6741_Lab_3 a roboprof:Lab ;
    dbo:name "Lab 3 : FOAF" ;
    dbo:number 3 ;
    roboprof:coversCourseContent <file:///./dataset/Lab%20Content/COMP%206741/Lab%20Material/Lab%203.pdf> .

roboprof_data:COMP_6741_Lecture_1 a roboprof:Lecture ;
    dbo:name "Introduction to Intelligent Systems" ;
    dbo:number 1 ;
    roboprof:coversCourseContent <file:///./dataset/Lecture%20Content/COMP%206741/Lectures/slides01.pdf>,
        <file:///./dataset/Lecture%20Content/COMP%206741/OtherMaterial/BagOfWords.pdf>,
        <file:///./dataset/Lecture%20Content/COMP%206741/Readings/DeepLearning.pdf>,
        <file:///./dataset/Lecture%20Content/COMP%206741/Worksheets/worksheet01.pdf> ;
    rdfs:seeAlso <https://moodle.concordia.ca/moodle/course/view.php?id=162041#section-2> .

roboprof_data:COMP_6741_Lecture_2 a roboprof:Lecture ;
    dbo:name "Knowledge Graphs" ;
    dbo:number 2 ;
    roboprof:coversCourseContent <file:///./dataset/Lecture%20Content/COMP%206741/Lectures/slides02.pdf>,
        <file:///./dataset/Lecture%20Content/COMP%206741/OtherMaterial/LinguisticLinkedOpenData.pdf>,
        <file:///./dataset/Lecture%20Content/COMP%206741/Readings/KnowledgeGraph.pdf>,
        <file:///./dataset/Lecture%20Content/COMP%206741/Worksheets/worksheet02.pdf> ;
    rdfs:seeAlso <https://moodle.concordia.ca/moodle/course/view.php?id=162041#section-3> .

roboprof_data:COMP_6741_Lecture_3 a roboprof:Lecture ;
    dbo:name "Knowledge Graphs : Vocabulary" ;
    dbo:number 3 ;
    roboprof:coversCourseContent <file:///./dataset/Lecture%20Content/COMP%206741/Lectures/slides03.pdf>,
        <file:///./dataset/Lecture%20Content/COMP%206741/OtherMaterial/MachineLearning.pdf>,
        <file:///./dataset/Lecture%20Content/COMP%206741/Readings/NLP.pdf>,
        <file:///./dataset/Lecture%20Content/COMP%206741/Worksheets/worksheet03.pdf> ;
    rdfs:seeAlso <https://moodle.concordia.ca/moodle/course/view.php?id=162041#section-4> .

roboprof_data:COMP_6741_Lecture_4 a roboprof:Lecture ;
    dbo:name "Knowledge Base Queries" ;
    dbo:number 4 ;
    roboprof:coversCourseContent <file:///./dataset/Lecture%20Content/COMP%206741/Lectures/slides04.pdf>,
        <file:///./dataset/Lecture%20Content/COMP%206741/OtherMaterial/TextMining.pdf>,
        <file:///./dataset/Lecture%20Content/COMP%206741/Readings/SPARQL.pdf>,
        <file:///./dataset/Lecture%20Content/COMP%206741/Worksheets/worksheet04.pdf> ;
    rdfs:seeAlso <https://moodle.concordia.ca/moodle/course/view.php?id=162041#section-5> .

roboprof_data:COMP_6741_Lecture_5 a roboprof:Lecture ;
    dbo:name "Recommender Systems" ;
    dbo:number 5 ;
    roboprof:coversCourseContent <file:///./dataset/Lecture%20Content/COMP%206741/Lectures/slides05.pdf>,
        <file:///./dataset/Lecture%20Content/COMP%206741/OtherMaterial/WordEmbeddings.pdf>,
        <file:///./dataset/Lecture%20Content/COMP%206741/Readings/RecommenderSystem.pdf>,
        <file:///./dataset/Lecture%20Content/COMP%206741/Worksheets/worksheet05.pdf> ;
    rdfs:seeAlso <https://moodle.concordia.ca/moodle/course/view.php?id=162041#section-7> .

roboprof_data:COMP_6741_Lecture_6 a roboprof:Lecture ;
    dbo:name "Intelligent Agents" ;
    dbo:number 6 ;
    roboprof:coversCourseContent <file:///./dataset/Lecture%20Content/COMP%206741/Lectures/slides06.pdf>,
        <file:///./dataset/Lecture%20Content/COMP%206741/OtherMaterial/TextMining.pdf>,
        <file:///./dataset/Lecture%20Content/COMP%206741/Readings/IntelligentAgent.pdf>,
        <file:///./dataset/Lecture%20Content/COMP%206741/Worksheets/worksheet05.pdf> ;
    rdfs:seeAlso <https://moodle.concordia.ca/moodle/course/view.php?id=162041#section-7> .

roboprof_data:COMP_6761_A a roboprof:InitialGrade ;
    roboprof:gradeInCourse roboprof_data:COMP_6761 ;
    roboprof:gradeValue "A" .

roboprof_data:COMP_6771_A- a roboprof:InitialGrade ;
    roboprof:gradeInCourse roboprof_data:COMP_6771 ;
    roboprof:gradeValue "A-" .

<http://roboprof.ca/data/COMP_6791_B+> a roboprof:InitialGrade ;
    roboprof:gradeInCourse roboprof_data:COMP_6791 ;
    roboprof:gradeValue "B+" .

roboprof_data:COMS_274 a vivo:Course ;
    dbo:name "Communication Media: Intermedia I" ;
    dbo:number 274 ;
    dcterms:description "Practicum course" ;
    vivo:courseCredits 3 ;
    vivo:hasSubjectArea "COMS" .

roboprof_data:COMS_276 a vivo:Course ;
    dbo:name "Communication Media: Sound I" ;
    dbo:number 276 ;
    dcterms:description "Practicum course" ;
    vivo:courseCredits 3 ;
    vivo:hasSubjectArea "COMS" .

roboprof_data:COMS_284 a vivo:Course ;
    dbo:name "Communication Media: Moving Images I" ;
    dbo:number 284 ;
    dcterms:description "Practicum course" ;
    vivo:courseCredits 4 ;
    vivo:hasSubjectArea "COMS" .

roboprof_data:COMS_307 a vivo:Course ;
    dbo:name "Scriptwriting for the Media" ;
    dbo:number 307 ;
    dcterms:description "Practicum course" ;
    vivo:courseCredits 4 ;
    vivo:hasSubjectArea "COMS" .

roboprof_data:COMS_324 a vivo:Course ;
    dbo:name "Communication Analysis of Environment" ;
    dbo:number 324 ;
    dcterms:description "Workshops, Montreal locations site analysis" ;
    vivo:courseCredits 3 ;
    vivo:hasSubjectArea "COMS" .

roboprof_data:COMS_361 a vivo:Course ;
    dbo:name "Propaganda" ;
    dbo:number 361 ;
    dcterms:description "Projects" ;
    vivo:courseCredits 4 ;
    vivo:hasSubjectArea "COMS" .

roboprof_data:COMS_374 a vivo:Course ;
    dbo:name "Communication Media: Intermedia II" ;
    dbo:number 374 ;
    dcterms:description "Practicum course" ;
    vivo:courseCredits 3 ;
    vivo:hasSubjectArea "COMS" .

roboprof_data:COMS_376 a vivo:Course ;
    dbo:name "Communication Media: Sound II" ;
    dbo:number 376 ;
    dcterms:description "Practicum course" ;
    vivo:courseCredits 4 ;
    vivo:hasSubjectArea "COMS" .

roboprof_data:COMS_384 a vivo:Course ;
    dbo:name "Communication Media: Moving Images II" ;
    dbo:number 384 ;
    dcterms:description "Practicum course" ;
    vivo:courseCredits 4 ;
    vivo:hasSubjectArea "COMS" .

roboprof_data:COMS_393 a vivo:Course ;
    dbo:name "Communication Media: Special Topics" ;
    dbo:number 393 ;
    dcterms:description "Practicum course" ;
    vivo:courseCredits 4 ;
    vivo:hasSubjectArea "COMS" .

roboprof_data:COMS_407 a vivo:Course ;
    dbo:name "Scriptwriting for the Media" ;
    dbo:number 407 ;
    dcterms:description "Practicum course" ;
    vivo:courseCredits 4 ;
    vivo:hasSubjectArea "COMS" .

roboprof_data:COMS_475 a vivo:Course ;
    dbo:name "Communication Media: Intermedia III" ;
    dbo:number 475 ;
    dcterms:description "Practicum course" ;
    vivo:courseCredits 4 ;
    vivo:hasSubjectArea "COMS" .

roboprof_data:COMS_477 a vivo:Course ;
    dbo:name "Communication Media: Sound III" ;
    dbo:number 477 ;
    dcterms:description "Practicum course" ;
    vivo:courseCredits 4 ;
    vivo:hasSubjectArea "COMS" .

roboprof_data:COMS_484 a vivo:Course ;
    dbo:name "Communication Media: Moving Images III" ;
    dbo:number 484 ;
    dcterms:description "Practicum course" ;
    vivo:courseCredits 3 ;
    vivo:hasSubjectArea "COMS" .

roboprof_data:COMS_493 a vivo:Course ;
    dbo:name "Communication Media: Advanced Topics" ;
    dbo:number 493 ;
    dcterms:description "Practicum course" ;
    vivo:courseCredits 4 ;
    vivo:hasSubjectArea "COMS" .

roboprof_data:COMS_506 a vivo:Course ;
    dbo:name "In the Field: Methods" ;
    dbo:number 506 ;
    dcterms:description "Practicum course" ;
    vivo:courseCredits 3 ;
    vivo:hasSubjectArea "COMS" .

roboprof_data:COMS_507 a vivo:Course ;
    dbo:name "Scriptwriting for the Media" ;
    dbo:number 507 ;
    dcterms:description "Practicum course" ;
    vivo:courseCredits 3 ;
    vivo:hasSubjectArea "COMS" .

roboprof_data:COMS_513 a vivo:Course ;
    dbo:name "Cultures of Production" ;
    dbo:number 513 ;
    dcterms:description "Field research projects" ;
    vivo:courseCredits 4 ;
    vivo:hasSubjectArea "COMS" .

roboprof_data:COMS_562 a vivo:Course ;
    dbo:name "Media Production: Sound" ;
    dbo:number 562 ;
    dcterms:description "Lectures and Laboratory: average 6 hours per week" ;
    vivo:courseCredits 4 ;
    vivo:hasSubjectArea "COMS" .

roboprof_data:COMS_569 a vivo:Course ;
    dbo:name "Media Production: Moving Images" ;
    dbo:number 569 ;
    dcterms:description "Lectures and Laboratory: average 6 hours per week" ;
    vivo:courseCredits 4 ;
    vivo:hasSubjectArea "COMS" .

roboprof_data:COMS_570 a vivo:Course ;
    dbo:name "Media Production: Intermedia" ;
    dbo:number 570 ;
    dcterms:description "Lectures and Laboratory: average 6 hours per week" ;
    vivo:courseCredits 4 ;
    vivo:hasSubjectArea "COMS" .

roboprof_data:COMS_606 a vivo:Course ;
    dbo:name "Media Research Practicum" ;
    dbo:number 606 ;
    dcterms:description "Individual research practicum offered on a tutorial basis under faculty supervision" ;
    vivo:courseCredits 4 ;
    vivo:hasSubjectArea "COMS" .

roboprof_data:COMS_684 a vivo:Course ;
    dbo:name "Media Research Laboratory" ;
    dbo:number 684 ;
    dcterms:description "Research-creation Laboratory" ;
    vivo:courseCredits 3 ;
    vivo:hasSubjectArea "COMS" .

roboprof_data:COMS_876 a vivo:Course ;
    dbo:name "Media Technology as Practice" ;
    dbo:number 876 ;
    dcterms:description "Research-creation Laboratory" ;
    vivo:courseCredits 4 ;
    vivo:hasSubjectArea "COMS" .

roboprof_data:DANC_201 a vivo:Course ;
    dbo:name "Creative Process I" ;
    dbo:number 201 ;
    dcterms:description "Students learn to explore, observe, and structure ideas and movements through improvisations and specific exercises which cover such fundamentals as kinetics, rhythm and dynamics, spatial organization, perceptual skills, integration of acoustic, visual and verbal elements, and the use of technology as a creative tool." ;
    vivo:courseCredits 4 ;
    vivo:hasSubjectArea "DANC" .

roboprof_data:DANC_205 a vivo:Course ;
    dbo:name "Technique I" ;
    dbo:number 205 ;
    dcterms:description "Emphasis is placed on the proper alignment and placement of the body in stillness and in motion. Integration and execution of movement fundamentals and sequences are taught as a preparation for dance." ;
    vivo:courseCredits 3 ;
    vivo:hasSubjectArea "DANC" .

roboprof_data:DANC_240 a vivo:Course ;
    dbo:name "Principles of Contemporary Dance" ;
    dbo:number 240 ;
    dcterms:description "A survey of technical skills, improvisation, and dance composition." ;
    vivo:courseCredits 3 ;
    vivo:hasSubjectArea "DANC" .

roboprof_data:DANC_301 a vivo:Course ;
    dbo:name "Creative Process II" ;
    dbo:number 301 ;
    dcterms:description "Students further develop the practical and theoretical aspects of the creative process in dance and the elaboration of an individualized kinetic language. Methods of research and their application to concepts, themes, collaborations, projects, and the use of technology are evolved in studio and laboratories." ;
    vivo:courseCredits 4 ;
    vivo:hasSubjectArea "DANC" .

roboprof_data:DANC_305 a vivo:Course ;
    dbo:name "Technique II" ;
    dbo:number 305 ;
    dcterms:description "Emphasis is placed on the technical development of suppleness, strength, coordination, rhythm, and kinetic fundamentals." ;
    vivo:courseCredits 4 ;
    vivo:hasSubjectArea "DANC" .

roboprof_data:DANC_320 a vivo:Course ;
    dbo:name "Choreography I" ;
    dbo:number 320 ;
    dcterms:description "This course develops personal creativity and broadens the students physical and expressive potential into public performances." ;
    vivo:courseCredits 3 ;
    vivo:hasSubjectArea "DANC" .

roboprof_data:DANC_350 a vivo:Course ;
    dbo:name "Practical Anatomy for the Moving Body" ;
    dbo:number 350 ;
    dcterms:description "Students experience the human anatomy in relation to movement and dance through studio practices." ;
    vivo:courseCredits 4 ;
    vivo:hasSubjectArea "DANC" .

roboprof_data:DANC_398 a vivo:Course ;
    dbo:name "Special Topics in Dance" ;
    dbo:number 398 ;
    dcterms:description "Studio based exploration of dance as real-world." ;
    vivo:courseCredits 4 ;
    vivo:hasSubjectArea "DANC" .

roboprof_data:DANC_401 a vivo:Course ;
    dbo:name "Creative Process III" ;
    dbo:number 401 ;
    dcterms:description "This course enables students to advance their creative process and practice as movement artists through kinetic exploration, improvisation, performance coaching, extended studio projects, and lab reports." ;
    vivo:courseCredits 3 ;
    vivo:hasSubjectArea "DANC" .

roboprof_data:DANC_405 a vivo:Course ;
    dbo:name "Technique III " ;
    dbo:number 405 ;
    dcterms:description "Emphasis is placed on refining and consolidating the students practical understanding of kinetics in relation to placement, locomotion, movement patterns, dynamics, and phrasing." ;
    vivo:courseCredits 4 ;
    vivo:hasSubjectArea "DANC" .

roboprof_data:DANC_420 a vivo:Course ;
    dbo:name "Choreography II" ;
    dbo:number 420 ;
    dcterms:description "Building on initial research carried out in DANC 320, further exploration is conducted into the use of technology within the choreographic process as well as an examination of the role that it plays in all aspects of production." ;
    vivo:courseCredits 3 ;
    vivo:hasSubjectArea "DANC" .

roboprof_data:DFTT_209 a vivo:Course ;
    dbo:name "Design for Live Performance l" ;
    dbo:number 209 ;
    dcterms:description "Examination of the theatrical design process" ;
    vivo:courseCredits 3 ;
    vivo:hasSubjectArea "DFTT" .

roboprof_data:DFTT_210 a vivo:Course ;
    dbo:name "Design for Live Performance ll" ;
    dbo:number 210 ;
    dcterms:description "Examination of the theatrical design process" ;
    vivo:courseCredits 4 ;
    vivo:hasSubjectArea "DFTT" .

roboprof_data:DFTT_211 a vivo:Course ;
    dbo:name "Drawing for the Theatre" ;
    dbo:number 211 ;
    dcterms:description "Study drawing and drafting techniques for the stage" ;
    vivo:courseCredits 4 ;
    vivo:hasSubjectArea "DFTT" .

roboprof_data:DFTT_212 a vivo:Course ;
    dbo:name "Introduction to Elements of Production" ;
    dbo:number 212 ;
    dcterms:description "Elements of stage management, production management and technical direction" ;
    vivo:courseCredits 4 ;
    vivo:hasSubjectArea "DFTT" .

roboprof_data:DFTT_298 a vivo:Course ;
    dbo:name "Special Topics in Design for the Theatre" ;
    dbo:number 298 ;
    dcterms:description "The study of specialized aspects of theatre design" ;
    vivo:courseCredits 3 ;
    vivo:hasSubjectArea "DFTT" .

roboprof_data:DFTT_299 a vivo:Course ;
    dbo:name "Special Topics in Design for the Theatre" ;
    dbo:number 299 ;
    dcterms:description "The study of specialized aspects of theatre design" ;
    vivo:courseCredits 4 ;
    vivo:hasSubjectArea "DFTT" .

roboprof_data:DFTT_301 a vivo:Course ;
    dbo:name "Introduction to Designer's Studio: Conception" ;
    dbo:number 301 ;
    dcterms:description "Students apply their design knowledge to special projects" ;
    vivo:courseCredits 3 ;
    vivo:hasSubjectArea "DFTT" .

roboprof_data:DFTT_305 a vivo:Course ;
    dbo:name "Independent Study I" ;
    dbo:number 305 ;
    dcterms:description "The independent study of specialized aspects of theatre design" ;
    vivo:courseCredits 4 ;
    vivo:hasSubjectArea "DFTT" .

roboprof_data:DFTT_311 a vivo:Course ;
    dbo:name "Lighting Design Conception" ;
    dbo:number 311 ;
    dcterms:description "Students study lighting design for the theatre" ;
    vivo:courseCredits 3 ;
    vivo:hasSubjectArea "DFTT" .

roboprof_data:DFTT_315 a vivo:Course ;
    dbo:name "Lighting Design Realization" ;
    dbo:number 315 ;
    dcterms:description "Focus is on basic realization methods" ;
    vivo:courseCredits 3 ;
    vivo:hasSubjectArea "DFTT" .

roboprof_data:DFTT_321 a vivo:Course ;
    dbo:name "Costume Design Conception" ;
    dbo:number 321 ;
    dcterms:description "Students study costume design for the theatre" ;
    vivo:courseCredits 3 ;
    vivo:hasSubjectArea "DFTT" .

roboprof_data:DFTT_325 a vivo:Course ;
    dbo:name "Costume Design Realization" ;
    dbo:number 325 ;
    dcterms:description "Focus is on basic realization methods" ;
    vivo:courseCredits 3 ;
    vivo:hasSubjectArea "DFTT" .

roboprof_data:DFTT_326 a vivo:Course ;
    dbo:name "Costume Accessories Realization" ;
    dbo:number 326 ;
    dcterms:description "Students study costume accessory design for the stage" ;
    vivo:courseCredits 4 ;
    vivo:hasSubjectArea "DFTT" .

roboprof_data:DFTT_331 a vivo:Course ;
    dbo:name "Set Design Conception" ;
    dbo:number 331 ;
    dcterms:description "Students study set design for the theatre with emphasis on imaginative and analytical processes" ;
    vivo:courseCredits 4 ;
    vivo:hasSubjectArea "DFTT" .

roboprof_data:DFTT_335 a vivo:Course ;
    dbo:name "Set Design Realization" ;
    dbo:number 335 ;
    dcterms:description "Students study stage scenery with emphasis on analysis, development, and execution of design ideas" ;
    vivo:courseCredits 4 ;
    vivo:hasSubjectArea "DFTT" .

roboprof_data:DFTT_336 a vivo:Course ;
    dbo:name "Stage Properties Realization" ;
    dbo:number 336 ;
    dcterms:description "Students study stage properties with an emphasis on analysis, development, and execution of design ideas" ;
    vivo:courseCredits 4 ;
    vivo:hasSubjectArea "DFTT" .

roboprof_data:DFTT_337 a vivo:Course ;
    dbo:name "Scene Painting Realization" ;
    dbo:number 337 ;
    dcterms:description "This studio course includes the study of the materials and technology of scene painting." ;
    vivo:courseCredits 4 ;
    vivo:hasSubjectArea "DFTT" .

roboprof_data:DFTT_341 a vivo:Course ;
    dbo:name "Elements of Multimedia Conception" ;
    dbo:number 341 ;
    dcterms:description "Students study design with a variety of media, with an emphasis on imaginative and analytical processes" ;
    vivo:courseCredits 3 ;
    vivo:hasSubjectArea "DFTT" .

roboprof_data:DFTT_345 a vivo:Course ;
    dbo:name "Elements of Multimedia Realization" ;
    dbo:number 345 ;
    dcterms:description "Students study elements of analog and digital media with an emphasis on the execution of design ideas" ;
    vivo:courseCredits 3 ;
    vivo:hasSubjectArea "DFTT" .

roboprof_data:DFTT_350 a vivo:Course ;
    dbo:name "Introduction to Public Performance Design" ;
    dbo:number 350 ;
    dcterms:description "Students learn to collaborate with directors, other designers, and technical staff to creatively realize set, costume, lighting, properties, video, and sound designs for live performance." ;
    vivo:courseCredits 3 ;
    vivo:hasSubjectArea "DFTT" .

roboprof_data:DFTT_351 a vivo:Course ;
    dbo:name "Introduction to Public Performance Design" ;
    dbo:number 351 ;
    dcterms:description "Students learn to collaborate with directors, other designers, and technical staff to creatively realize set, costume, lighting, properties, video, and sound designs for live performance." ;
    vivo:courseCredits 4 ;
    vivo:hasSubjectArea "DFTT" .

roboprof_data:DFTT_370 a vivo:Course ;
    dbo:name "Elements of Production" ;
    dbo:number 370 ;
    dcterms:description "Students are introduced to the language, tools, and techniques used in rehearsal halls, shops, and backstage." ;
    vivo:courseCredits 4 ;
    vivo:hasSubjectArea "DFTT" .

roboprof_data:DFTT_371 a vivo:Course ;
    dbo:name "Elements of Production" ;
    dbo:number 371 ;
    dcterms:description "Students are introduced to the language, tools, and techniques used in rehearsal halls, shops, and backstage." ;
    vivo:courseCredits 4 ;
    vivo:hasSubjectArea "DFTT" .

roboprof_data:DFTT_398 a vivo:Course ;
    dbo:name "Special Topics in Design for the Theatre: Realization" ;
    dbo:number 398 ;
    dcterms:description "The study of specialized aspects of theatre design realization" ;
    vivo:courseCredits 4 ;
    vivo:hasSubjectArea "DFTT" .

roboprof_data:DFTT_399 a vivo:Course ;
    dbo:name "Special Topics in Design for the Theatre" ;
    dbo:number 399 ;
    dcterms:description "The study of specialized aspects of theatre design" ;
    vivo:courseCredits 3 ;
    vivo:hasSubjectArea "DFTT" .

roboprof_data:DFTT_401 a vivo:Course ;
    dbo:name "Advanced Designer's Studio" ;
    dbo:number 401 ;
    dcterms:description "Students apply their design knowledge to special projects" ;
    vivo:courseCredits 3 ;
    vivo:hasSubjectArea "DFTT" .

roboprof_data:DFTT_405 a vivo:Course ;
    dbo:name "Independent Study II" ;
    dbo:number 405 ;
    dcterms:description "The independent study of specialized aspects of theatre design" ;
    vivo:courseCredits 4 ;
    vivo:hasSubjectArea "DFTT" .

roboprof_data:DFTT_450 a vivo:Course ;
    dbo:name "Advanced Public Performance Design" ;
    dbo:number 450 ;
    dcterms:description "Students collaborate with directors, other designers, and technical staff" ;
    vivo:courseCredits 4 ;
    vivo:hasSubjectArea "DFTT" .

roboprof_data:DFTT_451 a vivo:Course ;
    dbo:name "ADV. PUBLIC PERF. DESIGN",
        "Advanced Public Performance Design" ;
    dbo:number 451 ;
    dcterms:description "NaN"^^xsd:double,
        "Students collaborate with directors, other designers, and technical staff" ;
    vivo:courseCredits 3,
        4 ;
    vivo:hasSubjectArea "DFTT" .

roboprof_data:DFTT_470 a vivo:Course ;
    dbo:name "Advanced Elements of Production" ;
    dbo:number 470 ;
    dcterms:description "Students study advanced theories and practices of stage management, production management, and technical direction." ;
    vivo:courseCredits 3 ;
    vivo:hasSubjectArea "DFTT" .

roboprof_data:DFTT_471 a vivo:Course ;
    dbo:name "Advanced Elements of Production" ;
    dbo:number 471 ;
    dcterms:description "Students study advanced theories and practices of stage management, production management, and technical direction." ;
    vivo:courseCredits 3 ;
    vivo:hasSubjectArea "DFTT" .

roboprof_data:DFTT_498 a vivo:Course ;
    dbo:name "Special Topics in Design for the Theatre: Conception" ;
    dbo:number 498 ;
    dcterms:description "The study of specialized aspects of theatre design conception" ;
    vivo:courseCredits 3 ;
    vivo:hasSubjectArea "DFTT" .

roboprof_data:DFTT_499 a vivo:Course ;
    dbo:name "Special Topics in Design for the Theatre" ;
    dbo:number 499 ;
    dcterms:description "The study of specialized aspects of theatre design" ;
    vivo:courseCredits 4 ;
    vivo:hasSubjectArea "DFTT" .

roboprof_data:DRAW_200 a vivo:Course ;
    dbo:name "Drawing I" ;
    dbo:number 200 ;
    dcterms:description "A studio course which provides a technical and conceptual introduction to drawing focusing on the distinctive and interdisciplinary nature of the practice." ;
    vivo:courseCredits 3 ;
    vivo:hasSubjectArea "DRAW " .

roboprof_data:DRAW_201 a vivo:Course ;
    dbo:name "Introduction to Drawing" ;
    dbo:number 201 ;
    dcterms:description "This course introduces students to elementary skills required by the art of drawing. It covers fundamental drawing techniques and explores various mediums and concepts of drawing in th historical and contemporary art world." ;
    vivo:courseCredits 3 ;
    vivo:hasSubjectArea "DRAW " .

roboprof_data:DRAW_298 a vivo:Course ;
    dbo:name "Special Topics in Drawing " ;
    dbo:number 298 ;
    dcterms:description "A studio course which provides an opportunity for the study of more specialized aspects of drawing." ;
    vivo:courseCredits 3 ;
    vivo:hasSubjectArea "DRAW " .

roboprof_data:DRAW_299 a vivo:Course ;
    dbo:name "Special Topics in Drawing" ;
    dbo:number 299 ;
    dcterms:description "A studio course which provides an opportunity for the study of more specialized aspects of drawing." ;
    vivo:courseCredits 3 ;
    vivo:hasSubjectArea "DRAW " .

roboprof_data:DRAW_300 a vivo:Course ;
    dbo:name "Drawing II" ;
    dbo:number 300 ;
    dcterms:description "This studio course is an intermediate drawing course in which directed projects allow students to explore different approaches to drawing and to begin to develop a more personal visual language based on the skill sets acquired at the 200 level. Historical and contemporary issues in art practice are addressed in this course." ;
    vivo:courseCredits 3 ;
    vivo:hasSubjectArea "DRAW " .

roboprof_data:DRAW_310 a vivo:Course ;
    dbo:name "Narration, Time, Stories I" ;
    dbo:number 310 ;
    dcterms:description "This studio course encourages drawing based on personal experience or fictitious content, and the influence of film, books, diaries and illustration." ;
    vivo:courseCredits 4 ;
    vivo:hasSubjectArea "DRAW " .

roboprof_data:DRAW_312 a vivo:Course ;
    dbo:name "Drawing and Knowledge I" ;
    dbo:number 312 ;
    dcterms:description "This studio course explores a range of conceptual approaches to drawing using both traditional and experimental methods. " ;
    vivo:courseCredits 4 ;
    vivo:hasSubjectArea "DRAW " .

roboprof_data:DRAW_314 a vivo:Course ;
    dbo:name "Life in the Round: Drawing the Figure from Observation I" ;
    dbo:number 314 ;
    dcterms:description "This studio course focuses on the experience of seeing and depicting the living human body in all its complexity and presence." ;
    vivo:courseCredits 3 ;
    vivo:hasSubjectArea "DRAW " .

roboprof_data:DRAW_398 a vivo:Course ;
    dbo:name "Special Topics in Drawing" ;
    dbo:number 398 ;
    dcterms:description "A studio course which provides an opportunity for the study of more specialized aspects of drawing." ;
    vivo:courseCredits 3 ;
    vivo:hasSubjectArea "DRAW " .

roboprof_data:DRAW_399 a vivo:Course ;
    dbo:name "Special Topics in Drawing" ;
    dbo:number 399 ;
    dcterms:description "A studio course which provides an opportunity for the study of more specialized aspects of drawing." ;
    vivo:courseCredits 4 ;
    vivo:hasSubjectArea "DRAW " .

roboprof_data:DRAW_400 a vivo:Course ;
    dbo:name "Drawing III " ;
    dbo:number 400 ;
    dcterms:description "An advanced drawing class in which students develop a series of selfdirected projects in order to create a coherent body of work in drawing and to situate it within contemporary practice." ;
    vivo:courseCredits 3 ;
    vivo:hasSubjectArea "DRAW " .

roboprof_data:DRAW_410 a vivo:Course ;
    dbo:name "Narration, Time, Stories II " ;
    dbo:number 410 ;
    dcterms:description "This advancedlevel studio course encourages drawing based on personal experience or fictitious content, and the influence of film, books, diaries and illustration." ;
    vivo:courseCredits 4 ;
    vivo:hasSubjectArea "DRAW " .

roboprof_data:DRAW_412 a vivo:Course ;
    dbo:name "Drawing and Knowledge II" ;
    dbo:number 412 ;
    dcterms:description "This advancedlevel studio course explores a range of conceptual approaches to drawing using both traditional and experimental methods." ;
    vivo:courseCredits 3 ;
    vivo:hasSubjectArea "DRAW " .

roboprof_data:DRAW_414 a vivo:Course ;
    dbo:name "Life in the Round: Drawing the Figure from Observation II" ;
    dbo:number 414 ;
    dcterms:description "This advancedlevel studio course focuses on the experience of seeing and depicting the living human body in all its complexity and presence." ;
    vivo:courseCredits 4 ;
    vivo:hasSubjectArea "DRAW " .

roboprof_data:DRAW_418 a vivo:Course ;
    dbo:name "Life in the Round: Drawing the Figure from Observation II" ;
    dbo:number 418 ;
    dcterms:description "An installation studio course taught by the Painting and Drawing area that encourages students to create work in the context of an expanded field." ;
    vivo:courseCredits 3 ;
    vivo:hasSubjectArea "DRAW " .

roboprof_data:DRAW_420 a vivo:Course ;
    dbo:name "Seminar/Workshop in Drawing" ;
    dbo:number 420 ;
    dcterms:description "An advanced studio in drawing having its principal emphasis in studio practice, but developing further the theoretical concepts introduced in PTNG 320." ;
    vivo:courseCredits 4 ;
    vivo:hasSubjectArea "DRAW " .

roboprof_data:DRAW_450 a vivo:Course ;
    dbo:name "Drawing IV" ;
    dbo:number 450 ;
    dcterms:description "An advanced drawing class in which students develop a series of independent projects that allow them to create a coherent body of work in drawing and to situate it within contemporary practice." ;
    vivo:courseCredits 4 ;
    vivo:hasSubjectArea "DRAW " .

roboprof_data:DRAW_470 a vivo:Course ;
    dbo:name "Independent Study" ;
    dbo:number 470 ;
    dcterms:description "This course provides a limited number of students the opportunity to pursue advanced studies in drawing under the supervision of a fulltime drawing faculty member." ;
    vivo:courseCredits 4 ;
    vivo:hasSubjectArea "DRAW " .

roboprof_data:DRAW_471 a vivo:Course ;
    dbo:name "Independent Study I " ;
    dbo:number 471 ;
    dcterms:description "This course provides a limited number of students the opportunity to pursue advanced studies in drawing under the supervision of a fulltime drawing faculty member." ;
    vivo:courseCredits 4 ;
    vivo:hasSubjectArea "DRAW " .

roboprof_data:DRAW_472 a vivo:Course ;
    dbo:name "Independent Study II " ;
    dbo:number 472 ;
    dcterms:description "This course provides a limited number of students the opportunity to pursue advanced studies in drawing under the supervision of a fulltime drawing faculty member. " ;
    vivo:courseCredits 3 ;
    vivo:hasSubjectArea "DRAW " .

roboprof_data:DRAW_498 a vivo:Course ;
    dbo:name "Special Topics in Drawing" ;
    dbo:number 498 ;
    dcterms:description "A course for advanced students which provides an opportunity for the study of more specialized areas in drawing." ;
    vivo:courseCredits 3 ;
    vivo:hasSubjectArea "DRAW " .

roboprof_data:DRAW_499 a vivo:Course ;
    dbo:name "Special Topics in Drawing " ;
    dbo:number 499 ;
    dcterms:description "A course for advanced students which provides an opportunity for the study of more specialized areas in drawing. " ;
    vivo:courseCredits 4 ;
    vivo:hasSubjectArea "DRAW " .

roboprof_data:EAST_203 a vivo:Course ;
    dbo:name "DIGITAL AUDIO EDITING" ;
    dbo:number 203 ;
    dcterms:description "NaN"^^xsd:double ;
    vivo:courseCredits 3 ;
    vivo:hasSubjectArea "EAST" .

roboprof_data:EAST_451 a vivo:Course ;
    dbo:name "ADVANCED RECORDING I" ;
    dbo:number 451 ;
    dcterms:description "NaN"^^xsd:double ;
    vivo:courseCredits 4 ;
    vivo:hasSubjectArea "EAST" .

roboprof_data:EAST_463 a vivo:Course ;
    dbo:name "Concordia Laptop Orchestra II" ;
    dbo:number 463 ;
    dcterms:description "Co-creation, collaboration with artists, public performance" ;
    vivo:courseCredits 3 ;
    vivo:hasSubjectArea "EAST" .

roboprof_data:EAST_481 a vivo:Course ;
    dbo:name "Supervised Internship I" ;
    dbo:number 481 ;
    dcterms:description "Supervised internship at an industry/community partner" ;
    vivo:courseCredits 4 ;
    vivo:hasSubjectArea "EAST" .

roboprof_data:EAST_482 a vivo:Course ;
    dbo:name "Supervised Internship II" ;
    dbo:number 482 ;
    dcterms:description "Supervised internship at an industry/community partner" ;
    vivo:courseCredits 3 ;
    vivo:hasSubjectArea "EAST" .

roboprof_data:ECON_200 a vivo:Course ;
    dbo:name "Economics and Social Issues" ;
    dbo:number 200 ;
    dcterms:description "case studies" ;
    vivo:courseCredits 4 ;
    vivo:hasSubjectArea "ECON" .

roboprof_data:ECON_318 a vivo:Course ;
    dbo:name "Canadian Economic Policy and Institutions" ;
    dbo:number 318 ;
    dcterms:description "case studies; role-play" ;
    vivo:courseCredits 3 ;
    vivo:hasSubjectArea "ECON" .

roboprof_data:ECON_319 a vivo:Course ;
    dbo:name "International Economic Policy and Institutions" ;
    dbo:number 319 ;
    dcterms:description "case studies; role-play" ;
    vivo:courseCredits 3 ;
    vivo:hasSubjectArea "ECON" .

roboprof_data:ECON_324 a vivo:Course ;
    dbo:name "Economic Data Analysis" ;
    dbo:number 324 ;
    dcterms:description "computer-based applications" ;
    vivo:courseCredits 3 ;
    vivo:hasSubjectArea "ECON" .

roboprof_data:ECON_330 a vivo:Course ;
    dbo:name "Economics in Practice" ;
    dbo:number 330 ;
    dcterms:description "case studies; role-play" ;
    vivo:courseCredits 3 ;
    vivo:hasSubjectArea "ECON" .

roboprof_data:ECON_421 a vivo:Course ;
    dbo:name "Econometrics I" ;
    dbo:number 421 ;
    dcterms:description "computer-based applications" ;
    vivo:courseCredits 3 ;
    vivo:hasSubjectArea "ECON" .

roboprof_data:ECON_422 a vivo:Course ;
    dbo:name "Econometrics II" ;
    dbo:number 422 ;
    dcterms:description "computer-based applications" ;
    vivo:courseCredits 4 ;
    vivo:hasSubjectArea "ECON" .

roboprof_data:ECON_423 a vivo:Course ;
    dbo:name "Applied Econometrics" ;
    dbo:number 423 ;
    dcterms:description "computer analysis; case studies; model building" ;
    vivo:courseCredits 4 ;
    vivo:hasSubjectArea "ECON" .

roboprof_data:ECON_680 a vivo:Course ;
    dbo:name "Econometric Theory I" ;
    dbo:number 680 ;
    dcterms:description "computer-based applications" ;
    vivo:courseCredits 3 ;
    vivo:hasSubjectArea "ECON" .

roboprof_data:ECON_683 a vivo:Course ;
    dbo:name "Applied Econometrics: Microeconometrics" ;
    dbo:number 683 ;
    dcterms:description "practical aspects of analysis" ;
    vivo:courseCredits 4 ;
    vivo:hasSubjectArea "ECON" .

roboprof_data:ECON_695 a vivo:Course ;
    dbo:name "Special Topics: Computational Economics" ;
    dbo:number 695 ;
    dcterms:description "computer analysis; model building; practical aspects of analysis" ;
    vivo:courseCredits 4 ;
    vivo:hasSubjectArea "ECON" .

roboprof_data:ECON_696 a vivo:Course ;
    dbo:name "Research Methodology in Economics" ;
    dbo:number 696 ;
    dcterms:description "Activities focus on academic research specific to Economics. Students learn how to write an academic-level paper in Economics." ;
    vivo:courseCredits 4 ;
    vivo:hasSubjectArea "ECON" .

roboprof_data:ECON_806 a vivo:Course ;
    dbo:name "Research Seminar" ;
    dbo:number 806 ;
    dcterms:description "Experience-based seminar for PhD students in first and second year. Activities focus on academic and professional practice for economists, with emphasis on the job market. " ;
    vivo:courseCredits 4 ;
    vivo:hasSubjectArea "ECON" .

roboprof_data:EDUC_264 a vivo:Course ;
    dbo:name "Communication: Child, Parent and Teacher" ;
    dbo:number 264 ;
    dcterms:description "Students interact with parents of the children in the observation nursery by conducting and participating in parent-teacher seminars" ;
    vivo:courseCredits 3 ;
    vivo:hasSubjectArea "EDUC" .

roboprof_data:EDUC_301 a vivo:Course ;
    dbo:name "Integrating Computers into the Elementary Classroom" ;
    dbo:number 301 ;
    dcterms:description "Hands-on experience with the computer" ;
    vivo:courseCredits 3 ;
    vivo:hasSubjectArea "EDUC" .

roboprof_data:EDUC_302 a vivo:Course ;
    dbo:name "Working in Childhood Settings: Leadership and Organizational Issues" ;
    dbo:number 302 ;
    dcterms:description "Course-integrated project: Drafting an advocacy letter to the Ministre de Famille et des Aines; preparing a handbook for parents and staff in an early childhood setting; role-playing to simulate professional development and leadership." ;
    vivo:courseCredits 4 ;
    vivo:hasSubjectArea "EDUC" .

roboprof_data:EDUC_303 a vivo:Course ;
    dbo:name "Children, Families and Social Policy" ;
    dbo:number 303 ;
    dcterms:description "Group Project: Drafting policy statements, linking theoretical concepts with real-life needs and issues" ;
    vivo:courseCredits 4 ;
    vivo:hasSubjectArea "EDUC" .

roboprof_data:EDUC_304 a vivo:Course ;
    dbo:name "Play in Childhood Settings" ;
    dbo:number 304 ;
    dcterms:description "Course-integrated project: Designing play activities/material/space; arranging classroom configuration to explore play space; engaging in hands-on, play-based activities; using photo-elicitation methods in play; inquiry-based learning sessions using video case examples" ;
    vivo:courseCredits 4 ;
    vivo:hasSubjectArea "EDUC" .

roboprof_data:EDUC_307 a vivo:Course ;
    dbo:name "Integrating Digital Technologies and Social Media in Learning Environments" ;
    dbo:number 307 ;
    dcterms:description "Practical project-based activities" ;
    vivo:courseCredits 3 ;
    vivo:hasSubjectArea "EDUC" .

roboprof_data:EDUC_360 a vivo:Course ;
    dbo:name "Introduction to Inclusive Practices" ;
    dbo:number 360 ;
    dcterms:description "Active Learning activities that include case discussions, role-playing, and presentations; Analyzing psychoeducational evaluations to identify children's strengths and needs" ;
    vivo:courseCredits 4 ;
    vivo:hasSubjectArea "EDUC" .

roboprof_data:EDUC_361 a vivo:Course ;
    dbo:name "Inclusive Practices in Early Childhood Settings" ;
    dbo:number 361 ;
    dcterms:description "Group Project: Analysis of case studies to identify short- and long-term objectives, intervention strategies and activities for children with exceptionalities in early childhood settings" ;
    vivo:courseCredits 4 ;
    vivo:hasSubjectArea "EDUC" .

roboprof_data:EDUC_362 a vivo:Course ;
    dbo:name "Inclusive Practices for School-Aged Populations" ;
    dbo:number 362 ;
    dcterms:description "Group Project: Analysis of case studies to identify short- and long-term objectives, intervention strategies and activities for children with exceptionalities in childhood settings" ;
    vivo:courseCredits 3 ;
    vivo:hasSubjectArea "EDUC" .

roboprof_data:EDUC_382 a vivo:Course ;
    dbo:name "Teaching Science Concepts in the Elementary Classroom" ;
    dbo:number 382 ;
    dcterms:description "Developing activities for classroom use" ;
    vivo:courseCredits 3 ;
    vivo:hasSubjectArea "EDUC" .

roboprof_data:EDUC_385 a vivo:Course ;
    dbo:name "Teaching a Second Language in Early Childhood and Elementary School" ;
    dbo:number 385 ;
    dcterms:description "Development of appropriate classroom activities at the elementary level." ;
    vivo:courseCredits 3 ;
    vivo:hasSubjectArea "EDUC" .

roboprof_data:EDUC_402 a vivo:Course ;
    dbo:name "Diversity Issues in Childhood" ;
    dbo:number 402 ;
    dcterms:description "Course-integrated project: Student interview a parent or primary caregiver or an educator, and interpret/analyze responses in terms of the concepts and ideas covered in the course" ;
    vivo:courseCredits 4 ;
    vivo:hasSubjectArea "EDUC" .

roboprof_data:EDUC_406 a vivo:Course ;
    dbo:name "Physical Activity: Health and Well-being in Early Childhood Settings" ;
    dbo:number 406 ;
    dcterms:description "Identifying safety strategies in indoor and outdoor environments in early childhood settings; simulation and role-playing activities to practice procedures for reporting suspected child-safety and child-abuse issues" ;
    vivo:courseCredits 3 ;
    vivo:hasSubjectArea "EDUC" .

roboprof_data:EDUC_461 a vivo:Course ;
    dbo:name "Child Studies Seminar: Early Childhood Settings" ;
    dbo:number 461 ;
    dcterms:description "improvisation and role-play of communication skills; Preparing lesson plans, activity plans, observation reports; In-class case discussions" ;
    vivo:courseCredits 3 ;
    vivo:hasSubjectArea "EDUC" .

roboprof_data:EDUC_463 a vivo:Course ;
    dbo:name "Child Studies Seminar: Inclusive Practices in Childhood Settings" ;
    dbo:number 463 ;
    dcterms:description "Improvisation and role-play of communication skills; Preparing intervention goals and plans; identifying remediation and rehabilitation materials; modifying activities plans in accordance with inclusive practices; writing intervention reports; In-class case discussions" ;
    vivo:courseCredits 4 ;
    vivo:hasSubjectArea "EDUC" .

roboprof_data:ELEC_273 a vivo:Course ;
    dbo:name "Basic Circuit Analysis" ;
    dbo:number 273 ;
    dcterms:description "Laboratory: 15 hours total" ;
    vivo:courseCredits 4 ;
    vivo:hasSubjectArea "ELEC" .

roboprof_data:ELEC_275 a vivo:Course ;
    dbo:name "Principles of Electrical Engineering" ;
    dbo:number 275 ;
    dcterms:description "Laboratory: 15 hours total" ;
    vivo:courseCredits 3,
        4 ;
    vivo:hasSubjectArea "ELEC" .

roboprof_data:ELEC_311 a vivo:Course ;
    dbo:name "Electronics I" ;
    dbo:number 311 ;
    dcterms:description """Laboratory: 15 hours total_x000D_
Laboratory pre-labs, extensive simulation exercises""" ;
    vivo:courseCredits 3 ;
    vivo:hasSubjectArea "ELEC" .

roboprof_data:ELEC_312 a vivo:Course ;
    dbo:name "Electronics II" ;
    dbo:number 312 ;
    dcterms:description """Laboratory: 15 hours total_x000D_
Laboratory pre-labs, extensive simulation exercises""" ;
    vivo:courseCredits 4 ;
    vivo:hasSubjectArea "ELEC" .

roboprof_data:ELEC_321 a vivo:Course ;
    dbo:name "Introduction to Semiconductor Materials and Devices" ;
    dbo:number 321 ;
    dcterms:description "Laboratory: 15 hours total" ;
    vivo:courseCredits 4 ;
    vivo:hasSubjectArea "ELEC" .

roboprof_data:ELEC_331 a vivo:Course ;
    dbo:name "Fundamentals of Electrical Power Engineering" ;
    dbo:number 331 ;
    dcterms:description "Laboratory: 15 hours total" ;
    vivo:courseCredits 3 ;
    vivo:hasSubjectArea "ELEC" .

roboprof_data:ELEC_342 a vivo:Course ;
    dbo:name "Discrete-Time Signals and Systems" ;
    dbo:number 342 ;
    dcterms:description "Laboratory: 15 hours total" ;
    vivo:courseCredits 4 ;
    vivo:hasSubjectArea "ELEC" .

roboprof_data:ELEC_367 a vivo:Course ;
    dbo:name "Introduction to Digital Communications" ;
    dbo:number 367 ;
    dcterms:description "Laboratory: 15 hours total" ;
    vivo:courseCredits 4 ;
    vivo:hasSubjectArea "ELEC" .

roboprof_data:ELEC_372 a vivo:Course ;
    dbo:name "Fundamentals of Control Systems" ;
    dbo:number 372 ;
    dcterms:description "Laboratory: 15 hours total" ;
    vivo:courseCredits 4 ;
    vivo:hasSubjectArea "ELEC" .

roboprof_data:ELEC_390 a vivo:Course ;
    dbo:name "Electrical Engineering Product Design Project" ;
    dbo:number 390 ;
    dcterms:description "Team, Build system/device, Equivalent laboratory time: 6 hours per week" ;
    vivo:courseCredits 3 ;
    vivo:hasSubjectArea "ELEC" .

roboprof_data:ELEC_421 a vivo:Course ;
    dbo:name "Solid State Devices" ;
    dbo:number 421 ;
    dcterms:description """Design, fabricate_x000D_
Laboratory: 15 hours total""" ;
    vivo:courseCredits 3 ;
    vivo:hasSubjectArea "ELEC" .

roboprof_data:ELEC_422 a vivo:Course ;
    dbo:name "Design of Integrated Circuit Components" ;
    dbo:number 422 ;
    dcterms:description """Design, fabricate_x000D_
Laboratory: 15 hours total""" ;
    vivo:courseCredits 4 ;
    vivo:hasSubjectArea "ELEC" .

roboprof_data:ELEC_423 a vivo:Course ;
    dbo:name "Introduction to Analog VLSI" ;
    dbo:number 423 ;
    dcterms:description "Design, Laboratory: 30 hours total" ;
    vivo:courseCredits 3 ;
    vivo:hasSubjectArea "ELEC" .

roboprof_data:ELEC_424 a vivo:Course ;
    dbo:name "VLSI Process Technology" ;
    dbo:number 424 ;
    dcterms:description "Device fabrication, Laboratory: 15 hours total" ;
    vivo:courseCredits 3 ;
    vivo:hasSubjectArea "ELEC" .

roboprof_data:ELEC_425 a vivo:Course ;
    dbo:name "Optical Devices for High-Speed Communications" ;
    dbo:number 425 ;
    dcterms:description "Laboratory: 15 hours total" ;
    vivo:courseCredits 4 ;
    vivo:hasSubjectArea "ELEC" .

roboprof_data:ELEC_430 a vivo:Course ;
    dbo:name "Electrical Power Equipment" ;
    dbo:number 430 ;
    dcterms:description "Laboratory: 15 hours total" ;
    vivo:courseCredits 4 ;
    vivo:hasSubjectArea "ELEC" .

roboprof_data:ELEC_431 a vivo:Course ;
    dbo:name "Electrical Power Systems" ;
    dbo:number 431 ;
    dcterms:description "Laboratory: 15 hours total" ;
    vivo:courseCredits 3 ;
    vivo:hasSubjectArea "ELEC" .

roboprof_data:ELEC_432 a vivo:Course ;
    dbo:name "Control of Electrical Power Conversion Systems" ;
    dbo:number 432 ;
    dcterms:description "System design, Laboratory: 15 hours total" ;
    vivo:courseCredits 4 ;
    vivo:hasSubjectArea "ELEC" .

roboprof_data:ELEC_433 a vivo:Course ;
    dbo:name "Power Electronics" ;
    dbo:number 433 ;
    dcterms:description "Laboratory: 15 hours total" ;
    vivo:courseCredits 4 ;
    vivo:hasSubjectArea "ELEC" .

roboprof_data:ELEC_434 a vivo:Course ;
    dbo:name "Behaviour of Power Systems" ;
    dbo:number 434 ;
    dcterms:description "Laboratory: 15 hours total" ;
    vivo:courseCredits 3 ;
    vivo:hasSubjectArea "ELEC" .

roboprof_data:ELEC_435 a vivo:Course ;
    dbo:name "Electromechanical Energy Conversion Systems" ;
    dbo:number 435 ;
    dcterms:description "Laboratory: 15 hours total" ;
    vivo:courseCredits 4 ;
    vivo:hasSubjectArea "ELEC" .

roboprof_data:ELEC_436 a vivo:Course ;
    dbo:name "Protection of Power Systems" ;
    dbo:number 436 ;
    dcterms:description "Laboratory: 15 hours total" ;
    vivo:courseCredits 4 ;
    vivo:hasSubjectArea "ELEC" .

roboprof_data:ELEC_438 a vivo:Course ;
    dbo:name "Industrial Electrical Systems" ;
    dbo:number 438 ;
    dcterms:description "Laboratory: 15 hours total" ;
    vivo:courseCredits 4 ;
    vivo:hasSubjectArea "ELEC" .

roboprof_data:ELEC_440 a vivo:Course ;
    dbo:name "Controlled Electric Drives" ;
    dbo:number 440 ;
    dcterms:description "Laboratory: 15 hours total" ;
    vivo:courseCredits 4 ;
    vivo:hasSubjectArea "ELEC" .

roboprof_data:ELEC_441 a vivo:Course ;
    dbo:name "Modern Analog Filter Design" ;
    dbo:number 441 ;
    dcterms:description "Laboratory: 15 hours total" ;
    vivo:courseCredits 3 ;
    vivo:hasSubjectArea "ELEC" .

roboprof_data:ELEC_442 a vivo:Course ;
    dbo:name "Digital Signal Processing" ;
    dbo:number 442 ;
    dcterms:description "Laboratory: 15 hours total" ;
    vivo:courseCredits 3 ;
    vivo:hasSubjectArea "ELEC" .

roboprof_data:ELEC_453 a vivo:Course ;
    dbo:name "Microwave Engineering" ;
    dbo:number 453 ;
    dcterms:description "Laboratory: 15 hours total" ;
    vivo:courseCredits 4 ;
    vivo:hasSubjectArea "ELEC" .

roboprof_data:ELEC_456 a vivo:Course ;
    dbo:name "Antennas" ;
    dbo:number 456 ;
    dcterms:description "Laboratory: 15 hours total" ;
    vivo:courseCredits 4 ;
    vivo:hasSubjectArea "ELEC" .

roboprof_data:ELEC_463 a vivo:Course ;
    dbo:name "Telecommunication Network" ;
    dbo:number 463 ;
    dcterms:description "Laboratory: 15 hours total" ;
    vivo:courseCredits 4 ;
    vivo:hasSubjectArea "ELEC" .

roboprof_data:ELEC_465 a vivo:Course ;
    dbo:name "Networks Security and Management" ;
    dbo:number 465 ;
    dcterms:description "Laboratory: 15 hours total" ;
    vivo:courseCredits 4 ;
    vivo:hasSubjectArea "ELEC" .

roboprof_data:ELEC_466 a vivo:Course ;
    dbo:name "Introduction to Optical Communication Systems" ;
    dbo:number 466 ;
    dcterms:description "Laboratory: 15 hours total" ;
    vivo:courseCredits 3 ;
    vivo:hasSubjectArea "ELEC" .

roboprof_data:ELEC_472 a vivo:Course ;
    dbo:name "Advanced Telecommunication Network" ;
    dbo:number 472 ;
    dcterms:description "Laboratory: 15 hours total" ;
    vivo:courseCredits 4 ;
    vivo:hasSubjectArea "ELEC" .

roboprof_data:ELEC_481 a vivo:Course ;
    dbo:name "Linear Systems" ;
    dbo:number 481 ;
    dcterms:description "Laboratory: 15 hours total" ;
    vivo:courseCredits 3 ;
    vivo:hasSubjectArea "ELEC" .

roboprof_data:ELEC_482 a vivo:Course ;
    dbo:name "System Optimization" ;
    dbo:number 482 ;
    dcterms:description "Laboratory: 15 hours total" ;
    vivo:courseCredits 4 ;
    vivo:hasSubjectArea "ELEC" .

roboprof_data:ELEC_483 a vivo:Course ;
    dbo:name "Real-Time Computer Control Systems" ;
    dbo:number 483 ;
    dcterms:description "Laboratory: 15 hours total" ;
    vivo:courseCredits 3 ;
    vivo:hasSubjectArea "ELEC" .

roboprof_data:ELEC_490 a vivo:Course ;
    dbo:name "Capstone Electrical Engineering Design Project" ;
    dbo:number 490 ;
    dcterms:description "capstone, group project" ;
    vivo:courseCredits 4 ;
    vivo:hasSubjectArea "ELEC" .

roboprof_data:ELEC_6041 a vivo:Course ;
    dbo:name "Large-scale Control Systems" ;
    dbo:number 6041 ;
    dcterms:description "A project is required" ;
    vivo:courseCredits 4 ;
    vivo:hasSubjectArea "ELEC" .

roboprof_data:ELEC_6051 a vivo:Course ;
    dbo:name "Introduction to Analog VLSI" ;
    dbo:number 6051 ;
    dcterms:description "A project is required" ;
    vivo:courseCredits 4 ;
    vivo:hasSubjectArea "ELEC" .

roboprof_data:ELEC_6061 a vivo:Course ;
    dbo:name "Real-time Computer Control Systems" ;
    dbo:number 6061 ;
    dcterms:description "A project is required" ;
    vivo:courseCredits 4 ;
    vivo:hasSubjectArea "ELEC" .

roboprof_data:ELEC_6081 a vivo:Course ;
    dbo:name "Modern Analog Filter Design" ;
    dbo:number 6081 ;
    dcterms:description "A project is required" ;
    vivo:courseCredits 3 ;
    vivo:hasSubjectArea "ELEC" .

roboprof_data:ELEC_6091 a vivo:Course ;
    dbo:name "Discrete Event Systems" ;
    dbo:number 6091 ;
    dcterms:description "A project is required" ;
    vivo:courseCredits 4 ;
    vivo:hasSubjectArea "ELEC" .

roboprof_data:ELEC_6111 a vivo:Course ;
    dbo:name "Detection and Estimation Theory" ;
    dbo:number 6111 ;
    dcterms:description "A project is required" ;
    vivo:courseCredits 3 ;
    vivo:hasSubjectArea "ELEC" .

roboprof_data:ELEC_6131 a vivo:Course ;
    dbo:name "Error Detecting and Correcting Codes" ;
    dbo:number 6131 ;
    dcterms:description "A project is required" ;
    vivo:courseCredits 3 ;
    vivo:hasSubjectArea "ELEC" .

roboprof_data:ELEC_6141 a vivo:Course ;
    dbo:name "Wireless Communications" ;
    dbo:number 6141 ;
    dcterms:description "A project is required" ;
    vivo:courseCredits 4 ;
    vivo:hasSubjectArea "ELEC" .

roboprof_data:ELEC_6151 a vivo:Course ;
    dbo:name "Information Theory and Source Coding" ;
    dbo:number 6151 ;
    dcterms:description "A project is required" ;
    vivo:courseCredits 3 ;
    vivo:hasSubjectArea "ELEC" .

roboprof_data:ELEC_6171 a vivo:Course ;
    dbo:name "Modelling and Analysis of Telecommunications Networks" ;
    dbo:number 6171 ;
    dcterms:description "A project is required" ;
    vivo:courseCredits 4 ;
    vivo:hasSubjectArea "ELEC" .

roboprof_data:ELEC_6181 a vivo:Course ;
    dbo:name "Real-time and Multimedia Communication over Internet" ;
    dbo:number 6181 ;
    dcterms:description "A project is required" ;
    vivo:courseCredits 3 ;
    vivo:hasSubjectArea "ELEC" .

roboprof_data:ELEC_6221 a vivo:Course ;
    dbo:name "Solid State Devices" ;
    dbo:number 6221 ;
    dcterms:description "A project is required" ;
    vivo:courseCredits 4 ;
    vivo:hasSubjectArea "ELEC" .

roboprof_data:ELEC_6231 a vivo:Course ;
    dbo:name "Design of Integrated Circuit Components" ;
    dbo:number 6231 ;
    dcterms:description "A project is required" ;
    vivo:courseCredits 4 ;
    vivo:hasSubjectArea "ELEC" .

roboprof_data:ELEC_6241 a vivo:Course ;
    dbo:name "VLSI Process Technology" ;
    dbo:number 6241 ;
    dcterms:description "A project is required" ;
    vivo:courseCredits 4 ;
    vivo:hasSubjectArea "ELEC" .

roboprof_data:ELEC_6251 a vivo:Course ;
    dbo:name "Microtransducer Process Technology" ;
    dbo:number 6251 ;
    dcterms:description "A project is required" ;
    vivo:courseCredits 3 ;
    vivo:hasSubjectArea "ELEC" .

roboprof_data:ELEC_6261 a vivo:Course ;
    dbo:name "Optical Devices for High-Speed Communications" ;
    dbo:number 6261 ;
    dcterms:description "A project is required" ;
    vivo:courseCredits 3 ;
    vivo:hasSubjectArea "ELEC" .

roboprof_data:ELEC_6271 a vivo:Course ;
    dbo:name "Nanoscience and Nanotechnology: Opto-Electronic Devices" ;
    dbo:number 6271 ;
    dcterms:description "A project is required" ;
    vivo:courseCredits 3 ;
    vivo:hasSubjectArea "ELEC" .

roboprof_data:ELEC_6281 a vivo:Course ;
    dbo:name "Principles of Solid State Nanodevices" ;
    dbo:number 6281 ;
    dcterms:description "A project is required" ;
    vivo:courseCredits 4 ;
    vivo:hasSubjectArea "ELEC" .

roboprof_data:ELEC_6301 a vivo:Course ;
    dbo:name "Advanced Electromagnetics" ;
    dbo:number 6301 ;
    dcterms:description "A project is required" ;
    vivo:courseCredits 3 ;
    vivo:hasSubjectArea "ELEC" .

roboprof_data:ELEC_6311 a vivo:Course ;
    dbo:name "Radiation and Scattering of Waves" ;
    dbo:number 6311 ;
    dcterms:description "A project is required" ;
    vivo:courseCredits 3 ;
    vivo:hasSubjectArea "ELEC" .

roboprof_data:ELEC_6341 a vivo:Course ;
    dbo:name "Antennas" ;
    dbo:number 6341 ;
    dcterms:description "A project is required" ;
    vivo:courseCredits 4 ;
    vivo:hasSubjectArea "ELEC" .

roboprof_data:ELEC_6351 a vivo:Course ;
    dbo:name "Modern Antenna Theory" ;
    dbo:number 6351 ;
    dcterms:description "A project is required" ;
    vivo:courseCredits 3 ;
    vivo:hasSubjectArea "ELEC" .

roboprof_data:ELEC_6361 a vivo:Course ;
    dbo:name "Acoustics" ;
    dbo:number 6361 ;
    dcterms:description "A project is required" ;
    vivo:courseCredits 3 ;
    vivo:hasSubjectArea "ELEC" .

roboprof_data:ELEC_6371 a vivo:Course ;
    dbo:name "Design of Wireless RF Systems" ;
    dbo:number 6371 ;
    dcterms:description "A project is required" ;
    vivo:courseCredits 4 ;
    vivo:hasSubjectArea "ELEC" .

roboprof_data:ELEC_6381 a vivo:Course ;
    dbo:name "Techniques in Electromagnetic Compatibility" ;
    dbo:number 6381 ;
    dcterms:description "A project is required" ;
    vivo:courseCredits 4 ;
    vivo:hasSubjectArea "ELEC" .

roboprof_data:ELEC_6391 a vivo:Course ;
    dbo:name "Microwave Engineering" ;
    dbo:number 6391 ;
    dcterms:description "A project is required" ;
    vivo:courseCredits 3 ;
    vivo:hasSubjectArea "ELEC" .

roboprof_data:ELEC_6411 a vivo:Course ;
    dbo:name "Power Electronics I" ;
    dbo:number 6411 ;
    dcterms:description "A project is required" ;
    vivo:courseCredits 3 ;
    vivo:hasSubjectArea "ELEC" .

roboprof_data:ELEC_6421 a vivo:Course ;
    dbo:name "Renewable Energy Systems" ;
    dbo:number 6421 ;
    dcterms:description "A project is required" ;
    vivo:courseCredits 3 ;
    vivo:hasSubjectArea "ELEC" .

roboprof_data:ELEC_6431 a vivo:Course ;
    dbo:name "Advanced Electrical Machines and Drives" ;
    dbo:number 6431 ;
    dcterms:description "A project is required" ;
    vivo:courseCredits 3 ;
    vivo:hasSubjectArea "ELEC" .

roboprof_data:ELEC_6461 a vivo:Course ;
    dbo:name "Power Electronics II" ;
    dbo:number 6461 ;
    dcterms:description "A project is required" ;
    vivo:courseCredits 4 ;
    vivo:hasSubjectArea "ELEC" .

roboprof_data:ELEC_6471 a vivo:Course ;
    dbo:name "Hybrid Electric Vehicle Power System Design and Control" ;
    dbo:number 6471 ;
    dcterms:description "A project is required" ;
    vivo:courseCredits 3 ;
    vivo:hasSubjectArea "ELEC" .

roboprof_data:ELEC_6481 a vivo:Course ;
    dbo:name "Computer-aided Analysis of Power Electronic Systems" ;
    dbo:number 6481 ;
    dcterms:description "A project is required" ;
    vivo:courseCredits 4 ;
    vivo:hasSubjectArea "ELEC" .

roboprof_data:ELEC_6491 a vivo:Course ;
    dbo:name "Controlled Electric Drives" ;
    dbo:number 6491 ;
    dcterms:description "A project is required" ;
    vivo:courseCredits 3 ;
    vivo:hasSubjectArea "ELEC" .

roboprof_data:ELEC_6601 a vivo:Course ;
    dbo:name "Digital Signal Processing" ;
    dbo:number 6601 ;
    dcterms:description "A project is required" ;
    vivo:courseCredits 3 ;
    vivo:hasSubjectArea "ELEC" .

roboprof_data:ELEC_6611 a vivo:Course ;
    dbo:name "Digital Filters" ;
    dbo:number 6611 ;
    dcterms:description "A project is required" ;
    vivo:courseCredits 3 ;
    vivo:hasSubjectArea "ELEC" .

roboprof_data:ELEC_6621 a vivo:Course ;
    dbo:name "Digital Waveform Compression" ;
    dbo:number 6621 ;
    dcterms:description "A project is required" ;
    vivo:courseCredits 3 ;
    vivo:hasSubjectArea "ELEC" .

roboprof_data:ELEC_6631 a vivo:Course ;
    dbo:name "Video Processing and Compression" ;
    dbo:number 6631 ;
    dcterms:description "A project is required" ;
    vivo:courseCredits 3 ;
    vivo:hasSubjectArea "ELEC" .

roboprof_data:ELEC_6641 a vivo:Course ;
    dbo:name "Two-dimensional Signal and Image Processing" ;
    dbo:number 6641 ;
    dcterms:description "A project is required" ;
    vivo:courseCredits 4 ;
    vivo:hasSubjectArea "ELEC" .

roboprof_data:ELEC_6651 a vivo:Course ;
    dbo:name "Adaptive Signal Processing" ;
    dbo:number 6651 ;
    dcterms:description "A project is required" ;
    vivo:courseCredits 3 ;
    vivo:hasSubjectArea "ELEC" .

roboprof_data:ELEC_6661 a vivo:Course ;
    dbo:name "Medical Image Processing" ;
    dbo:number 6661 ;
    dcterms:description "A project is required" ;
    vivo:courseCredits 3 ;
    vivo:hasSubjectArea "ELEC" .

roboprof_data:ELEC_6831 a vivo:Course ;
    dbo:name "Digital Communications" ;
    dbo:number 6831 ;
    dcterms:description "A project is required" ;
    vivo:courseCredits 3 ;
    vivo:hasSubjectArea "ELEC" .

roboprof_data:ELEC_6841 a vivo:Course ;
    dbo:name "Advanced Digital Communications" ;
    dbo:number 6841 ;
    dcterms:description "A project is required" ;
    vivo:courseCredits 4 ;
    vivo:hasSubjectArea "ELEC" .

roboprof_data:ELEC_6851 a vivo:Course ;
    dbo:name "Telecommunications Networks" ;
    dbo:number 6851 ;
    dcterms:description "A project is required" ;
    vivo:courseCredits 3 ;
    vivo:hasSubjectArea "ELEC" .

roboprof_data:ELEC_6861 a vivo:Course ;
    dbo:name "Higher Layer Telecommunications Protocols" ;
    dbo:number 6861 ;
    dcterms:description "A project is required" ;
    vivo:courseCredits 4 ;
    vivo:hasSubjectArea "ELEC" .

roboprof_data:ELEC_6871 a vivo:Course ;
    dbo:name "Fiber-Optic Communication Systems and Networks" ;
    dbo:number 6871 ;
    dcterms:description "A project is required" ;
    vivo:courseCredits 3 ;
    vivo:hasSubjectArea "ELEC" .

roboprof_data:ELEC_6881 a vivo:Course ;
    dbo:name "Fundamentals and Applications of MIMO Communications" ;
    dbo:number 6881 ;
    dcterms:description "A project is required" ;
    vivo:courseCredits 4 ;
    vivo:hasSubjectArea "ELEC" .

roboprof_data:ELEC_7151 a vivo:Course ;
    dbo:name "Broadband Communications Networks" ;
    dbo:number 7151 ;
    dcterms:description "A project is required" ;
    vivo:courseCredits 4 ;
    vivo:hasSubjectArea "ELEC" .

roboprof_data:ELEC_7441 a vivo:Course ;
    dbo:name "Design of Power Electronic Circuits" ;
    dbo:number 7441 ;
    dcterms:description "A project is required" ;
    vivo:courseCredits 4 ;
    vivo:hasSubjectArea "ELEC" .

roboprof_data:ELEC_7451 a vivo:Course ;
    dbo:name "Power System Compensation" ;
    dbo:number 7451 ;
    dcterms:description "A project is required" ;
    vivo:courseCredits 4 ;
    vivo:hasSubjectArea "ELEC" .

roboprof_data:EMBA_610 a vivo:Course ;
    dbo:name "Measuring and Reporting Financial Performance" ;
    dbo:number 610 ;
    dcterms:description "Case method" ;
    vivo:courseCredits 4 ;
    vivo:hasSubjectArea "EMBA" .

roboprof_data:EMBA_611 a vivo:Course ;
    dbo:name "Managing Talent" ;
    dbo:number 611 ;
    dcterms:description "Case studies" ;
    vivo:courseCredits 3 ;
    vivo:hasSubjectArea "EMBA" .

roboprof_data:EMBA_612 a vivo:Course ;
    dbo:name "Marketing Management" ;
    dbo:number 612 ;
    dcterms:description "Case discussions & application-oriented readings" ;
    vivo:courseCredits 3 ;
    vivo:hasSubjectArea "EMBA" .

roboprof_data:EMBA_621 a vivo:Course ;
    dbo:name "Information Technology and Analytics" ;
    dbo:number 621 ;
    dcterms:description "Projects & case studies" ;
    vivo:courseCredits 3 ;
    vivo:hasSubjectArea "EMBA" .

roboprof_data:EMBA_625 a vivo:Course ;
    dbo:name "Global Experience" ;
    dbo:number 625 ;
    dcterms:description "Experience doing business abroad" ;
    vivo:courseCredits 4 ;
    vivo:hasSubjectArea "EMBA" .

roboprof_data:EMBA_630 a vivo:Course ;
    dbo:name "Financial Decisions Under Uncertainty" ;
    dbo:number 630 ;
    dcterms:description "Cases & projects" ;
    vivo:courseCredits 3 ;
    vivo:hasSubjectArea "EMBA" .

roboprof_data:EMBA_631 a vivo:Course ;
    dbo:name "Management Control Systems" ;
    dbo:number 631 ;
    dcterms:description "Practical cases & applications reflecting real organizational issues" ;
    vivo:courseCredits 4 ;
    vivo:hasSubjectArea "EMBA" .

roboprof_data:EMBA_632 a vivo:Course ;
    dbo:name "Creativity and Innovation" ;
    dbo:number 632 ;
    dcterms:description "Case studies & experiential exercises" ;
    vivo:courseCredits 3 ;
    vivo:hasSubjectArea "EMBA" .

roboprof_data:EMBA_633 a vivo:Course ;
    dbo:name "Applied Field Project I" ;
    dbo:number 633 ;
    dcterms:description "Field project and business project proposal" ;
    vivo:courseCredits 3 ;
    vivo:hasSubjectArea "EMBA" .

roboprof_data:EMBA_635 a vivo:Course ;
    dbo:name "Starting a New Venture" ;
    dbo:number 635 ;
    dcterms:description "Business plans to a board of potential investors" ;
    vivo:courseCredits 3 ;
    vivo:hasSubjectArea "EMBA" .

roboprof_data:EMBA_640 a vivo:Course ;
    dbo:name "Leadership" ;
    dbo:number 640 ;
    dcterms:description "Practical exercises, case studies, simulations & role-playing activities" ;
    vivo:courseCredits 3 ;
    vivo:hasSubjectArea "EMBA" .

roboprof_data:EMBA_645 a vivo:Course ;
    dbo:name "Applied Field Project II" ;
    dbo:number 645 ;
    dcterms:description "Field project" ;
    vivo:courseCredits 3 ;
    vivo:hasSubjectArea "EMBA" .

roboprof_data:EMBA_676 a vivo:Course ;
    dbo:name "International Study Trip" ;
    dbo:number 676 ;
    dcterms:description "Field school" ;
    vivo:courseCredits 4 ;
    vivo:hasSubjectArea "EMBA" .

roboprof_data:EMBA_690 a vivo:Course ;
    dbo:name "Management Consulting Project" ;
    dbo:number 690 ;
    dcterms:description "Course" ;
    vivo:courseCredits 4 ;
    vivo:hasSubjectArea "EMBA" .

roboprof_data:ENCS_272 a vivo:Course ;
    dbo:name "Argumentation and Composition for Engineers" ;
    dbo:number 272 ;
    dcterms:description "Course-integrated projects; Team project" ;
    vivo:courseCredits 4 ;
    vivo:hasSubjectArea "ENCS" .

roboprof_data:ENCS_282 a vivo:Course ;
    dbo:name "Technical Communication" ;
    dbo:number 282 ;
    dcterms:description "Course-integrated project; Simulations; Case Studies" ;
    vivo:courseCredits 3 ;
    vivo:hasSubjectArea "ENCS" .

roboprof_data:ENCS_393 a vivo:Course ;
    dbo:name "Impact of information and Communication Technologies on Society" ;
    dbo:number 393 ;
    dcterms:description "Course-integrated project; Games/Role Playing; Case Studies; Simulations" ;
    vivo:courseCredits 3 ;
    vivo:hasSubjectArea "ENCS" .

roboprof_data:ENCS_483 a vivo:Course ;
    dbo:name "Innovation and Critical Thinking in Science and Technology (also listed as ENCS 6041)" ;
    dbo:number 483 ;
    dcterms:description "Simulations, course-integrated projects, case studies & real time innovation challenges" ;
    vivo:courseCredits 3 ;
    vivo:hasSubjectArea "ENCS" .

roboprof_data:ENCS_484 a vivo:Course ;
    dbo:name "Development & Global Engineering (also listed as ENCS 6821)" ;
    dbo:number 484 ;
    dcterms:description "Course-integrated project; Games; Case Studies;" ;
    vivo:courseCredits 3 ;
    vivo:hasSubjectArea "ENCS" .

roboprof_data:ENCS_485 a vivo:Course ;
    dbo:name "Rwanda Field School in Engineering and Sustainable Development" ;
    dbo:number 485 ;
    dcterms:description "Intensive course with three classroom sessions in Montreal, followed by a 3-week trip to Rwanda. Based on contemporary scholarship around development initiatives that focus on technological intervention. Site visits in rural and urban settings. conversations with Rwandan stakeholders, and interactions with students and professors at University of Rwanda campuses in Kigali and Huye." ;
    vivo:courseCredits 4 ;
    vivo:hasSubjectArea "ENCS" .

roboprof_data:ENCS_5721 a vivo:Course ;
    dbo:name "Argumentation and Composition for Engineers" ;
    dbo:number 5721 ;
    dcterms:description "Course-integrated project; Case Studies" ;
    vivo:courseCredits 4 ;
    vivo:hasSubjectArea "ENCS" .

roboprof_data:ENCS_6041 a vivo:Course ;
    dbo:name "Innovation and Critical Thinking in Science and Technology (also listed as ENCS 6041)" ;
    dbo:number 6041 ;
    dcterms:description "Simulations, course-integrated projects, case studies & real time innovation challenges" ;
    vivo:courseCredits 3 ;
    vivo:hasSubjectArea "ENCS" .

roboprof_data:ENCS_6042 a vivo:Course ;
    dbo:name "Communication for the Innovation Process" ;
    dbo:number 6042 ;
    dcterms:description "Simulations, course-integrated projects, case studies & real time innovation challenges" ;
    vivo:courseCredits 4 ;
    vivo:hasSubjectArea "ENCS" .

roboprof_data:ENCS_6043 a vivo:Course ;
    dbo:name "Seminar in Innovation Process" ;
    dbo:number 6043 ;
    dcterms:description "Building network with industry, real time case studies with industry" ;
    vivo:courseCredits 4 ;
    vivo:hasSubjectArea "ENCS" .

roboprof_data:ENCS_6044 a vivo:Course ;
    dbo:name "Practicum in Innovation" ;
    dbo:number 6044 ;
    dcterms:description "Fully integrated practicum project" ;
    vivo:courseCredits 4 ;
    vivo:hasSubjectArea "ENCS" .

roboprof_data:ENCS_6721 a vivo:Course ;
    dbo:name "Technical Writing and Research Methods for Engineers and Computer Scientists" ;
    dbo:number 6721 ;
    dcterms:description "Major research project" ;
    vivo:courseCredits 4 ;
    vivo:hasSubjectArea "ENCS" .

roboprof_data:ENCS_6821 a vivo:Course ;
    dbo:name "Development & Global Engineering (also listed as ENCS 6821)" ;
    dbo:number 6821 ;
    dcterms:description "Course-integrated project; Games; Case Studies;" ;
    vivo:courseCredits 4 ;
    vivo:hasSubjectArea "ENCS" .

roboprof_data:ENCS_691 a vivo:Course ;
    dbo:name "Technology Policy Immersion" ;
    dbo:number 691 ;
    dcterms:description "Course-integrated project; Case Studies" ;
    vivo:courseCredits 4 ;
    vivo:hasSubjectArea "ENCS" .

roboprof_data:ENCS_8511 a vivo:Course ;
    dbo:name "Doctoral Research Proposal" ;
    dbo:number 8511 ;
    dcterms:description "Doctoral research proposal" ;
    vivo:courseCredits 3 ;
    vivo:hasSubjectArea "ENCS" .

roboprof_data:ENGL_215 a vivo:Course ;
    dbo:name "Editing II" ;
    dbo:number 215 ;
    dcterms:description "Advanced editing with emphasis on copyediting, stylistic editing, and structural editing; student manage an editing project with a student author from Creative or Professional writing." ;
    vivo:courseCredits 4 ;
    vivo:hasSubjectArea "ENGL" .

roboprof_data:ENGL_224 a vivo:Course ;
    dbo:name "The Creative Process" ;
    dbo:number 224 ;
    dcterms:description "This course introduces students to some options for developing their own process of literary creation, from the ENGLISH development of an idea through to the writing and editing of works of prose fiction, poetry, and/or drama." ;
    vivo:courseCredits 3 ;
    vivo:hasSubjectArea "ENGL" .

roboprof_data:ENGL_225 a vivo:Course ;
    dbo:name "Introductory Creative Writing: Poetry" ;
    dbo:number 225 ;
    dcterms:description "Writing workshop (peer critique, revision, ongoing development)" ;
    vivo:courseCredits 3 ;
    vivo:hasSubjectArea "ENGL" .

roboprof_data:ENGL_226 a vivo:Course ;
    dbo:name "Introductory Creative Writing: Prose Fiction" ;
    dbo:number 226 ;
    dcterms:description "Writing workshop (peer critique, revision, ongoing development)" ;
    vivo:courseCredits 3 ;
    vivo:hasSubjectArea "ENGL" .

roboprof_data:ENGL_227 a vivo:Course ;
    dbo:name "Introductory Creative Writing: Playwriting" ;
    dbo:number 227 ;
    dcterms:description "Writing workshop (peer critique, revision, ongoing development)" ;
    vivo:courseCredits 3 ;
    vivo:hasSubjectArea "ENGL" .

roboprof_data:ENGL_342 a vivo:Course ;
    dbo:name "Creative Writing: Prose Fiction" ;
    dbo:number 342 ;
    dcterms:description "Writing workshop (peer critique, revision, ongoing development)" ;
    vivo:courseCredits 3 ;
    vivo:hasSubjectArea "ENGL" .

roboprof_data:ENGL_347 a vivo:Course ;
    dbo:name "Creative Non-Fiction Writing" ;
    dbo:number 347 ;
    dcterms:description "Writing workshop (peer critique, revision, ongoing development)" ;
    vivo:courseCredits 3 ;
    vivo:hasSubjectArea "ENGL" .

roboprof_data:ENGL_348 a vivo:Course ;
    dbo:name "Creative Writing: Poetry" ;
    dbo:number 348 ;
    dcterms:description "Writing workshop (peer critique, revision, ongoing development)" ;
    vivo:courseCredits 3 ;
    vivo:hasSubjectArea "ENGL" .

roboprof_data:ENGL_384 a vivo:Course ;
    dbo:name "Creative Writing: Playwriting" ;
    dbo:number 384 ;
    dcterms:description "Writing workshop (peer critique, revision, ongoing development)" ;
    vivo:courseCredits 4 ;
    vivo:hasSubjectArea "ENGL" .

roboprof_data:ENGL_396 a vivo:Course ;
    dbo:name "Content Creation and Management in Professional Writing" ;
    dbo:number 396 ;
    dcterms:description "Students create and curate material for different platforms, primarily digital." ;
    vivo:courseCredits 3 ;
    vivo:hasSubjectArea "ENGL" .

roboprof_data:ENGL_414 a vivo:Course ;
    dbo:name "Literary Publishing and Editing" ;
    dbo:number 414 ;
    dcterms:description "Workshop in publishing and editing, involving hands-on projects" ;
    vivo:courseCredits 4 ;
    vivo:hasSubjectArea "ENGL" .

roboprof_data:ENGL_415 a vivo:Course ;
    dbo:name "Literary Production: Curating and Archiving the Literary Event" ;
    dbo:number 415 ;
    dcterms:description "Students aid in the development and maintenance of a related blog and an archive of current and previous reading series" ;
    vivo:courseCredits 4 ;
    vivo:hasSubjectArea "ENGL" .

roboprof_data:ENGL_416 a vivo:Course ;
    dbo:name "The Solo Play" ;
    dbo:number 416 ;
    dcterms:description "Writing workshop (peer critique, revision, ongoing development)" ;
    vivo:courseCredits 3 ;
    vivo:hasSubjectArea "ENGL" .

roboprof_data:ENGL_417 a vivo:Course ;
    dbo:name "Writing for Media" ;
    dbo:number 417 ;
    dcterms:description "Writing workshop (peer critique, revision, ongoing development)" ;
    vivo:courseCredits 4 ;
    vivo:hasSubjectArea "ENGL" .

roboprof_data:ENGL_428 a vivo:Course ;
    dbo:name "Advanced Studies in Creative Writing" ;
    dbo:number 428 ;
    dcterms:description "Writing workshop (peer critique, revision, ongoing development)" ;
    vivo:courseCredits 3 ;
    vivo:hasSubjectArea "ENGL" .

roboprof_data:ENGL_429 a vivo:Course ;
    dbo:name "Advanced Studies in Creative Writing" ;
    dbo:number 429 ;
    dcterms:description "Writing workshop (peer critique, revision, ongoing development)" ;
    vivo:courseCredits 4 ;
    vivo:hasSubjectArea "ENGL" .

roboprof_data:ENGL_470 a vivo:Course ;
    dbo:name "Honours Seminar" ;
    dbo:number 470 ;
    dcterms:description "With the permission of the Department, a student may arrange a tutorial program with a faculty member." ;
    vivo:courseCredits 3 ;
    vivo:hasSubjectArea "ENGL" .

roboprof_data:ENGL_474 a vivo:Course ;
    dbo:name "Honours Essay" ;
    dbo:number 474 ;
    dcterms:description "With the permission of the Department, an honours student may arrange a tutorial program with a faculty member, culminating in the writing of a long paper." ;
    vivo:courseCredits 4 ;
    vivo:hasSubjectArea "ENGL" .

roboprof_data:ENGL_480 a vivo:Course ;
    dbo:name "Independent Studies" ;
    dbo:number 480 ;
    dcterms:description "With the permission of the Department, a student may arrange a tutorial program with a faculty member." ;
    vivo:courseCredits 3 ;
    vivo:hasSubjectArea "ENGL" .

roboprof_data:ENGL_601 a vivo:Course ;
    dbo:name "Literary Pedagogies" ;
    dbo:number 601 ;
    dcterms:description "Special Topics in English Literature" ;
    vivo:courseCredits 3 ;
    vivo:hasSubjectArea "ENGL" .

roboprof_data:ENGL_636 a vivo:Course ;
    dbo:name "Writing about/on/with/at/the contemporary circus: A seminar on Research-Creation, Creative process and Meaning-Making (intensive Faculty of Arts and Science international graduate seminar)" ;
    dbo:number 636 ;
    dcterms:description "Writing and live performance workshop" ;
    vivo:courseCredits 3 ;
    vivo:hasSubjectArea "ENGL" .

roboprof_data:ENGL_637 a vivo:Course ;
    dbo:name "Experiential learning in Contemporary Circus Practice and Physical Theatre: Methods in research-creation, action-research and participant observation (intensive Faculty of Arts and Science international graduate seminar)" ;
    dbo:number 637 ;
    dcterms:description "Writing and life performance workshop" ;
    vivo:courseCredits 4 ;
    vivo:hasSubjectArea "ENGL " .

roboprof_data:ENGL_670 a vivo:Course ;
    dbo:name "Seminar in Creative Writing: Prose Fiction, Poetry and Drama " ;
    dbo:number 670 ;
    dcterms:description "Writing workshop (peer critique, revision, ongoing development)" ;
    vivo:courseCredits 4 ;
    vivo:hasSubjectArea "ENGL" .

roboprof_data:ENGL_671 a vivo:Course ;
    dbo:name "Seminar in Creative Writing: Prose Fiction, Poetry and Drama " ;
    dbo:number 671 ;
    dcterms:description "Writing workshop (peer critique, revision, ongoing development)" ;
    vivo:courseCredits 4 ;
    vivo:hasSubjectArea "ENGL" .

roboprof_data:ENGL_672 a vivo:Course ;
    dbo:name "Seminar in Creative Writing: Prose Fiction, Poetry and Drama " ;
    dbo:number 672 ;
    dcterms:description "Writing workshop (peer critique, revision, ongoing development)" ;
    vivo:courseCredits 3 ;
    vivo:hasSubjectArea "ENGL" .

roboprof_data:ENGL_673 a vivo:Course ;
    dbo:name "Seminar in Creative Writing: Prose Fiction, Poetry and Drama " ;
    dbo:number 673 ;
    dcterms:description "Writing workshop (peer critique, revision, ongoing development)" ;
    vivo:courseCredits 4 ;
    vivo:hasSubjectArea "ENGL" .

roboprof_data:ENGL_674 a vivo:Course ;
    dbo:name "Seminar in Creative Writing: Prose Fiction, Poetry and Drama " ;
    dbo:number 674 ;
    dcterms:description "Writing workshop (peer critique, revision, ongoing development)" ;
    vivo:courseCredits 4 ;
    vivo:hasSubjectArea "ENGL" .

roboprof_data:ENGL_802 a vivo:Course ;
    dbo:name "Professional Development Workshops" ;
    dbo:number 802 ;
    dcterms:description "Workshops" ;
    vivo:courseCredits 3 ;
    vivo:hasSubjectArea "ENGL" .

roboprof_data:ENGR_107 a vivo:Course ;
    dbo:name "Engineering Industrial Experience Work Term I" ;
    dbo:number 107 ;
    dcterms:description "Industrial experience work term" ;
    vivo:courseCredits 3,
        4 ;
    vivo:hasSubjectArea "ENGR" .

roboprof_data:ENGR_108 a vivo:Course ;
    dbo:name "Engineering Industrial Experience Reflective Learning I" ;
    dbo:number 108 ;
    dcterms:description "Associated reflective learning course to industrial experience work term I" ;
    vivo:courseCredits 4 ;
    vivo:hasSubjectArea "ENGR" .

roboprof_data:ENGR_201 a vivo:Course ;
    dbo:name "Professional Practice and Responsibility" ;
    dbo:number 201 ;
    dcterms:description "Case Studies" ;
    vivo:courseCredits 3 ;
    vivo:hasSubjectArea "ENGR" .

roboprof_data:ENGR_202 a vivo:Course ;
    dbo:name "Sustainable Development and Environmental Stewardship" ;
    dbo:number 202 ;
    dcterms:description "Case studies" ;
    vivo:courseCredits 3 ;
    vivo:hasSubjectArea "ENGR" .

roboprof_data:ENGR_207 a vivo:Course ;
    dbo:name "Engineering Industrial Experience Work Term II" ;
    dbo:number 207 ;
    dcterms:description "Industrial experience work term" ;
    vivo:courseCredits 3,
        4 ;
    vivo:hasSubjectArea "ENGR" .

roboprof_data:ENGR_208 a vivo:Course ;
    dbo:name "Engineering Industrial Experience Reflective Learning II" ;
    dbo:number 208 ;
    dcterms:description "Associated reflective learning course to industrial experience work term II" ;
    vivo:courseCredits 3,
        4 ;
    vivo:hasSubjectArea "ENGR" .

roboprof_data:ENGR_290 a vivo:Course ;
    dbo:name "Introductory Engineering Team Design Project" ;
    dbo:number 290 ;
    dcterms:description "Team project" ;
    vivo:courseCredits 3 ;
    vivo:hasSubjectArea "ENGR" .

roboprof_data:ENGR_307 a vivo:Course ;
    dbo:name "Engineering Industrial Experience Work Term III" ;
    dbo:number 307 ;
    dcterms:description "Industrial experience work term" ;
    vivo:courseCredits 3 ;
    vivo:hasSubjectArea "ENGR" .

roboprof_data:ENGR_308 a vivo:Course ;
    dbo:name "Engineering Industrial Experience Reflective Learning III" ;
    dbo:number 308 ;
    dcterms:description "Associated reflective learning course to industrial experience work term III" ;
    vivo:courseCredits 4 ;
    vivo:hasSubjectArea "ENGR" .

roboprof_data:ENGR_392 a vivo:Course ;
    dbo:name "Impact of Technology on Society" ;
    dbo:number 392 ;
    dcterms:description "Course-integrated project; Games/Role Playing; Case Studies; Simulations" ;
    vivo:courseCredits 3 ;
    vivo:hasSubjectArea "ENGR" .

roboprof_data:ENGR_412 a vivo:Course ;
    dbo:name "Honours Research Project" ;
    dbo:number 412 ;
    dcterms:description "Research project in area of concentration, selected in consultation with & conducted under the supervision of a faculty member",
        "Research project in their area of concentration" ;
    vivo:courseCredits 4 ;
    vivo:hasSubjectArea "ENGR" .

roboprof_data:ENGR_472 a vivo:Course ;
    dbo:name "Robot Manipulators" ;
    dbo:number 472 ;
    dcterms:description "Laboratory: 15 hours total" ;
    vivo:courseCredits 4 ;
    vivo:hasSubjectArea "ENGR" .

roboprof_data:ENGR_8901 a vivo:Course ;
    dbo:name "Master of Applied Science Research and Thesis" ;
    dbo:number 8901 ;
    dcterms:description "Research, thesis" ;
    vivo:courseCredits 3 ;
    vivo:hasSubjectArea "ENGR" .

roboprof_data:ENGR_8911 a vivo:Course ;
    dbo:name "Doctoral Research and Thesis" ;
    dbo:number 8911 ;
    dcterms:description "Research, thesis" ;
    vivo:courseCredits 3 ;
    vivo:hasSubjectArea "ENGR" .

roboprof_data:ENVS_608 a vivo:Course ;
    dbo:name "Getting Ready for the EA Internship" ;
    dbo:number 608 ;
    dcterms:description "Workshop" ;
    vivo:courseCredits 4 ;
    vivo:hasSubjectArea "ENVS" .

roboprof_data:ENVS_664 a vivo:Course ;
    dbo:name "Field Course in EA" ;
    dbo:number 664 ;
    dcterms:description "1-week field trip" ;
    vivo:courseCredits 3 ;
    vivo:hasSubjectArea "ENVS" .

roboprof_data:ESL_205 a vivo:Course ;
    dbo:name "Academic Oral Communication I" ;
    dbo:number 205 ;
    dcterms:description "Multimedia language lab",
        "This course helps students develop the oral skills necessary for speaking and listening in an English-speaking academic environment." ;
    vivo:courseCredits 4 ;
    vivo:hasSubjectArea "ESL" .

roboprof_data:ESL_206 a vivo:Course ;
    dbo:name "Academic Oral Communication II" ;
    dbo:number 206 ;
    dcterms:description "Multimedia language lab",
        "This course helps students achieve greater intelligibility and fluency by practising oral communication skills in meaningful discourse, as part of communicative activities and public-speaking assignments." ;
    vivo:courseCredits 3 ;
    vivo:hasSubjectArea "ESL" .

roboprof_data:ESTU_670 a vivo:Course ;
    dbo:name "Adult Education as a Field of Study" ;
    dbo:number 670 ;
    dcterms:description "A Canadian and Quebec perspective" ;
    vivo:courseCredits 3 ;
    vivo:hasSubjectArea "ESTU" .

roboprof_data:ETEC_613 a vivo:Course ;
    dbo:name "Learning Theories" ;
    dbo:number 613 ;
    dcterms:description "Conduct design sprints to determine a theoretically sound response to a real-world problem of performance and instruction" ;
    vivo:courseCredits 4 ;
    vivo:hasSubjectArea "ETEC" .

roboprof_data:ETEC_637 a vivo:Course ;
    dbo:name "Educational Gaming and Modeling" ;
    dbo:number 637 ;
    dcterms:description "Given a real-world prompt, design and develop an educational game" ;
    vivo:courseCredits 3 ;
    vivo:hasSubjectArea "ETEC" .

roboprof_data:ETEC_650 a vivo:Course ;
    dbo:name "Fundamentals of Instructional Design" ;
    dbo:number 650 ;
    dcterms:description "Real-world project" ;
    vivo:courseCredits 3 ;
    vivo:hasSubjectArea "ETEC" .

roboprof_data:ETEC_651 a vivo:Course ;
    dbo:name "Fundamentals of Human Performance Technology" ;
    dbo:number 651 ;
    dcterms:description "Real-world project" ;
    vivo:courseCredits 4 ;
    vivo:hasSubjectArea "ETEC" .

roboprof_data:ETEC_665 a vivo:Course ;
    dbo:name "Introduction to Digital Media" ;
    dbo:number 665 ;
    dcterms:description "Convert real-world documents into learning programs" ;
    vivo:courseCredits 4 ;
    vivo:hasSubjectArea "ETEC" .

roboprof_data:ETEC_669 a vivo:Course ;
    dbo:name "Designing and Developing Interactive Instruction" ;
    dbo:number 669 ;
    dcterms:description "Given a real-world prompt, design and develop a learning program " ;
    vivo:courseCredits 3 ;
    vivo:hasSubjectArea "ETEC" .

roboprof_data:ETEC_671 a vivo:Course ;
    dbo:name "Administering Educational Technology Groups" ;
    dbo:number 671 ;
    dcterms:description "Real-world practice of educational technology, experiential learning activities" ;
    vivo:courseCredits 3 ;
    vivo:hasSubjectArea "ETEC" .

roboprof_data:ETEC_681 a vivo:Course ;
    dbo:name "Foundations of Distance Education" ;
    dbo:number 681 ;
    dcterms:description "Real-world projects in educational technology found using the software Riipen." ;
    vivo:courseCredits 3 ;
    vivo:hasSubjectArea "ETEC" .

roboprof_data:EXCI_252 a vivo:Course ;
    dbo:name "Introduction to Physical Activity, Health and Fitness" ;
    dbo:number 252 ;
    dcterms:description "Laboratory" ;
    vivo:courseCredits 4 ;
    vivo:hasSubjectArea "EXCI" .

roboprof_data:EXCI_253 a vivo:Course ;
    dbo:name "Human Anatomy I: Musculoskeletal Anatomy" ;
    dbo:number 253 ;
    dcterms:description "Laboratory" ;
    vivo:courseCredits 3 ;
    vivo:hasSubjectArea "EXCI" .

roboprof_data:EXCI_254 a vivo:Course ;
    dbo:name "Human Anatomy II: Systemic Anatomy" ;
    dbo:number 254 ;
    dcterms:description "Laboratory" ;
    vivo:courseCredits 3 ;
    vivo:hasSubjectArea "EXCI" .

roboprof_data:EXCI_258 a vivo:Course ;
    dbo:name "Human Physiology I: Musculoskeletal, Neuromuscular and Bioenergetic Systems: From Rest to Exercise" ;
    dbo:number 258 ;
    dcterms:description "Laboratory" ;
    vivo:courseCredits 3 ;
    vivo:hasSubjectArea "EXCI" .

roboprof_data:EXCI_259 a vivo:Course ;
    dbo:name "Human Physiology II: Cardiovascular and Respiratory Systems: From Rest to Exercise" ;
    dbo:number 259 ;
    dcterms:description "Laboratory" ;
    vivo:courseCredits 4 ;
    vivo:hasSubjectArea "EXCI" .

roboprof_data:EXCI_323 a vivo:Course ;
    dbo:name "Research Experience in Exercise Science" ;
    dbo:number 323 ;
    dcterms:description "Hands-on research experience, Laboratory" ;
    vivo:courseCredits 4 ;
    vivo:hasSubjectArea "EXCI" .

roboprof_data:EXCI_351 a vivo:Course ;
    dbo:name "Introduction to the Biomechanics of Human Movement" ;
    dbo:number 351 ;
    dcterms:description "Laboratory" ;
    vivo:courseCredits 4 ;
    vivo:hasSubjectArea "EXCI" .

roboprof_data:EXCI_352 a vivo:Course ;
    dbo:name "Essentials of Exercise Testing and Training in Athletic Populations" ;
    dbo:number 352 ;
    dcterms:description "Laboratory" ;
    vivo:courseCredits 4 ;
    vivo:hasSubjectArea "EXCI" .

roboprof_data:EXCI_357 a vivo:Course ;
    dbo:name "Human Physiology II: The Cardiovascular and Respiratory Systems" ;
    dbo:number 357 ;
    dcterms:description "Laboratory" ;
    vivo:courseCredits 3 ;
    vivo:hasSubjectArea "EXCI" .

roboprof_data:EXCI_358 a vivo:Course ;
    dbo:name "Physiology of Exercise" ;
    dbo:number 358 ;
    dcterms:description "Laboratory" ;
    vivo:courseCredits 4 ;
    vivo:hasSubjectArea "EXCI" .

roboprof_data:EXCI_455 a vivo:Course ;
    dbo:name "Physical Activity, Health and Aging" ;
    dbo:number 455 ;
    dcterms:description "Laboratory" ;
    vivo:courseCredits 4 ;
    vivo:hasSubjectArea "EXCI" .

roboprof_data:FBRS_201 a vivo:Course ;
    dbo:name "INTRO TO FBRS&MATERIAL PRACT",
        "Introduction to Fibres and Material Practices" ;
    dbo:number 201 ;
    dcterms:description "NaN"^^xsd:double,
        "This course introduces students to elementary fibres processes and related tools." ;
    vivo:courseCredits 3 ;
    vivo:hasSubjectArea "FBRS" .

roboprof_data:FBRS_240 a vivo:Course ;
    dbo:name "Fibre Structures I" ;
    dbo:number 240 ;
    dcterms:description "An introductory course in which students explore the expressive potential of various materials and processes of fibre structures such as loom weaving, feltmaking, basketry, surface applications, and other experimental constructions." ;
    vivo:courseCredits 3 ;
    vivo:hasSubjectArea "FBRS" .

roboprof_data:FBRS_260 a vivo:Course ;
    dbo:name "Textile Printing and Dyeing I" ;
    dbo:number 260 ;
    dcterms:description "An introductory course in which students explore the creative potential of printing, painting, dyeing, resist work, and construction with fabric." ;
    vivo:courseCredits 4 ;
    vivo:hasSubjectArea "FBRS" .

roboprof_data:FBRS_341 a vivo:Course ;
    dbo:name "Intermediate Fibre Structures" ;
    dbo:number 341 ;
    dcterms:description "An intermediatelevel studio course, which emphasizes the visual and conceptual development in fibre media." ;
    vivo:courseCredits 4 ;
    vivo:hasSubjectArea "FBRS" .

roboprof_data:FBRS_361 a vivo:Course ;
    dbo:name "Intermediate Textile Printing and Dyeing" ;
    dbo:number 361 ;
    dcterms:description "An intermediatelevel studio course in textile printing and dyeing with an emphasis on the development of content." ;
    vivo:courseCredits 4 ;
    vivo:hasSubjectArea "FBRS" .

roboprof_data:FBRS_371 a vivo:Course ;
    dbo:name "Paper: Surface and Object " ;
    dbo:number 371 ;
    dcterms:description "This studio course introduces both Western and Eastern (Japanese) methods of processing raw materials to make pulp and form sheets of paper to be used in expressive art forms." ;
    vivo:courseCredits 4 ;
    vivo:hasSubjectArea "FBRS" .

roboprof_data:FBRS_372 a vivo:Course ;
    dbo:name "Paper Works" ;
    dbo:number 372 ;
    dcterms:description "This studio course introduces students to making paper as part of an expressive material practice." ;
    vivo:courseCredits 3 ;
    vivo:hasSubjectArea "FBRS" .

roboprof_data:FBRS_385 a vivo:Course ;
    dbo:name "Issues in Material Practices" ;
    dbo:number 385 ;
    dcterms:description "This studio course explores contemporary social, material and cultural issues addressed through fibre and interdisciplinary studio art practices." ;
    vivo:courseCredits 4 ;
    vivo:hasSubjectArea "FBRS" .

roboprof_data:FBRS_386 a vivo:Course ;
    dbo:name "Digital Technologies and Material Practices " ;
    dbo:number 386 ;
    dcterms:description "This studio course combines digital and material approaches within the context of contemporary studio practice. " ;
    vivo:courseCredits 4 ;
    vivo:hasSubjectArea "FBRS" .

roboprof_data:FBRS_395 a vivo:Course ;
    dbo:name "Extreme Fibres" ;
    dbo:number 395 ;
    dcterms:description "This studio course tests the boundaries of fibres practices to produce innovative and experimental studio work." ;
    vivo:courseCredits 4 ;
    vivo:hasSubjectArea "FBRS" .

roboprof_data:FBRS_396 a vivo:Course ;
    dbo:name "Topics in Fibre Surfaces" ;
    dbo:number 396 ;
    dcterms:description "A studio course providing an opportunity for specialized study and practice in fibres surfaces, to explore theoretical, critical, and practical issues of interest to the student towards developing their individual aesthetic in contemporary art." ;
    vivo:courseCredits 3 ;
    vivo:hasSubjectArea "FBRS" .

roboprof_data:FBRS_397 a vivo:Course ;
    dbo:name "Topics in Fibre Structures" ;
    dbo:number 397 ;
    dcterms:description "A studio course providing an opportunity for specialized study and practice in fibres structures, in which to explore contemporary theoretical, critical, and practical issues of interest to the student towards developing a personal aesthetic in art practice." ;
    vivo:courseCredits 4 ;
    vivo:hasSubjectArea "FBRS" .

roboprof_data:FBRS_398 a vivo:Course ;
    dbo:name "Special Topics in Fibres and Material Practices" ;
    dbo:number 398 ;
    dcterms:description "A workshop/seminar course providing an opportunity for study of specialized aspects of fibres." ;
    vivo:courseCredits 4 ;
    vivo:hasSubjectArea "FBRS" .

roboprof_data:FBRS_399 a vivo:Course ;
    dbo:name "Special Topics in Fibres and Material Practices" ;
    dbo:number 399 ;
    dcterms:description "A workshop/seminar course providing an opportunity for the study of specialized aspects in fibres." ;
    vivo:courseCredits 4 ;
    vivo:hasSubjectArea "FBRS" .

roboprof_data:FBRS_450 a vivo:Course ;
    dbo:name "Independent Study " ;
    dbo:number 450 ;
    dcterms:description "This course provides a limited number of students the opportunity to pursue advanced studies in fibres under the supervision of a fulltime fibres faculty member. " ;
    vivo:courseCredits 4 ;
    vivo:hasSubjectArea "FBRS" .

roboprof_data:FBRS_451 a vivo:Course ;
    dbo:name "INDEPENDENT STUDY I",
        "Independent Study I" ;
    dbo:number 451 ;
    dcterms:description "NaN"^^xsd:double,
        "This course provides a limited number of students the opportunity to pursue advanced studies in fibres under the supervision of a fulltime fibres faculty member." ;
    vivo:courseCredits 3,
        4 ;
    vivo:hasSubjectArea "FBRS" .

roboprof_data:FBRS_452 a vivo:Course ;
    dbo:name "Independent Study II " ;
    dbo:number 452 ;
    dcterms:description "This course provides a limited number of students the opportunity to pursue advanced studies in fibres under the supervision of a fulltime fibres faculty member." ;
    vivo:courseCredits 4 ;
    vivo:hasSubjectArea "FBRS" .

roboprof_data:FBRS_480 a vivo:Course ;
    dbo:name "Advanced Fibres" ;
    dbo:number 480 ;
    dcterms:description "An advancedlevel course in which students create a personal body or work, refine technical expertise, and develop a visual and critical language related to fibres and textiles." ;
    vivo:courseCredits 3 ;
    vivo:hasSubjectArea "FBRS" .

roboprof_data:FBRS_481 a vivo:Course ;
    dbo:name "Professional Internship I" ;
    dbo:number 481 ;
    dcterms:description "Internships are designed to provide professional experience to students. Students seeking to work in an apprentice capacity with an established artist, or wishing to pursue research in a fibres studio, or research in fibres criticism, museum work, publication, or other related endeavours, may apply for academic credit." ;
    vivo:courseCredits 3 ;
    vivo:hasSubjectArea "FBRS" .

roboprof_data:FBRS_482 a vivo:Course ;
    dbo:name "Professional Internship II" ;
    dbo:number 482 ;
    dcterms:description "Internships are designed to provide professional experience to students. Students seeking to work in an apprentice capacity with an established artist, or wishing to pursue research in a fibres studio, or research in fibres criticism, museum work, publication, or other related endeavours, may apply for academic credit." ;
    vivo:courseCredits 3 ;
    vivo:hasSubjectArea "FBRS" .

roboprof_data:FINA_385 a vivo:Course ;
    dbo:name "Theory of Finance I" ;
    dbo:number 385 ;
    dcterms:description "Portfolio project and hedging with futures contracts in select sections" ;
    vivo:courseCredits 4 ;
    vivo:hasSubjectArea "FINA" .

roboprof_data:FINA_395 a vivo:Course ;
    dbo:name "Theory of Finance II" ;
    dbo:number 395 ;
    dcterms:description "Team project with active application of theory" ;
    vivo:courseCredits 4 ;
    vivo:hasSubjectArea "FINA" .

roboprof_data:FINA_402 a vivo:Course ;
    dbo:name "Short Term Financial Management" ;
    dbo:number 402 ;
    dcterms:description "Case analysis" ;
    vivo:courseCredits 3 ;
    vivo:hasSubjectArea "FINA" .

roboprof_data:FINA_405 a vivo:Course ;
    dbo:name "Cases in Finance" ;
    dbo:number 405 ;
    dcterms:description "This course uses case discussions to focus on the application of the principles of finance learned in FINA 385 and 395 in real-world contexts." ;
    vivo:courseCredits 4 ;
    vivo:hasSubjectArea "FINA" .

roboprof_data:FINA_408 a vivo:Course ;
    dbo:name "Building and Testing Trading Systems Using Technical Analysis" ;
    dbo:number 408 ;
    dcterms:description "Group project to build and test a trading system using simulation and investment software" ;
    vivo:courseCredits 4 ;
    vivo:hasSubjectArea "FINA" .

roboprof_data:FINA_409 a vivo:Course ;
    dbo:name "Applied Investment Analysis" ;
    dbo:number 409 ;
    dcterms:description "Term paper and stock presentation" ;
    vivo:courseCredits 3 ;
    vivo:hasSubjectArea "FINA" .

roboprof_data:FINA_410 a vivo:Course ;
    dbo:name "Investment Analysis" ;
    dbo:number 410 ;
    dcterms:description "Group assignment and presentation; case study in select sections" ;
    vivo:courseCredits 3 ;
    vivo:hasSubjectArea "FINA" .

roboprof_data:FINA_411 a vivo:Course ;
    dbo:name "Portfolio Management" ;
    dbo:number 411 ;
    dcterms:description "Trading simulator (portfolio management simulator) and case study group report with presentation" ;
    vivo:courseCredits 4 ;
    vivo:hasSubjectArea "FINA" .

roboprof_data:FINA_413 a vivo:Course ;
    dbo:name "Advanced Topics in Derivative Markets" ;
    dbo:number 413 ;
    dcterms:description "Group presentation and report" ;
    vivo:courseCredits 4 ;
    vivo:hasSubjectArea "FINA" .

roboprof_data:FINA_415 a vivo:Course ;
    dbo:name "Mergers and Acquisitions" ;
    dbo:number 415 ;
    dcterms:description "Trading lab simulations and group project presentation" ;
    vivo:courseCredits 3 ;
    vivo:hasSubjectArea "FINA" .

roboprof_data:FINA_416 a vivo:Course ;
    dbo:name "Behavioral Finance" ;
    dbo:number 416 ;
    dcterms:description "Case studies, experiments and activities" ;
    vivo:courseCredits 4 ;
    vivo:hasSubjectArea "FINA" .

roboprof_data:FINA_465 a vivo:Course ;
    dbo:name "Trading in Financial Securities" ;
    dbo:number 465 ;
    dcterms:description "Practical skills in trading financial securities" ;
    vivo:courseCredits 3 ;
    vivo:hasSubjectArea "FINA" .

roboprof_data:FINA_470 a vivo:Course ;
    dbo:name "International Finance" ;
    dbo:number 470 ;
    dcterms:description "Case study" ;
    vivo:courseCredits 3 ;
    vivo:hasSubjectArea "FINA" .

roboprof_data:FINA_471 a vivo:Course ;
    dbo:name "International Financial Management" ;
    dbo:number 471 ;
    dcterms:description "Case study presentation" ;
    vivo:courseCredits 3 ;
    vivo:hasSubjectArea "FINA" .

roboprof_data:FINA_481 a vivo:Course ;
    dbo:name "Management of Financial Institutions" ;
    dbo:number 481 ;
    dcterms:description "Group presentation and case study" ;
    vivo:courseCredits 4 ;
    vivo:hasSubjectArea "FINA" .

roboprof_data:FINA_482 a vivo:Course ;
    dbo:name "International Banking: Operations, Policy and Strategy" ;
    dbo:number 482 ;
    dcterms:description "Group case presentation" ;
    vivo:courseCredits 4 ;
    vivo:hasSubjectArea "FINA" .

roboprof_data:FINA_663 a vivo:Course ;
    dbo:name "Seminar in Corporate Finance" ;
    dbo:number 663 ;
    dcterms:description "Team project with active application of theory" ;
    vivo:courseCredits 3 ;
    vivo:hasSubjectArea "FINA" .

roboprof_data:FINA_695 a vivo:Course ;
    dbo:name "Applied Investments: Business Analysis and Valuation" ;
    dbo:number 695 ;
    dcterms:description "Stock presentation, investment report and valuation model" ;
    vivo:courseCredits 3 ;
    vivo:hasSubjectArea "FINA" .

roboprof_data:FLIT_454 a vivo:Course ;
    dbo:name "Histoire du livre et de ldition" ;
    dbo:number 454 ;
    dcterms:description "mtiers (du livre), rapports (entre diteur et auteur)" ;
    vivo:courseCredits 3 ;
    vivo:hasSubjectArea "FLIT" .

roboprof_data:FLIT_486 a vivo:Course ;
    dbo:name "Cration littraire I" ;
    dbo:number 486 ;
    dcterms:description "ateliers et travaux (dcriture)" ;
    vivo:courseCredits 3 ;
    vivo:hasSubjectArea "FLIT" .

roboprof_data:FLIT_488 a vivo:Course ;
    dbo:name "Cration littraire II" ;
    dbo:number 488 ;
    dcterms:description "ateliers dcriture ainsi que par llaboration dun projet individuel" ;
    vivo:courseCredits 3 ;
    vivo:hasSubjectArea "FLIT" .

roboprof_data:FLIT_496 a vivo:Course ;
    dbo:name "Recherche dirige" ;
    dbo:number 496 ;
    dcterms:description "travaux individuels" ;
    vivo:courseCredits 3 ;
    vivo:hasSubjectArea "FLIT" .

roboprof_data:FLIT_690 a vivo:Course ;
    dbo:name "Prsentation du mmoire" ;
    dbo:number 690 ;
    dcterms:description "mmoire" ;
    vivo:courseCredits 4 ;
    vivo:hasSubjectArea "FLIT" .

roboprof_data:FLIT_691 a vivo:Course ;
    dbo:name "Prsentation du mmoire incluant une ralisation mdiatique" ;
    dbo:number 691 ;
    dcterms:description "mmoire, ralisation mdiatique" ;
    vivo:courseCredits 3 ;
    vivo:hasSubjectArea "FLIT" .

roboprof_data:FLIT_692 a vivo:Course ;
    dbo:name "Mmoire" ;
    dbo:number 692 ;
    dcterms:description "mmoire" ;
    vivo:courseCredits 4 ;
    vivo:hasSubjectArea "FLIT" .

roboprof_data:FLIT_693 a vivo:Course ;
    dbo:name "Mmoire incluant une ralisation mdiatique" ;
    dbo:number 693 ;
    dcterms:description "mmoire, ralisation mdiatique" ;
    vivo:courseCredits 4 ;
    vivo:hasSubjectArea "FLIT" .

roboprof_data:FMAN_203 a vivo:Course ;
    dbo:name "INTRO. TO ANIMATION I" ;
    dbo:number 203 ;
    dcterms:description "NaN"^^xsd:double ;
    vivo:courseCredits 4 ;
    vivo:hasSubjectArea "FMAN" .

roboprof_data:FMPR_451 a vivo:Course ;
    dbo:name "ADV. PROJECT INTERNSHIP I" ;
    dbo:number 451 ;
    dcterms:description "NaN"^^xsd:double ;
    vivo:courseCredits 3 ;
    vivo:hasSubjectArea "FMPR" .

roboprof_data:FMST_201 a vivo:Course ;
    dbo:name "FILM HISTORY I" ;
    dbo:number 201 ;
    dcterms:description "NaN"^^xsd:double ;
    vivo:courseCredits 3 ;
    vivo:hasSubjectArea "FMST" .

roboprof_data:FMST_202 a vivo:Course ;
    dbo:name "FILM HISTORY II" ;
    dbo:number 202 ;
    dcterms:description "NaN"^^xsd:double ;
    vivo:courseCredits 3 ;
    vivo:hasSubjectArea "FMST" .

roboprof_data:FMST_203 a vivo:Course ;
    dbo:name "FILM HISTORY III" ;
    dbo:number 203 ;
    dcterms:description "NaN"^^xsd:double ;
    vivo:courseCredits 3 ;
    vivo:hasSubjectArea "FMST" .

roboprof_data:FMST_204 a vivo:Course ;
    dbo:name "APPROACHES TO FILM STUDIES I" ;
    dbo:number 204 ;
    dcterms:description "NaN"^^xsd:double ;
    vivo:courseCredits 3 ;
    vivo:hasSubjectArea "FMST" .

roboprof_data:FPST_297 a vivo:Course ;
    dbo:name "Proseminar 1: Indigenous Ways of Knowing" ;
    dbo:number 297 ;
    dcterms:description "The course is based in learning Indigenous methods and professional skills that takes students out of the classroom and into Indigenous communities." ;
    vivo:courseCredits 3 ;
    vivo:hasSubjectArea "FPST" .

roboprof_data:FPST_397 a vivo:Course ;
    dbo:name "Proseminar 2: Ethics and First Peoples" ;
    dbo:number 397 ;
    dcterms:description "The course is based in learning Indigenous methods and professional skills that takes students out of the classroom and into Indigenous communities." ;
    vivo:courseCredits 3 ;
    vivo:hasSubjectArea "FPST" .

roboprof_data:FPST_497 a vivo:Course ;
    dbo:name "Proseminar 3: Oral Traditions as Methodology" ;
    dbo:number 497 ;
    dcterms:description "The course is based in learning Indigenous methods and professional skills that takes students out of the classroom and into Indigenous communities." ;
    vivo:courseCredits 4 ;
    vivo:hasSubjectArea "FPST" .

roboprof_data:FRAA_413 a vivo:Course ;
    dbo:name "Rdaction " ;
    dbo:number 413 ;
    dcterms:description "comptences (rdactionnelles)" ;
    vivo:courseCredits 3 ;
    vivo:hasSubjectArea "FRAA" .

roboprof_data:FRAA_419 a vivo:Course ;
    dbo:name "Le franais en Amrique du Nord, histoire et destins" ;
    dbo:number 419 ;
    dcterms:description "La prsence de la langue franaise en sol nordamricain ne se limite pas au Qubec,  lAcadie et  la Louisiane. En effet, il existe plusieurs autres varits de franais parles au Canada (le francoontarien, le francomanitobain, le franais mitchif ou encore le francoalbertain) et aux tatsUnis (le franais du Missouri, le francoamricain ou encore le francodakotain). Lobjectif de ce cours est doffrir aux tudiantes et aux tudiants un portrait  la fois historique, sociolinguistique et culturel de ces nombreuses varits nordamricaines du franais." ;
    vivo:courseCredits 3 ;
    vivo:hasSubjectArea "FRAA" .

roboprof_data:FRAA_423 a vivo:Course ;
    dbo:name "Rdaction avance" ;
    dbo:number 423 ;
    dcterms:description "comptences (rdactionnelles)" ;
    vivo:courseCredits 4 ;
    vivo:hasSubjectArea "FRAA" .

roboprof_data:FRAA_491 a vivo:Course ;
    dbo:name "Tutorat en langue ou linguistique" ;
    dbo:number 491 ;
    dcterms:description "sujet particulier" ;
    vivo:courseCredits 4 ;
    vivo:hasSubjectArea "FRAA" .

roboprof_data:FRAA_492 a vivo:Course ;
    dbo:name "Tutorat en langue ou linguistique" ;
    dbo:number 492 ;
    dcterms:description "sujet particulier" ;
    vivo:courseCredits 4 ;
    vivo:hasSubjectArea "FRAA" .

roboprof_data:FRAA_523 a vivo:Course ;
    dbo:name "Rdaction avance" ;
    dbo:number 523 ;
    dcterms:description "comptences (rdactionnelles)" ;
    vivo:courseCredits 4 ;
    vivo:hasSubjectArea "FRAA" .

roboprof_data:FRAA_623 a vivo:Course ;
    dbo:name "Rdaction avance" ;
    dbo:number 623 ;
    dcterms:description "comptences (rdactionnelles)" ;
    vivo:courseCredits 4 ;
    vivo:hasSubjectArea "FRAA" .

roboprof_data:FRAN_211 a vivo:Course ;
    dbo:name "French Language: Elementary" ;
    dbo:number 211 ;
    dcterms:description "This course includes a comprehensive introduction to the basic structures and vocabulary of French and should enable students to acquire an ability to speak and understand simple conversational French." ;
    vivo:courseCredits 4 ;
    vivo:hasSubjectArea "FRAN" .

roboprof_data:FRAN_212 a vivo:Course ;
    dbo:name "French Language: Transitional Level" ;
    dbo:number 212 ;
    dcterms:description "The aim of this course is to provide students who have studied either one year of French at the university or postsecondary level, or two years of French at the secondary level or equivalent, with an opportunity to improve their levels of comprehension and expression so that they will be able to communicate with greater ease in written and oral French." ;
    vivo:courseCredits 3 ;
    vivo:hasSubjectArea "FRAN" .

roboprof_data:FRAN_318 a vivo:Course ;
    dbo:name "Le franais des affaires ",
        "Le franais des affaires I" ;
    dbo:number 318 ;
    dcterms:description "Ce cours vise  faire acqurir des comptences ncessaires  une communication crite et orale efficace dans des situations complexes du march du travail.",
        "techniques de la correspondance commerciale; communications daffaires" ;
    vivo:courseCredits 3,
        4 ;
    vivo:hasSubjectArea "FRAN" .

roboprof_data:FRAN_319 a vivo:Course ;
    dbo:name "Le franais des affaires II" ;
    dbo:number 319 ;
    dcterms:description "Ce cours vise  faire acqurir des comptences ncessaires  une communication crite et orale efficace dans des situations complexes du march du travail." ;
    vivo:courseCredits 4 ;
    vivo:hasSubjectArea "FRAN" .

roboprof_data:FTRA_411 a vivo:Course ;
    dbo:name "Terminologie et mondialisation" ;
    dbo:number 411 ;
    dcterms:description "aspect pratique, utilisation doutils" ;
    vivo:courseCredits 4 ;
    vivo:hasSubjectArea "FTRA" .

roboprof_data:FTRA_416 a vivo:Course ;
    dbo:name "Informatique et traduction" ;
    dbo:number 416 ;
    dcterms:description "exercices, initiation aux outils informatiss" ;
    vivo:courseCredits 3 ;
    vivo:hasSubjectArea "FTRA" .

roboprof_data:FTRA_418 a vivo:Course ;
    dbo:name "Web, technologies, traduction : thories et critiques" ;
    dbo:number 418 ;
    dcterms:description "travail approfondi de recherche" ;
    vivo:courseCredits 4 ;
    vivo:hasSubjectArea "FTRA" .

roboprof_data:FTRA_438 a vivo:Course ;
    dbo:name "Initiation au sous-titrage" ;
    dbo:number 438 ;
    dcterms:description "volet pratique" ;
    vivo:courseCredits 4 ;
    vivo:hasSubjectArea "FTRA" .

roboprof_data:FTRA_452 a vivo:Course ;
    dbo:name "Traduction automatique (TA) et traduction assiste par ordinateur (TAO)" ;
    dbo:number 452 ;
    dcterms:description "exercises, appliquent des outils" ;
    vivo:courseCredits 4 ;
    vivo:hasSubjectArea "FTRA" .

roboprof_data:FTRA_455 a vivo:Course ;
    dbo:name "Gestion de projets" ;
    dbo:number 455 ;
    dcterms:description "mises en situation" ;
    vivo:courseCredits 4 ;
    vivo:hasSubjectArea "FTRA" .

roboprof_data:FTRA_492 a vivo:Course ;
    dbo:name "Tutorat en traduction" ;
    dbo:number 492 ;
    dcterms:description "sujet particulier" ;
    vivo:courseCredits 3 ;
    vivo:hasSubjectArea "FTRA" .

roboprof_data:FTRA_534 a vivo:Course ;
    dbo:name "Terminologie et mondialisation" ;
    dbo:number 534 ;
    dcterms:description "aspect pratique, utilisation doutils" ;
    vivo:courseCredits 4 ;
    vivo:hasSubjectArea "FTRA" .

roboprof_data:FTRA_538 a vivo:Course ;
    dbo:name """Initiation au sous-titrage_x000D_
Co-list : FTRA 538""" ;
    dbo:number 538 ;
    dcterms:description "volet pratique" ;
    vivo:courseCredits 4 ;
    vivo:hasSubjectArea "FTRA" .

roboprof_data:FTRA_555 a vivo:Course ;
    dbo:name "Gestion de projets" ;
    dbo:number 555 ;
    dcterms:description "mises en situation" ;
    vivo:courseCredits 4 ;
    vivo:hasSubjectArea "FTRA" .

roboprof_data:FTRA_556 a vivo:Course ;
    dbo:name "Programmation en localisation" ;
    dbo:number 556 ;
    dcterms:description "manipulation, programmation" ;
    vivo:courseCredits 4 ;
    vivo:hasSubjectArea "FTRA" .

roboprof_data:FTRA_558 a vivo:Course ;
    dbo:name "Pratique de la localisation" ;
    dbo:number 558 ;
    dcterms:description "pratique, logiciels" ;
    vivo:courseCredits 3 ;
    vivo:hasSubjectArea "FTRA" .

roboprof_data:FTRA_613 a vivo:Course ;
    dbo:name "Advanced translation in social sciences and the humanities Co-list : FTRA 542 ou FTRA 543" ;
    dbo:number 613 ;
    dcterms:description "sminaire pratique" ;
    vivo:courseCredits 3 ;
    vivo:hasSubjectArea "FTRA" .

roboprof_data:FTRA_615 a vivo:Course ;
    dbo:name "Advanced literary translation Co-list : FTRA 544 ou 545" ;
    dbo:number 615 ;
    dcterms:description "sminaire pratique" ;
    vivo:courseCredits 3 ;
    vivo:hasSubjectArea "FTRA" .

roboprof_data:FTRA_631 a vivo:Course ;
    dbo:name "Initiation  la traduction gnrale Co-list : FTRA 531" ;
    dbo:number 631 ;
    dcterms:description "outils de travail" ;
    vivo:courseCredits 4 ;
    vivo:hasSubjectArea "FTRA" .

roboprof_data:FTRA_632 a vivo:Course ;
    dbo:name "Initiation  la traduction gnrale Co-list : FTRA 532" ;
    dbo:number 632 ;
    dcterms:description "outils de travail" ;
    vivo:courseCredits 4 ;
    vivo:hasSubjectArea "FTRA" .

roboprof_data:FTRA_633 a vivo:Course ;
    dbo:name "Aspects thoriques et pratiques de la terminologie Co-list : FTRA 533" ;
    dbo:number 633 ;
    dcterms:description "aspects pratiques, supports informatiss" ;
    vivo:courseCredits 3 ;
    vivo:hasSubjectArea "FTRA" .

roboprof_data:FTRA_636 a vivo:Course ;
    dbo:name "Informatique et traduction Co-list : FTRA 536" ;
    dbo:number 636 ;
    dcterms:description "exercises, initiation aux outils informatiss" ;
    vivo:courseCredits 4 ;
    vivo:hasSubjectArea "FTRA" .

roboprof_data:FTRA_638 a vivo:Course ;
    dbo:name """Initiation au sous-titrage_x000D_
Co-list : FTRA 538""" ;
    dbo:number 638 ;
    dcterms:description "volet pratique" ;
    vivo:courseCredits 4 ;
    vivo:hasSubjectArea "FTRA" .

roboprof_data:FTRA_655 a vivo:Course ;
    dbo:name "Gestion de projets Co-list : FTRA 555" ;
    dbo:number 655 ;
    dcterms:description "mises en situation" ;
    vivo:courseCredits 4 ;
    vivo:hasSubjectArea "FTRA" .

roboprof_data:FTRA_658 a vivo:Course ;
    dbo:name "Pratique de la localisation Co-list : FTRA 558" ;
    dbo:number 658 ;
    dcterms:description "pratique" ;
    vivo:courseCredits 3 ;
    vivo:hasSubjectArea "FTRA" .

roboprof_data:FTRA_668 a vivo:Course ;
    dbo:name "Web, technologies, traduction : thories et critiques" ;
    dbo:number 668 ;
    dcterms:description "travail approfondi de recherche" ;
    vivo:courseCredits 4 ;
    vivo:hasSubjectArea "FTRA" .

roboprof_data:FTRA_681 a vivo:Course ;
    dbo:name "Tutorial in literature" ;
    dbo:number 681 ;
    dcterms:description "tutorial" ;
    vivo:courseCredits 4 ;
    vivo:hasSubjectArea "FTRA" .

roboprof_data:FTRA_682 a vivo:Course ;
    dbo:name "Tutorat en traduction" ;
    dbo:number 682 ;
    dcterms:description "tutorat" ;
    vivo:courseCredits 4 ;
    vivo:hasSubjectArea "FTRA" .

roboprof_data:FTRA_683 a vivo:Course ;
    dbo:name "Tutorial in translation" ;
    dbo:number 683 ;
    dcterms:description "tutorial" ;
    vivo:courseCredits 4 ;
    vivo:hasSubjectArea "FTRA" .

roboprof_data:FTRA_684 a vivo:Course ;
    dbo:name "Tutorat en linguistique" ;
    dbo:number 684 ;
    dcterms:description "tutorat" ;
    vivo:courseCredits 3 ;
    vivo:hasSubjectArea "FTRA" .

roboprof_data:FTRA_685 a vivo:Course ;
    dbo:name "Tutorial in linguistics" ;
    dbo:number 685 ;
    dcterms:description "tutorial" ;
    vivo:courseCredits 4 ;
    vivo:hasSubjectArea "FTRA" .

roboprof_data:GEOG_210 a vivo:Course ;
    dbo:name "Geography of Global Change" ;
    dbo:number 210 ;
    dcterms:description "This course examines a variety of geographical changes related to globalization. It focuses mainly on the global political system and the global economy, and also considers transport and communications systems, culture, and environmental issues." ;
    vivo:courseCredits 3 ;
    vivo:hasSubjectArea "GEOG" .

roboprof_data:GEOG_260 a vivo:Course ;
    dbo:name "Mapping the Environment" ;
    dbo:number 260 ;
    dcterms:description "Practical assignments, Laboratory" ;
    vivo:courseCredits 3 ;
    vivo:hasSubjectArea "GEOG" .

roboprof_data:GEOG_264 a vivo:Course ;
    dbo:name "Programming for Environmental Sciences" ;
    dbo:number 264 ;
    dcterms:description "Laboratory" ;
    vivo:courseCredits 4 ;
    vivo:hasSubjectArea "GEOG" .

roboprof_data:GEOG_301 a vivo:Course ;
    dbo:name "The Sustainable University Campus" ;
    dbo:number 301 ;
    dcterms:description "Campus as the laboratory,  workshops, project work" ;
    vivo:courseCredits 4 ;
    vivo:hasSubjectArea "GEOG" .

roboprof_data:GEOG_323 a vivo:Course ;
    dbo:name "Urban Agriculture" ;
    dbo:number 323 ;
    dcterms:description "Field work - working in community gardens" ;
    vivo:courseCredits 3 ;
    vivo:hasSubjectArea "GEOG" .

roboprof_data:GEOG_361 a vivo:Course ;
    dbo:name "Research Design and Qualitative Methods" ;
    dbo:number 361 ;
    dcterms:description "Involvement in fieldwork outside of class time" ;
    vivo:courseCredits 4 ;
    vivo:hasSubjectArea "GEOG" .

roboprof_data:GEOG_362 a vivo:Course ;
    dbo:name "Statistical Methods" ;
    dbo:number 362 ;
    dcterms:description "Laboratory" ;
    vivo:courseCredits 3 ;
    vivo:hasSubjectArea "GEOG" .

roboprof_data:GEOG_363 a vivo:Course ;
    dbo:name "Geographic Information Systems" ;
    dbo:number 363 ;
    dcterms:description "Real-world problem, Laboratory" ;
    vivo:courseCredits 3 ;
    vivo:hasSubjectArea "GEOG" .

roboprof_data:GEOG_371 a vivo:Course ;
    dbo:name "Landscape Ecology" ;
    dbo:number 371 ;
    dcterms:description "Laboratory" ;
    vivo:courseCredits 3 ;
    vivo:hasSubjectArea "GEOG" .

roboprof_data:GEOG_374 a vivo:Course ;
    dbo:name "Plant Ecology" ;
    dbo:number 374 ;
    dcterms:description "Laboratory, mandatory one-day field trip" ;
    vivo:courseCredits 4 ;
    vivo:hasSubjectArea "GEOG" .

roboprof_data:GEOG_377 a vivo:Course ;
    dbo:name "Landform Evolution" ;
    dbo:number 377 ;
    dcterms:description "Laboratory" ;
    vivo:courseCredits 3 ;
    vivo:hasSubjectArea "GEOG" .

roboprof_data:GEOG_463 a vivo:Course ;
    dbo:name "Advanced Geographic Information Systems" ;
    dbo:number 463 ;
    dcterms:description "Hands-on use of ArcGIS software, Laboratory" ;
    vivo:courseCredits 3 ;
    vivo:hasSubjectArea "GEOG" .

roboprof_data:GEOG_464 a vivo:Course ;
    dbo:name "Programming for Geospatial Technologies" ;
    dbo:number 464 ;
    dcterms:description "Laboratory" ;
    vivo:courseCredits 3 ;
    vivo:hasSubjectArea "GEOG" .

roboprof_data:GEOG_465 a vivo:Course ;
    dbo:name "Remote Sensing" ;
    dbo:number 465 ;
    dcterms:description "Laboratory" ;
    vivo:courseCredits 4 ;
    vivo:hasSubjectArea "GEOG" .

roboprof_data:GEOG_466 a vivo:Course ;
    dbo:name "Geomedia and the Geoweb" ;
    dbo:number 466 ;
    dcterms:description "Laboratory" ;
    vivo:courseCredits 3 ;
    vivo:hasSubjectArea "GEOG" .

roboprof_data:GEOG_467 a vivo:Course ;
    dbo:name "Environmental Modelling" ;
    dbo:number 467 ;
    dcterms:description "Laboratory" ;
    vivo:courseCredits 3 ;
    vivo:hasSubjectArea "GEOG" .

roboprof_data:GEOG_474 a vivo:Course ;
    dbo:name "Sustainable Forest Management" ;
    dbo:number 474 ;
    dcterms:description "Mandatory field trip" ;
    vivo:courseCredits 3 ;
    vivo:hasSubjectArea "GEOG" .

roboprof_data:GEOG_490 a vivo:Course ;
    dbo:name "Internship in Geography" ;
    dbo:number 490 ;
    dcterms:description "Case study or practicum of 120 hours" ;
    vivo:courseCredits 3 ;
    vivo:hasSubjectArea "GEOG " .

roboprof_data:GEOL_210 a vivo:Course ;
    dbo:name "Introduction to the Earth" ;
    dbo:number 210 ;
    dcterms:description "Laboratory" ;
    vivo:courseCredits 3 ;
    vivo:hasSubjectArea "GEOL" .

roboprof_data:GEOL_216 a vivo:Course ;
    dbo:name "Field Methods" ;
    dbo:number 216 ;
    dcterms:description "2-week field school" ;
    vivo:courseCredits 4 ;
    vivo:hasSubjectArea "GEOL" .

roboprof_data:GEOL_302 a vivo:Course ;
    dbo:name "Palaeobiology" ;
    dbo:number 302 ;
    dcterms:description "Laboratory" ;
    vivo:courseCredits 3 ;
    vivo:hasSubjectArea "GEOL" .

roboprof_data:GEOL_331 a vivo:Course ;
    dbo:name "Evolution of the Earth" ;
    dbo:number 331 ;
    dcterms:description "Laboratory" ;
    vivo:courseCredits 3 ;
    vivo:hasSubjectArea "GEOL" .

roboprof_data:GEOL_415 a vivo:Course ;
    dbo:name "Plate Tectonics and Crustal Evolution" ;
    dbo:number 415 ;
    dcterms:description "Laboratory" ;
    vivo:courseCredits 4 ;
    vivo:hasSubjectArea "GEOL" .

roboprof_data:GERM_200 a vivo:Course ;
    dbo:name "Introductory German: Intensive" ;
    dbo:number 200 ;
    dcterms:description "lab work" ;
    vivo:courseCredits 4 ;
    vivo:hasSubjectArea "GERM" .

roboprof_data:GERM_201 a vivo:Course ;
    dbo:name "Introductory German I" ;
    dbo:number 201 ;
    dcterms:description "lab work" ;
    vivo:courseCredits 4 ;
    vivo:hasSubjectArea "GERM" .

roboprof_data:GERM_202 a vivo:Course ;
    dbo:name "Introductory German II" ;
    dbo:number 202 ;
    dcterms:description "lab work" ;
    vivo:courseCredits 4 ;
    vivo:hasSubjectArea "GERM" .

roboprof_data:GERM_240 a vivo:Course ;
    dbo:name "Intermediate German: Intensive Course " ;
    dbo:number 240 ;
    dcterms:description "lab work" ;
    vivo:courseCredits 3 ;
    vivo:hasSubjectArea "GERM" .

roboprof_data:GIIM_637 a vivo:Course ;
    dbo:name "Strategic Management" ;
    dbo:number 637 ;
    dcterms:description "Case studies" ;
    vivo:courseCredits 4 ;
    vivo:hasSubjectArea "GIIM" .

roboprof_data:GIIM_655 a vivo:Course ;
    dbo:name "Socially Responsible & Sustainable Investment" ;
    dbo:number 655 ;
    dcterms:description "Case studies" ;
    vivo:courseCredits 3 ;
    vivo:hasSubjectArea "GIIM" .

roboprof_data:HENV_655 a vivo:Course ;
    dbo:name "Environmental Modelling" ;
    dbo:number 655 ;
    dcterms:description "Laboratory" ;
    vivo:courseCredits 4 ;
    vivo:hasSubjectArea "HENV" .

roboprof_data:HENV_801 a vivo:Course ;
    dbo:name "Pedagogical Training" ;
    dbo:number 801 ;
    dcterms:description "Teaching training and in-class practice" ;
    vivo:courseCredits 3 ;
    vivo:hasSubjectArea "HENV" .

roboprof_data:HENV_802 a vivo:Course ;
    dbo:name "Experiential Learning" ;
    dbo:number 802 ;
    dcterms:description "Minimum of 200 hours in a research laboratory based outside Concordia University" ;
    vivo:courseCredits 4 ;
    vivo:hasSubjectArea "HENV" .

roboprof_data:HEXS_801 a vivo:Course ;
    dbo:name "Scientific Communication and Pedagogy in Health and Exercise Science" ;
    dbo:number 801 ;
    dcterms:description "Development of course objectives and a course outline, along with preparing and presenting a lecture at the undergraduate level" ;
    vivo:courseCredits 4 ;
    vivo:hasSubjectArea "HEXS" .

roboprof_data:HIST_200 a vivo:Course ;
    dbo:name "Introduction to History" ;
    dbo:number 200 ;
    dcterms:description "The course offers an introduction to historical argumentation, research skills, and the interpretation of primary and secondary sources. The course will build skills in persuasive writing, library research, critical reading of documents, and the analysis of historical problems." ;
    vivo:courseCredits 3 ;
    vivo:hasSubjectArea "HIST" .

roboprof_data:HIST_281 a vivo:Course ;
    dbo:name "Film in History" ;
    dbo:number 281 ;
    dcterms:description "This course examines how selected commercial films interpret historical events or provide insight into the politics, society, and culture of the times in which they were produced." ;
    vivo:courseCredits 3 ;
    vivo:hasSubjectArea "HIST" .

roboprof_data:HIST_306 a vivo:Course ;
    dbo:name "History and the Public" ;
    dbo:number 306 ;
    dcterms:description "This course is an examination of the practice of history outside the academy and an introduction to the critical analysis of presentations of history in public and popular culture." ;
    vivo:courseCredits 3 ;
    vivo:hasSubjectArea "HIST" .

roboprof_data:HIST_307 a vivo:Course ;
    dbo:name "History of Montreal" ;
    dbo:number 307 ;
    dcterms:description "A study of the origins of the city, its role in the Empire of the St. Lawrence, and its rise to metropolitan dominance in Canada." ;
    vivo:courseCredits 4 ;
    vivo:hasSubjectArea "HIST" .

roboprof_data:HIST_329 a vivo:Course ;
    dbo:name "Music in History" ;
    dbo:number 329 ;
    dcterms:description "This course examines music as a medium for understanding the past. Depending on the historical focus, issues such as colonialism, nationalism, social movements, urban culture, youth culture, race, gender, and class through the prism of contemporaneous music genres may be considered." ;
    vivo:courseCredits 4 ;
    vivo:hasSubjectArea "HIST" .

roboprof_data:HIST_338 a vivo:Course ;
    dbo:name "History and the Graphic Novel" ;
    dbo:number 338 ;
    dcterms:description "This course explores the ways comics and graphic novels express and interpret history." ;
    vivo:courseCredits 3 ;
    vivo:hasSubjectArea "HIST" .

roboprof_data:HIST_368 a vivo:Course ;
    dbo:name "African Popular Culture" ;
    dbo:number 368 ;
    dcterms:description "This course explores the varied terrain of African popular culture in the 19th and 20th centuries." ;
    vivo:courseCredits 4 ;
    vivo:hasSubjectArea "HIST" .

roboprof_data:HIST_379 a vivo:Course ;
    dbo:name "History Through Visual Media and Material Culture" ;
    dbo:number 379 ;
    dcterms:description "This course explores the relationship between the public and the past by examining issues in the production, distribution, and reception of history via these new and changing technologies." ;
    vivo:courseCredits 3 ;
    vivo:hasSubjectArea "HIST" .

roboprof_data:HIST_380 a vivo:Course ;
    dbo:name "History and Digital Media" ;
    dbo:number 380 ;
    dcterms:description "Hands-on, pilot online history projects" ;
    vivo:courseCredits 4 ;
    vivo:hasSubjectArea "HIST" .

roboprof_data:HIST_381 a vivo:Course ;
    dbo:name "The Politics of the Past" ;
    dbo:number 381 ;
    dcterms:description "This course examines the uses of history and the role of the historian in the political arena, focusing on cases in which the past has underwritten social movements or mediated public controversies." ;
    vivo:courseCredits 4 ;
    vivo:hasSubjectArea "HIST" .

roboprof_data:HIST_387 a vivo:Course ;
    dbo:name "Selected Topics in Public History" ;
    dbo:number 387 ;
    dcterms:description "Specific topics for this course, and relevant prerequisites, are stated in the Undergraduate Class Schedule." ;
    vivo:courseCredits 4 ;
    vivo:hasSubjectArea "HIST" .

roboprof_data:HIST_388 a vivo:Course ;
    dbo:name "Telling Stories: Oral History, Memoryscapes, and Digital Storytelling" ;
    dbo:number 388 ;
    dcterms:description "Course introduces oral history theory, ethics and practice. As part of the course, students create projects that are based in the community and are designed to apply course material to a real-world situation." ;
    vivo:courseCredits 3 ;
    vivo:hasSubjectArea "HIST" .

roboprof_data:HIST_390 a vivo:Course ;
    dbo:name "Urban History Laboratory" ;
    dbo:number 390 ;
    dcterms:description "Students conduct original archival and/or oral history research on a selected aspect of Montreals history and then go public with their research in creative and engaging ways." ;
    vivo:courseCredits 3 ;
    vivo:hasSubjectArea "HIST" .

roboprof_data:HIST_397 a vivo:Course ;
    dbo:name "History and Sound" ;
    dbo:number 397 ;
    dcterms:description "This course examines sound as a historical subject and a medium for understanding the past. The course may include training in the production of radio documentaries, urban sound walks, and audio podcasts." ;
    vivo:courseCredits 4 ;
    vivo:hasSubjectArea "HIST" .

roboprof_data:HIST_403 a vivo:Course ;
    dbo:name "Methodology and History" ;
    dbo:number 403 ;
    dcterms:description "This course examines the variety of sources, methods, and modes of analysis used in the research and writing of history. It addresses both theoretical and practical aspects of method." ;
    vivo:courseCredits 3 ;
    vivo:hasSubjectArea "HIST" .

roboprof_data:HIST_481 a vivo:Course ;
    dbo:name "Advanced Topics in Public History" ;
    dbo:number 481 ;
    dcterms:description "Advanced seminar in a selected topic in public history. In addition to weekly discussions of relevant readings, the emphasis is on encouraging students to conduct historical investigation on their own, under a professors guidance." ;
    vivo:courseCredits 4 ;
    vivo:hasSubjectArea "HIST" .

roboprof_data:HIST_485 a vivo:Course ;
    dbo:name "Public History Workshop" ;
    dbo:number 485 ;
    dcterms:description "Project that presents a historical subject to the public" ;
    vivo:courseCredits 4 ;
    vivo:hasSubjectArea "HIST" .

roboprof_data:HIST_486 a vivo:Course ;
    dbo:name "Public History Internship" ;
    dbo:number 486 ;
    dcterms:description "This internship in public history is designed to allow students to test and hone their skills in a nonacademic situation." ;
    vivo:courseCredits 3 ;
    vivo:hasSubjectArea "HIST" .

roboprof_data:HIST_493 a vivo:Course ;
    dbo:name "Honours Essay Tutorial" ;
    dbo:number 493 ;
    dcterms:description "Tutorial, written work, 40 pages in length" ;
    vivo:courseCredits 4 ;
    vivo:hasSubjectArea "HIST" .

roboprof_data:HIST_498 a vivo:Course ;
    dbo:name "Critical Museology (also listed as HIST 670)",
        "Edible Environments: In and Beyond Montreal (also listed as HIST 670)" ;
    dbo:number 498 ;
    dcterms:description "International Graduate Summer School (2017)",
        "International Graduate Summer School (2018)" ;
    vivo:courseCredits 3 ;
    vivo:hasSubjectArea "HIST" .

roboprof_data:HIST_685 a vivo:Course ;
    dbo:name "Masters Thesis" ;
    dbo:number 685 ;
    dcterms:description "Master's Thesis" ;
    vivo:courseCredits 3 ;
    vivo:hasSubjectArea "HIST" .

roboprof_data:HIST_889 a vivo:Course ;
    dbo:name "Doctoral Seminar" ;
    dbo:number 889 ;
    dcterms:description "Experience-based seminar for PhD students  in first and second year. Activities focus on professional practice for historians: preparing fellowship and grant applications; presenting conference papers; assessing journal submissions, etc. " ;
    vivo:courseCredits 3 ;
    vivo:hasSubjectArea "HIST" .

roboprof_data:HIST_890 a vivo:Course ;
    dbo:name "Thesis Research" ;
    dbo:number 890 ;
    dcterms:description "Thesis Research" ;
    vivo:courseCredits 3 ;
    vivo:hasSubjectArea "HIST" .

roboprof_data:IADI_301 a vivo:Course ;
    dbo:name "Undergraduate Aerospace Industry Project I" ;
    dbo:number 301 ;
    dcterms:description "Project, industry training and tours" ;
    vivo:courseCredits 3 ;
    vivo:hasSubjectArea "IADI" .

roboprof_data:IADI_401 a vivo:Course ;
    dbo:name "Undergraduate Aerospace Industry Project II" ;
    dbo:number 401 ;
    dcterms:description "Project, industry training and tours" ;
    vivo:courseCredits 4 ;
    vivo:hasSubjectArea "IADI" .

roboprof_data:IMCA_201 a vivo:Course ;
    dbo:name "Introduction to Intermedia Arts" ;
    dbo:number 201 ;
    dcterms:description "This introductory-level course covers fundamental ideas and techniques related to Video Art, Performance Art and Electronic Art." ;
    vivo:courseCredits 3 ;
    vivo:hasSubjectArea "IMCA" .

roboprof_data:IMCA_210 a vivo:Course ;
    dbo:name "Introduction to Video Production" ;
    dbo:number 210 ;
    dcterms:description "This studio/seminar course introduces video technology as a tool for aesthetic investigations. " ;
    vivo:courseCredits 3 ;
    vivo:hasSubjectArea "IMCA" .

roboprof_data:IMCA_220 a vivo:Course ;
    dbo:name "Introduction to Digital Media and Electronic Arts" ;
    dbo:number 220 ;
    dcterms:description "This studio course is an introduction to the interface between the real world and the computer. " ;
    vivo:courseCredits 4 ;
    vivo:hasSubjectArea "IMCA" .

roboprof_data:IMCA_221 a vivo:Course ;
    dbo:name "Programming for Artists" ;
    dbo:number 221 ;
    dcterms:description "This studio course is an introduction to basic programming techniques used to create interactive art projects." ;
    vivo:courseCredits 3 ;
    vivo:hasSubjectArea "IMCA" .

roboprof_data:IMCA_222 a vivo:Course ;
    dbo:name "Electronics for Artists" ;
    dbo:number 222 ;
    dcterms:description "This studio course is an introduction to electronics as applied to artistic projects. It focuses on practical applications of basic electronic principles and techniques and the integration of electronic components and circuits in works of art." ;
    vivo:courseCredits 4 ;
    vivo:hasSubjectArea "IMCA" .

roboprof_data:IMCA_230 a vivo:Course ;
    dbo:name "Performance Art" ;
    dbo:number 230 ;
    dcterms:description "This studio course investigates performance art as a form of social and artistic intervention that crosses between the visual and performing arts." ;
    vivo:courseCredits 4 ;
    vivo:hasSubjectArea "IMCA" .

roboprof_data:IMCA_310 a vivo:Course ;
    dbo:name "Intermediate Video Production" ;
    dbo:number 310 ;
    dcterms:description "This studio/seminar course introduces video technology as a tool for aesthetic investigations." ;
    vivo:courseCredits 4 ;
    vivo:hasSubjectArea "IMCA" .

roboprof_data:IMCA_321 a vivo:Course ;
    dbo:name "Electronic Arts Workshop" ;
    dbo:number 321 ;
    dcterms:description "This studio course focuses on interactive technologies in relation to contemporary art practices (for example, installation, performance, kinetic sculpture, and sound art)." ;
    vivo:courseCredits 3 ;
    vivo:hasSubjectArea "IMCA" .

roboprof_data:IMCA_322 a vivo:Course ;
    dbo:name "Robotics for Artists" ;
    dbo:number 322 ;
    dcterms:description "This studio course focuses on robotic technologies applied to the arts and electronics, mechanics and programming integration." ;
    vivo:courseCredits 4 ;
    vivo:hasSubjectArea "IMCA" .

roboprof_data:IMCA_331 a vivo:Course ;
    dbo:name "Intermedia and Interventionist Performance Practices" ;
    dbo:number 331 ;
    dcterms:description "An intermediatelevel studio class with a seminar component focusing on the development of sitespecific projects based on video, performance and electronic arts." ;
    vivo:courseCredits 3 ;
    vivo:hasSubjectArea "IMCA" .

roboprof_data:IMCA_332 a vivo:Course ;
    dbo:name "Intermedia, Performance Practices and Performative Video" ;
    dbo:number 332 ;
    dcterms:description "This intermediate-level studio class with a seminar component focuses on the development of intermedia projects based on video, expanded moving image practices, sound, performance and electronic arts. " ;
    vivo:courseCredits 4 ;
    vivo:hasSubjectArea "IMCA" .

roboprof_data:IMCA_398 a vivo:Course ;
    dbo:name "Special Topics in Intermedia" ;
    dbo:number 398 ;
    dcterms:description "This studio course provides an opportunity for study and practice of specialized aspects of intermedia." ;
    vivo:courseCredits 4 ;
    vivo:hasSubjectArea "IMCA" .

roboprof_data:IMCA_399 a vivo:Course ;
    dbo:name "Special Topics in Intermedia" ;
    dbo:number 399 ;
    dcterms:description "This studio course provides an opportunity for study and practice of specialized aspects of intermedia." ;
    vivo:courseCredits 3 ;
    vivo:hasSubjectArea "IMCA" .

roboprof_data:IMCA_400 a vivo:Course ;
    dbo:name "Advanced Practices in Video, Performance and Electronic Arts " ;
    dbo:number 400 ;
    dcterms:description "An advanced studio class in which students create a personal body of work, refine technical expertise, and develop a visual and critical language related to video, performance, and electronic arts." ;
    vivo:courseCredits 4 ;
    vivo:hasSubjectArea "IMCA" .

roboprof_data:IMCA_470 a vivo:Course ;
    dbo:name "Independent Study in Intermedia" ;
    dbo:number 470 ;
    dcterms:description "This course provides a limited number of students the opportunity to pursue advanced studies in intermedia under the supervision of a full-time intermedia faculty member." ;
    vivo:courseCredits 4 ;
    vivo:hasSubjectArea "IMCA" .

roboprof_data:IMCA_471 a vivo:Course ;
    dbo:name "Independent Study in Intermedia I" ;
    dbo:number 471 ;
    dcterms:description "This course provides a limited number of students the opportunity to pursue advanced studies in intermedia under the supervision of a full-time intermedia faculty member." ;
    vivo:courseCredits 3 ;
    vivo:hasSubjectArea "IMCA" .

roboprof_data:IMCA_472 a vivo:Course ;
    dbo:name "Independent Study in Intermedia II " ;
    dbo:number 472 ;
    dcterms:description "This course provides a limited number of students the opportunity to pursue advanced studies in intermedia under the supervision of a full-time intermedia faculty member." ;
    vivo:courseCredits 4 ;
    vivo:hasSubjectArea "IMCA" .

roboprof_data:IMCA_480 a vivo:Course ;
    dbo:name "Professional Internship in Intermedia" ;
    dbo:number 480 ;
    dcterms:description "Under the joint supervision of a qualified professional and a full-time faculty member, the student is employed within industry or by a professional organization or other relevant institution." ;
    vivo:courseCredits 4 ;
    vivo:hasSubjectArea "IMCA" .

roboprof_data:IMCA_481 a vivo:Course ;
    dbo:name "Professional Internship in Intermedia I" ;
    dbo:number 481 ;
    dcterms:description "Under the joint supervision of a qualified professional and a full-time faculty member, the student is employed within industry or by a professional organization or other relevant institution." ;
    vivo:courseCredits 3 ;
    vivo:hasSubjectArea "IMCA" .

roboprof_data:IMCA_482 a vivo:Course ;
    dbo:name "Professional Internship in Intermedia II" ;
    dbo:number 482 ;
    dcterms:description "Under the joint supervision of a qualified professional and a full-time faculty member, the student is employed within industry or by a professional organization or other relevant institution." ;
    vivo:courseCredits 4 ;
    vivo:hasSubjectArea "IMCA" .

roboprof_data:IMCA_498 a vivo:Course ;
    dbo:name "Special Topics in Intermedia " ;
    dbo:number 498 ;
    dcterms:description "This studio course provides an opportunity for study and practice of specialized aspects of intermedia." ;
    vivo:courseCredits 3 ;
    vivo:hasSubjectArea "IMCA" .

roboprof_data:IMCA_499 a vivo:Course ;
    dbo:name "Special Topics in Intermedia" ;
    dbo:number 499 ;
    dcterms:description "This studio course provides an opportunity for study and practice of specialized aspects of intermedia." ;
    vivo:courseCredits 3 ;
    vivo:hasSubjectArea "IMCA" .

roboprof_data:INDU_311 a vivo:Course ;
    dbo:name "Simulation of Industrial Systems" ;
    dbo:number 311 ;
    dcterms:description "Simulation,  Laboratory: 2 hours per week" ;
    vivo:courseCredits 4 ;
    vivo:hasSubjectArea "INDU" .

roboprof_data:INDU_323 a vivo:Course ;
    dbo:name "Operations Research I" ;
    dbo:number 323 ;
    dcterms:description "Laboratory: 2 hours per week, alternate weeks" ;
    vivo:courseCredits 3 ;
    vivo:hasSubjectArea "INDU" .

roboprof_data:INDU_324 a vivo:Course ;
    dbo:name "Operations Research II" ;
    dbo:number 324 ;
    dcterms:description "Laboratory: 2 hours per week, alternate weeks" ;
    vivo:courseCredits 3 ;
    vivo:hasSubjectArea "INDU" .

roboprof_data:INDU_410 a vivo:Course ;
    dbo:name "Safety Engineering" ;
    dbo:number 410 ;
    dcterms:description "Laboratory: 2 hours per week, alternate weeks" ;
    vivo:courseCredits 4 ;
    vivo:hasSubjectArea "INDU" .

roboprof_data:INDU_411 a vivo:Course ;
    dbo:name "Computer Integrated Manufacturing" ;
    dbo:number 411 ;
    dcterms:description "Laboratory: 2 hours per week, alternate weeks" ;
    vivo:courseCredits 4 ;
    vivo:hasSubjectArea "INDU" .

roboprof_data:INDU_412 a vivo:Course ;
    dbo:name "Human Factors Engineering" ;
    dbo:number 412 ;
    dcterms:description "Laboratory: 2 hours per week, alternate weeks" ;
    vivo:courseCredits 3 ;
    vivo:hasSubjectArea "INDU" .

roboprof_data:INDU_421 a vivo:Course ;
    dbo:name "Facilities Design and Material Handling Systems" ;
    dbo:number 421 ;
    dcterms:description "Laboratory: 2 hours per week, alternate weeks" ;
    vivo:courseCredits 4 ;
    vivo:hasSubjectArea "INDU" .

roboprof_data:INDU_423 a vivo:Course ;
    dbo:name "Inventory Control" ;
    dbo:number 423 ;
    dcterms:description "Laboratory: 2 hours per week, alternate weeks" ;
    vivo:courseCredits 4 ;
    vivo:hasSubjectArea "INDU" .

roboprof_data:INDU_480 a vivo:Course ;
    dbo:name "Cases in Industrial Engineering" ;
    dbo:number 480 ;
    dcterms:description "Real-world situations, problem posed by the client" ;
    vivo:courseCredits 4 ;
    vivo:hasSubjectArea "INDU" .

roboprof_data:INDU_490 a vivo:Course ;
    dbo:name "Capstone Industrial Engineering Design Project" ;
    dbo:number 490 ;
    dcterms:description "capstone, group project" ;
    vivo:courseCredits 4 ;
    vivo:hasSubjectArea "INDU" .

roboprof_data:INDU_6111 a vivo:Course ;
    dbo:name "Theory of Operations Research" ;
    dbo:number 6111 ;
    dcterms:description "Project: 2 hours per week" ;
    vivo:courseCredits 3 ;
    vivo:hasSubjectArea "INDU" .

roboprof_data:INDU_6121 a vivo:Course ;
    dbo:name "Advanced Operations Research" ;
    dbo:number 6121 ;
    dcterms:description "A design project is required" ;
    vivo:courseCredits 4 ;
    vivo:hasSubjectArea "INDU" .

roboprof_data:INDU_6131 a vivo:Course ;
    dbo:name "Graph Theory with System Applications" ;
    dbo:number 6131 ;
    dcterms:description "Project: 2 hours per week" ;
    vivo:courseCredits 3 ;
    vivo:hasSubjectArea "INDU" .

roboprof_data:INDU_6141 a vivo:Course ;
    dbo:name "Logistics Network Models" ;
    dbo:number 6141 ;
    dcterms:description "A project is required" ;
    vivo:courseCredits 3 ;
    vivo:hasSubjectArea "INDU" .

roboprof_data:INDU_6151 a vivo:Course ;
    dbo:name "Decision Models in Service Sector" ;
    dbo:number 6151 ;
    dcterms:description "A project is required" ;
    vivo:courseCredits 4 ;
    vivo:hasSubjectArea "INDU" .

roboprof_data:INDU_6211 a vivo:Course ;
    dbo:name "Production Systems and Inventory Control" ;
    dbo:number 6211 ;
    dcterms:description "A project is required" ;
    vivo:courseCredits 4 ;
    vivo:hasSubjectArea "INDU" .

roboprof_data:INDU_6221 a vivo:Course ;
    dbo:name "Lean Enterprise" ;
    dbo:number 6221 ;
    dcterms:description "A project is required" ;
    vivo:courseCredits 4 ;
    vivo:hasSubjectArea "INDU" .

roboprof_data:INDU_6231 a vivo:Course ;
    dbo:name "Scheduling Theory" ;
    dbo:number 6231 ;
    dcterms:description "Project: 2 hours per week" ;
    vivo:courseCredits 4 ;
    vivo:hasSubjectArea "INDU" .

roboprof_data:INDU_6241 a vivo:Course ;
    dbo:name "Lean Manufacturing" ;
    dbo:number 6241 ;
    dcterms:description "A project is required" ;
    vivo:courseCredits 3 ;
    vivo:hasSubjectArea "INDU" .

roboprof_data:INDU_6311 a vivo:Course ;
    dbo:name "Discrete System Simulation" ;
    dbo:number 6311 ;
    dcterms:description "Computer simulation, A project is required" ;
    vivo:courseCredits 3 ;
    vivo:hasSubjectArea "INDU" .

roboprof_data:INDU_6321 a vivo:Course ;
    dbo:name "Introduction to Six Sigma" ;
    dbo:number 6321 ;
    dcterms:description "A project is required" ;
    vivo:courseCredits 4 ;
    vivo:hasSubjectArea "INDU" .

roboprof_data:INDU_6331 a vivo:Course ;
    dbo:name "Advanced Quality Control" ;
    dbo:number 6331 ;
    dcterms:description "A project is required" ;
    vivo:courseCredits 4 ;
    vivo:hasSubjectArea "INDU" .

roboprof_data:INDU_6341 a vivo:Course ;
    dbo:name "Advanced Concepts in Quality Improvement" ;
    dbo:number 6341 ;
    dcterms:description "A project on selected topics is required" ;
    vivo:courseCredits 4 ;
    vivo:hasSubjectArea "INDU" .

roboprof_data:INDU_6351 a vivo:Course ;
    dbo:name "System Reliability" ;
    dbo:number 6351 ;
    dcterms:description "Project: 2 hours per week" ;
    vivo:courseCredits 3 ;
    vivo:hasSubjectArea "INDU" .

roboprof_data:INDU_6361 a vivo:Course ;
    dbo:name "Discrete Optimization" ;
    dbo:number 6361 ;
    dcterms:description "A project is required" ;
    vivo:courseCredits 3 ;
    vivo:hasSubjectArea "INDU" .

roboprof_data:INDU_6411 a vivo:Course ;
    dbo:name "Human Factors Engineering" ;
    dbo:number 6411 ;
    dcterms:description "A project on a current topic is required" ;
    vivo:courseCredits 3 ;
    vivo:hasSubjectArea "INDU" .

roboprof_data:INDU_6421 a vivo:Course ;
    dbo:name "Occupational Safety Engineering" ;
    dbo:number 6421 ;
    dcterms:description "A project on a current topic is required" ;
    vivo:courseCredits 3 ;
    vivo:hasSubjectArea "INDU" .

roboprof_data:INSE_6100 a vivo:Course ;
    dbo:name "Advanced Java Platforms" ;
    dbo:number 6100 ;
    dcterms:description "A project is required" ;
    vivo:courseCredits 3 ;
    vivo:hasSubjectArea "INSE" .

roboprof_data:INSE_6110 a vivo:Course ;
    dbo:name "Foundations of Cryptography" ;
    dbo:number 6110 ;
    dcterms:description "A project is required" ;
    vivo:courseCredits 3 ;
    vivo:hasSubjectArea "INSE" .

roboprof_data:INSE_6120 a vivo:Course ;
    dbo:name "Crypto-Protocol and Network Security" ;
    dbo:number 6120 ;
    dcterms:description "A project is required" ;
    vivo:courseCredits 4 ;
    vivo:hasSubjectArea "INSE" .

roboprof_data:INSE_6130 a vivo:Course ;
    dbo:name "Operating Systems Security" ;
    dbo:number 6130 ;
    dcterms:description "A project is required" ;
    vivo:courseCredits 3 ;
    vivo:hasSubjectArea "INSE" .

roboprof_data:INSE_6140 a vivo:Course ;
    dbo:name "Malware Defenses and Application Security" ;
    dbo:number 6140 ;
    dcterms:description "A project is required" ;
    vivo:courseCredits 4 ;
    vivo:hasSubjectArea "INSE" .

roboprof_data:INSE_6150 a vivo:Course ;
    dbo:name "Security Evaluation Methodologies" ;
    dbo:number 6150 ;
    dcterms:description "A project is required" ;
    vivo:courseCredits 3 ;
    vivo:hasSubjectArea "INSE" .

roboprof_data:INSE_6160 a vivo:Course ;
    dbo:name "Database Security and Privacy" ;
    dbo:number 6160 ;
    dcterms:description "A project is required" ;
    vivo:courseCredits 4 ;
    vivo:hasSubjectArea "INSE" .

roboprof_data:INSE_6170 a vivo:Course ;
    dbo:name "Network Security Architecture and Management" ;
    dbo:number 6170 ;
    dcterms:description "A project is required" ;
    vivo:courseCredits 3 ;
    vivo:hasSubjectArea "INSE" .

roboprof_data:INSE_6180 a vivo:Course ;
    dbo:name "Security and Privacy Implications of Data Mining" ;
    dbo:number 6180 ;
    dcterms:description "A project is required" ;
    vivo:courseCredits 4 ;
    vivo:hasSubjectArea "INSE" .

roboprof_data:INSE_6190 a vivo:Course ;
    dbo:name "Wireless Network Security" ;
    dbo:number 6190 ;
    dcterms:description "A project is required" ;
    vivo:courseCredits 4 ;
    vivo:hasSubjectArea "INSE" .

roboprof_data:INSE_6210 a vivo:Course ;
    dbo:name "Total Quality Methodologies in Engineering" ;
    dbo:number 6210 ;
    dcterms:description "A project is required" ;
    vivo:courseCredits 4 ;
    vivo:hasSubjectArea "INSE" .

roboprof_data:INSE_6220 a vivo:Course ;
    dbo:name "Advanced Statistical Approaches to Quality" ;
    dbo:number 6220 ;
    dcterms:description "A project is required" ;
    vivo:courseCredits 3 ;
    vivo:hasSubjectArea "INSE" .

roboprof_data:INSE_6230 a vivo:Course ;
    dbo:name "Total Quality Project Management" ;
    dbo:number 6230 ;
    dcterms:description "A project is required" ;
    vivo:courseCredits 4 ;
    vivo:hasSubjectArea "INSE" .

roboprof_data:INSE_6240 a vivo:Course ;
    dbo:name "Executive Communication" ;
    dbo:number 6240 ;
    dcterms:description "A project is required" ;
    vivo:courseCredits 3 ;
    vivo:hasSubjectArea "INSE" .

roboprof_data:INSE_6250 a vivo:Course ;
    dbo:name "Quality Methodologies for Software" ;
    dbo:number 6250 ;
    dcterms:description "A project is required" ;
    vivo:courseCredits 3 ;
    vivo:hasSubjectArea "INSE" .

roboprof_data:INSE_6260 a vivo:Course ;
    dbo:name "Software Quality Assurance" ;
    dbo:number 6260 ;
    dcterms:description "A project is required" ;
    vivo:courseCredits 4 ;
    vivo:hasSubjectArea "INSE" .

roboprof_data:INSE_6270 a vivo:Course ;
    dbo:name "Quality-Based System Engineering" ;
    dbo:number 6270 ;
    dcterms:description "A project is required" ;
    vivo:courseCredits 3 ;
    vivo:hasSubjectArea "INSE" .

roboprof_data:INSE_6280 a vivo:Course ;
    dbo:name "Quality Assurance for System Engineering" ;
    dbo:number 6280 ;
    dcterms:description "A project is required" ;
    vivo:courseCredits 3 ;
    vivo:hasSubjectArea "INSE" .

roboprof_data:INSE_6290 a vivo:Course ;
    dbo:name "Quality in Supply Chain Design" ;
    dbo:number 6290 ;
    dcterms:description "A project is required" ;
    vivo:courseCredits 4 ;
    vivo:hasSubjectArea "INSE" .

roboprof_data:INSE_6300 a vivo:Course ;
    dbo:name "Quality Assurance in Supply Chain Management" ;
    dbo:number 6300 ;
    dcterms:description "A project is required" ;
    vivo:courseCredits 3 ;
    vivo:hasSubjectArea "INSE" .

roboprof_data:INSE_6310 a vivo:Course ;
    dbo:name "Systems Engineering Maintenance Management" ;
    dbo:number 6310 ;
    dcterms:description "A project is required" ;
    vivo:courseCredits 3 ;
    vivo:hasSubjectArea "INSE" .

roboprof_data:INSE_6311 a vivo:Course ;
    dbo:name "Sustainable Infrastructure Planning and Management Systems" ;
    dbo:number 6311 ;
    dcterms:description "Projects" ;
    vivo:courseCredits 3 ;
    vivo:hasSubjectArea "INSE" .

roboprof_data:INSE_6320 a vivo:Course ;
    dbo:name "Risk Analysis for Information and Systems Engineering" ;
    dbo:number 6320 ;
    dcterms:description "A project is required" ;
    vivo:courseCredits 3 ;
    vivo:hasSubjectArea "INSE" .

roboprof_data:INSE_6400 a vivo:Course ;
    dbo:name "Principles of Systems Engineering" ;
    dbo:number 6400 ;
    dcterms:description "A project is required" ;
    vivo:courseCredits 3 ;
    vivo:hasSubjectArea "INSE" .

roboprof_data:INSE_6411 a vivo:Course ;
    dbo:name "Product Design Theory and Methodology" ;
    dbo:number 6411 ;
    dcterms:description "A project is required" ;
    vivo:courseCredits 3 ;
    vivo:hasSubjectArea "INSE" .

roboprof_data:INSE_6421 a vivo:Course ;
    dbo:name "Systems Integration and Testing" ;
    dbo:number 6421 ;
    dcterms:description "A project is required" ;
    vivo:courseCredits 4 ;
    vivo:hasSubjectArea "INSE" .

roboprof_data:INSE_6431 a vivo:Course ;
    dbo:name "Ad Hoc Wireless Networks: Architectures and Protocols" ;
    dbo:number 6431 ;
    dcterms:description "A project is required" ;
    vivo:courseCredits 4 ;
    vivo:hasSubjectArea "INSE" .

roboprof_data:INSE_6441 a vivo:Course ;
    dbo:name "Applied Game Theory and Mechanism Design" ;
    dbo:number 6441 ;
    dcterms:description "A project is required" ;
    vivo:courseCredits 4 ;
    vivo:hasSubjectArea "INSE" .

roboprof_data:INSE_6510 a vivo:Course ;
    dbo:name "Video Game Technology and Development" ;
    dbo:number 6510 ;
    dcterms:description "A project is required" ;
    vivo:courseCredits 4 ;
    vivo:hasSubjectArea "INSE" .

roboprof_data:INSE_6530 a vivo:Course ;
    dbo:name "3D Graphics and Computer Animation for Game Design" ;
    dbo:number 6530 ;
    dcterms:description "A project is required" ;
    vivo:courseCredits 3 ;
    vivo:hasSubjectArea "INSE" .

roboprof_data:INSE_6610 a vivo:Course ;
    dbo:name "Cybercrime Investigations" ;
    dbo:number 6610 ;
    dcterms:description "A project is required" ;
    vivo:courseCredits 4 ;
    vivo:hasSubjectArea "INSE" .

roboprof_data:INSE_6630 a vivo:Course ;
    dbo:name "Recent Developments in Information Systems Security" ;
    dbo:number 6630 ;
    dcterms:description "A project is required" ;
    vivo:courseCredits 4 ;
    vivo:hasSubjectArea "INSE" .

roboprof_data:INSE_6640 a vivo:Course ;
    dbo:name "Smart Grids and Control System Security" ;
    dbo:number 6640 ;
    dcterms:description "A project is required" ;
    vivo:courseCredits 3 ;
    vivo:hasSubjectArea "INSE" .

roboprof_data:INSE_6650 a vivo:Course ;
    dbo:name "Trusted Computing" ;
    dbo:number 6650 ;
    dcterms:description "A project is required" ;
    vivo:courseCredits 3 ;
    vivo:hasSubjectArea "INSE" .

roboprof_data:INSE_6660 a vivo:Course ;
    dbo:name "Secure programsming" ;
    dbo:number 6660 ;
    dcterms:description "A project is required" ;
    vivo:courseCredits 3 ;
    vivo:hasSubjectArea "INSE" .

roboprof_data:INSE_6670 a vivo:Course ;
    dbo:name "Embedded Systems Security" ;
    dbo:number 6670 ;
    dcterms:description "A project is required" ;
    vivo:courseCredits 4 ;
    vivo:hasSubjectArea "INSE" .

roboprof_data:INSE_6680 a vivo:Course ;
    dbo:name "Systems Physical Security" ;
    dbo:number 6680 ;
    dcterms:description "A project is required" ;
    vivo:courseCredits 3 ;
    vivo:hasSubjectArea "INSE" .

roboprof_data:INSE_7100 a vivo:Course ;
    dbo:name "Design and Analysis of Security Protocols" ;
    dbo:number 7100 ;
    dcterms:description "A project is required" ;
    vivo:courseCredits 3 ;
    vivo:hasSubjectArea "INSE" .

roboprof_data:INSE_7110 a vivo:Course ;
    dbo:name "Value Added Service Engineering in Next Generation Networks" ;
    dbo:number 7110 ;
    dcterms:description "A project is required" ;
    vivo:courseCredits 4 ;
    vivo:hasSubjectArea "INSE" .

roboprof_data:INSE_7120 a vivo:Course ;
    dbo:name "Advanced Network Management" ;
    dbo:number 7120 ;
    dcterms:description "A project is required" ;
    vivo:courseCredits 4 ;
    vivo:hasSubjectArea "INSE" .

roboprof_data:INSE_8901 a vivo:Course ;
    dbo:name "Master of Applied Science Research and Thesis" ;
    dbo:number 8901 ;
    dcterms:description "Research, thesis" ;
    vivo:courseCredits 3 ;
    vivo:hasSubjectArea "INSE" .

roboprof_data:IRST_299 a vivo:Course ;
    dbo:name "Selected Topics: Introduction to Spoken Irish" ;
    dbo:number 299 ;
    dcterms:description "Applied language projects" ;
    vivo:courseCredits 3 ;
    vivo:hasSubjectArea "IRST" .

roboprof_data:IRST_300 a vivo:Course ;
    dbo:name "Research Methods in Irish Studies" ;
    dbo:number 300 ;
    dcterms:description "Participation in community events followed by anthropological analysis and reflection; final project includes self-driven bibliographic research with primary sources and material objects reflecting on the process in a final reflection paper on the problem or challenge of approaching a topic from at least three disciplinary perspectives. Final presentation could include a performance or creative dimension." ;
    vivo:courseCredits 3 ;
    vivo:hasSubjectArea "IRST" .

roboprof_data:IRST_344 a vivo:Course ;
    dbo:name "Classics of Irish Theatre" ;
    dbo:number 344 ;
    dcterms:description "Performance-based activities" ;
    vivo:courseCredits 4 ;
    vivo:hasSubjectArea "IRST" .

roboprof_data:IRST_346 a vivo:Course ;
    dbo:name "Irish Performance Studies" ;
    dbo:number 346 ;
    dcterms:description "Performance-based activities" ;
    vivo:courseCredits 4 ;
    vivo:hasSubjectArea "IRST" .

roboprof_data:IRST_347 a vivo:Course ;
    dbo:name "Contemporary Irish Theatre" ;
    dbo:number 347 ;
    dcterms:description "Performance-based activities" ;
    vivo:courseCredits 4 ;
    vivo:hasSubjectArea "IRST" .

roboprof_data:IRST_390 a vivo:Course ;
    dbo:name "Field Studies in Ireland" ;
    dbo:number 390 ;
    dcterms:description "Self-directed field study " ;
    vivo:courseCredits 4 ;
    vivo:hasSubjectArea "IRST" .

roboprof_data:ITAL_200 a vivo:Course ;
    dbo:name "Introductory Italian: Intensive" ;
    dbo:number 200 ;
    dcterms:description "lab work" ;
    vivo:courseCredits 3 ;
    vivo:hasSubjectArea "ITAL" .

roboprof_data:ITAL_201 a vivo:Course ;
    dbo:name "Introductory Italian I" ;
    dbo:number 201 ;
    dcterms:description "lab work" ;
    vivo:courseCredits 4 ;
    vivo:hasSubjectArea "ITAL" .

roboprof_data:ITAL_202 a vivo:Course ;
    dbo:name "Introductory Italian II" ;
    dbo:number 202 ;
    dcterms:description "lab work" ;
    vivo:courseCredits 3 ;
    vivo:hasSubjectArea "ITAL" .

roboprof_data:ITAL_240 a vivo:Course ;
    dbo:name "Intermediate Italian: Intensive Course " ;
    dbo:number 240 ;
    dcterms:description "lab work" ;
    vivo:courseCredits 4 ;
    vivo:hasSubjectArea "ITAL" .

roboprof_data:JAZZ_481 a vivo:Course ;
    dbo:name "Supervised Internship I" ;
    dbo:number 481 ;
    dcterms:description "Supervised internship at an industry/community partner" ;
    vivo:courseCredits 3 ;
    vivo:hasSubjectArea "JAZZ" .

roboprof_data:JAZZ_482 a vivo:Course ;
    dbo:name "Supervised Internship II" ;
    dbo:number 482 ;
    dcterms:description "Supervised internship at an industry/community partner" ;
    vivo:courseCredits 4 ;
    vivo:hasSubjectArea "JAZZ" .

roboprof_data:JOUR_206 a vivo:Course ;
    dbo:name "Introduction to Reporting" ;
    dbo:number 206 ;
    dcterms:description "Workshop course, practical out-of-class assignments" ;
    vivo:courseCredits 4 ;
    vivo:hasSubjectArea "JOUR" .

roboprof_data:JOUR_207 a vivo:Course ;
    dbo:name "Introduction to Multimedia" ;
    dbo:number 207 ;
    dcterms:description "Workshop course, practical out-of-class assignments" ;
    vivo:courseCredits 3 ;
    vivo:hasSubjectArea "JOUR" .

roboprof_data:JOUR_208 a vivo:Course ;
    dbo:name "Intermediate Reporting" ;
    dbo:number 208 ;
    dcterms:description "Workshop course, practical out-of-class assignments" ;
    vivo:courseCredits 3 ;
    vivo:hasSubjectArea "JOUR" .

roboprof_data:JOUR_209 a vivo:Course ;
    dbo:name "Intermediate Multimedia" ;
    dbo:number 209 ;
    dcterms:description "Workshop course, practical out-of-class assignments" ;
    vivo:courseCredits 4 ;
    vivo:hasSubjectArea "JOUR" .

roboprof_data:JOUR_303 a vivo:Course ;
    dbo:name "Feature Writing" ;
    dbo:number 303 ;
    dcterms:description "Workshop course, practical out-of-class assignments" ;
    vivo:courseCredits 4 ;
    vivo:hasSubjectArea "JOUR" .

roboprof_data:JOUR_309 a vivo:Course ;
    dbo:name "Editing and Page Design" ;
    dbo:number 309 ;
    dcterms:description "Workshop course, practical out-of-class assignments" ;
    vivo:courseCredits 4 ;
    vivo:hasSubjectArea "JOUR" .

roboprof_data:JOUR_321 a vivo:Course ;
    dbo:name "Visual Journalism" ;
    dbo:number 321 ;
    dcterms:description "Workshop course, practical out-of-class assignments" ;
    vivo:courseCredits 4 ;
    vivo:hasSubjectArea "JOUR" .

roboprof_data:JOUR_325 a vivo:Course ;
    dbo:name "Social Media and Mobile Reporting" ;
    dbo:number 325 ;
    dcterms:description "Workshop course, practical out-of-class assignments" ;
    vivo:courseCredits 3 ;
    vivo:hasSubjectArea "JOUR" .

roboprof_data:JOUR_330 a vivo:Course ;
    dbo:name "Radio Newsroom" ;
    dbo:number 330 ;
    dcterms:description "Course replicates the working conditions and journalistic experience of a digital newsroom" ;
    vivo:courseCredits 3 ;
    vivo:hasSubjectArea "JOUR" .

roboprof_data:JOUR_402 a vivo:Course ;
    dbo:name "Specialist Reporting" ;
    dbo:number 402 ;
    dcterms:description "Workshop course, practical out-of-class assignments" ;
    vivo:courseCredits 3 ;
    vivo:hasSubjectArea "JOUR" .

roboprof_data:JOUR_404 a vivo:Course ;
    dbo:name "Magazine Writing" ;
    dbo:number 404 ;
    dcterms:description "Workshop course, practical out-of-class assignments" ;
    vivo:courseCredits 3 ;
    vivo:hasSubjectArea "JOUR" .

roboprof_data:JOUR_421 a vivo:Course ;
    dbo:name "Advanced Video Journalism" ;
    dbo:number 421 ;
    dcterms:description "Workshop course, practical out-of-class assignments" ;
    vivo:courseCredits 4 ;
    vivo:hasSubjectArea "JOUR" .

roboprof_data:JOUR_432 a vivo:Course ;
    dbo:name "Documentary Video and Radio" ;
    dbo:number 432 ;
    dcterms:description "Workshop course, practical out-of-class assignments" ;
    vivo:courseCredits 3 ;
    vivo:hasSubjectArea "JOUR" .

roboprof_data:JOUR_443 a vivo:Course ;
    dbo:name "The Digital Magazine" ;
    dbo:number 443 ;
    dcterms:description "Capstone course" ;
    vivo:courseCredits 3 ;
    vivo:hasSubjectArea "JOUR" .

roboprof_data:JOUR_445 a vivo:Course ;
    dbo:name "Advanced Photojournalism" ;
    dbo:number 445 ;
    dcterms:description "Workshop course, practical out-of-class assignments" ;
    vivo:courseCredits 3 ;
    vivo:hasSubjectArea "JOUR" .

roboprof_data:JOUR_450 a vivo:Course ;
    dbo:name "Journalism Practicum" ;
    dbo:number 450 ;
    dcterms:description "Practicum at a recognized media outlet" ;
    vivo:courseCredits 4 ;
    vivo:hasSubjectArea "JOUR" .

roboprof_data:JOUR_502 a vivo:Course ;
    dbo:name "Introduction to Reporting" ;
    dbo:number 502 ;
    dcterms:description "Lecture/laboratory course, students receive assignments both in class and in the field" ;
    vivo:courseCredits 3 ;
    vivo:hasSubjectArea "JOUR" .

roboprof_data:JOUR_503 a vivo:Course ;
    dbo:name "Introduction to Visual Journalism" ;
    dbo:number 503 ;
    dcterms:description "Workshop course" ;
    vivo:courseCredits 3 ;
    vivo:hasSubjectArea "JOUR" .

roboprof_data:JOUR_504 a vivo:Course ;
    dbo:name "Intermediate Reporting" ;
    dbo:number 504 ;
    dcterms:description "Workshop course, practical out-of-class assignments" ;
    vivo:courseCredits 3 ;
    vivo:hasSubjectArea "JOUR" .

roboprof_data:JOUR_505 a vivo:Course ;
    dbo:name "Advanced Reporting" ;
    dbo:number 505 ;
    dcterms:description "Workshop course, practical out-of-class assignments" ;
    vivo:courseCredits 4 ;
    vivo:hasSubjectArea "JOUR" .

roboprof_data:JOUR_507 a vivo:Course ;
    dbo:name "Basics of Digital Imaging" ;
    dbo:number 507 ;
    dcterms:description "Workshop course, practical out-of-class assignments" ;
    vivo:courseCredits 3 ;
    vivo:hasSubjectArea "JOUR" .

roboprof_data:JOUR_521 a vivo:Course ;
    dbo:name "Visual Story-Telling" ;
    dbo:number 521 ;
    dcterms:description "Workshop course, practical out-of-class assignments" ;
    vivo:courseCredits 4 ;
    vivo:hasSubjectArea "JOUR" .

roboprof_data:JOUR_523 a vivo:Course ;
    dbo:name "News and Feature Photography" ;
    dbo:number 523 ;
    dcterms:description "Workshop course, practical out-of-class assignments" ;
    vivo:courseCredits 3 ;
    vivo:hasSubjectArea "JOUR" .

roboprof_data:JOUR_527 a vivo:Course ;
    dbo:name "Elements of Lighting for Visual Journalism" ;
    dbo:number 527 ;
    dcterms:description "Workshop course, practical out-of-class assignments" ;
    vivo:courseCredits 3 ;
    vivo:hasSubjectArea "JOUR" .

roboprof_data:JOUR_528 a vivo:Course ;
    dbo:name "The Digital Magazine" ;
    dbo:number 528 ;
    dcterms:description "Course replicates the working conditions and journalistic experience of a digital newsroom" ;
    vivo:courseCredits 4 ;
    vivo:hasSubjectArea "JOUR" .

roboprof_data:JOUR_530 a vivo:Course ;
    dbo:name "Advanced Radio News" ;
    dbo:number 530 ;
    dcterms:description "Course replicates the working conditions and journalistic experience of a digital newsroom" ;
    vivo:courseCredits 4 ;
    vivo:hasSubjectArea "JOUR" .

roboprof_data:JOUR_531 a vivo:Course ;
    dbo:name "Visual Journalism Photo Editing" ;
    dbo:number 531 ;
    dcterms:description "Workshop course, practical out-of-class assignments" ;
    vivo:courseCredits 4 ;
    vivo:hasSubjectArea "JOUR" .

roboprof_data:JOUR_532 a vivo:Course ;
    dbo:name "Documentary Video and Radio" ;
    dbo:number 532 ;
    dcterms:description "Workshop course, practical out-of-class assignments" ;
    vivo:courseCredits 4 ;
    vivo:hasSubjectArea "JOUR" .

roboprof_data:JOUR_535 a vivo:Course ;
    dbo:name "Documentary and Photographic Series" ;
    dbo:number 535 ;
    dcterms:description "Workshop course, practical out-of-class assignments" ;
    vivo:courseCredits 4 ;
    vivo:hasSubjectArea "JOUR" .

roboprof_data:JOUR_537 a vivo:Course ;
    dbo:name "Visual Journalism Portfolio" ;
    dbo:number 537 ;
    dcterms:description "Workshop course, practical out-of-class assignments" ;
    vivo:courseCredits 4 ;
    vivo:hasSubjectArea "JOUR" .

roboprof_data:JOUR_605 a vivo:Course ;
    dbo:name "Digital Innovation in Journalism" ;
    dbo:number 605 ;
    dcterms:description "Real-world project/assignment, Case studies" ;
    vivo:courseCredits 4 ;
    vivo:hasSubjectArea "JOUR" .

roboprof_data:JOUR_630 a vivo:Course ;
    dbo:name "Mediating Diversity through Audio Story-telling" ;
    dbo:number 630 ;
    dcterms:description "Workshop course, practical out-of-class assignments" ;
    vivo:courseCredits 3 ;
    vivo:hasSubjectArea "JOUR" .

roboprof_data:JPER_223 a vivo:Course ;
    dbo:name "Big Band I" ;
    dbo:number 223 ;
    dcterms:description "A performance course in which students participate in the Big Band Jazz Ensemble. Students are required to participate in public performances." ;
    vivo:courseCredits 3 ;
    vivo:hasSubjectArea "JPER" .

roboprof_data:JPER_224 a vivo:Course ;
    dbo:name "Eclectic Ensemble I" ;
    dbo:number 224 ;
    dcterms:description "A performance course in which students participate in the Eclectic Ensemble. Students are required to participate in public performances." ;
    vivo:courseCredits 4 ;
    vivo:hasSubjectArea "JPER " .

roboprof_data:JPER_225 a vivo:Course ;
    dbo:name "Jazz Choir" ;
    dbo:number 225 ;
    dcterms:description "A performance course in which students participate in the Jazz Choir. Students are required to participate in public performances." ;
    vivo:courseCredits 3 ;
    vivo:hasSubjectArea "JPER " .

roboprof_data:JPER_323 a vivo:Course ;
    dbo:name "Big Band II" ;
    dbo:number 323 ;
    dcterms:description "A continuation ofJPER 223. Students are required to participate in public performances." ;
    vivo:courseCredits 4 ;
    vivo:hasSubjectArea "JPER " .

roboprof_data:JPER_324 a vivo:Course ;
    dbo:name "Eclectic Ensemble II" ;
    dbo:number 324 ;
    dcterms:description "A continuation ofJPER 224. Students are required to participate in public performances." ;
    vivo:courseCredits 3 ;
    vivo:hasSubjectArea "JPER " .

roboprof_data:JPER_325 a vivo:Course ;
    dbo:name "Jazz Choir II" ;
    dbo:number 325 ;
    dcterms:description "A continuation ofJPER 225. Students are required to participate in public performances." ;
    vivo:courseCredits 3 ;
    vivo:hasSubjectArea "JPER " .

roboprof_data:JPER_341 a vivo:Course ;
    dbo:name "Jazz Vocal Repertoire I" ;
    dbo:number 341 ;
    dcterms:description "Public performance" ;
    vivo:courseCredits 4 ;
    vivo:hasSubjectArea "JPER" .

roboprof_data:JPER_423 a vivo:Course ;
    dbo:name "Big Band III" ;
    dbo:number 423 ;
    dcterms:description "A continuation ofJPER 323. Students are required to participate in public performances." ;
    vivo:courseCredits 4 ;
    vivo:hasSubjectArea "JPER " .

roboprof_data:JPER_424 a vivo:Course ;
    dbo:name "Eclectic Ensemble III" ;
    dbo:number 424 ;
    dcterms:description "A continuation ofJPER 324. Students are required to participate in public performances." ;
    vivo:courseCredits 3 ;
    vivo:hasSubjectArea "JPER" .

roboprof_data:JPER_425 a vivo:Course ;
    dbo:name "Jazz Choir III" ;
    dbo:number 425 ;
    dcterms:description "A continuation ofJPER 325. Students are required to participate in public performances." ;
    vivo:courseCredits 3 ;
    vivo:hasSubjectArea "JPER " .

roboprof_data:JPER_441 a vivo:Course ;
    dbo:name "Jazz Vocal Repertoire II" ;
    dbo:number 441 ;
    dcterms:description "Public performance" ;
    vivo:courseCredits 3 ;
    vivo:hasSubjectArea "JPER" .

roboprof_data:JPER_451 a vivo:Course ;
    dbo:name "JAZZ PRIVATE STUDY V" ;
    dbo:number 451 ;
    dcterms:description "NaN"^^xsd:double ;
    vivo:courseCredits 4 ;
    vivo:hasSubjectArea "JPER" .

roboprof_data:KCEP_349 a vivo:Course ;
    dbo:name "Assessment, Interpretation, and Rehabilitation in Neuromuscular Physiology" ;
    dbo:number 349 ;
    dcterms:description "Laboratory" ;
    vivo:courseCredits 4 ;
    vivo:hasSubjectArea "KCEP " .

roboprof_data:KCEP_383 a vivo:Course ;
    dbo:name "Kinesiology and Clinical Exercise Physiology Internship I" ;
    dbo:number 383 ;
    dcterms:description "Internship (200 hours)" ;
    vivo:courseCredits 4 ;
    vivo:hasSubjectArea "KCEP " .

roboprof_data:KCEP_449 a vivo:Course ;
    dbo:name "Physical Fitness Assessment, Exercise Prescription and Rehabilitation in Special Populations" ;
    dbo:number 449 ;
    dcterms:description "Laboratory" ;
    vivo:courseCredits 3 ;
    vivo:hasSubjectArea "KCEP " .

roboprof_data:KCEP_483 a vivo:Course ;
    dbo:name "Kinesiology and Clinical Exercise Physiology Internship II" ;
    dbo:number 483 ;
    dcterms:description "Internship (200 hours)" ;
    vivo:courseCredits 4 ;
    vivo:hasSubjectArea "KCEP " .

roboprof_data:LBCL_295 a vivo:Course ;
    dbo:name "History of Art" ;
    dbo:number 295 ;
    dcterms:description "Museum Field Work Project" ;
    vivo:courseCredits 4 ;
    vivo:hasSubjectArea "LBCL" .

roboprof_data:LIBS_495 a vivo:Course ;
    dbo:name "Field Practice" ;
    dbo:number 495 ;
    dcterms:description "5-week placement at a local library system" ;
    vivo:courseCredits 3 ;
    vivo:hasSubjectArea "LIBS" .

roboprof_data:LING_372 a vivo:Course ;
    dbo:name "Descriptive and Instrumental Phonetics" ;
    dbo:number 372 ;
    dcterms:description "lab/experiments built into course" ;
    vivo:courseCredits 4 ;
    vivo:hasSubjectArea "LING" .

roboprof_data:LING_421 a vivo:Course ;
    dbo:name "Non-Indo-European Structures" ;
    dbo:number 421 ;
    dcterms:description "The course involves working with a native speaker and/or from textual material." ;
    vivo:courseCredits 4 ;
    vivo:hasSubjectArea "LING" .

roboprof_data:LING_472 a vivo:Course ;
    dbo:name "Advanced Phonetics  " ;
    dbo:number 472 ;
    dcterms:description "NaN"^^xsd:double ;
    vivo:courseCredits 3 ;
    vivo:hasSubjectArea "LING" .

roboprof_data:LING_490 a vivo:Course ;
    dbo:name "Honours Thesis" ;
    dbo:number 490 ;
    dcterms:description "NaN"^^xsd:double ;
    vivo:courseCredits 4 ;
    vivo:hasSubjectArea "LING" .

roboprof_data:LOYC_205 a vivo:Course ;
    dbo:name "Introduction to Sustainability Studies (also listed as BIOL 205)" ;
    dbo:number 205 ;
    dcterms:description "Optional hands-on applied project. " ;
    vivo:courseCredits 3 ;
    vivo:hasSubjectArea "LOYC" .

roboprof_data:LOYC_240 a vivo:Course ;
    dbo:name "Global Environmental Issues and Ecological Justice (also listed as POLI 208)" ;
    dbo:number 240 ;
    dcterms:description "Groupwork simulation of the international climate change negotiations through the United Nations Framework Convention on Climate Change (UNFCCC).  Groups must come to an agreement for further reducing fossil fuel emissions following the success of the Paris Climate Accords in 2015." ;
    vivo:courseCredits 3 ;
    vivo:hasSubjectArea "LOYC" .

roboprof_data:LOYC_298 a vivo:Course ;
    dbo:name "Ecocide and Dystopias" ;
    dbo:number 298 ;
    dcterms:description "Film production and exhibition" ;
    vivo:courseCredits 4 ;
    vivo:hasSubjectArea "LOYC" .

roboprof_data:LOYC_320 a vivo:Course ;
    dbo:name "Biodiversity on Earth" ;
    dbo:number 320 ;
    dcterms:description "Fieldwork on biodiversity in the neighbourhood" ;
    vivo:courseCredits 4 ;
    vivo:hasSubjectArea "LOYC" .

roboprof_data:LOYC_420 a vivo:Course ;
    dbo:name "Integrative Project" ;
    dbo:number 420 ;
    dcterms:description "Most students (about 3/4 of the students) do a hands-on internship of relevance to Sustainability or Diversity Studies in the community and then reflect on their learning through classroom assignments. The rest of the students do a directed-study research project." ;
    vivo:courseCredits 4 ;
    vivo:hasSubjectArea "LOYC" .

roboprof_data:MACF_401 a vivo:Course ;
    dbo:name "Mathematical and Computational Finance I" ;
    dbo:number 401 ;
    dcterms:description "Modeling financial variables and pricing assets, calibration to real world financial data" ;
    vivo:courseCredits 4 ;
    vivo:hasSubjectArea "MACF" .

roboprof_data:MACF_402 a vivo:Course ;
    dbo:name "Mathematical and Computational Finance I" ;
    dbo:number 402 ;
    dcterms:description "Modeling financial variables and pricing assets, calibration to real world data, simulation and other numerical methods" ;
    vivo:courseCredits 4 ;
    vivo:hasSubjectArea "MACF" .

roboprof_data:MANA_300 a vivo:Course ;
    dbo:name "Entrepreneurship: Launching Your Business" ;
    dbo:number 300 ;
    dcterms:description "Students formulate their own business plans" ;
    vivo:courseCredits 4 ;
    vivo:hasSubjectArea "MANA" .

roboprof_data:MANA_343 a vivo:Course ;
    dbo:name "Negotiation and Conflict Resolution" ;
    dbo:number 343 ;
    dcterms:description "Practice, role play, and simulations" ;
    vivo:courseCredits 4 ;
    vivo:hasSubjectArea "MANA" .

roboprof_data:MANA_362 a vivo:Course ;
    dbo:name "Human Resource Management " ;
    dbo:number 362 ;
    dcterms:description "Includes a group project that requires students to go into companies and interview workers and prepare a report that produces a job description with either an interview guide or performance assessment" ;
    vivo:courseCredits 4 ;
    vivo:hasSubjectArea "MANA " .

roboprof_data:MANA_366 a vivo:Course ;
    dbo:name "Industrial Relations and Collective Bargaining" ;
    dbo:number 366 ;
    dcterms:description "Cases, role-playing, and simulations" ;
    vivo:courseCredits 3 ;
    vivo:hasSubjectArea "MANA" .

roboprof_data:MANA_420 a vivo:Course ;
    dbo:name "Management Research for Decision Making" ;
    dbo:number 420 ;
    dcterms:description "Handson experience with basic research techniques" ;
    vivo:courseCredits 3 ;
    vivo:hasSubjectArea "MANA" .

roboprof_data:MANA_443 a vivo:Course ;
    dbo:name "Compensation and Benefits" ;
    dbo:number 443 ;
    dcterms:description "Role play salary negotiation exercise to develop pay negotiation skills. Team paper consists of a consulting project where students create a compensation policy and salary structure based on actual pay data, company  and industry research. Presentation requires defending recommendations." ;
    vivo:courseCredits 4 ;
    vivo:hasSubjectArea "MANA" .

roboprof_data:MANA_444 a vivo:Course ;
    dbo:name "Training and Development" ;
    dbo:number 444 ;
    dcterms:description "Topics covered in this course include how training needs are assessed, how effective training programs are designed, how to ensure that learning achieved in training is transferred to the work, and how training programs are evaluated." ;
    vivo:courseCredits 3 ;
    vivo:hasSubjectArea "MANA" .

roboprof_data:MANA_446 a vivo:Course ;
    dbo:name "Workplace Planning and Staffing" ;
    dbo:number 446 ;
    dcterms:description "Real-world exploration of staffing in a specific company" ;
    vivo:courseCredits 4 ;
    vivo:hasSubjectArea "MANA" .

roboprof_data:MANA_447 a vivo:Course ;
    dbo:name "Leadership and Motivation" ;
    dbo:number 447 ;
    dcterms:description "Cases and simulations" ;
    vivo:courseCredits 4 ;
    vivo:hasSubjectArea "MANA" .

roboprof_data:MANA_481 a vivo:Course ;
    dbo:name "Introduction to Management Consulting" ;
    dbo:number 481 ;
    dcterms:description "Realworld consulting project that students conduct with a client firm" ;
    vivo:courseCredits 3 ;
    vivo:hasSubjectArea "MANA" .

roboprof_data:MANA_668 a vivo:Course ;
    dbo:name "Sustainable Business Strategy" ;
    dbo:number 668 ;
    dcterms:description "Case based pedagogy, hands-on experience using and developing relevant tools and practices, often directly with Montreal-based organizations" ;
    vivo:courseCredits 3 ;
    vivo:hasSubjectArea "MANA" .

roboprof_data:MANA_684 a vivo:Course ;
    dbo:name "Entrepreneurship through Acquisition" ;
    dbo:number 684 ;
    dcterms:description "Students evaluate opportunities to acquire firms and alternative strategies to successfully acquire and manage these firms." ;
    vivo:courseCredits 3 ;
    vivo:hasSubjectArea "MANA" .

roboprof_data:MARA_200 a vivo:Course ;
    dbo:name "Introduction to Modern Standard Arabic I      " ;
    dbo:number 200 ;
    dcterms:description "lab work" ;
    vivo:courseCredits 3 ;
    vivo:hasSubjectArea "MARA" .

roboprof_data:MARA_203 a vivo:Course ;
    dbo:name "Modern Standard Arabic for Heritage Speakers I " ;
    dbo:number 203 ;
    dcterms:description "lab work" ;
    vivo:courseCredits 3 ;
    vivo:hasSubjectArea "MARA" .

roboprof_data:MARA_206 a vivo:Course ;
    dbo:name "Introduction to Modern Standard Arabic II" ;
    dbo:number 206 ;
    dcterms:description "lab work" ;
    vivo:courseCredits 4 ;
    vivo:hasSubjectArea "MARA" .

roboprof_data:MARA_207 a vivo:Course ;
    dbo:name "Modern Standard Arabic for Heritage Speakers II " ;
    dbo:number 207 ;
    dcterms:description "lab work" ;
    vivo:courseCredits 3 ;
    vivo:hasSubjectArea "MARA" .

roboprof_data:MARA_240 a vivo:Course ;
    dbo:name "Intermediate Modern Standard Arabic I      " ;
    dbo:number 240 ;
    dcterms:description "lab work" ;
    vivo:courseCredits 3 ;
    vivo:hasSubjectArea "MARA" .

roboprof_data:MARA_250 a vivo:Course ;
    dbo:name "Intermediate Modern Standard Arabic I      " ;
    dbo:number 250 ;
    dcterms:description "lab work" ;
    vivo:courseCredits 4 ;
    vivo:hasSubjectArea "MARA" .

roboprof_data:MARK_301 a vivo:Course ;
    dbo:name "Marketing Management II" ;
    dbo:number 301 ;
    dcterms:description "Active application of theory and case studies" ;
    vivo:courseCredits 3 ;
    vivo:hasSubjectArea "MARK" .

roboprof_data:MARK_305 a vivo:Course ;
    dbo:name "Consumer Behaviour" ;
    dbo:number 305 ;
    dcterms:description "This course analyzes the motivations, roles, and behaviour of the consumers, how they are affected by economic, social, and cultural influences, and how the marketer may model this behaviour for decision-making purposes." ;
    vivo:courseCredits 4 ;
    vivo:hasSubjectArea "MARK" .

roboprof_data:MARK_444 a vivo:Course ;
    dbo:name "Sports Marketing" ;
    dbo:number 444 ;
    dcterms:description "The overall objective of the course is to familiarize students with the keys to success in each facet of sports marketing. It covers all aspects of the marketing management process in the particular context of sports marketing and allocates attention to the two major aspects: marketing through sports and marketing of sports." ;
    vivo:courseCredits 4 ;
    vivo:hasSubjectArea "MARK" .

roboprof_data:MARK_451 a vivo:Course ;
    dbo:name "Marketing of Services" ;
    dbo:number 451 ;
    dcterms:description "The whole spectrum is covered, including the active application of theory, a high degree of realism, facilitated reflection, the identification of skills, connection to life after graduation, case studies, and real-world projects/assignments." ;
    vivo:courseCredits 3 ;
    vivo:hasSubjectArea "MARK" .

roboprof_data:MARK_452 a vivo:Course ;
    dbo:name "E-Marketing" ;
    dbo:number 452 ;
    dcterms:description "This course offers an introduction to e-marketing strategies and tools that are required for effective marketing via electronic media." ;
    vivo:courseCredits 4 ;
    vivo:hasSubjectArea "MARK" .

roboprof_data:MARK_453 a vivo:Course ;
    dbo:name "Marketing Communications" ;
    dbo:number 453 ;
    dcterms:description "Cases and role-playing" ;
    vivo:courseCredits 4 ;
    vivo:hasSubjectArea "MARK" .

roboprof_data:MARK_454 a vivo:Course ;
    dbo:name "Personal Selling" ;
    dbo:number 454 ;
    dcterms:description "Real world project, sales presentations, role playing, social style simulation, and reflective writing " ;
    vivo:courseCredits 3 ;
    vivo:hasSubjectArea "MARK" .

roboprof_data:MARK_457 a vivo:Course ;
    dbo:name "Marketing Channels" ;
    dbo:number 457 ;
    dcterms:description "This course focuses on the different ways in which organizations make their goods and services available for consumption: the inter-organizational system that makes up channels of distribution." ;
    vivo:courseCredits 3 ;
    vivo:hasSubjectArea "MARK" .

roboprof_data:MARK_458 a vivo:Course ;
    dbo:name "The Marketing of Food" ;
    dbo:number 458 ;
    dcterms:description "Real world project managed as capstone project involving real client organizations in agri-food; 5 to 9 guest speakers from industry, each discussing real and recent projects in agri-food marketing; 1 to 2 case studies each term; industry-focused weekly readings." ;
    vivo:courseCredits 4 ;
    vivo:hasSubjectArea "MARK" .

roboprof_data:MARK_462 a vivo:Course ;
    dbo:name "Environment of World Business" ;
    dbo:number 462 ;
    dcterms:description "This is a foundation course in international business; the objective is to present information which exposes the student to cultural, social, political, economic, legal, and financial environments in which Canadian business executives manage their operations abroad." ;
    vivo:courseCredits 4 ;
    vivo:hasSubjectArea "MARK" .

roboprof_data:MARK_463 a vivo:Course ;
    dbo:name "Retailing" ;
    dbo:number 463 ;
    dcterms:description "Includes a project where students create an innovative retail product/service that also serves a social cause" ;
    vivo:courseCredits 3 ;
    vivo:hasSubjectArea "MARK" .

roboprof_data:MARK_465 a vivo:Course ;
    dbo:name "International Marketing Management" ;
    dbo:number 465 ;
    dcterms:description "This course studies the management approach to international marketing, with emphasis on key variables that are controllable by the international marketing manager. " ;
    vivo:courseCredits 4 ;
    vivo:hasSubjectArea "MARK" .

roboprof_data:MARK_485 a vivo:Course ;
    dbo:name "Business to Business Marketing" ;
    dbo:number 485 ;
    dcterms:description "The whole spectrum is covered, including the active application of theory, a high degree of realism, facilitated reflection, the identification of skills, connection to life after graduation, case studies, and real-world projects/assignments." ;
    vivo:courseCredits 4 ;
    vivo:hasSubjectArea "MARK" .

roboprof_data:MARK_486 a vivo:Course ;
    dbo:name "Product Innovation and Strategy" ;
    dbo:number 486 ;
    dcterms:description "Real world project, workshops, case studies, product pitches, and reflective writing" ;
    vivo:courseCredits 4 ;
    vivo:hasSubjectArea "MARK" .

roboprof_data:MARK_491 a vivo:Course ;
    dbo:name "Brand Management (Seminar)" ;
    dbo:number 491 ;
    dcterms:description "This course focuses on issues of current and potential concern to marketers. " ;
    vivo:courseCredits 3 ;
    vivo:hasSubjectArea "MARK" .

roboprof_data:MARK_492 a vivo:Course ;
    dbo:name "Cross-Cultural Communications" ;
    dbo:number 492 ;
    dcterms:description "This course deals with the multicultural dimensions of international business operations. The objective is to develop Canadian managerial skills for effective performance in an international setting. " ;
    vivo:courseCredits 4 ;
    vivo:hasSubjectArea "MARK" .

roboprof_data:MARK_493 a vivo:Course ;
    dbo:name "Current Issues in Marketing" ;
    dbo:number 493 ;
    dcterms:description "This course focuses on issues of current and potential concern to marketers. " ;
    vivo:courseCredits 4 ;
    vivo:hasSubjectArea "MARK" .

roboprof_data:MARK_495 a vivo:Course ;
    dbo:name "Strategic Marketing Planning" ;
    dbo:number 495 ;
    dcterms:description "Capstone course with computer-based marketing strategy simulation cases" ;
    vivo:courseCredits 4 ;
    vivo:hasSubjectArea "MARK" .

roboprof_data:MARK_671 a vivo:Course ;
    dbo:name "Consumer Behaviour" ;
    dbo:number 671 ;
    dcterms:description "This course introduces frameworks, tools, and concepts that are relevant to the consumption of goods and services. The focus in on understanding consumer behaviour in order to develop and execute effective marketing strategies." ;
    vivo:courseCredits 3 ;
    vivo:hasSubjectArea "MARK" .

roboprof_data:MAST_232 a vivo:Course ;
    dbo:name "Mathematics with Computer Algebra" ;
    dbo:number 232 ;
    dcterms:description "Interactive, in the computer laboratory" ;
    vivo:courseCredits 4 ;
    vivo:hasSubjectArea "MAST" .

roboprof_data:MAST_324 a vivo:Course ;
    dbo:name "Introduction to Optimization" ;
    dbo:number 324 ;
    dcterms:description "Use of computing software" ;
    vivo:courseCredits 4 ;
    vivo:hasSubjectArea "MAST" .

roboprof_data:MAST_333 a vivo:Course ;
    dbo:name "Applied Statistics" ;
    dbo:number 333 ;
    dcterms:description "Use of statistical software" ;
    vivo:courseCredits 3 ;
    vivo:hasSubjectArea "MAST" .

roboprof_data:MAST_397 a vivo:Course ;
    dbo:name "Topics in Mathematics and Statistics (Topic in 2021 - Sports Analytics)" ;
    dbo:number 397 ;
    dcterms:description "Python programming, analysis of real data related to sports projects" ;
    vivo:courseCredits 4 ;
    vivo:hasSubjectArea "MAST" .

roboprof_data:MAST_677 a vivo:Course ;
    dbo:name "Time Series" ;
    dbo:number 677 ;
    dcterms:description "Computer analysis of time series using computer packages" ;
    vivo:courseCredits 4 ;
    vivo:hasSubjectArea "MAST" .

roboprof_data:MATH_387 a vivo:Course ;
    dbo:name "Mathematics Lab III" ;
    dbo:number 387 ;
    dcterms:description "Lab" ;
    vivo:courseCredits 3 ;
    vivo:hasSubjectArea "MATH" .

roboprof_data:MBA_642 a vivo:Course ;
    dbo:name "Financial Reporting for Responsible Decision Making" ;
    dbo:number 642 ;
    dcterms:description "Case analysis" ;
    vivo:courseCredits 3 ;
    vivo:hasSubjectArea "MBA" .

roboprof_data:MBA_644 a vivo:Course ;
    dbo:name "Marketing Management" ;
    dbo:number 644 ;
    dcterms:description "Case discussions and application-oriented readings" ;
    vivo:courseCredits 4 ;
    vivo:hasSubjectArea "MBA" .

roboprof_data:MBA_645 a vivo:Course ;
    dbo:name "Economics for Organizational Decision Making" ;
    dbo:number 645 ;
    dcterms:description "Cases and projects" ;
    vivo:courseCredits 3 ;
    vivo:hasSubjectArea "MBA" .

roboprof_data:MBA_647 a vivo:Course ;
    dbo:name "Managing People in Organizations" ;
    dbo:number 647 ;
    dcterms:description "This course informs students about core concepts that help to explain and predict how people behave in organizations, including discussions of perception, motivation, team dynamics, conflict, stress management, leadership, and change." ;
    vivo:courseCredits 4 ;
    vivo:hasSubjectArea "MBA" .

roboprof_data:MBA_649 a vivo:Course ;
    dbo:name "Strategic Managerial Accounting and Control" ;
    dbo:number 649 ;
    dcterms:description "Case analysis" ;
    vivo:courseCredits 3 ;
    vivo:hasSubjectArea "MBA" .

roboprof_data:MBA_650 a vivo:Course ;
    dbo:name "Crafting and Implementing Successful Strategies" ;
    dbo:number 650 ;
    dcterms:description "Cases and projects" ;
    vivo:courseCredits 4 ;
    vivo:hasSubjectArea "MBA" .

roboprof_data:MBA_654 a vivo:Course ;
    dbo:name "MBA Research Projects" ;
    dbo:number 654 ;
    dcterms:description "Case-based research and analysis, often working directly with the organizations being studied  " ;
    vivo:courseCredits 4 ;
    vivo:hasSubjectArea "MBA" .

roboprof_data:MBA_657 a vivo:Course ;
    dbo:name "International Case Competition - Executive Assistant" ;
    dbo:number 657 ;
    dcterms:description "Case Competition" ;
    vivo:courseCredits 4 ;
    vivo:hasSubjectArea "MBA" .

roboprof_data:MBA_658 a vivo:Course ;
    dbo:name "Van Berkon Case Competition - Executive Assistant" ;
    dbo:number 658 ;
    dcterms:description "Case Competition" ;
    vivo:courseCredits 4 ;
    vivo:hasSubjectArea "MBA" .

roboprof_data:MBA_659 a vivo:Course ;
    dbo:name "Strategies in Action (Case Competition)" ;
    dbo:number 659 ;
    dcterms:description "Case Competition" ;
    vivo:courseCredits 3 ;
    vivo:hasSubjectArea "MBA" .

roboprof_data:MBA_660 a vivo:Course ;
    dbo:name "Small Business Consulting Bureau" ;
    dbo:number 660 ;
    dcterms:description "The Concordia Small Business Consulting Bureau provides professional consulting services to start-ups and small businesses at competitive rates." ;
    vivo:courseCredits 3 ;
    vivo:hasSubjectArea "MBA" .

roboprof_data:MBA_662 a vivo:Course ;
    dbo:name "MBA Surgical Innovation II" ;
    dbo:number 662 ;
    dcterms:description "This is the second of two courses on Surgical Innovation introducing concepts and performing needs analyses right through to exploring the entrepreneurial skills needed to launch a start-up company." ;
    vivo:courseCredits 3 ;
    vivo:hasSubjectArea "MBA" .

roboprof_data:MBA_663 a vivo:Course ;
    dbo:name "District 3 Start Up Consulting" ;
    dbo:number 663 ;
    dcterms:description "The District 3 Startup Consulting course is a non-credit experiential learning opportunity. Students provide ad-hoc consulting services to startup entrepreneurs in the District 3 incubator." ;
    vivo:courseCredits 4 ;
    vivo:hasSubjectArea "MBA" .

roboprof_data:MBA_695 a vivo:Course ;
    dbo:name "Seminar in Special Topics" ;
    dbo:number 695 ;
    dcterms:description "The subject matter for this course will vary from term to term." ;
    vivo:courseCredits 4 ;
    vivo:hasSubjectArea "MBA" .

roboprof_data:MCHI_200 a vivo:Course ;
    dbo:name "Introductory Modern Chinese " ;
    dbo:number 200 ;
    dcterms:description "lab work" ;
    vivo:courseCredits 4 ;
    vivo:hasSubjectArea "MCHI" .

roboprof_data:MCHI_206 a vivo:Course ;
    dbo:name "Introduction to Modern Chinese II " ;
    dbo:number 206 ;
    dcterms:description "lab work" ;
    vivo:courseCredits 3 ;
    vivo:hasSubjectArea "MCHI" .

roboprof_data:MCHI_240 a vivo:Course ;
    dbo:name "Intermediate Modern Chinese I " ;
    dbo:number 240 ;
    dcterms:description "lab work" ;
    vivo:courseCredits 4 ;
    vivo:hasSubjectArea "MCHI" .

roboprof_data:MCHI_250 a vivo:Course ;
    dbo:name "Intermediate Modern Chinese II" ;
    dbo:number 250 ;
    dcterms:description "lab work" ;
    vivo:courseCredits 3 ;
    vivo:hasSubjectArea "MCHI" .

roboprof_data:MECH_211 a vivo:Course ;
    dbo:name "Mechanical Engineering Drawing" ;
    dbo:number 211 ;
    dcterms:description "Laboratory: 2 hours per week, alternate weeks" ;
    vivo:courseCredits 4 ;
    vivo:hasSubjectArea "MECH" .

roboprof_data:MECH_215 a vivo:Course ;
    dbo:name "Programming for Mechanical and Industrial Engineers" ;
    dbo:number 215 ;
    dcterms:description """Laboratory: 1 hour per week_x000D_
Using Arduino - a type of microcontroller board used for mechatronics and robotics""" ;
    vivo:courseCredits 3 ;
    vivo:hasSubjectArea "MECH" .

roboprof_data:MECH_311 a vivo:Course ;
    dbo:name "Manufacturing Processes" ;
    dbo:number 311 ;
    dcterms:description "Industrial visits, field trips to local industries, Laboratory: 3 hours per week, alternate weeks" ;
    vivo:courseCredits 3 ;
    vivo:hasSubjectArea "MECH" .

roboprof_data:MECH_321 a vivo:Course ;
    dbo:name "Properties and Failure of Materials" ;
    dbo:number 321 ;
    dcterms:description "Laboratory: 2 hours per week, alternate weeks" ;
    vivo:courseCredits 4 ;
    vivo:hasSubjectArea "MECH" .

roboprof_data:MECH_343 a vivo:Course ;
    dbo:name "Theory of Machines" ;
    dbo:number 343 ;
    dcterms:description "Laboratory: 2 hours per week, alternate weeks" ;
    vivo:courseCredits 4 ;
    vivo:hasSubjectArea "MECH" .

roboprof_data:MECH_351 a vivo:Course ;
    dbo:name "Thermodynamics II" ;
    dbo:number 351 ;
    dcterms:description """Laboratory: 2 hours per week, alternate weeks_x000D_
Micro Steam Car Competition: students design & build a car powered by a soda-can water boiler, a pin-sized nozzle and a turbine which drives the front wheels""" ;
    vivo:courseCredits 4 ;
    vivo:hasSubjectArea "MECH" .

roboprof_data:MECH_352 a vivo:Course ;
    dbo:name "Heat Transfer I" ;
    dbo:number 352 ;
    dcterms:description "Laboratory: 2 hours per week, alternate weeks" ;
    vivo:courseCredits 4 ;
    vivo:hasSubjectArea "MECH" .

roboprof_data:MECH_361 a vivo:Course ;
    dbo:name "Fluid Mechanics II" ;
    dbo:number 361 ;
    dcterms:description "Laboratory: 2 hours per week, alternate weeks" ;
    vivo:courseCredits 3 ;
    vivo:hasSubjectArea "MECH" .

roboprof_data:MECH_368 a vivo:Course ;
    dbo:name "Electronics for Mechanical Engineers" ;
    dbo:number 368 ;
    dcterms:description "Laboratory: 2 hours per week, alternate weeks" ;
    vivo:courseCredits 4 ;
    vivo:hasSubjectArea "MECH" .

roboprof_data:MECH_370 a vivo:Course ;
    dbo:name "Modelling and Analysis of Dynamic Systems" ;
    dbo:number 370 ;
    dcterms:description "Laboratory: 2 hours per week, alternate weeks" ;
    vivo:courseCredits 4 ;
    vivo:hasSubjectArea "MECH" .

roboprof_data:MECH_371 a vivo:Course ;
    dbo:name "Analysis and Design of Control Systems" ;
    dbo:number 371 ;
    dcterms:description "Laboratory: 3 hours per week, alternate weeks" ;
    vivo:courseCredits 3 ;
    vivo:hasSubjectArea "MECH" .

roboprof_data:MECH_375 a vivo:Course ;
    dbo:name "Mechanical Vibrations" ;
    dbo:number 375 ;
    dcterms:description "Laboratory: 2 hours per week, alternate weeks" ;
    vivo:courseCredits 4 ;
    vivo:hasSubjectArea "MECH" .

roboprof_data:MECH_390 a vivo:Course ;
    dbo:name "Mechanical Engineering Design Project" ;
    dbo:number 390 ;
    dcterms:description "Team-based design project" ;
    vivo:courseCredits 3 ;
    vivo:hasSubjectArea "MECH" .

roboprof_data:MECH_411 a vivo:Course ;
    dbo:name "Instrumentation and Measurements" ;
    dbo:number 411 ;
    dcterms:description "Laboratory: 2 hours per week, alternate weeks" ;
    vivo:courseCredits 4 ;
    vivo:hasSubjectArea "MECH" .

roboprof_data:MECH_412 a vivo:Course ;
    dbo:name "Computer-Aided Mechanical Design" ;
    dbo:number 412 ;
    dcterms:description "Laboratory: 2 hours per week, alternate weeks" ;
    vivo:courseCredits 3 ;
    vivo:hasSubjectArea "MECH" .

roboprof_data:MECH_414 a vivo:Course ;
    dbo:name "Computer Numerically Controlled Machining" ;
    dbo:number 414 ;
    dcterms:description "Laboratory: 2 hours per week, alternate weeks" ;
    vivo:courseCredits 3 ;
    vivo:hasSubjectArea "MECH" .

roboprof_data:MECH_421 a vivo:Course ;
    dbo:name "Mechanical Shaping of Metals and Plastics" ;
    dbo:number 421 ;
    dcterms:description "Laboratory: 2 hours per week, alternate weeks" ;
    vivo:courseCredits 3 ;
    vivo:hasSubjectArea "MECH" .

roboprof_data:MECH_423 a vivo:Course ;
    dbo:name "Casting, Welding, Heat Treating, and Non-Destructive Testing" ;
    dbo:number 423 ;
    dcterms:description "Laboratory: 2 hours per week, alternate weeks" ;
    vivo:courseCredits 4 ;
    vivo:hasSubjectArea "MECH" .

roboprof_data:MECH_424 a vivo:Course ;
    dbo:name "MEMS - Design and Fabrication" ;
    dbo:number 424 ;
    dcterms:description "Laboratory: 2 hours per week, alternate weeks" ;
    vivo:courseCredits 4 ;
    vivo:hasSubjectArea "MECH" .

roboprof_data:MECH_425 a vivo:Course ;
    dbo:name "Manufacturing of Composites" ;
    dbo:number 425 ;
    dcterms:description "Simulation,  Laboratory: 2 hours per week, alternate weeks" ;
    vivo:courseCredits 3 ;
    vivo:hasSubjectArea "MECH" .

roboprof_data:MECH_447 a vivo:Course ;
    dbo:name "Fundamentals of Vehicle System Design" ;
    dbo:number 447 ;
    dcterms:description "Laboratory: 2 hours per week, alternate weeks" ;
    vivo:courseCredits 3 ;
    vivo:hasSubjectArea "MECH" .

roboprof_data:MECH_452 a vivo:Course ;
    dbo:name "Heat Transfer II" ;
    dbo:number 452 ;
    dcterms:description "Laboratory: 2 hours per week, alternate weeks" ;
    vivo:courseCredits 3 ;
    vivo:hasSubjectArea "MECH" .

roboprof_data:MECH_460 a vivo:Course ;
    dbo:name "Finite Element Analysis" ;
    dbo:number 460 ;
    dcterms:description "Laboratory: 3 hours per week, alternate weeks" ;
    vivo:courseCredits 4 ;
    vivo:hasSubjectArea "MECH" .

roboprof_data:MECH_461 a vivo:Course ;
    dbo:name "Gas Dynamics" ;
    dbo:number 461 ;
    dcterms:description "Laboratory: 2 hours per week, alternate weeks" ;
    vivo:courseCredits 4 ;
    vivo:hasSubjectArea "MECH" .

roboprof_data:MECH_463 a vivo:Course ;
    dbo:name "Fluid Power Control" ;
    dbo:number 463 ;
    dcterms:description "Laboratory: 2 hours per week, alternate weeks" ;
    vivo:courseCredits 3 ;
    vivo:hasSubjectArea "MECH" .

roboprof_data:MECH_471 a vivo:Course ;
    dbo:name "Microcontrollers for Mechatronics" ;
    dbo:number 471 ;
    dcterms:description "Hands-on project, Laboratory: 2 hours per week, alternate weeks, 3D printer project incorporated" ;
    vivo:courseCredits 3 ;
    vivo:hasSubjectArea "MECH" .

roboprof_data:MECH_472 a vivo:Course ;
    dbo:name "Mechatronics and Automation" ;
    dbo:number 472 ;
    dcterms:description "Laboratory: 2 hours per week, alternate weeks" ;
    vivo:courseCredits 3 ;
    vivo:hasSubjectArea "MECH" .

roboprof_data:MECH_473 a vivo:Course ;
    dbo:name "Control System Design" ;
    dbo:number 473 ;
    dcterms:description "Lab project, Laboratory: 2 hours per week, alternate weeks, 3D printer project incorporated" ;
    vivo:courseCredits 3 ;
    vivo:hasSubjectArea "MECH" .

roboprof_data:MECH_474 a vivo:Course ;
    dbo:name "Mechatronics" ;
    dbo:number 474 ;
    dcterms:description "Laboratory: 3 hours per week, alternate weeks" ;
    vivo:courseCredits 3 ;
    vivo:hasSubjectArea "MECH" .

roboprof_data:MECH_6011 a vivo:Course ;
    dbo:name "Analysis and Design of Pneumatic Systems" ;
    dbo:number 6011 ;
    dcterms:description "A project on selected topics is required" ;
    vivo:courseCredits 4 ;
    vivo:hasSubjectArea "MECH" .

roboprof_data:MECH_6021 a vivo:Course ;
    dbo:name "Design of Industrial Control Systems" ;
    dbo:number 6021 ;
    dcterms:description "A project on specific topic or applications is required" ;
    vivo:courseCredits 3 ;
    vivo:hasSubjectArea "MECH" .

roboprof_data:MECH_6041 a vivo:Course ;
    dbo:name "Virtual Systems Engineering" ;
    dbo:number 6041 ;
    dcterms:description "A project is required" ;
    vivo:courseCredits 4 ;
    vivo:hasSubjectArea "MECH" .

roboprof_data:MECH_6051 a vivo:Course ;
    dbo:name "Process Dynamics and Control" ;
    dbo:number 6051 ;
    dcterms:description "A project on selected topics of current interest is required" ;
    vivo:courseCredits 3 ;
    vivo:hasSubjectArea "MECH" .

roboprof_data:MECH_6061 a vivo:Course ;
    dbo:name "Analysis and Design of Hydraulic Control Systems" ;
    dbo:number 6061 ;
    dcterms:description "A projects on selected topics is required" ;
    vivo:courseCredits 4 ;
    vivo:hasSubjectArea "MECH" .

roboprof_data:MECH_6081 a vivo:Course ;
    dbo:name "Fuel Control Systems for Combustion Engines" ;
    dbo:number 6081 ;
    dcterms:description "Demonstration in lab" ;
    vivo:courseCredits 3 ;
    vivo:hasSubjectArea "MECH" .

roboprof_data:MECH_6091 a vivo:Course ;
    dbo:name "Flight Control Systems" ;
    dbo:number 6091 ;
    dcterms:description "Flight simulation, Projects on selected topics are required" ;
    vivo:courseCredits 4 ;
    vivo:hasSubjectArea "MECH" .

roboprof_data:MECH_6101 a vivo:Course ;
    dbo:name "Kinetic Theory of Gases" ;
    dbo:number 6101 ;
    dcterms:description "A project on specific topic or applications is required" ;
    vivo:courseCredits 4 ;
    vivo:hasSubjectArea "MECH" .

roboprof_data:MECH_6111 a vivo:Course ;
    dbo:name "Gas Dynamics" ;
    dbo:number 6111 ;
    dcterms:description "A project on specific applications is required" ;
    vivo:courseCredits 3 ;
    vivo:hasSubjectArea "MECH" .

roboprof_data:MECH_6121 a vivo:Course ;
    dbo:name "Aerodynamics" ;
    dbo:number 6121 ;
    dcterms:description "A project on specific topic or applications is required" ;
    vivo:courseCredits 4 ;
    vivo:hasSubjectArea "MECH" .

roboprof_data:MECH_6131 a vivo:Course ;
    dbo:name "Conduction and Radiation Heat Transfer" ;
    dbo:number 6131 ;
    dcterms:description "A project on selected topics is required" ;
    vivo:courseCredits 4 ;
    vivo:hasSubjectArea "MECH" .

roboprof_data:MECH_6141 a vivo:Course ;
    dbo:name "Heat Exchanger Design" ;
    dbo:number 6141 ;
    dcterms:description "A project on selected topics is required" ;
    vivo:courseCredits 3 ;
    vivo:hasSubjectArea "MECH" .

roboprof_data:MECH_6161 a vivo:Course ;
    dbo:name "Gas Turbine Design" ;
    dbo:number 6161 ;
    dcterms:description "A project on specific topic or applications is required" ;
    vivo:courseCredits 3 ;
    vivo:hasSubjectArea "MECH" .

roboprof_data:MECH_6171 a vivo:Course ;
    dbo:name "Turbomachinery and Propulsion" ;
    dbo:number 6171 ;
    dcterms:description "Projects on selected topics are required" ;
    vivo:courseCredits 4 ;
    vivo:hasSubjectArea "MECH" .

roboprof_data:MECH_6181 a vivo:Course ;
    dbo:name "Heating, Air Conditioning and Ventilation" ;
    dbo:number 6181 ;
    dcterms:description "A project on selected applications is required" ;
    vivo:courseCredits 3 ;
    vivo:hasSubjectArea "MECH" .

roboprof_data:MECH_6191 a vivo:Course ;
    dbo:name "Combustion" ;
    dbo:number 6191 ;
    dcterms:description "Projects on selected topics are required" ;
    vivo:courseCredits 4 ;
    vivo:hasSubjectArea "MECH" .

roboprof_data:MECH_6231 a vivo:Course ;
    dbo:name "Helicopter Flight Dynamics" ;
    dbo:number 6231 ;
    dcterms:description "Case studies and projects on selected topics are required" ;
    vivo:courseCredits 3 ;
    vivo:hasSubjectArea "MECH" .

roboprof_data:MECH_6241 a vivo:Course ;
    dbo:name "Operational Performance of Aircraft" ;
    dbo:number 6241 ;
    dcterms:description "Projects on selected topics are required" ;
    vivo:courseCredits 3 ;
    vivo:hasSubjectArea "MECH" .

roboprof_data:MECH_6251 a vivo:Course ;
    dbo:name "Space Flight Mechanics and Propulsion Systems" ;
    dbo:number 6251 ;
    dcterms:description "A project is required" ;
    vivo:courseCredits 4 ;
    vivo:hasSubjectArea "MECH" .

roboprof_data:MECH_6301 a vivo:Course ;
    dbo:name "Vibration Problems in Rotating Machinery" ;
    dbo:number 6301 ;
    dcterms:description "Projects on selected applications are required" ;
    vivo:courseCredits 4 ;
    vivo:hasSubjectArea "MECH" .

roboprof_data:MECH_6311 a vivo:Course ;
    dbo:name "Noise and Vibration Control" ;
    dbo:number 6311 ;
    dcterms:description "Projects on selected applications are required" ;
    vivo:courseCredits 3 ;
    vivo:hasSubjectArea "MECH" .

roboprof_data:MECH_6321 a vivo:Course ;
    dbo:name "Optimum Design of Mechanical Systems" ;
    dbo:number 6321 ;
    dcterms:description "An optimization project on selected topics is required" ;
    vivo:courseCredits 4 ;
    vivo:hasSubjectArea "MECH" .

roboprof_data:MECH_6341 a vivo:Course ;
    dbo:name "Engineering Analysis of Smart Materials and Structures" ;
    dbo:number 6341 ;
    dcterms:description "A project is required" ;
    vivo:courseCredits 3 ;
    vivo:hasSubjectArea "MECH" .

roboprof_data:MECH_6351 a vivo:Course ;
    dbo:name "Modal Analysis of Mechanical Systems" ;
    dbo:number 6351 ;
    dcterms:description "Projects on selected applications are required" ;
    vivo:courseCredits 3 ;
    vivo:hasSubjectArea "MECH" .

roboprof_data:MECH_6361 a vivo:Course ;
    dbo:name "Mechanics of Biological Tissues" ;
    dbo:number 6361 ;
    dcterms:description "A project on current topic is required" ;
    vivo:courseCredits 3 ;
    vivo:hasSubjectArea "MECH" .

roboprof_data:MECH_6421 a vivo:Course ;
    dbo:name "Metal Machining and Surface Technology" ;
    dbo:number 6421 ;
    dcterms:description "A project on selected topics is required" ;
    vivo:courseCredits 3 ;
    vivo:hasSubjectArea "MECH" .

roboprof_data:MECH_6431 a vivo:Course ;
    dbo:name "Introduction to Tribology (Wear, Friction and Lubrication)" ;
    dbo:number 6431 ;
    dcterms:description "A project on specific topic or applications is required" ;
    vivo:courseCredits 3 ;
    vivo:hasSubjectArea "MECH" .

roboprof_data:MECH_6441 a vivo:Course ;
    dbo:name "Stress Analysis in Mechanical Design" ;
    dbo:number 6441 ;
    dcterms:description "Case studies, and project from selected applications are required" ;
    vivo:courseCredits 4 ;
    vivo:hasSubjectArea "MECH" .

roboprof_data:MECH_6451 a vivo:Course ;
    dbo:name "Computer-Aided Mechanical Design" ;
    dbo:number 6451 ;
    dcterms:description "A project is required" ;
    vivo:courseCredits 4 ;
    vivo:hasSubjectArea "MECH" .

roboprof_data:MECH_6481 a vivo:Course ;
    dbo:name "Aeroelasticity" ;
    dbo:number 6481 ;
    dcterms:description "A project on specific applications is required" ;
    vivo:courseCredits 3 ;
    vivo:hasSubjectArea "MECH" .

roboprof_data:MECH_6491 a vivo:Course ;
    dbo:name "Engineering Metrology and Measurement Systems" ;
    dbo:number 6491 ;
    dcterms:description "A project is required" ;
    vivo:courseCredits 4 ;
    vivo:hasSubjectArea "MECH" .

roboprof_data:MECH_6501 a vivo:Course ;
    dbo:name "Advanced Materials" ;
    dbo:number 6501 ;
    dcterms:description "A project on selected topics of current interest is required" ;
    vivo:courseCredits 4 ;
    vivo:hasSubjectArea "MECH" .

roboprof_data:MECH_6511 a vivo:Course ;
    dbo:name "Mechanical Forming of Metals" ;
    dbo:number 6511 ;
    dcterms:description "A project on current research topics and selected applications is required" ;
    vivo:courseCredits 4 ;
    vivo:hasSubjectArea "MECH" .

roboprof_data:MECH_6521 a vivo:Course ;
    dbo:name "Manufacturing of Composites" ;
    dbo:number 6521 ;
    dcterms:description "A project on selected topics of current interest is required" ;
    vivo:courseCredits 3 ;
    vivo:hasSubjectArea "MECH" .

roboprof_data:MECH_6531 a vivo:Course ;
    dbo:name "Casting" ;
    dbo:number 6531 ;
    dcterms:description "A project on current research topic and selected applications is required" ;
    vivo:courseCredits 3 ;
    vivo:hasSubjectArea "MECH" .

roboprof_data:MECH_6541 a vivo:Course ;
    dbo:name "Joining Processes and Nondestructive Testing" ;
    dbo:number 6541 ;
    dcterms:description "A project on current research topic or selected applications is required" ;
    vivo:courseCredits 4 ;
    vivo:hasSubjectArea "MECH" .

roboprof_data:MECH_6551 a vivo:Course ;
    dbo:name "Fracture" ;
    dbo:number 6551 ;
    dcterms:description "A project on current research topics and selected applications is required" ;
    vivo:courseCredits 3 ;
    vivo:hasSubjectArea "MECH" .

roboprof_data:MECH_6561 a vivo:Course ;
    dbo:name "High Strength Materials" ;
    dbo:number 6561 ;
    dcterms:description "A project on current research topics and selected applications is required" ;
    vivo:courseCredits 3 ;
    vivo:hasSubjectArea "MECH" .

roboprof_data:MECH_6571 a vivo:Course ;
    dbo:name "Corrosion and Oxidation of Metals" ;
    dbo:number 6571 ;
    dcterms:description "A project on current research topics and selected applications is required" ;
    vivo:courseCredits 4 ;
    vivo:hasSubjectArea "MECH" .

roboprof_data:MECH_6581 a vivo:Course ;
    dbo:name "Mechanical Behaviour of Polymer Composite Materials" ;
    dbo:number 6581 ;
    dcterms:description "Projects on selected applications are required" ;
    vivo:courseCredits 3 ;
    vivo:hasSubjectArea "MECH" .

roboprof_data:MECH_6601 a vivo:Course ;
    dbo:name "Testing and Evaluation of Polymer Composite Materials and Structures" ;
    dbo:number 6601 ;
    dcterms:description "A project on selected topics of current interest is required" ;
    vivo:courseCredits 3 ;
    vivo:hasSubjectArea "MECH" .

roboprof_data:MECH_6611 a vivo:Course ;
    dbo:name "Numerically Controlled Machines" ;
    dbo:number 6611 ;
    dcterms:description "A design project on multi-surface machine parts is required" ;
    vivo:courseCredits 4 ;
    vivo:hasSubjectArea "MECH" .

roboprof_data:MECH_6621 a vivo:Course ;
    dbo:name "Microprocessors and Applications" ;
    dbo:number 6621 ;
    dcterms:description "A project on specific topic or applications is required" ;
    vivo:courseCredits 3 ;
    vivo:hasSubjectArea "MECH" .

roboprof_data:MECH_6631 a vivo:Course ;
    dbo:name "Industrial Automation" ;
    dbo:number 6631 ;
    dcterms:description "A project on specific topic or applications is required" ;
    vivo:courseCredits 3 ;
    vivo:hasSubjectArea "MECH" .

roboprof_data:MECH_6641 a vivo:Course ;
    dbo:name "Engineering Fracture Mechanics and Fatigue" ;
    dbo:number 6641 ;
    dcterms:description "A case study or project on selected applications is required" ;
    vivo:courseCredits 3 ;
    vivo:hasSubjectArea "MECH" .

roboprof_data:MECH_6651 a vivo:Course ;
    dbo:name "Structural Composite" ;
    dbo:number 6651 ;
    dcterms:description "A project on selected applications is required" ;
    vivo:courseCredits 4 ;
    vivo:hasSubjectArea "MECH" .

roboprof_data:MECH_6661 a vivo:Course ;
    dbo:name "Thermodynamics and Phase Equilibria of Materials" ;
    dbo:number 6661 ;
    dcterms:description "A project is required" ;
    vivo:courseCredits 4 ;
    vivo:hasSubjectArea "MECH" .

roboprof_data:MECH_6671 a vivo:Course ;
    dbo:name "Finite Element Method in Machine Design" ;
    dbo:number 6671 ;
    dcterms:description "A case study or project on selected applications is required" ;
    vivo:courseCredits 3 ;
    vivo:hasSubjectArea "MECH" .

roboprof_data:MECH_6681 a vivo:Course ;
    dbo:name "Dynamics and Control of Nonholonomic Systems" ;
    dbo:number 6681 ;
    dcterms:description "A project is required" ;
    vivo:courseCredits 4 ;
    vivo:hasSubjectArea "MECH" .

roboprof_data:MECH_6691 a vivo:Course ;
    dbo:name "Optical Microsystems" ;
    dbo:number 6691 ;
    dcterms:description "A project is required" ;
    vivo:courseCredits 4 ;
    vivo:hasSubjectArea "MECH" .

roboprof_data:MECH_6741 a vivo:Course ;
    dbo:name "Mechatronics" ;
    dbo:number 6741 ;
    dcterms:description "A project is required" ;
    vivo:courseCredits 4 ;
    vivo:hasSubjectArea "MECH" .

roboprof_data:MECH_6751 a vivo:Course ;
    dbo:name "Vehicle Dynamics" ;
    dbo:number 6751 ;
    dcterms:description "A project on research topics is required" ;
    vivo:courseCredits 4 ;
    vivo:hasSubjectArea "MECH" .

roboprof_data:MECH_6761 a vivo:Course ;
    dbo:name "Vehicular Internal Combustion Engines" ;
    dbo:number 6761 ;
    dcterms:description "Modelling, Simulation, Demonstration in lab" ;
    vivo:courseCredits 4 ;
    vivo:hasSubjectArea "MECH" .

roboprof_data:MECH_6771 a vivo:Course ;
    dbo:name "Driverless Ground Vehicles" ;
    dbo:number 6771 ;
    dcterms:description "A project on selected topics is required" ;
    vivo:courseCredits 3 ;
    vivo:hasSubjectArea "MECH" .

roboprof_data:MECH_6781 a vivo:Course ;
    dbo:name "Guided Vehicle Systems" ;
    dbo:number 6781 ;
    dcterms:description "A project on selected topics is an integral part of the course" ;
    vivo:courseCredits 3 ;
    vivo:hasSubjectArea "MECH" .

roboprof_data:MECH_7011 a vivo:Course ;
    dbo:name "Dynamics of Hydraulic Control Systems" ;
    dbo:number 7011 ;
    dcterms:description "Projects on selected topics are required" ;
    vivo:courseCredits 4 ;
    vivo:hasSubjectArea "MECH" .

roboprof_data:MECH_7101 a vivo:Course ;
    dbo:name "Convection Heat Transfer" ;
    dbo:number 7101 ;
    dcterms:description "Project or term paper required" ;
    vivo:courseCredits 3 ;
    vivo:hasSubjectArea "MECH" .

roboprof_data:MECH_7501 a vivo:Course ;
    dbo:name "Design Using Composite Materials" ;
    dbo:number 7501 ;
    dcterms:description "A project on selected topics is required" ;
    vivo:courseCredits 4 ;
    vivo:hasSubjectArea "MECH" .

roboprof_data:MECH_7511 a vivo:Course ;
    dbo:name "Vehicle Vibration and Control" ;
    dbo:number 7511 ;
    dcterms:description "Projects on selected applications are required" ;
    vivo:courseCredits 3 ;
    vivo:hasSubjectArea "MECH" .

roboprof_data:MECH_7711 a vivo:Course ;
    dbo:name "Handling and Stability of Road Vehicles" ;
    dbo:number 7711 ;
    dcterms:description "Project on selected topics is an integral part of the course" ;
    vivo:courseCredits 3 ;
    vivo:hasSubjectArea "MECH" .

roboprof_data:MHIS_203 a vivo:Course ;
    dbo:name "MUSIC HISTORY TO 1800" ;
    dbo:number 203 ;
    dcterms:description "NaN"^^xsd:double ;
    vivo:courseCredits 3 ;
    vivo:hasSubjectArea "MHIS" .

roboprof_data:MPER_231 a vivo:Course ;
    dbo:name "Choir I" ;
    dbo:number 231 ;
    dcterms:description "Choir" ;
    vivo:courseCredits 4 ;
    vivo:hasSubjectArea "MPER" .

roboprof_data:MPER_321 a vivo:Course ;
    dbo:name "Chamber Ensemble I" ;
    dbo:number 321 ;
    dcterms:description "Public performance" ;
    vivo:courseCredits 3 ;
    vivo:hasSubjectArea "MPER" .

roboprof_data:MPER_322 a vivo:Course ;
    dbo:name "Chamber Ensemble II" ;
    dbo:number 322 ;
    dcterms:description "Public performance" ;
    vivo:courseCredits 4 ;
    vivo:hasSubjectArea "MPER" .

roboprof_data:MPER_332 a vivo:Course ;
    dbo:name "Choir II" ;
    dbo:number 332 ;
    dcterms:description "Choir" ;
    vivo:courseCredits 4 ;
    vivo:hasSubjectArea "MPER" .

roboprof_data:MPER_421 a vivo:Course ;
    dbo:name "Chamber Ensemble III" ;
    dbo:number 421 ;
    dcterms:description "Public performance" ;
    vivo:courseCredits 4 ;
    vivo:hasSubjectArea "MPER" .

roboprof_data:MPER_422 a vivo:Course ;
    dbo:name "Chamber Ensemble IV" ;
    dbo:number 422 ;
    dcterms:description "Public performance" ;
    vivo:courseCredits 4 ;
    vivo:hasSubjectArea "MPER" .

roboprof_data:MPER_451 a vivo:Course ;
    dbo:name "PRIVATE STUDY V" ;
    dbo:number 451 ;
    dcterms:description "NaN"^^xsd:double ;
    vivo:courseCredits 4 ;
    vivo:hasSubjectArea "MPER" .

roboprof_data:MSCA_602 a vivo:Course ;
    dbo:name "Applied Linear Statistical Models" ;
    dbo:number 602 ;
    dcterms:description "Case studies" ;
    vivo:courseCredits 4 ;
    vivo:hasSubjectArea "MSCA" .

roboprof_data:MSCA_611 a vivo:Course ;
    dbo:name "Research Methodology" ;
    dbo:number 611 ;
    dcterms:description "Research paper presentation and a separate research paper" ;
    vivo:courseCredits 3 ;
    vivo:hasSubjectArea "MSCA" .

roboprof_data:MSCA_625 a vivo:Course ;
    dbo:name "Seminar in Options and Futures" ;
    dbo:number 625 ;
    dcterms:description "Research proposal presentation" ;
    vivo:courseCredits 4 ;
    vivo:hasSubjectArea "MSCA" .

roboprof_data:MSCA_632 a vivo:Course ;
    dbo:name "Seminar in Special Topics in Finance" ;
    dbo:number 632 ;
    dcterms:description "Research paper and presentation" ;
    vivo:courseCredits 3 ;
    vivo:hasSubjectArea "MSCA" .

roboprof_data:MSCA_654 a vivo:Course ;
    dbo:name "Seminar in Consulting" ;
    dbo:number 654 ;
    dcterms:description "Team assignment with client firm" ;
    vivo:courseCredits 3 ;
    vivo:hasSubjectArea "MSCA" .

roboprof_data:MUSI_201 a vivo:Course ;
    dbo:name "INTRODUCTION TO MUSIC FUNDAMEN" ;
    dbo:number 201 ;
    dcterms:description "NaN"^^xsd:double ;
    vivo:courseCredits 3 ;
    vivo:hasSubjectArea "MUSI" .

roboprof_data:MUSI_481 a vivo:Course ;
    dbo:name "Supervised Internship I" ;
    dbo:number 481 ;
    dcterms:description "Supervised internship at an industry/community partner" ;
    vivo:courseCredits 3 ;
    vivo:hasSubjectArea "MUSI " .

roboprof_data:MUSI_482 a vivo:Course ;
    dbo:name "Supervised Internship II" ;
    dbo:number 482 ;
    dcterms:description "Supervised internship at an industry/community partner" ;
    vivo:courseCredits 4 ;
    vivo:hasSubjectArea "MUSI " .

roboprof_data:PERC_209 a vivo:Course ;
    dbo:name "The Engaged Theatre Artist" ;
    dbo:number 209 ;
    dcterms:description "Students explore basic skills and principles of performance creation and acting for the theatre" ;
    vivo:courseCredits 4 ;
    vivo:hasSubjectArea "PERC" .

roboprof_data:PERC_210 a vivo:Course ;
    dbo:name "Performance Creation Studio 1: Theory and Method" ;
    dbo:number 210 ;
    dcterms:description "Students study a wide range of theories and techniques for creating socially engaged, collaborative and community-based performance works." ;
    vivo:courseCredits 3 ;
    vivo:hasSubjectArea "PERC" .

roboprof_data:PERC_211 a vivo:Course ;
    dbo:name "Theatre in the City" ;
    dbo:number 211 ;
    dcterms:description "Students encounter the challenges of a small production project in collaboration with other students" ;
    vivo:courseCredits 4 ;
    vivo:hasSubjectArea "PERC" .

roboprof_data:PERC_212 a vivo:Course ;
    dbo:name "Introduction to Dramaturgy" ;
    dbo:number 212 ;
    dcterms:description "Course emphasis is on script analysis including elements such as structure, semiotics, genre, and style" ;
    vivo:courseCredits 4 ;
    vivo:hasSubjectArea "PERC" .

roboprof_data:PERC_298 a vivo:Course ;
    dbo:name "Special Topics in Performance Creation" ;
    dbo:number 298 ;
    dcterms:description "The study of specialized aspects of performance creation" ;
    vivo:courseCredits 3 ;
    vivo:hasSubjectArea "PERC" .

roboprof_data:PERC_311 a vivo:Course ;
    dbo:name "Directing 1" ;
    dbo:number 311 ;
    dcterms:description "Students learn basic organizational, analytical, and leadership skills for stage direction." ;
    vivo:courseCredits 4 ;
    vivo:hasSubjectArea "PERC" .

roboprof_data:PERC_318 a vivo:Course ;
    dbo:name "Playwriting 1" ;
    dbo:number 318 ;
    dcterms:description "Course focuses on building skills in writing for the stage" ;
    vivo:courseCredits 4 ;
    vivo:hasSubjectArea "PERC" .

roboprof_data:PERC_321 a vivo:Course ;
    dbo:name "Introduction to Performance Studies" ;
    dbo:number 321 ;
    dcterms:description "Course investigates a broad range of sites and practices from the realms of theatre, dance, and other cultural forms" ;
    vivo:courseCredits 4 ;
    vivo:hasSubjectArea "PERC" .

roboprof_data:PERC_322 a vivo:Course ;
    dbo:name "Gender and Sexuality in Performance" ;
    dbo:number 322 ;
    dcterms:description "Course provides a grounding in feminist and queer theory as critical tools for the analysis and creation of performance." ;
    vivo:courseCredits 4 ;
    vivo:hasSubjectArea "PERC" .

roboprof_data:PERC_324 a vivo:Course ;
    dbo:name "Queer Theatre and Performance" ;
    dbo:number 324 ;
    dcterms:description "Course examines how the stage has been, and continues to be, a necessary public forum for queer political activism and identity politics" ;
    vivo:courseCredits 4 ;
    vivo:hasSubjectArea "PERC" .

roboprof_data:PERC_351 a vivo:Course ;
    dbo:name "Community Arts: The Art of Engagement" ;
    dbo:number 351 ;
    dcterms:description "Course includes practical explorations of various approaches to creating socially engaged theatre and performance." ;
    vivo:courseCredits 3 ;
    vivo:hasSubjectArea "PERC" .

roboprof_data:PERC_356 a vivo:Course ;
    dbo:name "Puppetry and Performing Object Workshop" ;
    dbo:number 356 ;
    dcterms:description "Course combines building, basic manipulation, and showmaking techniques" ;
    vivo:courseCredits 4 ;
    vivo:hasSubjectArea "PERC" .

roboprof_data:PERC_384 a vivo:Course ;
    dbo:name "Performance Creation Studio 11: Collaborative Practice" ;
    dbo:number 384 ;
    dcterms:description "Students generate and rehearse original material inspired by current events" ;
    vivo:courseCredits 4 ;
    vivo:hasSubjectArea "PERC" .

roboprof_data:PERC_386 a vivo:Course ;
    dbo:name "Site-specific Performance Practice" ;
    dbo:number 386 ;
    dcterms:description "Introduces students to interdisciplinary methods for developing solo or collaborative sitespecific works" ;
    vivo:courseCredits 3 ;
    vivo:hasSubjectArea "PERC" .

roboprof_data:PERC_398 a vivo:Course ;
    dbo:name "Special Topics in Performance Creation" ;
    dbo:number 398 ;
    dcterms:description "A seminar course exploring a topic in performance creation" ;
    vivo:courseCredits 3 ;
    vivo:hasSubjectArea "PERC" .

roboprof_data:PERC_399 a vivo:Course ;
    dbo:name "Special Topics in Performance Creation" ;
    dbo:number 399 ;
    dcterms:description "A seminar or studio course exploring a topic in performance creation" ;
    vivo:courseCredits 4 ;
    vivo:hasSubjectArea "PERC" .

roboprof_data:PERC_405 a vivo:Course ;
    dbo:name "Independent Study I" ;
    dbo:number 405 ;
    dcterms:description "Studentproposed research project supervised by a fulltime faculty member." ;
    vivo:courseCredits 4 ;
    vivo:hasSubjectArea "PERC" .

roboprof_data:PERC_408 a vivo:Course ;
    dbo:name "Supervised Internship I" ;
    dbo:number 408 ;
    dcterms:description "Course provides students with the opportunity to obtain credit for work completed for a recognized theatre company" ;
    vivo:courseCredits 4 ;
    vivo:hasSubjectArea "PERC" .

roboprof_data:PERC_409 a vivo:Course ;
    dbo:name "Supervised Internship II" ;
    dbo:number 409 ;
    dcterms:description "Course provides students with the opportunity to obtain credit for work completed for a recognized theatre company" ;
    vivo:courseCredits 4 ;
    vivo:hasSubjectArea "PERC" .

roboprof_data:PERC_415 a vivo:Course ;
    dbo:name "Independent Study II" ;
    dbo:number 415 ;
    dcterms:description "Studentproposed research project supervised by a fulltime faculty member." ;
    vivo:courseCredits 4 ;
    vivo:hasSubjectArea "PERC" .

roboprof_data:PERC_421 a vivo:Course ;
    dbo:name "Socially Engaged and Cctivist  Performance" ;
    dbo:number 421 ;
    dcterms:description "Theory and practice of approaches and genres selected from community arts, oral history performance, street theatre, performance art, and political theatre" ;
    vivo:courseCredits 4 ;
    vivo:hasSubjectArea "PERC" .

roboprof_data:PERC_422 a vivo:Course ;
    dbo:name "Indigenous Story Telling" ;
    dbo:number 422 ;
    dcterms:description "Studio course introduces students to foundational Indigenous stories as an exploration into worldview and philosophy, utilizing a variety of Indigenous performance methods" ;
    vivo:courseCredits 4 ;
    vivo:hasSubjectArea "PERC" .

roboprof_data:PERC_462 a vivo:Course ;
    dbo:name "Playwriting II" ;
    dbo:number 462 ;
    dcterms:description "Students work on an original performance text to be developed through a workshop process" ;
    vivo:courseCredits 3 ;
    vivo:hasSubjectArea "PERC" .

roboprof_data:PERC_464 a vivo:Course ;
    dbo:name "Oral History performance" ;
    dbo:number 464 ;
    dcterms:description "Hybrid seminarstudio course explores key ethical, dramaturgical, and performative dimensions of the emergent field of oral history performance" ;
    vivo:courseCredits 4 ;
    vivo:hasSubjectArea "PERC" .

roboprof_data:PERC_471 a vivo:Course ;
    dbo:name "Directing II" ;
    dbo:number 471 ;
    dcterms:description "Assignment involves directing a short work" ;
    vivo:courseCredits 3 ;
    vivo:hasSubjectArea "PERC" .

roboprof_data:PERC_488 a vivo:Course ;
    dbo:name "Short Works Festival" ;
    dbo:number 488 ;
    dcterms:description "Explores methods for conceiving and creating a new theatre work in relation to contemporary topics and/ or subject matter" ;
    vivo:courseCredits 4 ;
    vivo:hasSubjectArea "PERC" .

roboprof_data:PERC_490 a vivo:Course ;
    dbo:name "Performance Creation Mainstage" ;
    dbo:number 490 ;
    dcterms:description "Students working in ensemble on all aspects of the study and production of an existing theatre script, or the creation and production of an original piece of theatre" ;
    vivo:courseCredits 3 ;
    vivo:hasSubjectArea "PERC" .

roboprof_data:PERC_496 a vivo:Course ;
    dbo:name "Performance Creation Field School" ;
    dbo:number 496 ;
    dcterms:description "Experiential learning in performance creation or performance studies via faculty-led travel to and residency at a festival, conference, exhibition or partner institution" ;
    vivo:courseCredits 4 ;
    vivo:hasSubjectArea "PERC" .

roboprof_data:PERC_498 a vivo:Course ;
    dbo:name "Special Topics in Performance Creation" ;
    dbo:number 498 ;
    dcterms:description "A studio course exploring a topic in performance creation" ;
    vivo:courseCredits 3 ;
    vivo:hasSubjectArea "PERC" .

roboprof_data:PERC_499 a vivo:Course ;
    dbo:name "Special Topics in Performance Creation" ;
    dbo:number 499 ;
    dcterms:description "A seminar or studio course exploring a topic in performance creation" ;
    vivo:courseCredits 4 ;
    vivo:hasSubjectArea "PERC" .

roboprof_data:PHIL_214 a vivo:Course ;
    dbo:name "Deductive Logic" ;
    dbo:number 214 ;
    dcterms:description "This course presents the modern symbolic systems of sentential and predicate logic. Students transcribe English sentences into a logical form, analyze the concepts of logical truth, consistency, and validity, as well as learn to construct derivations in each system." ;
    vivo:courseCredits 3 ;
    vivo:hasSubjectArea "PHIL" .

roboprof_data:PHIL_220 a vivo:Course ;
    dbo:name "Introduction to the Philosophy of Science" ;
    dbo:number 220 ;
    dcterms:description "This course provides an introduction to the main problems in the philosophy of science. These include the structure of scientific theories, various models of scientific method and explanation, and the existence of unobservables." ;
    vivo:courseCredits 3 ;
    vivo:hasSubjectArea "PHIL" .

roboprof_data:PHIL_232 a vivo:Course ;
    dbo:name "Introduction to Ethics" ;
    dbo:number 232 ;
    dcterms:description "In this course, students are introduced to some representative approaches to ethical thought and action." ;
    vivo:courseCredits 3 ;
    vivo:hasSubjectArea "PHIL" .

roboprof_data:PHIL_260 a vivo:Course ;
    dbo:name "Presocratics and Plato" ;
    dbo:number 260 ;
    dcterms:description "This course is a study of ancient Greek philosophy from its beginnings to Plato." ;
    vivo:courseCredits 4 ;
    vivo:hasSubjectArea "PHIL" .

roboprof_data:PHIL_261 a vivo:Course ;
    dbo:name "Aristotle and Hellenistic Philosophy" ;
    dbo:number 261 ;
    dcterms:description "This course is an introduction to Aristotle and the main lines of thought in Hellenistic philosophy, including Stoicism, Epicureanism and Scepticism." ;
    vivo:courseCredits 3 ;
    vivo:hasSubjectArea "PHIL" .

roboprof_data:PHIL_263 a vivo:Course ;
    dbo:name "Introduction to Epistemology" ;
    dbo:number 263 ;
    dcterms:description "An introduction to the basic concepts and problems in epistemology, including belief, knowledge, scepticism, perception, and intentionality." ;
    vivo:courseCredits 4 ;
    vivo:hasSubjectArea "PHIL" .

roboprof_data:PHIL_265 a vivo:Course ;
    dbo:name "Introduction to Metaphysics" ;
    dbo:number 265 ;
    dcterms:description "This course is an introduction to metaphysics and the attempt to understand a mindindependent reality." ;
    vivo:courseCredits 4 ;
    vivo:hasSubjectArea "PHIL" .

roboprof_data:PHIL_495 a vivo:Course ;
    dbo:name "Honours Essay" ;
    dbo:number 495 ;
    dcterms:description "An honours student may arrange a tutorial program with a faculty member culminating in a research project not exceeding 40 pages." ;
    vivo:courseCredits 4 ;
    vivo:hasSubjectArea "PHIL" .

roboprof_data:PHIL_496 a vivo:Course ;
    dbo:name "Tutorial in Philosophy" ;
    dbo:number 496 ;
    dcterms:description "Personal intensive reading and research program under the supervision of a faculty member." ;
    vivo:courseCredits 4 ;
    vivo:hasSubjectArea "PHIL" .

roboprof_data:PHIL_497 a vivo:Course ;
    dbo:name "Tutorial in Philosophy" ;
    dbo:number 497 ;
    dcterms:description "Personal intensive reading and research program under the supervision of a faculty member." ;
    vivo:courseCredits 4 ;
    vivo:hasSubjectArea "PHIL" .

roboprof_data:PHOT_201 a vivo:Course ;
    dbo:name "INTRO TO COLOUR PHOTOGRAPHY",
        "Introduction to Colour Photography" ;
    dbo:number 201 ;
    dcterms:description "NaN"^^xsd:double,
        "This introductory-level course covers fundamental techniques specific to colour photography including basic camera functions, film exposure, and printing." ;
    vivo:courseCredits 3,
        4 ;
    vivo:hasSubjectArea "PHOT" .

roboprof_data:PHOT_210 a vivo:Course ;
    dbo:name "Foundations in Photographic Vision Theory and Practice I" ;
    dbo:number 210 ;
    dcterms:description "In this course, students investigate and examine the numerous aspects of photographys complex history, aesthetics, and processes, as well as different camera and darkroom techniques specific to colour photography. " ;
    vivo:courseCredits 4 ;
    vivo:hasSubjectArea "PHOT" .

roboprof_data:PHOT_221 a vivo:Course ;
    dbo:name "Colour Photography I" ;
    dbo:number 221 ;
    dcterms:description "In this course, students become aware of how colour contributes to the structure and meaning of photographs." ;
    vivo:courseCredits 3 ;
    vivo:hasSubjectArea "PHOT" .

roboprof_data:PHOT_300 a vivo:Course ;
    dbo:name "Photographic Vision: Theory and Practice II" ;
    dbo:number 300 ;
    dcterms:description "The purpose of this studio course is to provide a framework within which students pursue their photographic practice at an intermediate level." ;
    vivo:courseCredits 4 ;
    vivo:hasSubjectArea "PHOT" .

roboprof_data:PHOT_311 a vivo:Course ;
    dbo:name "Large Format Photography I" ;
    dbo:number 311 ;
    dcterms:description "A studio course introducing large format photography, its techniques and application. Demonstrations cover the basics of view camera operation, light metering, sheet film exposure, development, and advanced printing." ;
    vivo:courseCredits 3 ;
    vivo:hasSubjectArea "PHOT" .

roboprof_data:PHOT_312 a vivo:Course ;
    dbo:name "Large Format Photography II" ;
    dbo:number 312 ;
    dcterms:description "A studio course directed towards the development of an individual approach to view camera photography. " ;
    vivo:courseCredits 4 ;
    vivo:hasSubjectArea "PHOT" .

roboprof_data:PHOT_322 a vivo:Course ;
    dbo:name "Colour Photography II" ;
    dbo:number 322 ;
    dcterms:description "A continuation of PHOT 221 , this course explores further techniques in colour photography and advanced colour printing." ;
    vivo:courseCredits 3 ;
    vivo:hasSubjectArea "PHOT" .

roboprof_data:PHOT_331 a vivo:Course ;
    dbo:name "Digital Photography I" ;
    dbo:number 331 ;
    dcterms:description "An introductory studio course investigating the technical and creative aspects of digital photography. " ;
    vivo:courseCredits 4 ;
    vivo:hasSubjectArea "PHOT" .

roboprof_data:PHOT_332 a vivo:Course ;
    dbo:name "Digital Photography II" ;
    dbo:number 332 ;
    dcterms:description "This advanced course expands on the basic control skills and creative aspects of digital technology by implementing personal approaches to the use of technology." ;
    vivo:courseCredits 4 ;
    vivo:hasSubjectArea "PHOT" .

roboprof_data:PHOT_398 a vivo:Course ;
    dbo:name "Special Topics in Photography" ;
    dbo:number 398 ;
    dcterms:description "An opportunity for the study of limited and more specialized aspects of photography." ;
    vivo:courseCredits 4 ;
    vivo:hasSubjectArea "PHOT" .

roboprof_data:PHOT_399 a vivo:Course ;
    dbo:name "Special Topics in Photography" ;
    dbo:number 399 ;
    dcterms:description "An opportunity for the study of limited and more specialized aspects of photography." ;
    vivo:courseCredits 3 ;
    vivo:hasSubjectArea "PHOT" .

roboprof_data:PHOT_400 a vivo:Course ;
    dbo:name "Advanced Workshop in Photography" ;
    dbo:number 400 ;
    dcterms:description "A studio course in which students pursue one or more extended photographic projects in black and white and/or digital." ;
    vivo:courseCredits 3 ;
    vivo:hasSubjectArea "PHOT" .

roboprof_data:PHOT_470 a vivo:Course ;
    dbo:name "Professional Internship" ;
    dbo:number 470 ;
    dcterms:description "A student wishing to work in an apprentice capacity with an established photographic artist, or wishing to pursue research in photographic criticism, museum work, publication, or other related endeavours may apply for academic credit. " ;
    vivo:courseCredits 3 ;
    vivo:hasSubjectArea "PHOT" .

roboprof_data:PHOT_471 a vivo:Course ;
    dbo:name "Professional Internship I" ;
    dbo:number 471 ;
    dcterms:description "A student wishing to work in an apprentice capacity with an established photographic artist, or wishing to pursue research in photographic criticism, museum work, publication, or other related endeavours may apply for academic credit. " ;
    vivo:courseCredits 3 ;
    vivo:hasSubjectArea "PHOT" .

roboprof_data:PHOT_472 a vivo:Course ;
    dbo:name "Professional Internship II" ;
    dbo:number 472 ;
    dcterms:description "Students who wish additional internships in a professional milieu may take this course." ;
    vivo:courseCredits 3 ;
    vivo:hasSubjectArea "PHOT" .

roboprof_data:PHOT_480 a vivo:Course ;
    dbo:name "Independent Study" ;
    dbo:number 480 ;
    dcterms:description "This course provides a limited number of students the opportunity to pursue advanced studies in photography under the supervision of a fulltime photography faculty member." ;
    vivo:courseCredits 3 ;
    vivo:hasSubjectArea "PHOT" .

roboprof_data:PHOT_481 a vivo:Course ;
    dbo:name "Independent Study I " ;
    dbo:number 481 ;
    dcterms:description "This course provides a limited number of students the opportunity to pursue advanced studies in photography under the supervision of a fulltime photography faculty member." ;
    vivo:courseCredits 3 ;
    vivo:hasSubjectArea "PHOT" .

roboprof_data:PHOT_482 a vivo:Course ;
    dbo:name "Independent Study II" ;
    dbo:number 482 ;
    dcterms:description "This course provides a limited number of students the opportunity to pursue advanced studies in photography under the supervision of a fulltime photography faculty member." ;
    vivo:courseCredits 3 ;
    vivo:hasSubjectArea "PHOT" .

roboprof_data:PHOT_498 a vivo:Course ;
    dbo:name "Special Topics in Photography" ;
    dbo:number 498 ;
    dcterms:description "A course for advanced students which provides an opportunity for the study of limited and more specialized aspects of photography." ;
    vivo:courseCredits 3 ;
    vivo:hasSubjectArea "PHOT" .

roboprof_data:PHOT_499 a vivo:Course ;
    dbo:name "Special Topics in Photography" ;
    dbo:number 499 ;
    dcterms:description "A course for advanced students which provides an opportunity for the study of limited and more specialized aspects of photography." ;
    vivo:courseCredits 3 ;
    vivo:hasSubjectArea "PHOT" .

roboprof_data:PHYS_224 a vivo:Course ;
    dbo:name "Introductory Experimental Mechanics" ;
    dbo:number 224 ;
    dcterms:description "Experiment, lab" ;
    vivo:courseCredits 3 ;
    vivo:hasSubjectArea "PHYS" .

roboprof_data:PHYS_225 a vivo:Course ;
    dbo:name "Introductory Experimental Electricity" ;
    dbo:number 225 ;
    dcterms:description "Experiment, lab" ;
    vivo:courseCredits 4 ;
    vivo:hasSubjectArea "PHYS" .

roboprof_data:PHYS_226 a vivo:Course ;
    dbo:name "Introductory Experimental Waves and Modern Physics" ;
    dbo:number 226 ;
    dcterms:description "Experiment, lab" ;
    vivo:courseCredits 3 ;
    vivo:hasSubjectArea "PHYS" .

roboprof_data:PHYS_230 a vivo:Course ;
    dbo:name "Experimental Physics I" ;
    dbo:number 230 ;
    dcterms:description "Experiment, lab" ;
    vivo:courseCredits 3 ;
    vivo:hasSubjectArea "PHYS" .

roboprof_data:PHYS_236 a vivo:Course ;
    dbo:name "Numerical Methods in Physics with Python" ;
    dbo:number 236 ;
    dcterms:description "includes Programming project" ;
    vivo:courseCredits 4 ;
    vivo:hasSubjectArea "PHYS" .

roboprof_data:PHYS_289 a vivo:Course ;
    dbo:name "Honours Research Experience I" ;
    dbo:number 289 ;
    dcterms:description "Research Project" ;
    vivo:courseCredits 4 ;
    vivo:hasSubjectArea "PHYS" .

roboprof_data:PHYS_295 a vivo:Course ;
    dbo:name "Experimental Electronics I" ;
    dbo:number 295 ;
    dcterms:description "Experiments, practical laboratory course" ;
    vivo:courseCredits 3 ;
    vivo:hasSubjectArea "PHYS" .

roboprof_data:PHYS_330 a vivo:Course ;
    dbo:name "Experimental Physics II" ;
    dbo:number 330 ;
    dcterms:description "Experiment, lab" ;
    vivo:courseCredits 3 ;
    vivo:hasSubjectArea "PHYS" .

roboprof_data:PHYS_389 a vivo:Course ;
    dbo:name "Honours Research Experience II" ;
    dbo:number 389 ;
    dcterms:description "Research Project" ;
    vivo:courseCredits 4 ;
    vivo:hasSubjectArea "PHYS" .

roboprof_data:PHYS_390 a vivo:Course ;
    dbo:name "Electronics" ;
    dbo:number 390 ;
    dcterms:description "Experiment, lab" ;
    vivo:courseCredits 3 ;
    vivo:hasSubjectArea "PHYS" .

roboprof_data:PHYS_440 a vivo:Course ;
    dbo:name "Computational Methods in Physics with Python" ;
    dbo:number 440 ;
    dcterms:description "includes Programming project" ;
    vivo:courseCredits 3 ;
    vivo:hasSubjectArea "PHYS" .

roboprof_data:PHYS_496 a vivo:Course ;
    dbo:name "Honours Research Project (6 cr)" ;
    dbo:number 496 ;
    dcterms:description "Final Year Research Project" ;
    vivo:courseCredits 4 ;
    vivo:hasSubjectArea "PHYS" .

roboprof_data:PHYS_497 a vivo:Course ;
    dbo:name "Specialization Research Project (3 cr)" ;
    dbo:number 497 ;
    dcterms:description "Final Year Research Project" ;
    vivo:courseCredits 3 ;
    vivo:hasSubjectArea "PHYS" .

roboprof_data:PHYS_637 a vivo:Course ;
    dbo:name "Condensed Matter Physics II" ;
    dbo:number 637 ;
    dcterms:description "includes Individual project" ;
    vivo:courseCredits 3 ;
    vivo:hasSubjectArea "PHYS" .

roboprof_data:PHYS_660 a vivo:Course ;
    dbo:name "Chemical Aspects of Biophysics" ;
    dbo:number 660 ;
    dcterms:description "includes Individual project" ;
    vivo:courseCredits 4 ;
    vivo:hasSubjectArea "PHYS" .

roboprof_data:PHYS_663 a vivo:Course ;
    dbo:name "Quantitative Human Systems Physiology" ;
    dbo:number 663 ;
    dcterms:description "includes Individual project" ;
    vivo:courseCredits 3 ;
    vivo:hasSubjectArea "PHYS" .

roboprof_data:PHYS_665 a vivo:Course ;
    dbo:name "Principles of Medical Imaging" ;
    dbo:number 665 ;
    dcterms:description "includes Individual project" ;
    vivo:courseCredits 3 ;
    vivo:hasSubjectArea "PHYS" .

roboprof_data:PHYS_760 a vivo:Course ;
    dbo:name "MSc Seminar on Selected Topics" ;
    dbo:number 760 ;
    dcterms:description "includes workshops" ;
    vivo:courseCredits 3 ;
    vivo:hasSubjectArea "PHYS" .

roboprof_data:PHYS_862 a vivo:Course ;
    dbo:name "Doctoral Seminar on Selected Topics II" ;
    dbo:number 862 ;
    dcterms:description "includes workshops" ;
    vivo:courseCredits 4 ;
    vivo:hasSubjectArea "PHYS" .

roboprof_data:POLI_205 a vivo:Course ;
    dbo:name "Introduction to International Relations" ;
    dbo:number 205 ;
    dcterms:description "This course introduces the principal theories, concepts, and debates in the contemporary study of international relations. It provides an overview of issues in international security, international political economy and global governance." ;
    vivo:courseCredits 4 ;
    vivo:hasSubjectArea "POLI " .

roboprof_data:POLI_214 a vivo:Course ;
    dbo:name "Human Rights: An Overview" ;
    dbo:number 214 ;
    dcterms:description "This course introduces students to the historical origins of the concept of human rights; the international regime and the acceptance of several generations of rights such as civil and political rights, economic rights, group rights, and womens rights; the critiques of universalism and the problems of implementation of human rights." ;
    vivo:courseCredits 4 ;
    vivo:hasSubjectArea "POLI" .

roboprof_data:POLI_300 a vivo:Course ;
    dbo:name "NotforProfit Organizations and the Law" ;
    dbo:number 300 ;
    dcterms:description "This course introduces students to the legal regimes affecting notfor profit organizations (NPO). The course covers the legal structures, rules and procedures that govern NPOs, the vast diversity of NPOs, and practical questions such as how to set up an NPO." ;
    vivo:courseCredits 3 ;
    vivo:hasSubjectArea "POLI" .

roboprof_data:POLI_315 a vivo:Course ;
    dbo:name "International Organizations" ;
    dbo:number 315 ;
    dcterms:description "This course offers an overview of international institutions and global governance. It examines major theoretical perspectives on international organizations, and addresses the role of the United Nations system, regional organizations, and nongovernmental organizations in promoting international cooperation to address collective problems." ;
    vivo:courseCredits 3 ;
    vivo:hasSubjectArea "POLI" .

roboprof_data:POLI_328 a vivo:Course ;
    dbo:name "Public Policy and the Politics of Equality" ;
    dbo:number 328 ;
    dcterms:description "This course reviews theoretical debates about the role of the state and the individual, collective and individual rights, integration, and the role of cultural diversity and identity. It examines selected policy demands of women, the poor, refugees, and other constituencies." ;
    vivo:courseCredits 4 ;
    vivo:hasSubjectArea "POLI" .

roboprof_data:POLI_392 a vivo:Course ;
    dbo:name "Approaches to Social Science Inquiry" ;
    dbo:number 392 ;
    dcterms:description "This course introduces students to a variety of approaches to social scientific inquiry, focusing on their underlying logics. The course covers variablebased research of the qualitative and quantitative variety and alternatives to this approach such as critical theory, processtracing, modelling, ethnography, interpretivist analysis, and conceptual analysis." ;
    vivo:courseCredits 4 ;
    vivo:hasSubjectArea "POLI " .

roboprof_data:POLI_397 a vivo:Course ;
    dbo:name "Internship" ;
    dbo:number 397 ;
    dcterms:description "10hrs/week for 13 weeks of relevant work with an employer who trains, supervises and coaches the intern to better understand their field of study. A research paper is graded by a Faculty member. 3 credits." ;
    vivo:courseCredits 4 ;
    vivo:hasSubjectArea "POLI" .

roboprof_data:POLI_419 a vivo:Course ;
    dbo:name "Strategic Studies" ;
    dbo:number 419 ;
    dcterms:description "Simulations" ;
    vivo:courseCredits 4 ;
    vivo:hasSubjectArea "POLI" .

roboprof_data:POLI_480 a vivo:Course ;
    dbo:name "Workshops on Social Science Research Methods" ;
    dbo:number 480 ;
    dcterms:description "The Workshops on Social Science Research (WSSR) are short, intensive learning experiences and networking opportunities that allow you to develop your critical thinking skills, make new contacts, and succeed as future decision makers." ;
    vivo:courseCredits 3 ;
    vivo:hasSubjectArea "POLI" .

roboprof_data:POLI_487 a vivo:Course ;
    dbo:name "Advanced Seminar in Comparative Politics" ;
    dbo:number 487 ;
    dcterms:description "Advanced seminars deal with selected topics in sub-fields of political science. Topics vary from year to year." ;
    vivo:courseCredits 3 ;
    vivo:hasSubjectArea "POLI" .

roboprof_data:POLI_495 a vivo:Course ;
    dbo:name "Honours Thesis" ;
    dbo:number 495 ;
    dcterms:description "NaN"^^xsd:double ;
    vivo:courseCredits 4 ;
    vivo:hasSubjectArea "POLI" .

roboprof_data:POLI_644 a vivo:Course ;
    dbo:name "Research Methods" ;
    dbo:number 644 ;
    dcterms:description "This course is intended to introduce undergraduate students to quantitative analysis in political science. Key skills in univariate, bivariate, and multivariate analysis; inferential statistics; and graphing are demonstrated using statistical software in lab exercises." ;
    vivo:courseCredits 4 ;
    vivo:hasSubjectArea "POLI" .

roboprof_data:POLI_683 a vivo:Course ;
    dbo:name "Mechanics of Briefing Notes",
        "Minding the Gap",
        "Professional Development" ;
    dbo:number 683 ;
    dcterms:description "Students choose from a number of pre-selected workshops, including soft skills, teamwork, leadership, interviewing, communications, French, and data management and analytics, professional ethics, and gender analysis which will help prepare them for their professional careers.",
        "Taught by Public Servant in Residence (current or former) students practice how to prepare and deliver information needed by high level public servants via multiple case studies provided by past and current decision-makers in the Canadian and Quebec governments.",
        "This course provides students with a thorough understanding of the development and the requirements for writing and presenting policy ideas through government communication vehicles including Question Period notes, Briefing Notes, Memorandums to Cabinet, Treasury Board Submissions, and oral and written presentations to senior management." ;
    vivo:courseCredits 3 ;
    vivo:hasSubjectArea "POLI" .

roboprof_data:POLI_693 a vivo:Course ;
    dbo:name "Internship" ;
    dbo:number 693 ;
    dcterms:description "Students complete 8 public policy stream courses; compete for and attain a relevant paid internship as policy analyst or program evaluator. They complete one 16 week full-time internship, and can extend to 32 weeks.  21 credits divided in Professional Development/Internship/Academic Report." ;
    vivo:courseCredits 3 ;
    vivo:hasSubjectArea "POLI" .

roboprof_data:PRIN_211 a vivo:Course ;
    dbo:name "Intaglio I " ;
    dbo:number 211 ;
    dcterms:description "An introductory studio course in intaglio techniques with an emphasis on creative imagery. " ;
    vivo:courseCredits 4 ;
    vivo:hasSubjectArea "PRIN" .

roboprof_data:PRIN_221 a vivo:Course ;
    dbo:name "Lithography I" ;
    dbo:number 221 ;
    dcterms:description "An introductory studio course in lithographic techniques with an emphasis on creative imagery." ;
    vivo:courseCredits 3 ;
    vivo:hasSubjectArea "PRIN" .

roboprof_data:PRIN_231 a vivo:Course ;
    dbo:name "Screen Printing I" ;
    dbo:number 231 ;
    dcterms:description "An introductory studio course in the basic techniques of screen printing with an emphasis on creative imagery." ;
    vivo:courseCredits 4 ;
    vivo:hasSubjectArea "PRIN" .

roboprof_data:PRIN_241 a vivo:Course ;
    dbo:name "Processes in Digital Print Media I" ;
    dbo:number 241 ;
    dcterms:description "An introductory studio course in the basic concepts of contemporary digital imaging and print applications. " ;
    vivo:courseCredits 3 ;
    vivo:hasSubjectArea "PRIN" .

roboprof_data:PRIN_271 a vivo:Course ;
    dbo:name "Contemporary Print Processes I " ;
    dbo:number 271 ;
    dcterms:description "This introductory studio course addresses special topics in print processes and new technologies." ;
    vivo:courseCredits 3 ;
    vivo:hasSubjectArea "PRIN" .

roboprof_data:PRIN_291 a vivo:Course ;
    dbo:name "Contemporary Relief and Woodcut I" ;
    dbo:number 291 ;
    dcterms:description "An introductory studio course in the basic techniques of woodcut and relief printing with an emphasis on creative imagery." ;
    vivo:courseCredits 4 ;
    vivo:hasSubjectArea "PRIN" .

roboprof_data:PRIN_311 a vivo:Course ;
    dbo:name "Intaglio II" ;
    dbo:number 311 ;
    dcterms:description "An intermediate intaglio studio course with an emphasis on individual creative and theoretical development through experimentation and innovation." ;
    vivo:courseCredits 3 ;
    vivo:hasSubjectArea "PRIN" .

roboprof_data:PRIN_321 a vivo:Course ;
    dbo:name "Lithography II" ;
    dbo:number 321 ;
    dcterms:description "An intermediate lithography studio course with emphasis on individual creative and theoretical development through experimentation and innovation." ;
    vivo:courseCredits 4 ;
    vivo:hasSubjectArea "PRIN" .

roboprof_data:PRIN_331 a vivo:Course ;
    dbo:name "Screen Printing II" ;
    dbo:number 331 ;
    dcterms:description "An intermediate screenprinting studio course with an emphasis on individual creative and theoretical development through experimentation and innovation. " ;
    vivo:courseCredits 3 ;
    vivo:hasSubjectArea "PRIN" .

roboprof_data:PRIN_341 a vivo:Course ;
    dbo:name "Processes in Digital Print Media II" ;
    dbo:number 341 ;
    dcterms:description "An intermediate studio course with an emphasis on concepts of digital imaging, print applications, file creation, and layers for multiplate handprinting and file export to various digital print formats." ;
    vivo:courseCredits 4 ;
    vivo:hasSubjectArea "PRIN" .

roboprof_data:PRIN_366 a vivo:Course ;
    dbo:name "Aspects of the Artist Book" ;
    dbo:number 366 ;
    dcterms:description "An intermediate studio course with an emphasis on creative and theoretical development through experimentation and innovation." ;
    vivo:courseCredits 4 ;
    vivo:hasSubjectArea "PRIN" .

roboprof_data:PRIN_371 a vivo:Course ;
    dbo:name "Contemporary Print Processes II" ;
    dbo:number 371 ;
    dcterms:description "This intermediate studio course addresses topics in print processes and technologies. Students create a portfolio of artwork that demonstrates their research." ;
    vivo:courseCredits 4 ;
    vivo:hasSubjectArea "PRIN" .

roboprof_data:PRIN_381 a vivo:Course ;
    dbo:name "Aspects of Print Media" ;
    dbo:number 381 ;
    dcterms:description "An intermediate studio course that focuses on theoretical issues and practices in contemporary print media." ;
    vivo:courseCredits 4 ;
    vivo:hasSubjectArea "PRIN" .

roboprof_data:PRIN_391 a vivo:Course ;
    dbo:name "Contemporary Relief and Woodcut II" ;
    dbo:number 391 ;
    dcterms:description "An intermediate studio course in the techniques of woodcut and relief printing with an emphasis on creation." ;
    vivo:courseCredits 4 ;
    vivo:hasSubjectArea "PRIN" .

roboprof_data:PRIN_398 a vivo:Course ;
    dbo:name "Special Topics in Print Media" ;
    dbo:number 398 ;
    dcterms:description "An intermediate studio course that examines ideas and practices in contemporary print media, students produce printed images that reflect their research and critical thinking on the specific topic." ;
    vivo:courseCredits 3 ;
    vivo:hasSubjectArea "PRIN" .

roboprof_data:PRIN_399 a vivo:Course ;
    dbo:name "Special Topics in Print Media" ;
    dbo:number 399 ;
    dcterms:description "An intermediate studio course that examines ideas and practices in contemporary print media, students produce printed images that reflect their research and critical thinking on the specific topic." ;
    vivo:courseCredits 3 ;
    vivo:hasSubjectArea "PRIN" .

roboprof_data:PRIN_411 a vivo:Course ;
    dbo:name "Intaglio III " ;
    dbo:number 411 ;
    dcterms:description "An advanced intaglio studio course with an emphasis on individual creative and theoretical development through experimentation." ;
    vivo:courseCredits 3 ;
    vivo:hasSubjectArea "PRIN" .

roboprof_data:PRIN_421 a vivo:Course ;
    dbo:name "Lithography III " ;
    dbo:number 421 ;
    dcterms:description "An advanced lithography studio course with an emphasis on individual creative and theoretical development through experimentation and innovation. " ;
    vivo:courseCredits 3 ;
    vivo:hasSubjectArea "PRIN" .

roboprof_data:PRIN_431 a vivo:Course ;
    dbo:name "Screen Printing III" ;
    dbo:number 431 ;
    dcterms:description "An advanced screenprinting studio course with an emphasis on individual creative and theoretical development through experimentation and innovation." ;
    vivo:courseCredits 3 ;
    vivo:hasSubjectArea "PRIN" .

roboprof_data:PRIN_441 a vivo:Course ;
    dbo:name "Advanced Processes in Digital Print Media III" ;
    dbo:number 441 ;
    dcterms:description "An advanced digital studio course with an emphasis on individual creative and theoretical development through experimentation and innovation." ;
    vivo:courseCredits 3 ;
    vivo:hasSubjectArea "PRIN" .

roboprof_data:PRIN_451 a vivo:Course ;
    dbo:name "Advanced Projects in Print Media I" ;
    dbo:number 451 ;
    dcterms:description "An advanced studio course where students propose and complete print projects in consultation with the instructor. " ;
    vivo:courseCredits 4 ;
    vivo:hasSubjectArea "PRIN" .

roboprof_data:PRIN_452 a vivo:Course ;
    dbo:name "Advanced Projects in Print Media II" ;
    dbo:number 452 ;
    dcterms:description "An advanced studio course where students propose and complete print projects in consultation with the instructor. " ;
    vivo:courseCredits 4 ;
    vivo:hasSubjectArea "PRIN" .

roboprof_data:PRIN_470 a vivo:Course ;
    dbo:name "Independent Study in Print Media " ;
    dbo:number 470 ;
    dcterms:description "This course provides a limited number of students the opportunity to pursue advanced studies in print media under the supervision of a fulltime print faculty member. " ;
    vivo:courseCredits 4 ;
    vivo:hasSubjectArea "PRIN" .

roboprof_data:PRIN_471 a vivo:Course ;
    dbo:name "Independent Study in Print Media I" ;
    dbo:number 471 ;
    dcterms:description "This course provides a limited number of students the opportunity to pursue advanced studies in print media under the supervision of a fulltime print faculty member." ;
    vivo:courseCredits 4 ;
    vivo:hasSubjectArea "PRIN" .

roboprof_data:PRIN_472 a vivo:Course ;
    dbo:name "Independent Study in Print Media II" ;
    dbo:number 472 ;
    dcterms:description "This course provides a limited number of students the opportunity to pursue advanced studies in print media under the supervision of a fulltime print faculty member." ;
    vivo:courseCredits 3 ;
    vivo:hasSubjectArea "PRIN" .

roboprof_data:PRIN_481 a vivo:Course ;
    dbo:name "Professional Internship" ;
    dbo:number 481 ;
    dcterms:description "Internships are for students who wish to obtain practical experience by working as an apprentice in a professional environment, or who would like to pursue research in the curating of prints, print criticism, or other related experience in print media, and receive academic credit for the activity. " ;
    vivo:courseCredits 4 ;
    vivo:hasSubjectArea "PRIN" .

roboprof_data:PRIN_498 a vivo:Course ;
    dbo:name "Special Topics in Print Media" ;
    dbo:number 498 ;
    dcterms:description "An advanced studio course with an emphasis on individual creative and theoretical development through experimentation and innovation." ;
    vivo:courseCredits 4 ;
    vivo:hasSubjectArea "PRIN" .

roboprof_data:PRIN_499 a vivo:Course ;
    dbo:name "Special Topics in Print Media " ;
    dbo:number 499 ;
    dcterms:description "An advanced studio course with an emphasis on individual creative and theoretical development through experimentation and innovation. " ;
    vivo:courseCredits 4 ;
    vivo:hasSubjectArea "PRIN" .

roboprof_data:PSYC_311 a vivo:Course ;
    dbo:name "Research Methods and Designs II" ;
    dbo:number 311 ;
    dcterms:description "Experiment, Laboratory" ;
    vivo:courseCredits 4 ;
    vivo:hasSubjectArea "PSYC" .

roboprof_data:PSYC_315 a vivo:Course ;
    dbo:name "Statistical Analysis I" ;
    dbo:number 315 ;
    dcterms:description "Laboratory" ;
    vivo:courseCredits 4 ;
    vivo:hasSubjectArea "PSYC" .

roboprof_data:PSYC_316 a vivo:Course ;
    dbo:name "Statistical Analysis II" ;
    dbo:number 316 ;
    dcterms:description "Laboratory" ;
    vivo:courseCredits 4 ;
    vivo:hasSubjectArea "PSYC" .

roboprof_data:PSYC_387 a vivo:Course ;
    dbo:name "Directed Research in Psychology" ;
    dbo:number 387 ;
    dcterms:description "Students work in a research laboratory, gaining experience on current research methods in Psychology" ;
    vivo:courseCredits 4 ;
    vivo:hasSubjectArea "PSYC" .

roboprof_data:PSYC_485 a vivo:Course ;
    dbo:name "Specialization Project" ;
    dbo:number 485 ;
    dcterms:description "Students work in research lab on thesis. Course trains how to present their projects." ;
    vivo:courseCredits 4 ;
    vivo:hasSubjectArea "PSYC" .

roboprof_data:PSYC_487 a vivo:Course ;
    dbo:name "Advanced Directed Research in Psychology" ;
    dbo:number 487 ;
    dcterms:description "Students work in a research laboratory, gaining experience on current research methods in Psychology. Must have completed PSYC485 or PSYC495." ;
    vivo:courseCredits 3 ;
    vivo:hasSubjectArea "PSYC" .

roboprof_data:PSYC_495 a vivo:Course ;
    dbo:name "Honours Thesis" ;
    dbo:number 495 ;
    dcterms:description "Students work in research lab on thesis. Course trains how to present their projects." ;
    vivo:courseCredits 3 ;
    vivo:hasSubjectArea "PSYC" .

roboprof_data:PSYC_601 a vivo:Course ;
    dbo:name "Statistical Analysis and Experimental Design" ;
    dbo:number 601 ;
    dcterms:description "Laboratory" ;
    vivo:courseCredits 3 ;
    vivo:hasSubjectArea "PSYC" .

roboprof_data:PSYC_705 a vivo:Course ;
    dbo:name "APC Practicum I" ;
    dbo:number 705 ;
    dcterms:description "Case supervision, observe and/or assist with clients in therapy, case conferences at the Applied Psychology Centre" ;
    vivo:courseCredits 4 ;
    vivo:hasSubjectArea "PSYC" .

roboprof_data:PSYC_706 a vivo:Course ;
    dbo:name "Assessment Practicum I" ;
    dbo:number 706 ;
    dcterms:description "Administer intellectual tests under supervision" ;
    vivo:courseCredits 3 ;
    vivo:hasSubjectArea "PSYC" .

roboprof_data:PSYC_707 a vivo:Course ;
    dbo:name "Assessment Practicum II" ;
    dbo:number 707 ;
    dcterms:description "Administer intellectual tests under supervision" ;
    vivo:courseCredits 3 ;
    vivo:hasSubjectArea "PSYC" .

roboprof_data:PSYC_708 a vivo:Course ;
    dbo:name "APC Practicum II: General" ;
    dbo:number 708 ;
    dcterms:description "Assessment and treatment of selected clients of the Applied Psychology Centre under faculty supervision" ;
    vivo:courseCredits 3 ;
    vivo:hasSubjectArea "PSYC" .

roboprof_data:PSYC_709 a vivo:Course ;
    dbo:name "APC Practicum II: Adult" ;
    dbo:number 709 ;
    dcterms:description "Assessment and treatment of selected adult clients of the Applied Psychology Centre under faculty supervision" ;
    vivo:courseCredits 4 ;
    vivo:hasSubjectArea "PSYC" .

roboprof_data:PSYC_710 a vivo:Course ;
    dbo:name "APC Practicum II: Child" ;
    dbo:number 710 ;
    dcterms:description "Assessment and treatment of selected child clients of the Applied Psychology Centre under faculty supervision" ;
    vivo:courseCredits 4 ;
    vivo:hasSubjectArea "PSYC" .

roboprof_data:PSYC_711 a vivo:Course ;
    dbo:name "Extramural Practicum I: General" ;
    dbo:number 711 ;
    dcterms:description "4-month extramural practicum done under qualified supervisors" ;
    vivo:courseCredits 3 ;
    vivo:hasSubjectArea "PSYC" .

roboprof_data:PSYC_712 a vivo:Course ;
    dbo:name "Extramural Practicum I: Adult" ;
    dbo:number 712 ;
    dcterms:description "4-month extramural practicum with adult clients, done under qualified supervisors" ;
    vivo:courseCredits 4 ;
    vivo:hasSubjectArea "PSYC" .

roboprof_data:PSYC_713 a vivo:Course ;
    dbo:name "Extramural Practicum I: Child" ;
    dbo:number 713 ;
    dcterms:description "4-month extramural practicum with child clients, done under qualified supervisors" ;
    vivo:courseCredits 3 ;
    vivo:hasSubjectArea "PSYC" .

roboprof_data:PSYC_823 a vivo:Course ;
    dbo:name "APC Practicum III: General",
        "Multivariate Statistics" ;
    dbo:number 823 ;
    dcterms:description "Laboratory",
        "Practicum, clinical experience and supervision" ;
    vivo:courseCredits 4 ;
    vivo:hasSubjectArea "PSYC" .

roboprof_data:PSYC_824 a vivo:Course ;
    dbo:name "APC Practicum III: Adult" ;
    dbo:number 824 ;
    dcterms:description "Practicum, clinical experience and supervision" ;
    vivo:courseCredits 4 ;
    vivo:hasSubjectArea "PSYC" .

roboprof_data:PSYC_825 a vivo:Course ;
    dbo:name "APC Practicum III: Child" ;
    dbo:number 825 ;
    dcterms:description "Practicum, clinical experience and supervision" ;
    vivo:courseCredits 3 ;
    vivo:hasSubjectArea "PSYC" .

roboprof_data:PSYC_826 a vivo:Course ;
    dbo:name "APC Practicum IV: General" ;
    dbo:number 826 ;
    dcterms:description "Specialised practicum for advanced students involving clinical experience under supervision" ;
    vivo:courseCredits 4 ;
    vivo:hasSubjectArea "PSYC" .

roboprof_data:PSYC_827 a vivo:Course ;
    dbo:name "APC Practicum IV: Adult" ;
    dbo:number 827 ;
    dcterms:description "Specialised practicum for advanced students involving clinical experience with adult clients under supervision" ;
    vivo:courseCredits 3 ;
    vivo:hasSubjectArea "PSYC" .

roboprof_data:PSYC_828 a vivo:Course ;
    dbo:name "APC Practicum IV: Child" ;
    dbo:number 828 ;
    dcterms:description "Specialised practicum for advanced students involving clinical experience with child clients under supervision" ;
    vivo:courseCredits 3 ;
    vivo:hasSubjectArea "PSYC" .

roboprof_data:PSYC_838 a vivo:Course ;
    dbo:name "Extramural Practicum II: General" ;
    dbo:number 838 ;
    dcterms:description "Practicum" ;
    vivo:courseCredits 3 ;
    vivo:hasSubjectArea "PSYC" .

roboprof_data:PSYC_839 a vivo:Course ;
    dbo:name "Extramural Practicum II: Adult" ;
    dbo:number 839 ;
    dcterms:description "Practicum" ;
    vivo:courseCredits 4 ;
    vivo:hasSubjectArea "PSYC" .

roboprof_data:PSYC_840 a vivo:Course ;
    dbo:name "Extramural Practicum II: Child" ;
    dbo:number 840 ;
    dcterms:description "Practicum" ;
    vivo:courseCredits 3 ;
    vivo:hasSubjectArea "PSYC" .

roboprof_data:PSYC_841 a vivo:Course ;
    dbo:name "Extramural Practicum III: General" ;
    dbo:number 841 ;
    dcterms:description "Practicum" ;
    vivo:courseCredits 4 ;
    vivo:hasSubjectArea "PSYC" .

roboprof_data:PSYC_842 a vivo:Course ;
    dbo:name "Extramural Practicum III: Adult" ;
    dbo:number 842 ;
    dcterms:description "Practicum" ;
    vivo:courseCredits 4 ;
    vivo:hasSubjectArea "PSYC" .

roboprof_data:PSYC_843 a vivo:Course ;
    dbo:name "Extramural Practicum III: Child" ;
    dbo:number 843 ;
    dcterms:description "Practicum" ;
    vivo:courseCredits 3 ;
    vivo:hasSubjectArea "PSYC" .

roboprof_data:PSYC_850 a vivo:Course ;
    dbo:name "Practicum in Experimental Techniques" ;
    dbo:number 850 ;
    dcterms:description "Practicum" ;
    vivo:courseCredits 4 ;
    vivo:hasSubjectArea "PSYC" .

roboprof_data:PSYC_851 a vivo:Course ;
    dbo:name "Teaching of Laboratory Techniques" ;
    dbo:number 851 ;
    dcterms:description "Practicum" ;
    vivo:courseCredits 3 ;
    vivo:hasSubjectArea "PSYC" .

roboprof_data:PTNG_200 a vivo:Course ;
    dbo:name "Painting I" ;
    dbo:number 200 ;
    dcterms:description "A studio course which provides a technical and conceptual introduction to painting focusing on the distinctive nature of the medium." ;
    vivo:courseCredits 3 ;
    vivo:hasSubjectArea "PTNG" .

roboprof_data:PTNG_201 a vivo:Course ;
    dbo:name "Introduction to Painting" ;
    dbo:number 201 ;
    dcterms:description "This introductory-level course explores elementary concepts in the art of painting through a series of structured studio experiences." ;
    vivo:courseCredits 4 ;
    vivo:hasSubjectArea "PTNG" .

roboprof_data:PTNG_298 a vivo:Course ;
    dbo:name "Special Topics in Painting" ;
    dbo:number 298 ;
    dcterms:description "A studio course which provides an opportunity for the study of more specialized aspects of painting." ;
    vivo:courseCredits 3 ;
    vivo:hasSubjectArea "PTNG" .

roboprof_data:PTNG_299 a vivo:Course ;
    dbo:name "Special Topics in Painting " ;
    dbo:number 299 ;
    dcterms:description "A studio course which provides an opportunity for the study of more specialized aspects of painting." ;
    vivo:courseCredits 3 ;
    vivo:hasSubjectArea "PTNG" .

roboprof_data:PTNG_300 a vivo:Course ;
    dbo:name "Painting II" ;
    dbo:number 300 ;
    dcterms:description "This studio course is an intermediate painting class in which directed projects allow students to explore a variety of approaches to the medium and to begin to develop a more personal visual language based on the skill sets acquired at the 200 level." ;
    vivo:courseCredits 4 ;
    vivo:hasSubjectArea "PTNG" .

roboprof_data:PTNG_310 a vivo:Course ;
    dbo:name "Painting and Popular Culture I" ;
    dbo:number 310 ;
    dcterms:description "A studio course designed to focus on the relationship between painting and popular culture." ;
    vivo:courseCredits 4 ;
    vivo:hasSubjectArea "PTNG" .

roboprof_data:PTNG_312 a vivo:Course ;
    dbo:name "Body, Representation and Information I " ;
    dbo:number 312 ;
    dcterms:description "This studio course addresses contemporary art issues in painting, exploring body information in relation to questions of power, race, gender, and sexuality." ;
    vivo:courseCredits 3 ;
    vivo:hasSubjectArea "PTNG" .

roboprof_data:PTNG_314 a vivo:Course ;
    dbo:name "Life in the Round: Painting the Figure from Observation I" ;
    dbo:number 314 ;
    dcterms:description "This studio course focuses on the experience of seeing and depicting the living human body in all its complexity and presence." ;
    vivo:courseCredits 3 ;
    vivo:hasSubjectArea "PTNG" .

roboprof_data:PTNG_316 a vivo:Course ;
    dbo:name "Abstract Painting I" ;
    dbo:number 316 ;
    dcterms:description "A studio course designed to focus on the historical and contemporary practice of abstraction." ;
    vivo:courseCredits 3 ;
    vivo:hasSubjectArea "PTNG" .

roboprof_data:PTNG_320 a vivo:Course ;
    dbo:name "Studio/Seminar in Painting and Drawing" ;
    dbo:number 320 ;
    dcterms:description "A combination studio/seminar in which advanced ideas in painting and drawing are addressed. " ;
    vivo:courseCredits 4 ;
    vivo:hasSubjectArea "PTNG" .

roboprof_data:PTNG_398 a vivo:Course ;
    dbo:name "Special Topics in Painting" ;
    dbo:number 398 ;
    dcterms:description "A studio course which provides an opportunity for the study of more specialized aspects of painting." ;
    vivo:courseCredits 4 ;
    vivo:hasSubjectArea "PTNG" .

roboprof_data:PTNG_399 a vivo:Course ;
    dbo:name "Special Topics in Painting" ;
    dbo:number 399 ;
    dcterms:description "A studio course which provides an opportunity for the study of more specialized aspects of painting." ;
    vivo:courseCredits 4 ;
    vivo:hasSubjectArea "PTNG" .

roboprof_data:PTNG_400 a vivo:Course ;
    dbo:name "Painting III" ;
    dbo:number 400 ;
    dcterms:description "An advanced painting class in which students develop a series of independent projects that allow them to create a coherent body of work in painting and to situate it within contemporary practice." ;
    vivo:courseCredits 3 ;
    vivo:hasSubjectArea "PTNG" .

roboprof_data:PTNG_410 a vivo:Course ;
    dbo:name "Painting and Popular Culture II" ;
    dbo:number 410 ;
    dcterms:description "An advancedlevel studio course designed to focus on the relationship between painting and popular culture. " ;
    vivo:courseCredits 3 ;
    vivo:hasSubjectArea "PTNG" .

roboprof_data:PTNG_412 a vivo:Course ;
    dbo:name "Body, Representation and Information II " ;
    dbo:number 412 ;
    dcterms:description "This advancedlevel studio course addresses contemporary art issues and their representation in painting, exploring body information in relation to questions of power, race, gender, and sexuality." ;
    vivo:courseCredits 4 ;
    vivo:hasSubjectArea "PTNG" .

roboprof_data:PTNG_414 a vivo:Course ;
    dbo:name "Life in the Round: Painting the Figure from Observation II" ;
    dbo:number 414 ;
    dcterms:description "This advancedlevel studio course focuses on the experience of seeing and depicting the living human body in all its complexity and presence." ;
    vivo:courseCredits 4 ;
    vivo:hasSubjectArea "PTNG" .

roboprof_data:PTNG_416 a vivo:Course ;
    dbo:name "Abstract Painting II" ;
    dbo:number 416 ;
    dcterms:description "An advancedlevel studio class designed to focus on the historical and contemporary practice of abstraction." ;
    vivo:courseCredits 4 ;
    vivo:hasSubjectArea "PTNG" .

roboprof_data:PTNG_418 a vivo:Course ;
    dbo:name "Between the Wall and the Viewer" ;
    dbo:number 418 ;
    dcterms:description "An installation studio course taught by faculty in the Painting and Drawing area that encourages students to create work in the context of an expanded field." ;
    vivo:courseCredits 4 ;
    vivo:hasSubjectArea "PTNG" .

roboprof_data:PTNG_420 a vivo:Course ;
    dbo:name "Seminar/Workshop in Painting" ;
    dbo:number 420 ;
    dcterms:description "An advanced studio in painting having its principal emphasis in studio practice, but developing further the theoretical concepts introduced in PTNG 320." ;
    vivo:courseCredits 3 ;
    vivo:hasSubjectArea "PTNG" .

roboprof_data:PTNG_430 a vivo:Course ;
    dbo:name "Women and Painting" ;
    dbo:number 430 ;
    dcterms:description "A studio/seminar course in which students are encouraged to explore their world in painting and consider their practice from the point of view of womens experience, individually and collectively." ;
    vivo:courseCredits 4 ;
    vivo:hasSubjectArea "PTNG" .

roboprof_data:PTNG_440 a vivo:Course ;
    dbo:name "Collage" ;
    dbo:number 440 ;
    dcterms:description "An exploration of collage as a means of expression evolving from the historical and artistic traditions of painting and drawing." ;
    vivo:courseCredits 3 ;
    vivo:hasSubjectArea "PTNG" .

roboprof_data:PTNG_450 a vivo:Course ;
    dbo:name "Painting IV" ;
    dbo:number 450 ;
    dcterms:description "An advanced painting class in which students develop a series of independent projects that allow them to create a coherent body of work in painting and to situate it within contemporary practice. Independent studio production may be supplemented by readings, lectures, seminars, museum/gallery visits, and visiting artists." ;
    vivo:courseCredits 4 ;
    vivo:hasSubjectArea "PTNG" .

roboprof_data:PTNG_460 a vivo:Course ;
    dbo:name "Materials and Methods of the Artist" ;
    dbo:number 460 ;
    dcterms:description "Through a series of special projects in drawing and painting, this course familiarizes the student with historical materials and techniques, and with other aspects of the artists concerns." ;
    vivo:courseCredits 3 ;
    vivo:hasSubjectArea "PTNG" .

roboprof_data:PTNG_470 a vivo:Course ;
    dbo:name "Independent Study" ;
    dbo:number 470 ;
    dcterms:description "This course provides a limited number of students the opportunity to pursue advanced studies in painting under the supervision of a fulltime painting faculty member. " ;
    vivo:courseCredits 3 ;
    vivo:hasSubjectArea "PTNG" .

roboprof_data:PTNG_471 a vivo:Course ;
    dbo:name "Independent Study I" ;
    dbo:number 471 ;
    dcterms:description "This course provides a limited number of students the opportunity to pursue advanced studies in painting under the supervision of a fulltime painting faculty member." ;
    vivo:courseCredits 3 ;
    vivo:hasSubjectArea "PTNG" .

roboprof_data:PTNG_472 a vivo:Course ;
    dbo:name "Independent Study II" ;
    dbo:number 472 ;
    dcterms:description "This course provides a limited number of students the opportunity to pursue advanced studies in painting under the supervision of a fulltime painting faculty member." ;
    vivo:courseCredits 4 ;
    vivo:hasSubjectArea "PTNG" .

roboprof_data:PTNG_498 a vivo:Course ;
    dbo:name "Special Topics in Painting" ;
    dbo:number 498 ;
    dcterms:description "A course for advanced students which provides an opportunity for the study of more specialized areas in painting." ;
    vivo:courseCredits 3 ;
    vivo:hasSubjectArea "PTNG" .

roboprof_data:PTNG_499 a vivo:Course ;
    dbo:name "Special Topics in Painting" ;
    dbo:number 499 ;
    dcterms:description "A course for advanced students which provides an opportunity for the study of more specialized areas in painting." ;
    vivo:courseCredits 3 ;
    vivo:hasSubjectArea "PTNG" .

roboprof_data:RELI_210 a vivo:Course ;
    dbo:name "Religion in Practice" ;
    dbo:number 210 ;
    dcterms:description "create map of religious sites in students neighborhood; interview religious leader for practice portrait; field trips to religious sites" ;
    vivo:courseCredits 4 ;
    vivo:hasSubjectArea "RELI" .

roboprof_data:RELI_214 a vivo:Course ;
    dbo:name "Religions of the West" ;
    dbo:number 214 ;
    dcterms:description "field trip to places of workshop, creative project, group presentations" ;
    vivo:courseCredits 4 ;
    vivo:hasSubjectArea "RELI" .

roboprof_data:RELI_215 a vivo:Course ;
    dbo:name "Religions of Asia" ;
    dbo:number 215 ;
    dcterms:description "field trip to places of workshop, creative project, group presentations" ;
    vivo:courseCredits 3 ;
    vivo:hasSubjectArea "RELI" .

roboprof_data:RELI_220 a vivo:Course ;
    dbo:name "Introduction to Judaism" ;
    dbo:number 220 ;
    dcterms:description "real-life case studies, role-playing, fieldwork, facilitated reflection in response paper assignments" ;
    vivo:courseCredits 3 ;
    vivo:hasSubjectArea "RELI" .

roboprof_data:RELI_223 a vivo:Course ;
    dbo:name "Introduction to Christianity" ;
    dbo:number 223 ;
    dcterms:description "site visits to local churches and Christian communities" ;
    vivo:courseCredits 3 ;
    vivo:hasSubjectArea "RELI" .

roboprof_data:RELI_224 a vivo:Course ;
    dbo:name "Introduction to Hinduism" ;
    dbo:number 224 ;
    dcterms:description "field trip to places of workshop, creative project, group presentations" ;
    vivo:courseCredits 3 ;
    vivo:hasSubjectArea "RELI" .

roboprof_data:RELI_312 a vivo:Course ;
    dbo:name "Justice and Social Conflict in a Globalized World" ;
    dbo:number 312 ;
    dcterms:description "profile of a social justice organization" ;
    vivo:courseCredits 4 ;
    vivo:hasSubjectArea "RELI" .

roboprof_data:RELI_313 a vivo:Course ;
    dbo:name "Zoroastrianism" ;
    dbo:number 313 ;
    dcterms:description "participation in local communitys gahanbar rituals." ;
    vivo:courseCredits 4 ;
    vivo:hasSubjectArea "RELI" .

roboprof_data:RELI_318 a vivo:Course ;
    dbo:name "Shiite Islam" ;
    dbo:number 318 ;
    dcterms:description "team video preparation" ;
    vivo:courseCredits 4 ;
    vivo:hasSubjectArea "RELI" .

roboprof_data:RELI_378 a vivo:Course ;
    dbo:name "Death and Dying" ;
    dbo:number 378 ;
    dcterms:description "profile of death care issues or rituals in Montreal, field trips" ;
    vivo:courseCredits 3 ;
    vivo:hasSubjectArea "RELI" .

roboprof_data:RELI_387 a vivo:Course ;
    dbo:name "Goddesses and Religious Images of Women" ;
    dbo:number 387 ;
    dcterms:description "field report on contemporaneous experience related to course material" ;
    vivo:courseCredits 4 ;
    vivo:hasSubjectArea "RELI" .

roboprof_data:RELI_390 a vivo:Course ;
    dbo:name "Angels and Demons in Judaism" ;
    dbo:number 390 ;
    dcterms:description "Creative assignment (artwork; poetry; fiction), optional participation in exhibit; in-class presentation" ;
    vivo:courseCredits 4 ;
    vivo:hasSubjectArea "RELI" .

roboprof_data:RELI_392 a vivo:Course ;
    dbo:name "Women in Jewish History: Modern" ;
    dbo:number 392 ;
    dcterms:description "This course examines the lives and experiences of Jewish women in the modern period. The immigrations to North America and the subsequent development of the community provide the framework for investigating Jewish womens encounter with and contribution to modern Jewish life. The main focus is on North America, using primary sources such as fiction, biography, and autobiography. The influence of denominational differences and feminist challenges complete the survey.",
        "interviewing a woman whose life story is informative " ;
    vivo:courseCredits 4 ;
    vivo:hasSubjectArea "RELI",
        "RELI " .

roboprof_data:RELI_396 a vivo:Course ;
    dbo:name "Food and Religion" ;
    dbo:number 396 ;
    dcterms:description "field report on contemporaneous experience related to course material" ;
    vivo:courseCredits 4 ;
    vivo:hasSubjectArea "RELI" .

roboprof_data:RELI_409 a vivo:Course ;
    dbo:name "Methodology and the Study of Religion" ;
    dbo:number 409 ;
    dcterms:description "fieldwork project, 2 interviews, site visit to a religious community" ;
    vivo:courseCredits 3 ;
    vivo:hasSubjectArea "RELI" .

roboprof_data:RELI_6007 a vivo:Course ;
    dbo:name "Religion, Politics, Heritage" ;
    dbo:number 6007 ;
    dcterms:description "research project based on real world heritage site, data collection, survey, interviewing, ethnographic observation, archival and media research. Presentation and discussion moderation." ;
    vivo:courseCredits 3 ;
    vivo:hasSubjectArea "RELI" .

roboprof_data:RELI_6008 a vivo:Course ;
    dbo:name "Community Engagement" ;
    dbo:number 6008 ;
    dcterms:description "internship in local community organization or institution" ;
    vivo:courseCredits 4 ;
    vivo:hasSubjectArea "RELI" .

roboprof_data:RELI_6018 a vivo:Course ;
    dbo:name "Jewish Community Engagement" ;
    dbo:number 6018 ;
    dcterms:description "internship in local Jewish community organization/institution" ;
    vivo:courseCredits 3 ;
    vivo:hasSubjectArea "RELI" .

<http://roboprof.ca/data/Retake/COMP_6231_A> a roboprof:RetakeGrade ;
    roboprof:gradeInCourse roboprof_data:COMP_6231 ;
    roboprof:gradeValue "A" .

<http://roboprof.ca/data/Retake/COMP_6521_B+> a roboprof:RetakeGrade ;
    roboprof:gradeInCourse roboprof_data:COMP_6521 ;
    roboprof:gradeValue "B+" .

roboprof_data:SCEN_327 a vivo:Course ;
    dbo:name "Hair and Make up Design" ;
    dbo:number 327 ;
    dcterms:description "Students study hair and make-up design for the performing arts with emphasis on analysis, development and execution of design ideas" ;
    vivo:courseCredits 3 ;
    vivo:hasSubjectArea "SCEN" .

roboprof_data:SCEN_347 a vivo:Course ;
    dbo:name "Exhibition Scenography" ;
    dbo:number 347 ;
    dcterms:description "Introduces exhibition scenography as a practical, expressive, and interpretive form" ;
    vivo:courseCredits 4 ;
    vivo:hasSubjectArea "SCEN" .

roboprof_data:SCEN_411 a vivo:Course ;
    dbo:name "Urban Scenographies" ;
    dbo:number 411 ;
    dcterms:description "Contemporary theories and practices of scenography and performance design in the context and scale of cities and urban landscapes" ;
    vivo:courseCredits 4 ;
    vivo:hasSubjectArea "SCEN" .

roboprof_data:SCEN_412 a vivo:Course ;
    dbo:name "Art Direction" ;
    dbo:number 412 ;
    dcterms:description "This studio course examines art direction for films, television, music videos, and documentaries." ;
    vivo:courseCredits 3 ;
    vivo:hasSubjectArea "SCEN" .

roboprof_data:SCEN_448 a vivo:Course ;
    dbo:name "Design Field School" ;
    dbo:number 448 ;
    dcterms:description "Course offers students hands-on, experiential learning in aspects of scenography via travel to and residency at a festival, conference, or exhibition" ;
    vivo:courseCredits 3 ;
    vivo:hasSubjectArea "SCEN" .

roboprof_data:SCOL_290 a vivo:Course ;
    dbo:name "Directed and Independent Study I" ;
    dbo:number 290 ;
    dcterms:description "Practical laboratory project (one semester in length) intended to give students an introduction to the way a research group operates, as well as the factors that go into the design and execution of a research project." ;
    vivo:courseCredits 3 ;
    vivo:hasSubjectArea "SCOL" .

roboprof_data:SCOL_391 a vivo:Course ;
    dbo:name "Directed and Independent Study II" ;
    dbo:number 391 ;
    dcterms:description "Practical laboratory project (two semesters in length) to be carried out after the completion of SCOL 290, and in a field different from the SCOL 290 project" ;
    vivo:courseCredits 3 ;
    vivo:hasSubjectArea "SCOL" .

roboprof_data:SCOL_490 a vivo:Course ;
    dbo:name "Directed and Independent Study III" ;
    dbo:number 490 ;
    dcterms:description "Practical laboratory project (two semesters in length) to be carried out after the completion of SCOL 290 and SCOL 391, and in a field different from the SCOL 290 and 391 projects" ;
    vivo:courseCredits 4 ;
    vivo:hasSubjectArea "SCOL" .

roboprof_data:SCOM_374 a vivo:Course ;
    dbo:name "Supply Chain Logistics" ;
    dbo:number 374 ;
    dcterms:description "Logistics simulations and games used to illustrate integration and coordination issues in supply chain" ;
    vivo:courseCredits 3 ;
    vivo:hasSubjectArea "SCOM" .

roboprof_data:SCOM_492 a vivo:Course ;
    dbo:name "Supply Chain Simulation" ;
    dbo:number 492 ;
    dcterms:description "Use of simulation software to run realistic supply chain scenarios" ;
    vivo:courseCredits 3 ;
    vivo:hasSubjectArea "SCOM" .

roboprof_data:SCOM_498 a vivo:Course ;
    dbo:name "Supply Chain Project" ;
    dbo:number 498 ;
    dcterms:description "Project carried out in a real-life setting" ;
    vivo:courseCredits 4 ;
    vivo:hasSubjectArea "SCOM" .

roboprof_data:SCPA_301 a vivo:Course ;
    dbo:name "Social Debates and Issues in Public Affairs and Public Policy" ;
    dbo:number 301 ;
    dcterms:description "Case studies, public panel discussion" ;
    vivo:courseCredits 3 ;
    vivo:hasSubjectArea "SCPA" .

roboprof_data:SCPA_352 a vivo:Course ;
    dbo:name "Community and Local Activism" ;
    dbo:number 352 ;
    dcterms:description "Local and community activism" ;
    vivo:courseCredits 3 ;
    vivo:hasSubjectArea "SCPA" .

roboprof_data:SCPA_411 a vivo:Course ;
    dbo:name "Internship" ;
    dbo:number 411 ;
    dcterms:description "NaN"^^xsd:double ;
    vivo:courseCredits 3 ;
    vivo:hasSubjectArea "SCPA" .

roboprof_data:SCPA_412 a vivo:Course ;
    dbo:name "Senior Research Seminar" ;
    dbo:number 412 ;
    dcterms:description "Simulation, real-life interaction, one-day event at the end of term" ;
    vivo:courseCredits 4 ;
    vivo:hasSubjectArea "SCPA" .

roboprof_data:SCPA_482 a vivo:Course ;
    dbo:name "Field Project in Immigration, Migration and Diversity" ;
    dbo:number 482 ;
    dcterms:description "NaN"^^xsd:double ;
    vivo:courseCredits 3 ;
    vivo:hasSubjectArea "SCPA" .

roboprof_data:SCPA_509 a vivo:Course ;
    dbo:name "Financing CED Initiatives: Part II",
        "Le financement des initiatives de DC. Partie II" ;
    dbo:number 509 ;
    dcterms:description "Case study approach,  on site visits, interviews",
        "Visite de sites, entrevues" ;
    vivo:courseCredits 3,
        4 ;
    vivo:hasSubjectArea "SCPA" .

roboprof_data:SCPA_510 a vivo:Course ;
    dbo:name "CED Field Project Part 1" ;
    dbo:number 510 ;
    dcterms:description "NaN"^^xsd:double ;
    vivo:courseCredits 4 ;
    vivo:hasSubjectArea "SCPA" .

roboprof_data:SCPA_516 a vivo:Course ;
    dbo:name "Housing and Land Use from a CED Perspective: Part II" ;
    dbo:number 516 ;
    dcterms:description "Examine, evaluate existing housing projects, on site visits, interviews" ;
    vivo:courseCredits 3 ;
    vivo:hasSubjectArea "SCPA" .

roboprof_data:SCPA_537 a vivo:Course ;
    dbo:name "Aboriginal CED: Part II",
        "Le DC en milieu autochtone. Partie II" ;
    dbo:number 537 ;
    dcterms:description "On site visits",
        "Visite de sites" ;
    vivo:courseCredits 3,
        4 ;
    vivo:hasSubjectArea "SCPA" .

roboprof_data:SCUL_201 a vivo:Course ;
    dbo:name "Introduction to Sculpture and Installation" ;
    dbo:number 201 ;
    dcterms:description "This introductory-level course covers fundamental ideas and techniques central to 3-dimensional art making within the context of contemporary art." ;
    vivo:courseCredits 3 ;
    vivo:hasSubjectArea "SCUL" .

roboprof_data:SCUL_210 a vivo:Course ;
    dbo:name "Sculpture and Material Practices" ;
    dbo:number 210 ;
    dcterms:description "In this studiobased course, students explore the expansive field of contemporary sculpture and the range of materials and ideas employed by contemporary artists working in the discipline." ;
    vivo:courseCredits 4 ;
    vivo:hasSubjectArea "SCUL" .

roboprof_data:SCUL_251 a vivo:Course ;
    dbo:name "Sculpture/Mechanics" ;
    dbo:number 251 ;
    dcterms:description "This studio course introduces students to animating sculpture through a variety of techniques such as moving joints, gear, chain, and pulley systems, and motion converters, leading to more complex assemblies in animating static form. " ;
    vivo:courseCredits 4 ;
    vivo:hasSubjectArea "SCUL" .

roboprof_data:SCUL_310 a vivo:Course ;
    dbo:name "Sculpture and Spatial Practices" ;
    dbo:number 310 ;
    dcterms:description "This course builds upon the expansive field of contemporary sculpture, with an emphasis on the development of an individual art practice, including installation, intervention, public artworks, action/ performance, and object making." ;
    vivo:courseCredits 4 ;
    vivo:hasSubjectArea "SCUL" .

roboprof_data:SCUL_311 a vivo:Course ;
    dbo:name "Metal Casting: Bronze and Aluminum I" ;
    dbo:number 311 ;
    dcterms:description "This course includes an introduction to the sculptural histories and contemporary contexts of bronze casting, and the technical processes of casting." ;
    vivo:courseCredits 3 ;
    vivo:hasSubjectArea "SCUL" .

roboprof_data:SCUL_312 a vivo:Course ;
    dbo:name "Metal Casting: Bronze and Aluminum II" ;
    dbo:number 312 ;
    dcterms:description "A continuation of SCUL 311. In this advanced course, students learn to cast larger or more complex artworks in bronze or aluminum. " ;
    vivo:courseCredits 4 ;
    vivo:hasSubjectArea "SCUL" .

roboprof_data:SCUL_396 a vivo:Course ;
    dbo:name "Digital Sculpture" ;
    dbo:number 396 ;
    dcterms:description "This studio course introduces 3D software for sculptors, covering modelling, drafting, and rendering for both real and virtual output, using advanced manual and automated processes." ;
    vivo:courseCredits 3 ;
    vivo:hasSubjectArea "SCUL" .

roboprof_data:SCUL_397 a vivo:Course ;
    dbo:name "Intermediate Digital Sculpture II" ;
    dbo:number 397 ;
    dcterms:description "This course provides greater experience and advanced skills in 3D modelling." ;
    vivo:courseCredits 3 ;
    vivo:hasSubjectArea "SCUL" .

roboprof_data:SCUL_398 a vivo:Course ;
    dbo:name "Special Topics in Sculpture" ;
    dbo:number 398 ;
    dcterms:description "A workshop/seminar course providing an opportunity for the study of specialized aspects of sculpture." ;
    vivo:courseCredits 4 ;
    vivo:hasSubjectArea "SCUL" .

roboprof_data:SCUL_399 a vivo:Course ;
    dbo:name "Special Topics in Sculpture " ;
    dbo:number 399 ;
    dcterms:description "A workshop/seminar course providing an opportunity for the study of specialized aspects in sculpture." ;
    vivo:courseCredits 4 ;
    vivo:hasSubjectArea "SCUL" .

roboprof_data:SCUL_410 a vivo:Course ;
    dbo:name "Sculpture as Practice" ;
    dbo:number 410 ;
    dcterms:description "An advanced sculpture class in which students develop and create a body of artwork situated within the contexts of contemporary sculpture." ;
    vivo:courseCredits 3 ;
    vivo:hasSubjectArea "SCUL" .

roboprof_data:SCUL_450 a vivo:Course ;
    dbo:name "Independent Study" ;
    dbo:number 450 ;
    dcterms:description "This course provides a limited number of students the opportunity to pursue advanced studies in sculpture under the supervision of a fulltime sculpture faculty member." ;
    vivo:courseCredits 3 ;
    vivo:hasSubjectArea "SCUL" .

roboprof_data:SCUL_451 a vivo:Course ;
    dbo:name "INDEPENDENT STUDY I",
        "Independent Study I" ;
    dbo:number 451 ;
    dcterms:description "NaN"^^xsd:double,
        "This course provides a limited number of students the opportunity to pursue advanced studies in sculpture under the supervision of a fulltime sculpture faculty member." ;
    vivo:courseCredits 4 ;
    vivo:hasSubjectArea "SCUL" .

roboprof_data:SCUL_452 a vivo:Course ;
    dbo:name "Independent Study II" ;
    dbo:number 452 ;
    dcterms:description "This course provides a limited number of students the opportunity to pursue advanced studies in sculpture under the supervision of a fulltime sculpture faculty member." ;
    vivo:courseCredits 4 ;
    vivo:hasSubjectArea "SCUL" .

roboprof_data:SCUL_490 a vivo:Course ;
    dbo:name "Advanced Studio Practice" ;
    dbo:number 490 ;
    dcterms:description "A studio course providing an opportunity for the advanced student to work in an intimate context within a studio setting, structured around current topics of theoretical and practical importance." ;
    vivo:courseCredits 4 ;
    vivo:hasSubjectArea "SCUL" .

roboprof_data:SOCI_415 a vivo:Course ;
    dbo:name "Field Research" ;
    dbo:number 415 ;
    dcterms:description "Field, practice" ;
    vivo:courseCredits 3 ;
    vivo:hasSubjectArea "SOCI" .

roboprof_data:SOCI_450 a vivo:Course ;
    dbo:name "Social Economy & Sustainable Futures" ;
    dbo:number 450 ;
    dcterms:description "Community Service Learning & Group project" ;
    vivo:courseCredits 3 ;
    vivo:hasSubjectArea "SOCI" .

roboprof_data:SOEN_228 a vivo:Course ;
    dbo:name "System Hardware" ;
    dbo:number 228 ;
    dcterms:description "Laboratory: 24 hours total" ;
    vivo:courseCredits 4 ;
    vivo:hasSubjectArea "SOEN" .

roboprof_data:SOEN_341 a vivo:Course ;
    dbo:name "Software Process" ;
    dbo:number 341 ;
    dcterms:description "Group project" ;
    vivo:courseCredits 4 ;
    vivo:hasSubjectArea "SOEN" .

roboprof_data:SOEN_385 a vivo:Course ;
    dbo:name "Control Systems and Applications" ;
    dbo:number 385 ;
    dcterms:description "A project is required" ;
    vivo:courseCredits 4 ;
    vivo:hasSubjectArea "SOEN" .

roboprof_data:SOEN_390 a vivo:Course ;
    dbo:name "Software Engineering Team Design Project" ;
    dbo:number 390 ;
    dcterms:description "mini-capstone, group project, Laboratory: 36 hours total" ;
    vivo:courseCredits 4 ;
    vivo:hasSubjectArea "SOEN" .

roboprof_data:SOEN_422 a vivo:Course ;
    dbo:name "Embedded Systems and Software" ;
    dbo:number 422 ;
    dcterms:description "Laboratory: 24 hours total, project" ;
    vivo:courseCredits 4 ;
    vivo:hasSubjectArea "SOEN" .

roboprof_data:SOEN_423 a vivo:Course ;
    dbo:name "Distributed Systems" ;
    dbo:number 423 ;
    dcterms:description "Laboratory: 24 hours total, project" ;
    vivo:courseCredits 4 ;
    vivo:hasSubjectArea "SOEN" .

roboprof_data:SOEN_487 a vivo:Course ;
    dbo:name "Web Services and Applications" ;
    dbo:number 487 ;
    dcterms:description "Laboratory: 24 hours total, project" ;
    vivo:courseCredits 4 ;
    vivo:hasSubjectArea "SOEN" .

roboprof_data:SOEN_490 a vivo:Course ;
    dbo:name "Capstone Software Engineering Design Project" ;
    dbo:number 490 ;
    dcterms:description "capstone, group project" ;
    vivo:courseCredits 4 ;
    vivo:hasSubjectArea "SOEN" .

roboprof_data:SOEN_491 a vivo:Course ;
    dbo:name "Software Engineering Project" ;
    dbo:number 491 ;
    dcterms:description "project" ;
    vivo:courseCredits 4 ;
    vivo:hasSubjectArea "SOEN" .

roboprof_data:SOEN_6231 a vivo:Course ;
    dbo:name "Distributed Systems" ;
    dbo:number 6231 ;
    dcterms:description "Laboratory: 24 hours total, project" ;
    vivo:courseCredits 4 ;
    vivo:hasSubjectArea "SOEN" .

roboprof_data:SOEN_6441 a vivo:Course ;
    dbo:name "Advanced Programming Practices" ;
    dbo:number 6441 ;
    dcterms:description "Laboratory: 24 hours total, project" ;
    vivo:courseCredits 4 ;
    vivo:hasSubjectArea "SOEN" .

roboprof_data:SPAN_200 a vivo:Course ;
    dbo:name "Introductory Spanish: Intensive" ;
    dbo:number 200 ;
    dcterms:description "lab work" ;
    vivo:courseCredits 4 ;
    vivo:hasSubjectArea "SPAN" .

roboprof_data:SPAN_201 a vivo:Course ;
    dbo:name "Introductory Spanish I" ;
    dbo:number 201 ;
    dcterms:description "lab work" ;
    vivo:courseCredits 3 ;
    vivo:hasSubjectArea "SPAN" .

roboprof_data:SPAN_202 a vivo:Course ;
    dbo:name "Introductory Spanish II" ;
    dbo:number 202 ;
    dcterms:description "lab work" ;
    vivo:courseCredits 3 ;
    vivo:hasSubjectArea "SPAN" .

roboprof_data:SPAN_240 a vivo:Course ;
    dbo:name "Intermediate Spanish: Intensive Course " ;
    dbo:number 240 ;
    dcterms:description "lab work" ;
    vivo:courseCredits 3 ;
    vivo:hasSubjectArea "SPAN" .

roboprof_data:SSDB_220 a vivo:Course ;
    dbo:name "Introduction to Theories of Sexuality" ;
    dbo:number 220 ;
    dcterms:description "This course is a multidisciplinary introduction to the central problems in the study of sexuality. " ;
    vivo:courseCredits 3 ;
    vivo:hasSubjectArea "SSDB" .

roboprof_data:SSDB_275 a vivo:Course ;
    dbo:name "Introduction to Sexuality Research" ;
    dbo:number 275 ;
    dcterms:description "This course surveys interdisciplinary approaches to research in sexuality within the humanities, arts and social sciences. The course considers different research methodologies in sexuality research, with opportunities to apply multiple methods." ;
    vivo:courseCredits 4 ;
    vivo:hasSubjectArea "SSDB" .

roboprof_data:SSDB_425 a vivo:Course ;
    dbo:name "Ethics and Community Engagement" ;
    dbo:number 425 ;
    dcterms:description "This course examines the ethics, practices, and processes of working within and alongside of communities. Examining both theoretical and practical texts, case studies, and site-visits in the area of feminism and sexuality, the course prepares students to enter into the Practicum experience." ;
    vivo:courseCredits 4 ;
    vivo:hasSubjectArea "SSDB" .

roboprof_data:SSDB_426 a vivo:Course ;
    dbo:name "Practicum" ;
    dbo:number 426 ;
    dcterms:description "This course offers a 100-hour field experience over the course of one semester. The course involves a fieldwork project." ;
    vivo:courseCredits 4 ;
    vivo:hasSubjectArea "SSDB" .

roboprof_data:SSDB_428 a vivo:Course ;
    dbo:name "Independent Study" ;
    dbo:number 428 ;
    dcterms:description "This course provides the opportunity for an independent study in which the student may explore, from a feminist and intersectional perspective, a specific topic within the interdisciplinary field of sexuality." ;
    vivo:courseCredits 3 ;
    vivo:hasSubjectArea "SSDB" .

roboprof_data:SSDB_492 a vivo:Course ;
    dbo:name "Seminar in Advanced Topics in Sexuality I" ;
    dbo:number 492 ;
    dcterms:description "This seminar is designed to provide a setting for concentrated learning and an opportunity for advanced feminist and intersectional study on a research topic in sexuality." ;
    vivo:courseCredits 3 ;
    vivo:hasSubjectArea "SSDB" .

roboprof_data:STAT_280 a vivo:Course ;
    dbo:name "Introduction to Statistical Programming" ;
    dbo:number 280 ;
    dcterms:description "Introduction to statistical programming and computational statistics using the R programming language." ;
    vivo:courseCredits 4 ;
    vivo:hasSubjectArea "STAT" .

roboprof_data:STAT_287 a vivo:Course ;
    dbo:name "Statistics Lab I" ;
    dbo:number 287 ;
    dcterms:description "Lab" ;
    vivo:courseCredits 4 ;
    vivo:hasSubjectArea "STAT" .

roboprof_data:STAT_380 a vivo:Course ;
    dbo:name "Statistical Learning" ;
    dbo:number 380 ;
    dcterms:description "Introduction to methods in statistical/machine learning, computer programming, projects using data" ;
    vivo:courseCredits 4 ;
    vivo:hasSubjectArea "STAT" .

roboprof_data:STAT_388 a vivo:Course ;
    dbo:name "Statistics Lab II" ;
    dbo:number 388 ;
    dcterms:description "Lab" ;
    vivo:courseCredits 3 ;
    vivo:hasSubjectArea "STAT" .

roboprof_data:STAT_460 a vivo:Course ;
    dbo:name "Time Series and Forecasting" ;
    dbo:number 460 ;
    dcterms:description "Analysis of time series data using statistical software" ;
    vivo:courseCredits 3 ;
    vivo:hasSubjectArea "STAT" .

roboprof_data:STAT_461 a vivo:Course ;
    dbo:name "Statistical Simulation" ;
    dbo:number 461 ;
    dcterms:description "Simulations" ;
    vivo:courseCredits 3 ;
    vivo:hasSubjectArea "STAT" .

roboprof_data:STAT_480 a vivo:Course ;
    dbo:name "Statistical Consulting and Data Analysis" ;
    dbo:number 480 ;
    dcterms:description "Statistical software (SAS) projects using data" ;
    vivo:courseCredits 4 ;
    vivo:hasSubjectArea "STAT" .

roboprof_data:STAT_497 a vivo:Course ;
    dbo:name "Topics in Statistics (Topic in 2020, 2021 - Reinforcement Learning)" ;
    dbo:number 497 ;
    dcterms:description "Reinforcement Learning - Projects with real world applications, computer programming" ;
    vivo:courseCredits 3 ;
    vivo:hasSubjectArea "STAT" .

roboprof_data:TESL_201 a vivo:Course ;
    dbo:name "Introduction to Teaching English as a Second Language" ;
    dbo:number 201 ;
    dcterms:description "Project-based activities, apply course concepts & put teaching skills into practice" ;
    vivo:courseCredits 3 ;
    vivo:hasSubjectArea "TESL" .

roboprof_data:TESL_221 a vivo:Course ;
    dbo:name "Phonology for Teachers" ;
    dbo:number 221 ;
    dcterms:description "This course includes a practice component, called pronunciation tutorials. During this practical component of the course, students meet with a non-native speaker, learner of English as a second language (typically, an international student at Concordia), conduct an assessment of the learner's pronunciation skills, and design and implement a brief pronunciation course." ;
    vivo:courseCredits 3 ;
    vivo:hasSubjectArea "TESL" .

roboprof_data:TESL_231 a vivo:Course ;
    dbo:name "Modern English Grammar" ;
    dbo:number 231 ;
    dcterms:description "Practical teaching assignments based on ESL speech and writing samples" ;
    vivo:courseCredits 3 ;
    vivo:hasSubjectArea "TESL" .

roboprof_data:TESL_324 a vivo:Course ;
    dbo:name "Methodology I" ;
    dbo:number 324 ;
    dcterms:description "NaN"^^xsd:double ;
    vivo:courseCredits 3 ;
    vivo:hasSubjectArea "TESL" .

roboprof_data:TESL_326 a vivo:Course ;
    dbo:name "TESL Pedagogy: General" ;
    dbo:number 326 ;
    dcterms:description "Minimum 20 hours observing, teaching & assisting in adult ESL classes, classroom-based projects" ;
    vivo:courseCredits 4 ;
    vivo:hasSubjectArea "TESL" .

roboprof_data:TESL_330 a vivo:Course ;
    dbo:name "Computers in Language Learning" ;
    dbo:number 330 ;
    dcterms:description "Conceptualize, design and assess computer-based materials (including websites, online materials, digital games, virtual learning environments, etc.); develop a computer-assisted language learning curriculum;" ;
    vivo:courseCredits 4 ;
    vivo:hasSubjectArea "TESL" .

roboprof_data:TESL_331 a vivo:Course ;
    dbo:name "Grammar for Teachers" ;
    dbo:number 331 ;
    dcterms:description "Practical assignments: evaluate online grammar sources; prepare grammar lesson outlines and participate in teaching simulations. The work completed by students can be applied in their teaching careers" ;
    vivo:courseCredits 4 ;
    vivo:hasSubjectArea "TESL" .

roboprof_data:TESL_341 a vivo:Course ;
    dbo:name "Language acquisition" ;
    dbo:number 341 ;
    dcterms:description "Case studies. Hands-on workshops." ;
    vivo:courseCredits 4 ;
    vivo:hasSubjectArea "TESL" .

roboprof_data:TESL_415 a vivo:Course ;
    dbo:name "Testing, Evaluation, and Course Design" ;
    dbo:number 415 ;
    dcterms:description "Students analyze tests and rating scales, and create a set of thematic assessments for their final project." ;
    vivo:courseCredits 3 ;
    vivo:hasSubjectArea "TESL" .

roboprof_data:TESL_424 a vivo:Course ;
    dbo:name "Methodology II" ;
    dbo:number 424 ;
    dcterms:description "Conceptualize, create and assess pedagogical materials involving reading and writing (including lesson plans, activities, textbooks, virtual learning environments, website, games, etc.)" ;
    vivo:courseCredits 3 ;
    vivo:hasSubjectArea "TESL" .

roboprof_data:TESL_426 a vivo:Course ;
    dbo:name "Primary Pedagogy" ;
    dbo:number 426 ;
    dcterms:description "Games/role-plays. Case studies. Hands-on workshops." ;
    vivo:courseCredits 3 ;
    vivo:hasSubjectArea "TESL" .

roboprof_data:TESL_427 a vivo:Course ;
    dbo:name "Secondary Pedagogy" ;
    dbo:number 427 ;
    dcterms:description "Games/role-plays. Case studies. Hands-on workshops." ;
    vivo:courseCredits 4 ;
    vivo:hasSubjectArea "TESL" .

roboprof_data:TESL_433 a vivo:Course ;
    dbo:name "Practicum" ;
    dbo:number 433 ;
    dcterms:description "Observation of ESL classes taught by experienced teachers, lesson planning and evaluation of own's teaching style" ;
    vivo:courseCredits 3 ;
    vivo:hasSubjectArea "TESL" .

roboprof_data:TESL_471 a vivo:Course ;
    dbo:name "English Language Arts: Secondary" ;
    dbo:number 471 ;
    dcterms:description "Case studies. Hands-on workshops." ;
    vivo:courseCredits 4 ;
    vivo:hasSubjectArea "TESL" .

roboprof_data:TESL_488 a vivo:Course ;
    dbo:name "Internship Seminar" ;
    dbo:number 488 ;
    dcterms:description "Develop self-regulated learning of that of a professional in education. Develop the ability to make links between the knowledge acquired during the BEd & practice in the field." ;
    vivo:courseCredits 4 ;
    vivo:hasSubjectArea "TESL" .

roboprof_data:THEO_234 a vivo:Course ;
    dbo:name "Pilgrim Bodies, Sacred Journeys" ;
    dbo:number 234 ;
    dcterms:description "Individual and group fieldwork" ;
    vivo:courseCredits 3 ;
    vivo:hasSubjectArea "THEO" .

roboprof_data:THEO_243 a vivo:Course ;
    dbo:name "Indigenous Spirituality" ;
    dbo:number 243 ;
    dcterms:description "Group fieldwork" ;
    vivo:courseCredits 3 ;
    vivo:hasSubjectArea "THEO" .

roboprof_data:THEO_404 a vivo:Course ;
    dbo:name "Practicum in Pastoral  Care" ;
    dbo:number 404 ;
    dcterms:description "Internship and field exploration focused on an area in pastoral care" ;
    vivo:courseCredits 4 ;
    vivo:hasSubjectArea "THEO" .

roboprof_data:THEO_692 a vivo:Course ;
    dbo:name "Applied Project in Theology" ;
    dbo:number 692 ;
    dcterms:description "Practicum" ;
    vivo:courseCredits 3 ;
    vivo:hasSubjectArea "THEO" .

roboprof_data:URBS_250 a vivo:Course ;
    dbo:name "Representation Methods in Urban Studies" ;
    dbo:number 250 ;
    dcterms:description "Laboratory" ;
    vivo:courseCredits 3 ;
    vivo:hasSubjectArea "URBS" .

roboprof_data:URBS_260 a vivo:Course ;
    dbo:name "Analytical Methods in Urban Studies" ;
    dbo:number 260 ;
    dcterms:description "Laboratory" ;
    vivo:courseCredits 4 ;
    vivo:hasSubjectArea "URBS" .

roboprof_data:URBS_333 a vivo:Course ;
    dbo:name "Urban Laboratory" ;
    dbo:number 333 ;
    dcterms:description "First-hand knowledge, plans are evaluated by the peer group and experts in the field" ;
    vivo:courseCredits 3 ;
    vivo:hasSubjectArea "URBS" .

roboprof_data:URBS_335 a vivo:Course ;
    dbo:name "Geographic Information Systems" ;
    dbo:number 335 ;
    dcterms:description "Real-world problem, Laboratory" ;
    vivo:courseCredits 4 ;
    vivo:hasSubjectArea "URBS" .

roboprof_data:URBS_337 a vivo:Course ;
    dbo:name "Urban Agriculture" ;
    dbo:number 337 ;
    dcterms:description "Field work - working in community gardens" ;
    vivo:courseCredits 4 ;
    vivo:hasSubjectArea "URBS" .

roboprof_data:URBS_362 a vivo:Course ;
    dbo:name "Quantitative Research Methods" ;
    dbo:number 362 ;
    dcterms:description "Laboratory" ;
    vivo:courseCredits 3,
        4 ;
    vivo:hasSubjectArea "URBS" .

roboprof_data:URBS_420 a vivo:Course ;
    dbo:name "The Social and Cultural Geographies of Montreal" ;
    dbo:number 420 ;
    dcterms:description "Field trips" ;
    vivo:courseCredits 3 ;
    vivo:hasSubjectArea "URBS" .

roboprof_data:URBS_433 a vivo:Course ;
    dbo:name "Advanced Urban Laboratory" ;
    dbo:number 433 ;
    dcterms:description "Simulations" ;
    vivo:courseCredits 3 ;
    vivo:hasSubjectArea "URBS" .

roboprof_data:URBS_483 a vivo:Course ;
    dbo:name "Directed Studies / Practicum in Urban Planning I" ;
    dbo:number 483 ;
    dcterms:description "120 hours with a private or public institution, or community interest group" ;
    vivo:courseCredits 4 ;
    vivo:hasSubjectArea "URBS" .

roboprof_data:URBS_484 a vivo:Course ;
    dbo:name "Directed Studies / Practicum in Urban Planning II" ;
    dbo:number 484 ;
    dcterms:description "120 hours with a private or public institution, or community interest group" ;
    vivo:courseCredits 4 ;
    vivo:hasSubjectArea "URBS" .

roboprof_data:VDEO_350 a vivo:Course ;
    dbo:name "Video History and Theory" ;
    dbo:number 350 ;
    dcterms:description "A survey lecture course introducing the history and theory of art video practice since its inception in the 1960s." ;
    vivo:courseCredits 3 ;
    vivo:hasSubjectArea "VDEO" .

roboprof_data:WSDB_291 a vivo:Course ;
    dbo:name "Introduction to Contemporary Concerns in Womens Studies" ;
    dbo:number 291 ;
    dcterms:description "This course explores a range of current issues and debates within feminism. Using interdisciplinary feminist theories that consider how systems of power such as patriarchy, capitalism, racism, and heterosexism constitute one another, it examines particular local and global topics of interest/concern which may include health, education, work, violence against women, globalization, militarism, media and cultural representations, families, and feminist activism." ;
    vivo:courseCredits 4 ;
    vivo:hasSubjectArea "WSDB " .

roboprof_data:WSDB_292 a vivo:Course ;
    dbo:name "Feminism and Research Methods" ;
    dbo:number 292 ;
    dcterms:description "Practical, hands-on exercises" ;
    vivo:courseCredits 3 ;
    vivo:hasSubjectArea "WSDB" .

roboprof_data:WSDB_391 a vivo:Course ;
    dbo:name "Health Issues: Feminist Perspectives" ;
    dbo:number 391 ;
    dcterms:description "This course presents feminist, intersectional, postcolonialist, poststructuralist and queer examinations of a variety of womens health issues." ;
    vivo:courseCredits 4 ;
    vivo:hasSubjectArea "WSDB " .

roboprof_data:WSDB_491 a vivo:Course ;
    dbo:name "Feminist Perspectives on Culture" ;
    dbo:number 491 ;
    dcterms:description "This seminar explores the central concepts and theories in feminist cultural studies, as they inform feminist, postcolonial, queer, and poststructuralist understandings of culture." ;
    vivo:courseCredits 4 ;
    vivo:hasSubjectArea "WSDB" .

roboprof_data:WSDB_494 a vivo:Course ;
    dbo:name "Advanced Tutorial in Womens Studies" ;
    dbo:number 494 ;
    dcterms:description "Tutorial on topic not covered under normal curriculum, independent research ability required" ;
    vivo:courseCredits 4 ;
    vivo:hasSubjectArea "WSDB" .

<file:///./dataset/Lab%20Content/COMP%206741/Lab%20Material/Lab%201.pdf> a roboprof:LabMaterial ;
    dbo:name "Lab 1.pdf" .

<file:///./dataset/Lecture%20Content/COMP%206741/OtherMaterial/BagOfWords.pdf> a roboprof:OtherMaterial ;
    dbo:name "BagOfWords.pdf" .

<http://roboprof.ca/data/COMP_6741_A+> a roboprof:InitialGrade ;
    roboprof:gradeInCourse roboprof_data:COMP_6741 ;
    roboprof:gradeValue "A+" .

<file:///./dataset/Lecture%20Content/COMP%206461/OtherMaterial/NetworkLayer.pdf> a roboprof:OtherMaterial ;
    dbo:name "NetworkLayer.pdf" .

<file:///./dataset/Lecture%20Content/COMP%206741/Worksheets/worksheet02.pdf> a roboprof:Worksheet ;
    dbo:name "worksheet02.pdf" .

<file:///./dataset/Lecture%20Content/COMP%206741/Worksheets/worksheet04.pdf> a roboprof:Worksheet ;
    dbo:name "worksheet04.pdf" .

roboprof_data:COMP_6411 a vivo:Course ;
    dbo:name "Comparative Study of Programming Languages" ;
    dbo:number 6411 ;
    dcterms:description "Laboratory: 24 hours total, project" ;
    vivo:courseCredits 4 ;
    vivo:hasSubjectArea "COMP" .

roboprof_data:COMP_6421 a vivo:Course ;
    dbo:name "Compiler Design" ;
    dbo:number 6421 ;
    dcterms:description "Laboratory: 24 hours total, project" ;
    vivo:courseCredits 4 ;
    vivo:hasSubjectArea "COMP" .

roboprof_data:COMP_6481 a vivo:Course ;
    dbo:name "Programming and Problem Solving" ;
    dbo:number 6481 ;
    dcterms:description "Laboratory: 36 hours total" ;
    vivo:courseCredits 4 ;
    vivo:hasSubjectArea "COMP" .

roboprof_data:COMP_6551 a vivo:Course ;
    dbo:name "Algorithm Design & Techniques" ;
    dbo:number 6551 ;
    dcterms:description "Laboratory: 24 hours total, project" ;
    vivo:courseCredits 4 ;
    vivo:hasSubjectArea "COMP" .

roboprof_data:COMP_6721 a vivo:Course ;
    dbo:name "Applied Artificial Intelligence" ;
    dbo:number 6721 ;
    dcterms:description "Laboratory: 24 hours total, project" ;
    vivo:courseCredits 4 ;
    vivo:hasSubjectArea "COMP" .

roboprof_data:COMP_6731 a vivo:Course ;
    dbo:name "Pattern Recognition" ;
    dbo:number 6731 ;
    dcterms:description "Laboratory: 24 hours total, project" ;
    vivo:courseCredits 4 ;
    vivo:hasSubjectArea "COMP" .

roboprof_data:COMP_6761 a vivo:Course ;
    dbo:name "Advanced Computer Graphics" ;
    dbo:number 6761 ;
    dcterms:description "Laboratory: 24 hours total, project" ;
    vivo:courseCredits 4 ;
    vivo:hasSubjectArea "COMP" .

roboprof_data:COMP_6771 a vivo:Course ;
    dbo:name "Image Processing" ;
    dbo:number 6771 ;
    dcterms:description "Laboratory: 24 hours total, project" ;
    vivo:courseCredits 4 ;
    vivo:hasSubjectArea "COMP" .

roboprof_data:COMP_6791 a vivo:Course ;
    dbo:name "Information Retrieval and Web Search" ;
    dbo:number 6791 ;
    dcterms:description "Laboratory: 24 hours total, project" ;
    vivo:courseCredits 4 ;
    vivo:hasSubjectArea "COMP" .

roboprof_data:ConcordiaUniversity a dbo:University ;
    dbo:name "Concordia University" ;
    roboprof:offersCourse roboprof_data:ACCO_330,
        roboprof_data:ACCO_355,
        roboprof_data:ACCO_400,
        roboprof_data:ACCO_420,
        roboprof_data:ACCO_425,
        roboprof_data:ACCO_435,
        roboprof_data:ACCO_455,
        roboprof_data:ACCO_465,
        roboprof_data:ACCO_495,
        roboprof_data:ACCO_650,
        roboprof_data:ACCO_651,
        roboprof_data:ACCO_652,
        roboprof_data:ACCO_653,
        roboprof_data:ACCO_654,
        roboprof_data:ACCO_655,
        roboprof_data:ACCO_656,
        roboprof_data:ACCO_657,
        roboprof_data:ACCO_658,
        roboprof_data:ACCO_659,
        roboprof_data:ACTT_201,
        roboprof_data:ACTT_202,
        roboprof_data:ACTT_209,
        roboprof_data:ACTT_210,
        roboprof_data:ACTT_211,
        roboprof_data:ACTT_231,
        roboprof_data:ACTT_321,
        roboprof_data:ACTT_325,
        roboprof_data:ACTT_331,
        roboprof_data:ACTT_332,
        roboprof_data:ACTT_355,
        roboprof_data:ACTT_358,
        roboprof_data:ACTT_360,
        roboprof_data:ACTT_362,
        roboprof_data:ACTT_370,
        roboprof_data:ACTT_372,
        roboprof_data:ACTT_398,
        roboprof_data:ACTT_399,
        roboprof_data:ACTT_432,
        roboprof_data:ACTT_435,
        roboprof_data:ACTT_436,
        roboprof_data:ACTT_440,
        roboprof_data:ACTT_450,
        roboprof_data:ACTT_455,
        roboprof_data:ACTT_458,
        roboprof_data:ACTT_460,
        roboprof_data:ACTT_465,
        roboprof_data:ACTT_480,
        roboprof_data:ACTT_481,
        roboprof_data:ACTT_498,
        roboprof_data:ACTT_499,
        roboprof_data:ACTU_286,
        roboprof_data:ACTU_386,
        roboprof_data:ACTU_486,
        roboprof_data:ADED_230,
        roboprof_data:ADED_344,
        roboprof_data:ADED_345,
        roboprof_data:ADED_370,
        roboprof_data:AERO_201,
        roboprof_data:AERO_371,
        roboprof_data:AERO_390,
        roboprof_data:AERO_455,
        roboprof_data:AERO_465,
        roboprof_data:AERO_480,
        roboprof_data:AERO_481,
        roboprof_data:AERO_482,
        roboprof_data:AERO_490,
        roboprof_data:AHSC_225,
        roboprof_data:AHSC_232,
        roboprof_data:AHSC_260,
        roboprof_data:AHSC_322,
        roboprof_data:AHSC_332,
        roboprof_data:AHSC_350,
        roboprof_data:AHSC_360,
        roboprof_data:AHSC_361,
        roboprof_data:AHSC_371,
        roboprof_data:AHSC_384,
        roboprof_data:AHSC_410,
        roboprof_data:AHSC_422,
        roboprof_data:AHSC_425,
        roboprof_data:AHSC_432,
        roboprof_data:AHSC_435,
        roboprof_data:AHSC_436,
        roboprof_data:AHSC_437,
        roboprof_data:AHSC_438,
        roboprof_data:AHSC_439,
        roboprof_data:AHSC_442,
        roboprof_data:AHSC_443,
        roboprof_data:AHSC_444,
        roboprof_data:AHSC_451,
        roboprof_data:AHSC_456,
        roboprof_data:AHSC_470,
        roboprof_data:AHSC_490,
        roboprof_data:AHSC_491,
        roboprof_data:AHSC_498,
        roboprof_data:AHSC_510,
        roboprof_data:AHSC_525,
        roboprof_data:AHSC_527,
        roboprof_data:AHSC_530,
        roboprof_data:AHSC_533,
        roboprof_data:AHSC_537,
        roboprof_data:AHSC_538,
        roboprof_data:AHSC_599,
        roboprof_data:AHSC_610,
        roboprof_data:AHSC_620,
        roboprof_data:AHSC_631,
        roboprof_data:AHSC_632,
        roboprof_data:AHSC_660,
        roboprof_data:AHSC_670,
        roboprof_data:AHSC_675,
        roboprof_data:AHSC_680,
        roboprof_data:AHSC_685,
        roboprof_data:AHSC_690,
        roboprof_data:AHSC_691,
        roboprof_data:AHSC_698,
        roboprof_data:ANTH_315,
        roboprof_data:ANTH_450,
        roboprof_data:APLI_601,
        roboprof_data:APLI_604,
        roboprof_data:APLI_610,
        roboprof_data:APLI_616,
        roboprof_data:APLI_623,
        roboprof_data:APLI_626,
        roboprof_data:APLI_630,
        roboprof_data:APLI_634,
        roboprof_data:APLI_635,
        roboprof_data:APLI_636,
        roboprof_data:APLI_644,
        roboprof_data:APLI_647,
        roboprof_data:APLI_660,
        roboprof_data:ARTE_201,
        roboprof_data:ARTT_470,
        roboprof_data:ARTT_471,
        roboprof_data:ARTT_472,
        roboprof_data:ARTX_201,
        roboprof_data:ARTX_280,
        roboprof_data:ARTX_380,
        roboprof_data:ARTX_398,
        roboprof_data:ARTX_399,
        roboprof_data:ARTX_480,
        roboprof_data:ARTX_490,
        roboprof_data:ARTX_491,
        roboprof_data:ARTX_492,
        roboprof_data:BCEE_371,
        roboprof_data:BIOL_201,
        roboprof_data:BIOL_227,
        roboprof_data:BIOL_322,
        roboprof_data:BIOL_330,
        roboprof_data:BIOL_337,
        roboprof_data:BIOL_340,
        roboprof_data:BIOL_351,
        roboprof_data:BIOL_368,
        roboprof_data:BIOL_382,
        roboprof_data:BIOL_398,
        roboprof_data:BIOL_422,
        roboprof_data:BIOL_423,
        roboprof_data:BIOL_450,
        roboprof_data:BIOL_451,
        roboprof_data:BIOL_466,
        roboprof_data:BIOL_480,
        roboprof_data:BIOL_486,
        roboprof_data:BIOL_490,
        roboprof_data:BIOL_498,
        roboprof_data:BIOL_510,
        roboprof_data:BIOL_515,
        roboprof_data:BIOL_516,
        roboprof_data:BIOL_524,
        roboprof_data:BIOL_614,
        roboprof_data:BIOL_622,
        roboprof_data:BIOL_630,
        roboprof_data:BIOL_631,
        roboprof_data:BIOL_670,
        roboprof_data:BIOL_680,
        roboprof_data:BIOL_689,
        roboprof_data:BIOL_801,
        roboprof_data:BIOL_802,
        roboprof_data:BLDG_365,
        roboprof_data:BLDG_366,
        roboprof_data:BLDG_371,
        roboprof_data:BLDG_390,
        roboprof_data:BLDG_463,
        roboprof_data:BLDG_471,
        roboprof_data:BLDG_476,
        roboprof_data:BLDG_490,
        roboprof_data:BLDG_492,
        roboprof_data:BLDG_6071,
        roboprof_data:BLDG_6111,
        roboprof_data:BLDG_6151,
        roboprof_data:BLDG_6221,
        roboprof_data:BLDG_6231,
        roboprof_data:BLDG_6241,
        roboprof_data:BLDG_6561,
        roboprof_data:BLDG_6571,
        roboprof_data:BLDG_6581,
        roboprof_data:BLDG_6591,
        roboprof_data:BLDG_6601,
        roboprof_data:BLDG_6611,
        roboprof_data:BLDG_6621,
        roboprof_data:BLDG_6641,
        roboprof_data:BLDG_6651,
        roboprof_data:BLDG_6661,
        roboprof_data:BLDG_6701,
        roboprof_data:BLDG_6711,
        roboprof_data:BLDG_6721,
        roboprof_data:BLDG_6731,
        roboprof_data:BLDG_6741,
        roboprof_data:BLDG_6751,
        roboprof_data:BLDG_6761,
        roboprof_data:BLDG_6781,
        roboprof_data:BLDG_6791,
        roboprof_data:BLDG_6801,
        roboprof_data:BLDG_6851,
        roboprof_data:BLDG_6861,
        roboprof_data:BLDG_6951,
        roboprof_data:BLDG_7401,
        roboprof_data:BLDG_7511,
        roboprof_data:BLDG_7521,
        roboprof_data:BLDG_7601,
        roboprof_data:BLDG_7811,
        roboprof_data:BLDG_7831,
        roboprof_data:BLDG_7841,
        roboprof_data:BLDG_7861,
        roboprof_data:BLDG_7871,
        roboprof_data:BSTA_445,
        roboprof_data:BSTA_450,
        roboprof_data:BSTA_477,
        roboprof_data:BSTA_478,
        roboprof_data:BTM_430,
        roboprof_data:BTM_480,
        roboprof_data:BTM_481,
        roboprof_data:BTM_495,
        roboprof_data:BTM_496,
        roboprof_data:BTM_633,
        roboprof_data:CART_451,
        roboprof_data:CATA_262,
        roboprof_data:CATA_263,
        roboprof_data:CATA_337,
        roboprof_data:CATA_339,
        roboprof_data:CATA_348,
        roboprof_data:CATA_365,
        roboprof_data:CATA_437,
        roboprof_data:CATA_439,
        roboprof_data:CATA_441,
        roboprof_data:CATA_462,
        roboprof_data:CATA_475,
        roboprof_data:CATA_485,
        roboprof_data:CATA_495,
        roboprof_data:CERA_201,
        roboprof_data:CERA_230,
        roboprof_data:CERA_330,
        roboprof_data:CERA_391,
        roboprof_data:CERA_392,
        roboprof_data:CERA_398,
        roboprof_data:CERA_399,
        roboprof_data:CERA_430,
        roboprof_data:CERA_450,
        roboprof_data:CERA_451,
        roboprof_data:CERA_452,
        roboprof_data:CERA_498,
        roboprof_data:CERA_499,
        roboprof_data:CHEM_205,
        roboprof_data:CHEM_206,
        roboprof_data:CHEM_212,
        roboprof_data:CHEM_217,
        roboprof_data:CHEM_218,
        roboprof_data:CHEM_221,
        roboprof_data:CHEM_222,
        roboprof_data:CHEM_235,
        roboprof_data:CHEM_241,
        roboprof_data:CHEM_242,
        roboprof_data:CHEM_271,
        roboprof_data:CHEM_293,
        roboprof_data:CHEM_312,
        roboprof_data:CHEM_324,
        roboprof_data:CHEM_325,
        roboprof_data:CHEM_333,
        roboprof_data:CHEM_335,
        roboprof_data:CHEM_341,
        roboprof_data:CHEM_375,
        roboprof_data:CHEM_419,
        roboprof_data:CHEM_431,
        roboprof_data:CHEM_436,
        roboprof_data:CHEM_450,
        roboprof_data:CHEM_477,
        roboprof_data:CHEM_487,
        roboprof_data:CHEM_614,
        roboprof_data:CHEM_631,
        roboprof_data:CHEM_651,
        roboprof_data:CHEM_692,
        roboprof_data:CHST_605,
        roboprof_data:CHST_606,
        roboprof_data:CHST_608,
        roboprof_data:CHST_618,
        roboprof_data:CIVI_231,
        roboprof_data:CIVI_321,
        roboprof_data:CIVI_361,
        roboprof_data:CIVI_381,
        roboprof_data:CIVI_382,
        roboprof_data:CIVI_390,
        roboprof_data:CIVI_432,
        roboprof_data:CIVI_440,
        roboprof_data:CIVI_453,
        roboprof_data:CIVI_454,
        roboprof_data:CIVI_465,
        roboprof_data:CIVI_469,
        roboprof_data:CIVI_484,
        roboprof_data:CIVI_6001,
        roboprof_data:CIVI_6011,
        roboprof_data:CIVI_6021,
        roboprof_data:CIVI_6031,
        roboprof_data:CIVI_6051,
        roboprof_data:CIVI_6061,
        roboprof_data:CIVI_6071,
        roboprof_data:CIVI_6101,
        roboprof_data:CIVI_6301,
        roboprof_data:CIVI_6331,
        roboprof_data:CIVI_6381,
        roboprof_data:CIVI_6401,
        roboprof_data:CIVI_6411,
        roboprof_data:CIVI_6441,
        roboprof_data:CIVI_6451,
        roboprof_data:CIVI_6461,
        roboprof_data:CIVI_6481,
        roboprof_data:CIVI_6491,
        roboprof_data:CIVI_6501,
        roboprof_data:CIVI_6521,
        roboprof_data:CIVI_6531,
        roboprof_data:CIVI_6541,
        roboprof_data:CIVI_6601,
        roboprof_data:CIVI_6611,
        roboprof_data:CIVI_6621,
        roboprof_data:CIVI_6631,
        roboprof_data:CIVI_6641,
        roboprof_data:CIVI_6651,
        roboprof_data:CIVI_6661,
        roboprof_data:CIVI_6671,
        roboprof_data:CIVI_6681,
        roboprof_data:CIVI_6691,
        roboprof_data:CIVI_6711,
        roboprof_data:CIVI_7001,
        roboprof_data:CIVI_7031,
        roboprof_data:CIVI_7101,
        roboprof_data:CIVI_7111,
        roboprof_data:CIVI_7121,
        roboprof_data:CIVI_7311,
        roboprof_data:CIVI_7401,
        roboprof_data:CIVI_7901,
        roboprof_data:CLAS_370,
        roboprof_data:CLAS_383,
        roboprof_data:CLAS_384,
        roboprof_data:CLAS_391,
        roboprof_data:CLAS_392,
        roboprof_data:CLAS_410,
        roboprof_data:CLAS_411,
        roboprof_data:CLAS_420,
        roboprof_data:CLAS_421,
        roboprof_data:CLAS_460,
        roboprof_data:CLAS_470,
        roboprof_data:CLAS_490,
        roboprof_data:COEN_212,
        roboprof_data:COEN_311,
        roboprof_data:COEN_313,
        roboprof_data:COEN_315,
        roboprof_data:COEN_316,
        roboprof_data:COEN_317,
        roboprof_data:COEN_345,
        roboprof_data:COEN_346,
        roboprof_data:COEN_390,
        roboprof_data:COEN_421,
        roboprof_data:COEN_445,
        roboprof_data:COEN_451,
        roboprof_data:COEN_490,
        roboprof_data:COEN_6211,
        roboprof_data:COEN_6311,
        roboprof_data:COEN_6312,
        roboprof_data:COEN_6313,
        roboprof_data:COEN_6321,
        roboprof_data:COEN_6331,
        roboprof_data:COEN_6341,
        roboprof_data:COEN_6501,
        roboprof_data:COEN_6511,
        roboprof_data:COEN_6521,
        roboprof_data:COEN_6531,
        roboprof_data:COEN_6541,
        roboprof_data:COEN_6551,
        roboprof_data:COEN_6611,
        roboprof_data:COEN_6711,
        roboprof_data:COEN_6721,
        roboprof_data:COEN_6741,
        roboprof_data:COEN_7311,
        roboprof_data:COEN_7741,
        roboprof_data:COMM_205,
        roboprof_data:COMM_401,
        roboprof_data:COMM_499,
        roboprof_data:COMP_107,
        roboprof_data:COMP_108,
        roboprof_data:COMP_207,
        roboprof_data:COMP_208,
        roboprof_data:COMP_248,
        roboprof_data:COMP_249,
        roboprof_data:COMP_345,
        roboprof_data:COMP_346,
        roboprof_data:COMP_353,
        roboprof_data:COMP_354,
        roboprof_data:COMP_371,
        roboprof_data:COMP_376,
        roboprof_data:COMP_426,
        roboprof_data:COMP_428,
        roboprof_data:COMP_442,
        roboprof_data:COMP_444,
        roboprof_data:COMP_445,
        roboprof_data:COMP_451,
        roboprof_data:COMP_472,
        roboprof_data:COMP_473,
        roboprof_data:COMP_474,
        roboprof_data:COMP_476,
        roboprof_data:COMP_477,
        roboprof_data:COMP_478,
        roboprof_data:COMP_479,
        roboprof_data:COMP_490,
        roboprof_data:COMP_492,
        roboprof_data:COMP_5201,
        roboprof_data:COMP_5361,
        roboprof_data:COMP_5461,
        roboprof_data:COMP_5511,
        roboprof_data:COMP_5541,
        roboprof_data:COMP_6231,
        roboprof_data:COMP_628,
        roboprof_data:COMP_6311,
        roboprof_data:COMP_6321,
        roboprof_data:COMP_6331,
        roboprof_data:COMP_6411,
        roboprof_data:COMP_6421,
        roboprof_data:COMP_6461,
        roboprof_data:COMP_6481,
        roboprof_data:COMP_6521,
        roboprof_data:COMP_6551,
        roboprof_data:COMP_6721,
        roboprof_data:COMP_6731,
        roboprof_data:COMP_6741,
        roboprof_data:COMP_6761,
        roboprof_data:COMP_6771,
        roboprof_data:COMP_6791,
        roboprof_data:COMS_274,
        roboprof_data:COMS_276,
        roboprof_data:COMS_284,
        roboprof_data:COMS_307,
        roboprof_data:COMS_324,
        roboprof_data:COMS_361,
        roboprof_data:COMS_374,
        roboprof_data:COMS_376,
        roboprof_data:COMS_384,
        roboprof_data:COMS_393,
        roboprof_data:COMS_407,
        roboprof_data:COMS_475,
        roboprof_data:COMS_477,
        roboprof_data:COMS_484,
        roboprof_data:COMS_493,
        roboprof_data:COMS_506,
        roboprof_data:COMS_507,
        roboprof_data:COMS_513,
        roboprof_data:COMS_562,
        roboprof_data:COMS_569,
        roboprof_data:COMS_570,
        roboprof_data:COMS_606,
        roboprof_data:COMS_684,
        roboprof_data:COMS_876,
        roboprof_data:DANC_201,
        roboprof_data:DANC_205,
        roboprof_data:DANC_240,
        roboprof_data:DANC_301,
        roboprof_data:DANC_305,
        roboprof_data:DANC_320,
        roboprof_data:DANC_350,
        roboprof_data:DANC_398,
        roboprof_data:DANC_401,
        roboprof_data:DANC_405,
        roboprof_data:DANC_420,
        roboprof_data:DFTT_209,
        roboprof_data:DFTT_210,
        roboprof_data:DFTT_211,
        roboprof_data:DFTT_212,
        roboprof_data:DFTT_298,
        roboprof_data:DFTT_299,
        roboprof_data:DFTT_301,
        roboprof_data:DFTT_305,
        roboprof_data:DFTT_311,
        roboprof_data:DFTT_315,
        roboprof_data:DFTT_321,
        roboprof_data:DFTT_325,
        roboprof_data:DFTT_326,
        roboprof_data:DFTT_331,
        roboprof_data:DFTT_335,
        roboprof_data:DFTT_336,
        roboprof_data:DFTT_337,
        roboprof_data:DFTT_341,
        roboprof_data:DFTT_345,
        roboprof_data:DFTT_350,
        roboprof_data:DFTT_351,
        roboprof_data:DFTT_370,
        roboprof_data:DFTT_371,
        roboprof_data:DFTT_398,
        roboprof_data:DFTT_399,
        roboprof_data:DFTT_401,
        roboprof_data:DFTT_405,
        roboprof_data:DFTT_450,
        roboprof_data:DFTT_451,
        roboprof_data:DFTT_470,
        roboprof_data:DFTT_471,
        roboprof_data:DFTT_498,
        roboprof_data:DFTT_499,
        roboprof_data:DRAW_200,
        roboprof_data:DRAW_201,
        roboprof_data:DRAW_298,
        roboprof_data:DRAW_299,
        roboprof_data:DRAW_300,
        roboprof_data:DRAW_310,
        roboprof_data:DRAW_312,
        roboprof_data:DRAW_314,
        roboprof_data:DRAW_398,
        roboprof_data:DRAW_399,
        roboprof_data:DRAW_400,
        roboprof_data:DRAW_410,
        roboprof_data:DRAW_412,
        roboprof_data:DRAW_414,
        roboprof_data:DRAW_418,
        roboprof_data:DRAW_420,
        roboprof_data:DRAW_450,
        roboprof_data:DRAW_470,
        roboprof_data:DRAW_471,
        roboprof_data:DRAW_472,
        roboprof_data:DRAW_498,
        roboprof_data:DRAW_499,
        roboprof_data:EAST_203,
        roboprof_data:EAST_451,
        roboprof_data:EAST_463,
        roboprof_data:EAST_481,
        roboprof_data:EAST_482,
        roboprof_data:ECON_200,
        roboprof_data:ECON_318,
        roboprof_data:ECON_319,
        roboprof_data:ECON_324,
        roboprof_data:ECON_330,
        roboprof_data:ECON_421,
        roboprof_data:ECON_422,
        roboprof_data:ECON_423,
        roboprof_data:ECON_680,
        roboprof_data:ECON_683,
        roboprof_data:ECON_695,
        roboprof_data:ECON_696,
        roboprof_data:ECON_806,
        roboprof_data:EDUC_264,
        roboprof_data:EDUC_301,
        roboprof_data:EDUC_302,
        roboprof_data:EDUC_303,
        roboprof_data:EDUC_304,
        roboprof_data:EDUC_307,
        roboprof_data:EDUC_360,
        roboprof_data:EDUC_361,
        roboprof_data:EDUC_362,
        roboprof_data:EDUC_382,
        roboprof_data:EDUC_385,
        roboprof_data:EDUC_402,
        roboprof_data:EDUC_406,
        roboprof_data:EDUC_461,
        roboprof_data:EDUC_463,
        roboprof_data:ELEC_273,
        roboprof_data:ELEC_275,
        roboprof_data:ELEC_311,
        roboprof_data:ELEC_312,
        roboprof_data:ELEC_321,
        roboprof_data:ELEC_331,
        roboprof_data:ELEC_342,
        roboprof_data:ELEC_367,
        roboprof_data:ELEC_372,
        roboprof_data:ELEC_390,
        roboprof_data:ELEC_421,
        roboprof_data:ELEC_422,
        roboprof_data:ELEC_423,
        roboprof_data:ELEC_424,
        roboprof_data:ELEC_425,
        roboprof_data:ELEC_430,
        roboprof_data:ELEC_431,
        roboprof_data:ELEC_432,
        roboprof_data:ELEC_433,
        roboprof_data:ELEC_434,
        roboprof_data:ELEC_435,
        roboprof_data:ELEC_436,
        roboprof_data:ELEC_438,
        roboprof_data:ELEC_440,
        roboprof_data:ELEC_441,
        roboprof_data:ELEC_442,
        roboprof_data:ELEC_453,
        roboprof_data:ELEC_456,
        roboprof_data:ELEC_463,
        roboprof_data:ELEC_465,
        roboprof_data:ELEC_466,
        roboprof_data:ELEC_472,
        roboprof_data:ELEC_481,
        roboprof_data:ELEC_482,
        roboprof_data:ELEC_483,
        roboprof_data:ELEC_490,
        roboprof_data:ELEC_6041,
        roboprof_data:ELEC_6051,
        roboprof_data:ELEC_6061,
        roboprof_data:ELEC_6081,
        roboprof_data:ELEC_6091,
        roboprof_data:ELEC_6111,
        roboprof_data:ELEC_6131,
        roboprof_data:ELEC_6141,
        roboprof_data:ELEC_6151,
        roboprof_data:ELEC_6171,
        roboprof_data:ELEC_6181,
        roboprof_data:ELEC_6221,
        roboprof_data:ELEC_6231,
        roboprof_data:ELEC_6241,
        roboprof_data:ELEC_6251,
        roboprof_data:ELEC_6261,
        roboprof_data:ELEC_6271,
        roboprof_data:ELEC_6281,
        roboprof_data:ELEC_6301,
        roboprof_data:ELEC_6311,
        roboprof_data:ELEC_6341,
        roboprof_data:ELEC_6351,
        roboprof_data:ELEC_6361,
        roboprof_data:ELEC_6371,
        roboprof_data:ELEC_6381,
        roboprof_data:ELEC_6391,
        roboprof_data:ELEC_6411,
        roboprof_data:ELEC_6421,
        roboprof_data:ELEC_6431,
        roboprof_data:ELEC_6461,
        roboprof_data:ELEC_6471,
        roboprof_data:ELEC_6481,
        roboprof_data:ELEC_6491,
        roboprof_data:ELEC_6601,
        roboprof_data:ELEC_6611,
        roboprof_data:ELEC_6621,
        roboprof_data:ELEC_6631,
        roboprof_data:ELEC_6641,
        roboprof_data:ELEC_6651,
        roboprof_data:ELEC_6661,
        roboprof_data:ELEC_6831,
        roboprof_data:ELEC_6841,
        roboprof_data:ELEC_6851,
        roboprof_data:ELEC_6861,
        roboprof_data:ELEC_6871,
        roboprof_data:ELEC_6881,
        roboprof_data:ELEC_7151,
        roboprof_data:ELEC_7441,
        roboprof_data:ELEC_7451,
        roboprof_data:EMBA_610,
        roboprof_data:EMBA_611,
        roboprof_data:EMBA_612,
        roboprof_data:EMBA_621,
        roboprof_data:EMBA_625,
        roboprof_data:EMBA_630,
        roboprof_data:EMBA_631,
        roboprof_data:EMBA_632,
        roboprof_data:EMBA_633,
        roboprof_data:EMBA_635,
        roboprof_data:EMBA_640,
        roboprof_data:EMBA_645,
        roboprof_data:EMBA_676,
        roboprof_data:EMBA_690,
        roboprof_data:ENCS_272,
        roboprof_data:ENCS_282,
        roboprof_data:ENCS_393,
        roboprof_data:ENCS_483,
        roboprof_data:ENCS_484,
        roboprof_data:ENCS_485,
        roboprof_data:ENCS_5721,
        roboprof_data:ENCS_6041,
        roboprof_data:ENCS_6042,
        roboprof_data:ENCS_6043,
        roboprof_data:ENCS_6044,
        roboprof_data:ENCS_6721,
        roboprof_data:ENCS_6821,
        roboprof_data:ENCS_691,
        roboprof_data:ENCS_8511,
        roboprof_data:ENGL_215,
        roboprof_data:ENGL_224,
        roboprof_data:ENGL_225,
        roboprof_data:ENGL_226,
        roboprof_data:ENGL_227,
        roboprof_data:ENGL_342,
        roboprof_data:ENGL_347,
        roboprof_data:ENGL_348,
        roboprof_data:ENGL_384,
        roboprof_data:ENGL_396,
        roboprof_data:ENGL_414,
        roboprof_data:ENGL_415,
        roboprof_data:ENGL_416,
        roboprof_data:ENGL_417,
        roboprof_data:ENGL_428,
        roboprof_data:ENGL_429,
        roboprof_data:ENGL_470,
        roboprof_data:ENGL_474,
        roboprof_data:ENGL_480,
        roboprof_data:ENGL_601,
        roboprof_data:ENGL_636,
        roboprof_data:ENGL_637,
        roboprof_data:ENGL_670,
        roboprof_data:ENGL_671,
        roboprof_data:ENGL_672,
        roboprof_data:ENGL_673,
        roboprof_data:ENGL_674,
        roboprof_data:ENGL_802,
        roboprof_data:ENGR_107,
        roboprof_data:ENGR_108,
        roboprof_data:ENGR_201,
        roboprof_data:ENGR_202,
        roboprof_data:ENGR_207,
        roboprof_data:ENGR_208,
        roboprof_data:ENGR_290,
        roboprof_data:ENGR_307,
        roboprof_data:ENGR_308,
        roboprof_data:ENGR_392,
        roboprof_data:ENGR_412,
        roboprof_data:ENGR_472,
        roboprof_data:ENGR_8901,
        roboprof_data:ENGR_8911,
        roboprof_data:ENVS_608,
        roboprof_data:ENVS_664,
        roboprof_data:ESL_205,
        roboprof_data:ESL_206,
        roboprof_data:ESTU_670,
        roboprof_data:ETEC_613,
        roboprof_data:ETEC_637,
        roboprof_data:ETEC_650,
        roboprof_data:ETEC_651,
        roboprof_data:ETEC_665,
        roboprof_data:ETEC_669,
        roboprof_data:ETEC_671,
        roboprof_data:ETEC_681,
        roboprof_data:EXCI_252,
        roboprof_data:EXCI_253,
        roboprof_data:EXCI_254,
        roboprof_data:EXCI_258,
        roboprof_data:EXCI_259,
        roboprof_data:EXCI_323,
        roboprof_data:EXCI_351,
        roboprof_data:EXCI_352,
        roboprof_data:EXCI_357,
        roboprof_data:EXCI_358,
        roboprof_data:EXCI_455,
        roboprof_data:FBRS_201,
        roboprof_data:FBRS_240,
        roboprof_data:FBRS_260,
        roboprof_data:FBRS_341,
        roboprof_data:FBRS_361,
        roboprof_data:FBRS_371,
        roboprof_data:FBRS_372,
        roboprof_data:FBRS_385,
        roboprof_data:FBRS_386,
        roboprof_data:FBRS_395,
        roboprof_data:FBRS_396,
        roboprof_data:FBRS_397,
        roboprof_data:FBRS_398,
        roboprof_data:FBRS_399,
        roboprof_data:FBRS_450,
        roboprof_data:FBRS_451,
        roboprof_data:FBRS_452,
        roboprof_data:FBRS_480,
        roboprof_data:FBRS_481,
        roboprof_data:FBRS_482,
        roboprof_data:FINA_385,
        roboprof_data:FINA_395,
        roboprof_data:FINA_402,
        roboprof_data:FINA_405,
        roboprof_data:FINA_408,
        roboprof_data:FINA_409,
        roboprof_data:FINA_410,
        roboprof_data:FINA_411,
        roboprof_data:FINA_413,
        roboprof_data:FINA_415,
        roboprof_data:FINA_416,
        roboprof_data:FINA_465,
        roboprof_data:FINA_470,
        roboprof_data:FINA_471,
        roboprof_data:FINA_481,
        roboprof_data:FINA_482,
        roboprof_data:FINA_663,
        roboprof_data:FINA_695,
        roboprof_data:FLIT_454,
        roboprof_data:FLIT_486,
        roboprof_data:FLIT_488,
        roboprof_data:FLIT_496,
        roboprof_data:FLIT_690,
        roboprof_data:FLIT_691,
        roboprof_data:FLIT_692,
        roboprof_data:FLIT_693,
        roboprof_data:FMAN_203,
        roboprof_data:FMPR_451,
        roboprof_data:FMST_201,
        roboprof_data:FMST_202,
        roboprof_data:FMST_203,
        roboprof_data:FMST_204,
        roboprof_data:FPST_297,
        roboprof_data:FPST_397,
        roboprof_data:FPST_497,
        roboprof_data:FRAA_413,
        roboprof_data:FRAA_419,
        roboprof_data:FRAA_423,
        roboprof_data:FRAA_491,
        roboprof_data:FRAA_492,
        roboprof_data:FRAA_523,
        roboprof_data:FRAA_623,
        roboprof_data:FRAN_211,
        roboprof_data:FRAN_212,
        roboprof_data:FRAN_318,
        roboprof_data:FRAN_319,
        roboprof_data:FTRA_411,
        roboprof_data:FTRA_416,
        roboprof_data:FTRA_418,
        roboprof_data:FTRA_438,
        roboprof_data:FTRA_452,
        roboprof_data:FTRA_455,
        roboprof_data:FTRA_492,
        roboprof_data:FTRA_534,
        roboprof_data:FTRA_538,
        roboprof_data:FTRA_555,
        roboprof_data:FTRA_556,
        roboprof_data:FTRA_558,
        roboprof_data:FTRA_613,
        roboprof_data:FTRA_615,
        roboprof_data:FTRA_631,
        roboprof_data:FTRA_632,
        roboprof_data:FTRA_633,
        roboprof_data:FTRA_636,
        roboprof_data:FTRA_638,
        roboprof_data:FTRA_655,
        roboprof_data:FTRA_658,
        roboprof_data:FTRA_668,
        roboprof_data:FTRA_681,
        roboprof_data:FTRA_682,
        roboprof_data:FTRA_683,
        roboprof_data:FTRA_684,
        roboprof_data:FTRA_685,
        roboprof_data:GEOG_210,
        roboprof_data:GEOG_260,
        roboprof_data:GEOG_264,
        roboprof_data:GEOG_301,
        roboprof_data:GEOG_323,
        roboprof_data:GEOG_361,
        roboprof_data:GEOG_362,
        roboprof_data:GEOG_363,
        roboprof_data:GEOG_371,
        roboprof_data:GEOG_374,
        roboprof_data:GEOG_377,
        roboprof_data:GEOG_463,
        roboprof_data:GEOG_464,
        roboprof_data:GEOG_465,
        roboprof_data:GEOG_466,
        roboprof_data:GEOG_467,
        roboprof_data:GEOG_474,
        roboprof_data:GEOG_490,
        roboprof_data:GEOL_210,
        roboprof_data:GEOL_216,
        roboprof_data:GEOL_302,
        roboprof_data:GEOL_331,
        roboprof_data:GEOL_415,
        roboprof_data:GERM_200,
        roboprof_data:GERM_201,
        roboprof_data:GERM_202,
        roboprof_data:GERM_240,
        roboprof_data:GIIM_637,
        roboprof_data:GIIM_655,
        roboprof_data:HENV_655,
        roboprof_data:HENV_801,
        roboprof_data:HENV_802,
        roboprof_data:HEXS_801,
        roboprof_data:HIST_200,
        roboprof_data:HIST_281,
        roboprof_data:HIST_306,
        roboprof_data:HIST_307,
        roboprof_data:HIST_329,
        roboprof_data:HIST_338,
        roboprof_data:HIST_368,
        roboprof_data:HIST_379,
        roboprof_data:HIST_380,
        roboprof_data:HIST_381,
        roboprof_data:HIST_387,
        roboprof_data:HIST_388,
        roboprof_data:HIST_390,
        roboprof_data:HIST_397,
        roboprof_data:HIST_403,
        roboprof_data:HIST_481,
        roboprof_data:HIST_485,
        roboprof_data:HIST_486,
        roboprof_data:HIST_493,
        roboprof_data:HIST_498,
        roboprof_data:HIST_685,
        roboprof_data:HIST_889,
        roboprof_data:HIST_890,
        roboprof_data:IADI_301,
        roboprof_data:IADI_401,
        roboprof_data:IMCA_201,
        roboprof_data:IMCA_210,
        roboprof_data:IMCA_220,
        roboprof_data:IMCA_221,
        roboprof_data:IMCA_222,
        roboprof_data:IMCA_230,
        roboprof_data:IMCA_310,
        roboprof_data:IMCA_321,
        roboprof_data:IMCA_322,
        roboprof_data:IMCA_331,
        roboprof_data:IMCA_332,
        roboprof_data:IMCA_398,
        roboprof_data:IMCA_399,
        roboprof_data:IMCA_400,
        roboprof_data:IMCA_470,
        roboprof_data:IMCA_471,
        roboprof_data:IMCA_472,
        roboprof_data:IMCA_480,
        roboprof_data:IMCA_481,
        roboprof_data:IMCA_482,
        roboprof_data:IMCA_498,
        roboprof_data:IMCA_499,
        roboprof_data:INDU_311,
        roboprof_data:INDU_323,
        roboprof_data:INDU_324,
        roboprof_data:INDU_410,
        roboprof_data:INDU_411,
        roboprof_data:INDU_412,
        roboprof_data:INDU_421,
        roboprof_data:INDU_423,
        roboprof_data:INDU_480,
        roboprof_data:INDU_490,
        roboprof_data:INDU_6111,
        roboprof_data:INDU_6121,
        roboprof_data:INDU_6131,
        roboprof_data:INDU_6141,
        roboprof_data:INDU_6151,
        roboprof_data:INDU_6211,
        roboprof_data:INDU_6221,
        roboprof_data:INDU_6231,
        roboprof_data:INDU_6241,
        roboprof_data:INDU_6311,
        roboprof_data:INDU_6321,
        roboprof_data:INDU_6331,
        roboprof_data:INDU_6341,
        roboprof_data:INDU_6351,
        roboprof_data:INDU_6361,
        roboprof_data:INDU_6411,
        roboprof_data:INDU_6421,
        roboprof_data:INSE_6100,
        roboprof_data:INSE_6110,
        roboprof_data:INSE_6120,
        roboprof_data:INSE_6130,
        roboprof_data:INSE_6140,
        roboprof_data:INSE_6150,
        roboprof_data:INSE_6160,
        roboprof_data:INSE_6170,
        roboprof_data:INSE_6180,
        roboprof_data:INSE_6190,
        roboprof_data:INSE_6210,
        roboprof_data:INSE_6220,
        roboprof_data:INSE_6230,
        roboprof_data:INSE_6240,
        roboprof_data:INSE_6250,
        roboprof_data:INSE_6260,
        roboprof_data:INSE_6270,
        roboprof_data:INSE_6280,
        roboprof_data:INSE_6290,
        roboprof_data:INSE_6300,
        roboprof_data:INSE_6310,
        roboprof_data:INSE_6311,
        roboprof_data:INSE_6320,
        roboprof_data:INSE_6400,
        roboprof_data:INSE_6411,
        roboprof_data:INSE_6421,
        roboprof_data:INSE_6431,
        roboprof_data:INSE_6441,
        roboprof_data:INSE_6510,
        roboprof_data:INSE_6530,
        roboprof_data:INSE_6610,
        roboprof_data:INSE_6630,
        roboprof_data:INSE_6640,
        roboprof_data:INSE_6650,
        roboprof_data:INSE_6660,
        roboprof_data:INSE_6670,
        roboprof_data:INSE_6680,
        roboprof_data:INSE_7100,
        roboprof_data:INSE_7110,
        roboprof_data:INSE_7120,
        roboprof_data:INSE_8901,
        roboprof_data:IRST_299,
        roboprof_data:IRST_300,
        roboprof_data:IRST_344,
        roboprof_data:IRST_346,
        roboprof_data:IRST_347,
        roboprof_data:IRST_390,
        roboprof_data:ITAL_200,
        roboprof_data:ITAL_201,
        roboprof_data:ITAL_202,
        roboprof_data:ITAL_240,
        roboprof_data:JAZZ_481,
        roboprof_data:JAZZ_482,
        roboprof_data:JOUR_206,
        roboprof_data:JOUR_207,
        roboprof_data:JOUR_208,
        roboprof_data:JOUR_209,
        roboprof_data:JOUR_303,
        roboprof_data:JOUR_309,
        roboprof_data:JOUR_321,
        roboprof_data:JOUR_325,
        roboprof_data:JOUR_330,
        roboprof_data:JOUR_402,
        roboprof_data:JOUR_404,
        roboprof_data:JOUR_421,
        roboprof_data:JOUR_432,
        roboprof_data:JOUR_443,
        roboprof_data:JOUR_445,
        roboprof_data:JOUR_450,
        roboprof_data:JOUR_502,
        roboprof_data:JOUR_503,
        roboprof_data:JOUR_504,
        roboprof_data:JOUR_505,
        roboprof_data:JOUR_507,
        roboprof_data:JOUR_521,
        roboprof_data:JOUR_523,
        roboprof_data:JOUR_527,
        roboprof_data:JOUR_528,
        roboprof_data:JOUR_530,
        roboprof_data:JOUR_531,
        roboprof_data:JOUR_532,
        roboprof_data:JOUR_535,
        roboprof_data:JOUR_537,
        roboprof_data:JOUR_605,
        roboprof_data:JOUR_630,
        roboprof_data:JPER_223,
        roboprof_data:JPER_224,
        roboprof_data:JPER_225,
        roboprof_data:JPER_323,
        roboprof_data:JPER_324,
        roboprof_data:JPER_325,
        roboprof_data:JPER_341,
        roboprof_data:JPER_423,
        roboprof_data:JPER_424,
        roboprof_data:JPER_425,
        roboprof_data:JPER_441,
        roboprof_data:JPER_451,
        roboprof_data:KCEP_349,
        roboprof_data:KCEP_383,
        roboprof_data:KCEP_449,
        roboprof_data:KCEP_483,
        roboprof_data:LBCL_295,
        roboprof_data:LIBS_495,
        roboprof_data:LING_372,
        roboprof_data:LING_421,
        roboprof_data:LING_472,
        roboprof_data:LING_490,
        roboprof_data:LOYC_205,
        roboprof_data:LOYC_240,
        roboprof_data:LOYC_298,
        roboprof_data:LOYC_320,
        roboprof_data:LOYC_420,
        roboprof_data:MACF_401,
        roboprof_data:MACF_402,
        roboprof_data:MANA_300,
        roboprof_data:MANA_343,
        roboprof_data:MANA_362,
        roboprof_data:MANA_366,
        roboprof_data:MANA_420,
        roboprof_data:MANA_443,
        roboprof_data:MANA_444,
        roboprof_data:MANA_446,
        roboprof_data:MANA_447,
        roboprof_data:MANA_481,
        roboprof_data:MANA_668,
        roboprof_data:MANA_684,
        roboprof_data:MARA_200,
        roboprof_data:MARA_203,
        roboprof_data:MARA_206,
        roboprof_data:MARA_207,
        roboprof_data:MARA_240,
        roboprof_data:MARA_250,
        roboprof_data:MARK_301,
        roboprof_data:MARK_305,
        roboprof_data:MARK_444,
        roboprof_data:MARK_451,
        roboprof_data:MARK_452,
        roboprof_data:MARK_453,
        roboprof_data:MARK_454,
        roboprof_data:MARK_457,
        roboprof_data:MARK_458,
        roboprof_data:MARK_462,
        roboprof_data:MARK_463,
        roboprof_data:MARK_465,
        roboprof_data:MARK_485,
        roboprof_data:MARK_486,
        roboprof_data:MARK_491,
        roboprof_data:MARK_492,
        roboprof_data:MARK_493,
        roboprof_data:MARK_495,
        roboprof_data:MARK_671,
        roboprof_data:MAST_232,
        roboprof_data:MAST_324,
        roboprof_data:MAST_333,
        roboprof_data:MAST_397,
        roboprof_data:MAST_677,
        roboprof_data:MATH_387,
        roboprof_data:MBA_642,
        roboprof_data:MBA_644,
        roboprof_data:MBA_645,
        roboprof_data:MBA_647,
        roboprof_data:MBA_649,
        roboprof_data:MBA_650,
        roboprof_data:MBA_654,
        roboprof_data:MBA_657,
        roboprof_data:MBA_658,
        roboprof_data:MBA_659,
        roboprof_data:MBA_660,
        roboprof_data:MBA_662,
        roboprof_data:MBA_663,
        roboprof_data:MBA_695,
        roboprof_data:MCHI_200,
        roboprof_data:MCHI_206,
        roboprof_data:MCHI_240,
        roboprof_data:MCHI_250,
        roboprof_data:MECH_211,
        roboprof_data:MECH_215,
        roboprof_data:MECH_311,
        roboprof_data:MECH_321,
        roboprof_data:MECH_343,
        roboprof_data:MECH_351,
        roboprof_data:MECH_352,
        roboprof_data:MECH_361,
        roboprof_data:MECH_368,
        roboprof_data:MECH_370,
        roboprof_data:MECH_371,
        roboprof_data:MECH_375,
        roboprof_data:MECH_390,
        roboprof_data:MECH_411,
        roboprof_data:MECH_412,
        roboprof_data:MECH_414,
        roboprof_data:MECH_421,
        roboprof_data:MECH_423,
        roboprof_data:MECH_424,
        roboprof_data:MECH_425,
        roboprof_data:MECH_447,
        roboprof_data:MECH_452,
        roboprof_data:MECH_460,
        roboprof_data:MECH_461,
        roboprof_data:MECH_463,
        roboprof_data:MECH_471,
        roboprof_data:MECH_472,
        roboprof_data:MECH_473,
        roboprof_data:MECH_474,
        roboprof_data:MECH_6011,
        roboprof_data:MECH_6021,
        roboprof_data:MECH_6041,
        roboprof_data:MECH_6051,
        roboprof_data:MECH_6061,
        roboprof_data:MECH_6081,
        roboprof_data:MECH_6091,
        roboprof_data:MECH_6101,
        roboprof_data:MECH_6111,
        roboprof_data:MECH_6121,
        roboprof_data:MECH_6131,
        roboprof_data:MECH_6141,
        roboprof_data:MECH_6161,
        roboprof_data:MECH_6171,
        roboprof_data:MECH_6181,
        roboprof_data:MECH_6191,
        roboprof_data:MECH_6231,
        roboprof_data:MECH_6241,
        roboprof_data:MECH_6251,
        roboprof_data:MECH_6301,
        roboprof_data:MECH_6311,
        roboprof_data:MECH_6321,
        roboprof_data:MECH_6341,
        roboprof_data:MECH_6351,
        roboprof_data:MECH_6361,
        roboprof_data:MECH_6421,
        roboprof_data:MECH_6431,
        roboprof_data:MECH_6441,
        roboprof_data:MECH_6451,
        roboprof_data:MECH_6481,
        roboprof_data:MECH_6491,
        roboprof_data:MECH_6501,
        roboprof_data:MECH_6511,
        roboprof_data:MECH_6521,
        roboprof_data:MECH_6531,
        roboprof_data:MECH_6541,
        roboprof_data:MECH_6551,
        roboprof_data:MECH_6561,
        roboprof_data:MECH_6571,
        roboprof_data:MECH_6581,
        roboprof_data:MECH_6601,
        roboprof_data:MECH_6611,
        roboprof_data:MECH_6621,
        roboprof_data:MECH_6631,
        roboprof_data:MECH_6641,
        roboprof_data:MECH_6651,
        roboprof_data:MECH_6661,
        roboprof_data:MECH_6671,
        roboprof_data:MECH_6681,
        roboprof_data:MECH_6691,
        roboprof_data:MECH_6741,
        roboprof_data:MECH_6751,
        roboprof_data:MECH_6761,
        roboprof_data:MECH_6771,
        roboprof_data:MECH_6781,
        roboprof_data:MECH_7011,
        roboprof_data:MECH_7101,
        roboprof_data:MECH_7501,
        roboprof_data:MECH_7511,
        roboprof_data:MECH_7711,
        roboprof_data:MHIS_203,
        roboprof_data:MPER_231,
        roboprof_data:MPER_321,
        roboprof_data:MPER_322,
        roboprof_data:MPER_332,
        roboprof_data:MPER_421,
        roboprof_data:MPER_422,
        roboprof_data:MPER_451,
        roboprof_data:MSCA_602,
        roboprof_data:MSCA_611,
        roboprof_data:MSCA_625,
        roboprof_data:MSCA_632,
        roboprof_data:MSCA_654,
        roboprof_data:MUSI_201,
        roboprof_data:MUSI_481,
        roboprof_data:MUSI_482,
        roboprof_data:PERC_209,
        roboprof_data:PERC_210,
        roboprof_data:PERC_211,
        roboprof_data:PERC_212,
        roboprof_data:PERC_298,
        roboprof_data:PERC_311,
        roboprof_data:PERC_318,
        roboprof_data:PERC_321,
        roboprof_data:PERC_322,
        roboprof_data:PERC_324,
        roboprof_data:PERC_351,
        roboprof_data:PERC_356,
        roboprof_data:PERC_384,
        roboprof_data:PERC_386,
        roboprof_data:PERC_398,
        roboprof_data:PERC_399,
        roboprof_data:PERC_405,
        roboprof_data:PERC_408,
        roboprof_data:PERC_409,
        roboprof_data:PERC_415,
        roboprof_data:PERC_421,
        roboprof_data:PERC_422,
        roboprof_data:PERC_462,
        roboprof_data:PERC_464,
        roboprof_data:PERC_471,
        roboprof_data:PERC_488,
        roboprof_data:PERC_490,
        roboprof_data:PERC_496,
        roboprof_data:PERC_498,
        roboprof_data:PERC_499,
        roboprof_data:PHIL_214,
        roboprof_data:PHIL_220,
        roboprof_data:PHIL_232,
        roboprof_data:PHIL_260,
        roboprof_data:PHIL_261,
        roboprof_data:PHIL_263,
        roboprof_data:PHIL_265,
        roboprof_data:PHIL_495,
        roboprof_data:PHIL_496,
        roboprof_data:PHIL_497,
        roboprof_data:PHOT_201,
        roboprof_data:PHOT_210,
        roboprof_data:PHOT_221,
        roboprof_data:PHOT_300,
        roboprof_data:PHOT_311,
        roboprof_data:PHOT_312,
        roboprof_data:PHOT_322,
        roboprof_data:PHOT_331,
        roboprof_data:PHOT_332,
        roboprof_data:PHOT_398,
        roboprof_data:PHOT_399,
        roboprof_data:PHOT_400,
        roboprof_data:PHOT_470,
        roboprof_data:PHOT_471,
        roboprof_data:PHOT_472,
        roboprof_data:PHOT_480,
        roboprof_data:PHOT_481,
        roboprof_data:PHOT_482,
        roboprof_data:PHOT_498,
        roboprof_data:PHOT_499,
        roboprof_data:PHYS_224,
        roboprof_data:PHYS_225,
        roboprof_data:PHYS_226,
        roboprof_data:PHYS_230,
        roboprof_data:PHYS_236,
        roboprof_data:PHYS_289,
        roboprof_data:PHYS_295,
        roboprof_data:PHYS_330,
        roboprof_data:PHYS_389,
        roboprof_data:PHYS_390,
        roboprof_data:PHYS_440,
        roboprof_data:PHYS_496,
        roboprof_data:PHYS_497,
        roboprof_data:PHYS_637,
        roboprof_data:PHYS_660,
        roboprof_data:PHYS_663,
        roboprof_data:PHYS_665,
        roboprof_data:PHYS_760,
        roboprof_data:PHYS_862,
        roboprof_data:POLI_205,
        roboprof_data:POLI_214,
        roboprof_data:POLI_300,
        roboprof_data:POLI_315,
        roboprof_data:POLI_328,
        roboprof_data:POLI_392,
        roboprof_data:POLI_397,
        roboprof_data:POLI_419,
        roboprof_data:POLI_480,
        roboprof_data:POLI_487,
        roboprof_data:POLI_495,
        roboprof_data:POLI_644,
        roboprof_data:POLI_683,
        roboprof_data:POLI_693,
        roboprof_data:PRIN_211,
        roboprof_data:PRIN_221,
        roboprof_data:PRIN_231,
        roboprof_data:PRIN_241,
        roboprof_data:PRIN_271,
        roboprof_data:PRIN_291,
        roboprof_data:PRIN_311,
        roboprof_data:PRIN_321,
        roboprof_data:PRIN_331,
        roboprof_data:PRIN_341,
        roboprof_data:PRIN_366,
        roboprof_data:PRIN_371,
        roboprof_data:PRIN_381,
        roboprof_data:PRIN_391,
        roboprof_data:PRIN_398,
        roboprof_data:PRIN_399,
        roboprof_data:PRIN_411,
        roboprof_data:PRIN_421,
        roboprof_data:PRIN_431,
        roboprof_data:PRIN_441,
        roboprof_data:PRIN_451,
        roboprof_data:PRIN_452,
        roboprof_data:PRIN_470,
        roboprof_data:PRIN_471,
        roboprof_data:PRIN_472,
        roboprof_data:PRIN_481,
        roboprof_data:PRIN_498,
        roboprof_data:PRIN_499,
        roboprof_data:PSYC_311,
        roboprof_data:PSYC_315,
        roboprof_data:PSYC_316,
        roboprof_data:PSYC_387,
        roboprof_data:PSYC_485,
        roboprof_data:PSYC_487,
        roboprof_data:PSYC_495,
        roboprof_data:PSYC_601,
        roboprof_data:PSYC_705,
        roboprof_data:PSYC_706,
        roboprof_data:PSYC_707,
        roboprof_data:PSYC_708,
        roboprof_data:PSYC_709,
        roboprof_data:PSYC_710,
        roboprof_data:PSYC_711,
        roboprof_data:PSYC_712,
        roboprof_data:PSYC_713,
        roboprof_data:PSYC_823,
        roboprof_data:PSYC_824,
        roboprof_data:PSYC_825,
        roboprof_data:PSYC_826,
        roboprof_data:PSYC_827,
        roboprof_data:PSYC_828,
        roboprof_data:PSYC_838,
        roboprof_data:PSYC_839,
        roboprof_data:PSYC_840,
        roboprof_data:PSYC_841,
        roboprof_data:PSYC_842,
        roboprof_data:PSYC_843,
        roboprof_data:PSYC_850,
        roboprof_data:PSYC_851,
        roboprof_data:PTNG_200,
        roboprof_data:PTNG_201,
        roboprof_data:PTNG_298,
        roboprof_data:PTNG_299,
        roboprof_data:PTNG_300,
        roboprof_data:PTNG_310,
        roboprof_data:PTNG_312,
        roboprof_data:PTNG_314,
        roboprof_data:PTNG_316,
        roboprof_data:PTNG_320,
        roboprof_data:PTNG_398,
        roboprof_data:PTNG_399,
        roboprof_data:PTNG_400,
        roboprof_data:PTNG_410,
        roboprof_data:PTNG_412,
        roboprof_data:PTNG_414,
        roboprof_data:PTNG_416,
        roboprof_data:PTNG_418,
        roboprof_data:PTNG_420,
        roboprof_data:PTNG_430,
        roboprof_data:PTNG_440,
        roboprof_data:PTNG_450,
        roboprof_data:PTNG_460,
        roboprof_data:PTNG_470,
        roboprof_data:PTNG_471,
        roboprof_data:PTNG_472,
        roboprof_data:PTNG_498,
        roboprof_data:PTNG_499,
        roboprof_data:RELI_210,
        roboprof_data:RELI_214,
        roboprof_data:RELI_215,
        roboprof_data:RELI_220,
        roboprof_data:RELI_223,
        roboprof_data:RELI_224,
        roboprof_data:RELI_312,
        roboprof_data:RELI_313,
        roboprof_data:RELI_318,
        roboprof_data:RELI_378,
        roboprof_data:RELI_387,
        roboprof_data:RELI_390,
        roboprof_data:RELI_392,
        roboprof_data:RELI_396,
        roboprof_data:RELI_409,
        roboprof_data:RELI_6007,
        roboprof_data:RELI_6008,
        roboprof_data:RELI_6018,
        roboprof_data:SCEN_327,
        roboprof_data:SCEN_347,
        roboprof_data:SCEN_411,
        roboprof_data:SCEN_412,
        roboprof_data:SCEN_448,
        roboprof_data:SCOL_290,
        roboprof_data:SCOL_391,
        roboprof_data:SCOL_490,
        roboprof_data:SCOM_374,
        roboprof_data:SCOM_492,
        roboprof_data:SCOM_498,
        roboprof_data:SCPA_301,
        roboprof_data:SCPA_352,
        roboprof_data:SCPA_411,
        roboprof_data:SCPA_412,
        roboprof_data:SCPA_482,
        roboprof_data:SCPA_509,
        roboprof_data:SCPA_510,
        roboprof_data:SCPA_516,
        roboprof_data:SCPA_537,
        roboprof_data:SCUL_201,
        roboprof_data:SCUL_210,
        roboprof_data:SCUL_251,
        roboprof_data:SCUL_310,
        roboprof_data:SCUL_311,
        roboprof_data:SCUL_312,
        roboprof_data:SCUL_396,
        roboprof_data:SCUL_397,
        roboprof_data:SCUL_398,
        roboprof_data:SCUL_399,
        roboprof_data:SCUL_410,
        roboprof_data:SCUL_450,
        roboprof_data:SCUL_451,
        roboprof_data:SCUL_452,
        roboprof_data:SCUL_490,
        roboprof_data:SOCI_415,
        roboprof_data:SOCI_450,
        roboprof_data:SOEN_228,
        roboprof_data:SOEN_341,
        roboprof_data:SOEN_385,
        roboprof_data:SOEN_390,
        roboprof_data:SOEN_422,
        roboprof_data:SOEN_423,
        roboprof_data:SOEN_487,
        roboprof_data:SOEN_490,
        roboprof_data:SOEN_491,
        roboprof_data:SOEN_6231,
        roboprof_data:SOEN_6441,
        roboprof_data:SPAN_200,
        roboprof_data:SPAN_201,
        roboprof_data:SPAN_202,
        roboprof_data:SPAN_240,
        roboprof_data:SSDB_220,
        roboprof_data:SSDB_275,
        roboprof_data:SSDB_425,
        roboprof_data:SSDB_426,
        roboprof_data:SSDB_428,
        roboprof_data:SSDB_492,
        roboprof_data:STAT_280,
        roboprof_data:STAT_287,
        roboprof_data:STAT_380,
        roboprof_data:STAT_388,
        roboprof_data:STAT_460,
        roboprof_data:STAT_461,
        roboprof_data:STAT_480,
        roboprof_data:STAT_497,
        roboprof_data:TESL_201,
        roboprof_data:TESL_221,
        roboprof_data:TESL_231,
        roboprof_data:TESL_324,
        roboprof_data:TESL_326,
        roboprof_data:TESL_330,
        roboprof_data:TESL_331,
        roboprof_data:TESL_341,
        roboprof_data:TESL_415,
        roboprof_data:TESL_424,
        roboprof_data:TESL_426,
        roboprof_data:TESL_427,
        roboprof_data:TESL_433,
        roboprof_data:TESL_471,
        roboprof_data:TESL_488,
        roboprof_data:THEO_234,
        roboprof_data:THEO_243,
        roboprof_data:THEO_404,
        roboprof_data:THEO_692,
        roboprof_data:URBS_250,
        roboprof_data:URBS_260,
        roboprof_data:URBS_333,
        roboprof_data:URBS_335,
        roboprof_data:URBS_337,
        roboprof_data:URBS_362,
        roboprof_data:URBS_420,
        roboprof_data:URBS_433,
        roboprof_data:URBS_483,
        roboprof_data:URBS_484,
        roboprof_data:VDEO_350,
        roboprof_data:WSDB_291,
        roboprof_data:WSDB_292,
        roboprof_data:WSDB_391,
        roboprof_data:WSDB_491,
        roboprof_data:WSDB_494 ;
    rdfs:seeAlso <https://dbpedia.org/resource/Concordia_University> .

<file:///./dataset/Lecture%20Content/COMP%206461/Readings/NetworkCongestion.pdf> a roboprof:Reading ;
    dbo:name "NetworkCongestion.pdf" .

<file:///./dataset/Lecture%20Content/COMP%206461/Worksheets/TA3.pdf> a roboprof:Worksheet ;
    dbo:name "TA3.pdf" .

<file:///./dataset/Lecture%20Content/COMP%206461/Readings/GoBackN.pdf> a roboprof:Reading ;
    dbo:name "GoBackN.pdf" .

<file:///./dataset/Lecture%20Content/COMP%206741/OtherMaterial/LinguisticLinkedOpenData.pdf> a roboprof:OtherMaterial ;
    dbo:name "LinguisticLinkedOpenData.pdf" .

<file:///./dataset/Lecture%20Content/COMP%206741/OtherMaterial/WordEmbeddings.pdf> a roboprof:OtherMaterial ;
    dbo:name "WordEmbeddings.pdf" .

<file:///./dataset/Lecture%20Content/COMP%206741/Readings/RecommenderSystem.pdf> a roboprof:Reading ;
    dbo:name "RecommenderSystem.pdf" .

<file:///./dataset/Lecture%20Content/COMP%206741/Worksheets/worksheet05.pdf> a roboprof:Worksheet ;
    dbo:name "worksheet05.pdf" .

roboprof_data:COMP_6461 a vivo:Course ;
    dbo:name "Computer Networks and Protocols" ;
    dbo:number 6461 ;
    dcterms:description "The main objectives of this course are: 1. Introduce the basics of Data Communication, Information, Coding, and Transmission. 2. Understand the ISO OSI and Internet models and the role of layered protocols. 3. Understand and appreciate Networks, Protocols, Network-interconnection and Internet." ;
    roboprof:courseOutline <https://www.aimanhanna.com/concordia/index.htm> ;
    roboprof:hasCourseEvent roboprof_data:COMP_6461_Lab_1,
        roboprof_data:COMP_6461_Lab_2,
        roboprof_data:COMP_6461_Lab_3,
        roboprof_data:COMP_6461_Lecture_1,
        roboprof_data:COMP_6461_Lecture_2,
        roboprof_data:COMP_6461_Lecture_3,
        roboprof_data:COMP_6461_Lecture_4,
        roboprof_data:COMP_6461_Lecture_5,
        roboprof_data:COMP_6461_Lecture_6 ;
    vivo:courseCredits 4 ;
    vivo:hasSubjectArea "COMP" ;
    rdfs:seeAlso <https://www.concordia.ca/academics/graduate/calendar/current/gina-cody-school-of-engineering-and-computer-science-courses/computer-science-and-software-engineering-master-s-and-phd-courses.html> .

<file:///./dataset/Lecture%20Content/COMP%206741/Worksheets/worksheet03.pdf> a roboprof:Worksheet ;
    dbo:name "worksheet03.pdf" .

roboprof_data:COMP_6521 a vivo:Course ;
    dbo:name "Advanced Database Techniques and Applications" ;
    dbo:number 6521 ;
    dcterms:description "Laboratory: 24 hours total, project" ;
    vivo:courseCredits 4 ;
    vivo:hasSubjectArea "COMP" .

roboprof_data:COMP_6741 a vivo:Course ;
    dbo:name "Intelligent Systems" ;
    dbo:number 6741 ;
    dcterms:description "(COMP 474): Rule-based expert systems, blackboard architecture, and agent-based. Knowledge acquisition and representation. Uncertainty and conflict resolution. Reasoning and explanation. Design of intelligent systems. Project. (COMP 6741): Knowledge representation and reasoning. Uncertainty and conflict resolution. Design of intelligent systems. Grammar-based, rule-based, and blackboard architectures. A project is required. Component(s): Lecture 3 hours per week; Laboratory 2 hours per week Prerequisites: COMP 352 or COEN 352 (applies to COMP 474 only) Co-requisites: n/a Specific Knowledge and Skills Needed for this Course: To succeed in this course, you will need specific skills and knowledge in the following areas: Programming Skills:  Python: Proficiency in general programming using Python is essential for lab sessions and the course project. A brief introduction to Python will be provided during the first lab session, but pre-existing familiarity is strongly recommended.  APIs and Data Handling: Basic understanding of working with APIs and data formats (like JSON, XML) is important, especially for labs and the project involving knowledge graphs, NLP applications, and interfacing with Deep Learning frameworks. Mathematical Foundations:  Linear Algebra: Concepts from linear algebra will be utilized frequently, especially in machine learning and neural network modules. If you find yourself lacking in any of these areas, you are strongly encouraged to review these topics before the DNE (Did Not Enter) deadline" ;
    roboprof:courseOutline <https://moodle.concordia.ca/moodle/pluginfile.php/6419696/course/section/2181768/course_outline_comp474_6741_w2024.pdf> ;
    roboprof:hasCourseEvent roboprof_data:COMP_6741_Lab_1,
        roboprof_data:COMP_6741_Lab_2,
        roboprof_data:COMP_6741_Lab_3,
        roboprof_data:COMP_6741_Lecture_1,
        roboprof_data:COMP_6741_Lecture_2,
        roboprof_data:COMP_6741_Lecture_3,
        roboprof_data:COMP_6741_Lecture_4,
        roboprof_data:COMP_6741_Lecture_5,
        roboprof_data:COMP_6741_Lecture_6 ;
    vivo:courseCredits 4 ;
    vivo:hasSubjectArea "COMP" ;
    rdfs:seeAlso <https://www.concordia.ca/academics/graduate/calendar/current/gina-cody-school-of-engineering-and-computer-science-courses/computer-science-and-software-engineering-master-s-and-phd-courses.html> .

<file:///./dataset/Lecture%20Content/COMP%206741/OtherMaterial/MachineLearning.pdf> a roboprof:OtherMaterial ;
    dbo:name "MachineLearning.pdf" .

<file:///./dataset/Lecture%20Content/COMP%206741/OtherMaterial/TextMining.pdf> a roboprof:OtherMaterial ;
    dbo:name "TextMining.pdf" .

<file:///./dataset/Lecture%20Content/COMP%206741/Readings/IntelligentAgent.pdf> a roboprof:Reading ;
    dbo:name "IntelligentAgent.pdf" .

<file:///./dataset/Lecture%20Content/COMP%206741/Readings/SPARQL.pdf> a roboprof:Reading ;
    dbo:name "SPARQL.pdf" .

<file:///./dataset/Lecture%20Content/COMP%206741/Worksheets/worksheet01.pdf> a roboprof:Worksheet ;
    dbo:name "worksheet01.pdf" .

<file:///./dataset/Lecture%20Content/COMP%206461/Worksheets/TA2.pdf> a roboprof:Worksheet ;
    dbo:name "TA2.pdf" .

roboprof_data:COMP_6231 a vivo:Course ;
    dbo:name "Distributed Systems & Design" ;
    dbo:number 6231 ;
    dcterms:description "Laboratory: 24 hours total, project" ;
    vivo:courseCredits 4 ;
    vivo:hasSubjectArea "COMP" .

<file:///./dataset/Lecture%20Content/COMP%206461/Worksheets/TA1.pdf> a roboprof:Worksheet ;
    dbo:name "TA1.pdf" .

<file:///./dataset/Lab%20Content/COMP%206461/Lab%20Material/Lab%202.pdf> a roboprof:LabMaterial ;
    dbo:name "Lab 2.pdf" .

<file:///./dataset/Lab%20Content/COMP%206741/Lab%20Material/Lab%202.pdf> a roboprof:LabMaterial ;
    dbo:name "Lab 2.pdf" .

<file:///./dataset/Lecture%20Content/COMP%206461/OtherMaterial/ComputerNetwork.pdf> a roboprof:OtherMaterial ;
    dbo:name "ComputerNetwork.pdf" .

<file:///./dataset/Lecture%20Content/COMP%206461/Readings/InternetProtocolSuite.pdf> a roboprof:Reading ;
    dbo:name "InternetProtocolSuite.pdf" .

<file:///./dataset/Lecture%20Content/COMP%206461/OtherMaterial/TCP.pdf> a roboprof:OtherMaterial ;
    dbo:name "TCP.pdf" .

<file:///./dataset/Lab%20Content/COMP%206461/Lab%20Material/Lab%203.pdf> a roboprof:LabMaterial ;
    dbo:name "Lab 3.pdf" .

<file:///./dataset/Lecture%20Content/COMP%206461/Lectures/4.ppt> a roboprof:Slide ;
    dbo:name "4.ppt" .

<file:///./dataset/Lecture%20Content/COMP%206461/Readings/SelectiveRepeat.pdf> a roboprof:Reading ;
    dbo:name "SelectiveRepeat.pdf" .

<file:///./dataset/Lecture%20Content/COMP%206741/Readings/NLP.pdf> a roboprof:Reading ;
    dbo:name "NLP.pdf" .

<file:///./dataset/Lecture%20Content/COMP%206461/Lectures/5.ppt> a roboprof:Slide ;
    dbo:name "5.ppt" .

<file:///./dataset/Lecture%20Content/COMP%206461/OtherMaterial/UDP.pdf> a roboprof:OtherMaterial ;
    dbo:name "UDP.pdf" .

<file:///./dataset/Lab%20Content/COMP%206741/Lab%20Material/Lab%203.pdf> a roboprof:LabMaterial ;
    dbo:name "Lab 3.pdf" .

<file:///./dataset/Lecture%20Content/COMP%206461/Lectures/6.ppt> a roboprof:Slide ;
    dbo:name "6.ppt" .

<file:///./dataset/Lecture%20Content/COMP%206461/OtherMaterial/ApplicationLayer.pdf> a roboprof:OtherMaterial ;
    dbo:name "ApplicationLayer.pdf" .

<file:///./dataset/Lecture%20Content/COMP%206741/Readings/KnowledgeGraph.pdf> a roboprof:Reading ;
    dbo:name "KnowledgeGraph.pdf" .

<file:///./dataset/Lecture%20Content/COMP%206741/Lectures/slides05.pdf> a roboprof:Slide ;
    dbo:name "slides05.pdf" .

<file:///./dataset/Lecture%20Content/COMP%206461/Lectures/3.ppt> a roboprof:Slide ;
    dbo:name "3.ppt" .

<file:///./dataset/Lecture%20Content/COMP%206741/Lectures/slides06.pdf> a roboprof:Slide ;
    dbo:name "slides06.pdf" .

<file:///./dataset/Lecture%20Content/COMP%206741/Lectures/slides03.pdf> a roboprof:Slide ;
    dbo:name "slides03.pdf" .

<file:///./dataset/Lecture%20Content/COMP%206741/Lectures/slides04.pdf> a roboprof:Slide ;
    dbo:name "slides04.pdf" .

<file:///./dataset/Lab%20Content/COMP%206461/Lab%20Material/Lab%201.pdf> a roboprof:LabMaterial ;
    dbo:name "Lab 1.pdf" .

<file:///./dataset/Lecture%20Content/COMP%206741/Lectures/slides01.pdf> a roboprof:Slide ;
    dbo:name "slides01.pdf" .

<file:///./dataset/Lecture%20Content/COMP%206461/Lectures/2.ppt> a roboprof:Slide ;
    dbo:name "2.ppt" .

<file:///./dataset/Lecture%20Content/COMP%206741/Lectures/slides02.pdf> a roboprof:Slide ;
    dbo:name "slides02.pdf" .

